<rdf:RDF xmlns:rdf="http://www.w3.org/1999/02/22-rdf-syntax-ns#" xmlns:rdfs="http://www.w3.org/2000/01/rdf-schema#" xmlns:owl="http://www.w3.org/2002/07/owl#" xmlns:xsd="http://www.w3.org/2001/XMLSchema#" xmlns:dc="http://purl.org/dc/elements/1.1/" xmlns:abcd="http://rs.tdwg.org/abcd/terms/" xmlns:skos="http://www.w3.org/2004/02/skos/core#" xmlns:dwcattributes="http://rs.tdwg.org/dwc/terms/attributes/" xmlns:vann="http://purl.org/vocab/vann/" xmlns:dcterms="http://purl.org/dc/terms/" xmlns="http://rs.tdwg.org/abcd/terms/" xml:base="http://rs.tdwg.org/abcd/terms/">
    <owl:Ontology rdf:about="http://rs.tdwg.org/abcd/terms/">
        <dc:title>ABCD Base Ontology</dc:title>
        <dc:creator>TDWG ABCD Task Group</dc:creator>
        <dc:publisher>Biodiversity Information Standards (TDWG)</dc:publisher>
        <dcterms:issued>2019-01-31</dcterms:issued>
        <dcterms:modified>2019-01-31</dcterms:modified>
        <dc:description>The base ontology of the ABCD Standard.</dc:description>
        <owl:versionInfo>1.0</owl:versionInfo>
    </owl:Ontology>

    <owl:Class rdf:about="Accession">
        <rdfs:label xml:lang="en">Accession</rdfs:label>
        <rdfs:isDefinedBy rdf:resource="http://rs.tdwg.org/abcd/terms/"/>
        <dwcattributes:status>recommended</dwcattributes:status>
        <dcterms:issued>2019-01-31</dcterms:issued>
        <dcterms:modified>2019-01-31</dcterms:modified>
        <rdfs:comment>Triple to accommodate accession number in multiple catalogues.</rdfs:comment>
        <skos:definition>Triple to accommodate accession number in multiple catalogues.</skos:definition>
        <vann:termGroup rdf:resource="Specimen Unit"/>
    </owl:Class>

    <owl:Class rdf:about="Annotation">
        <rdfs:label xml:lang="en">Annotation</rdfs:label>
        <rdfs:isDefinedBy rdf:resource="http://rs.tdwg.org/abcd/terms/"/>
        <dwcattributes:status>recommended</dwcattributes:status>
        <dcterms:issued>2019-01-31</dcterms:issued>
        <dcterms:modified>2019-01-31</dcterms:modified>
        <rdfs:comment>An annotation for an instance of a class.</rdfs:comment>
        <skos:definition>An annotation for an instance of a class.</skos:definition>
        <vann:termGroup rdf:resource="Unit"/>
        <skos:relatedMatch rdf:resource="http://www.w3.org/ns/oa#Annotation"/>
    </owl:Class>

    <owl:Class rdf:about="Assemblage">
        <rdfs:label xml:lang="en">Assemblage</rdfs:label>
        <rdfs:isDefinedBy rdf:resource="http://rs.tdwg.org/abcd/terms/"/>
        <dwcattributes:status>recommended</dwcattributes:status>
        <dcterms:issued>2019-01-31</dcterms:issued>
        <dcterms:modified>2019-01-31</dcterms:modified>
        <rdfs:comment>A class to handle symmetric relationships between several Units i.e. herds of animals, batches of species.</rdfs:comment>
        <skos:definition>A class to handle symmetric relationships between several Units i.e. herds of animals, batches of species.</skos:definition>
        <vann:termGroup rdf:resource="Unit"/>
    </owl:Class>

    <owl:Class rdf:about="Association">
        <rdfs:label xml:lang="en">Association</rdfs:label>
        <rdfs:isDefinedBy rdf:resource="http://rs.tdwg.org/abcd/terms/"/>
        <dwcattributes:status>recommended</dwcattributes:status>
        <dcterms:issued>2019-01-31</dcterms:issued>
        <dcterms:modified>2019-01-31</dcterms:modified>
        <rdfs:comment>A class to describe an asymmetric relationship between two Units, e.g. host-parasite, parental relationships, observed pollinators, substrate, etc.</rdfs:comment>
        <skos:definition>A class to describe an asymmetric relationship between two Units, e.g. host-parasite, parental relationships, observed pollinators, substrate, etc.</skos:definition>
        <vann:termGroup rdf:resource="Unit"/>
    </owl:Class>

    <owl:Class rdf:about="AudioObject">
        <rdfs:label xml:lang="en">Audio Object</rdfs:label>
        <rdfs:isDefinedBy rdf:resource="http://rs.tdwg.org/abcd/terms/"/>
        <dwcattributes:status>recommended</dwcattributes:status>
        <dcterms:issued>2019-01-31</dcterms:issued>
        <dcterms:modified>2019-01-31</dcterms:modified>
        <rdfs:comment>Class to describe an audio recording.</rdfs:comment>
        <skos:definition>Class to describe an audio recording.</skos:definition>
        <rdfs:subClassOf rdf:resource="MultimediaObject"/>
        <vann:termGroup rdf:resource="Multimedia Object"/>
    </owl:Class>

    <owl:Class rdf:about="BacterialScientificName">
        <rdfs:label xml:lang="en">Bacterial Scientific Name</rdfs:label>
        <rdfs:isDefinedBy rdf:resource="http://rs.tdwg.org/abcd/terms/"/>
        <dwcattributes:status>recommended</dwcattributes:status>
        <dcterms:issued>2019-01-31</dcterms:issued>
        <dcterms:modified>2019-01-31</dcterms:modified>
        <rdfs:comment>Atomized bacterial name formed in the unit identification with elements according to the International Code of Nomenclature of Prokaryotes.</rdfs:comment>
        <skos:definition>Atomized bacterial name formed in the unit identification with elements according to the International Code of Nomenclature of Prokaryotes.</skos:definition>
        <rdfs:subClassOf rdf:resource="ScientificName"/>
        <vann:termGroup rdf:resource="Identification"/>
    </owl:Class>

    <owl:Class rdf:about="Biotope">
        <rdfs:label xml:lang="en">Biotope</rdfs:label>
        <rdfs:isDefinedBy rdf:resource="http://rs.tdwg.org/abcd/terms/"/>
        <dwcattributes:status>recommended</dwcattributes:status>
        <dcterms:issued>2019-01-31</dcterms:issued>
        <dcterms:modified>2019-01-31</dcterms:modified>
        <rdfs:comment>A class for citing biotope type terms and measurements related to a Unit's gathering site.</rdfs:comment>
        <skos:definition>A class for citing biotope type terms and measurements related to a Unit's gathering site.</skos:definition>
        <vann:termGroup rdf:resource="Gathering"/>
    </owl:Class>

    <owl:Class rdf:about="BotanicalGardenUnit">
        <rdfs:label xml:lang="en">Botanical Garden Unit</rdfs:label>
        <rdfs:isDefinedBy rdf:resource="http://rs.tdwg.org/abcd/terms/"/>
        <dwcattributes:status>recommended</dwcattributes:status>
        <dcterms:issued>2019-01-31</dcterms:issued>
        <dcterms:modified>2019-01-31</dcterms:modified>
        <rdfs:comment>Data specific to units in botanical live (horticultural) collections.</rdfs:comment>
        <skos:definition>Data specific to units in botanical live (horticultural) collections.</skos:definition>
        <rdfs:subClassOf rdf:resource="TypeSpecificInformation"/>
        <vann:termGroup rdf:resource="Unit Type Classes"/>
    </owl:Class>

    <owl:Class rdf:about="BotanicalScientificName">
        <rdfs:label xml:lang="en">Botanical Scientific Name</rdfs:label>
        <rdfs:isDefinedBy rdf:resource="http://rs.tdwg.org/abcd/terms/"/>
        <dwcattributes:status>recommended</dwcattributes:status>
        <dcterms:issued>2019-01-31</dcterms:issued>
        <dcterms:modified>2019-01-31</dcterms:modified>
        <rdfs:comment>Atomized botanical name formed in the unit identification, with elements according to the International Code of Botanical Nomenclature.</rdfs:comment>
        <skos:definition>Atomized botanical name formed in the unit identification, with elements according to the International Code of Botanical Nomenclature.</skos:definition>
        <rdfs:subClassOf rdf:resource="ScientificName"/>
        <vann:termGroup rdf:resource="Identification"/>
    </owl:Class>

    <owl:Class rdf:about="BotanicalTaxonRank">
        <rdfs:label xml:lang="en">Botanical Taxon Rank</rdfs:label>
        <rdfs:isDefinedBy rdf:resource="http://rs.tdwg.org/abcd/terms/"/>
        <dwcattributes:status>recommended</dwcattributes:status>
        <dcterms:issued>2019-01-31</dcterms:issued>
        <dcterms:modified>2019-01-31</dcterms:modified>
        <rdfs:comment>Taxonomic rank abbreviations as used in (botanical) name strings.</rdfs:comment>
        <skos:definition>Taxonomic rank abbreviations as used in (botanical) name strings.</skos:definition>
        <vann:termGroup rdf:resource="Identification"/>
    </owl:Class>

    <owl:Class rdf:about="Contact">
        <rdfs:label xml:lang="en">Contact</rdfs:label>
        <rdfs:isDefinedBy rdf:resource="http://rs.tdwg.org/abcd/terms/"/>
        <dwcattributes:status>recommended</dwcattributes:status>
        <dcterms:issued>2019-01-31</dcterms:issued>
        <dcterms:modified>2019-01-31</dcterms:modified>
        <rdfs:comment>A class to bundle contact information of a person or an organization.</rdfs:comment>
        <skos:definition>A class to bundle contact information of a person or an organization.</skos:definition>
        <vann:termGroup rdf:resource="Contact"/>
        <skos:exactMatch rdf:resource="http://xmlns.com/foaf/0.1/Agent"/>
    </owl:Class>

    <owl:Class rdf:about="Coordinates">
        <rdfs:label xml:lang="en">Coordinates</rdfs:label>
        <rdfs:isDefinedBy rdf:resource="http://rs.tdwg.org/abcd/terms/"/>
        <dwcattributes:status>recommended</dwcattributes:status>
        <dcterms:issued>2019-01-31</dcterms:issued>
        <dcterms:modified>2019-01-31</dcterms:modified>
        <rdfs:comment>A class to record coordinates that can be expressed in different systems.</rdfs:comment>
        <skos:definition>A class to record coordinates that can be expressed in different systems.</skos:definition>
        <vann:termGroup rdf:resource="Gathering"/>
    </owl:Class>

    <owl:Class rdf:about="Country">
        <rdfs:label xml:lang="en">Country</rdfs:label>
        <rdfs:isDefinedBy rdf:resource="http://rs.tdwg.org/abcd/terms/"/>
        <dwcattributes:status>recommended</dwcattributes:status>
        <dcterms:issued>2019-01-31</dcterms:issued>
        <dcterms:modified>2019-01-31</dcterms:modified>
        <rdfs:comment>Class to describe a country.</rdfs:comment>
        <skos:definition>Class to describe a country.</skos:definition>
        <vann:termGroup rdf:resource="Gathering"/>
    </owl:Class>

    <owl:Class rdf:about="CultureCollectionUnit">
        <rdfs:label xml:lang="en">Culture Collection Unit</rdfs:label>
        <rdfs:isDefinedBy rdf:resource="http://rs.tdwg.org/abcd/terms/"/>
        <dwcattributes:status>recommended</dwcattributes:status>
        <dcterms:issued>2019-01-31</dcterms:issued>
        <dcterms:modified>2019-01-31</dcterms:modified>
        <rdfs:comment>Data specific to microbial and similar culture methods used for the culture collection unit.</rdfs:comment>
        <skos:definition>Data specific to microbial and similar culture methods used for the culture collection unit.</skos:definition>
        <rdfs:subClassOf rdf:resource="TypeSpecificInformation"/>
        <vann:termGroup rdf:resource="Unit Type Classes"/>
    </owl:Class>

    <owl:Class rdf:about="DataSet">
        <rdfs:label xml:lang="en">Data Set</rdfs:label>
        <rdfs:isDefinedBy rdf:resource="http://rs.tdwg.org/abcd/terms/"/>
        <dwcattributes:status>recommended</dwcattributes:status>
        <dcterms:issued>2019-01-31</dcterms:issued>
        <dcterms:modified>2019-01-31</dcterms:modified>
        <rdfs:comment>A class cohering several data records and their shared metadata elements.</rdfs:comment>
        <skos:definition>A class cohering several data records and their shared metadata elements.</skos:definition>
        <vann:termGroup rdf:resource="Data Set"/>
    </owl:Class>

    <owl:Class rdf:about="Date">
        <rdfs:label xml:lang="en">Date</rdfs:label>
        <rdfs:isDefinedBy rdf:resource="http://rs.tdwg.org/abcd/terms/"/>
        <dwcattributes:status>recommended</dwcattributes:status>
        <dcterms:issued>2019-01-31</dcterms:issued>
        <dcterms:modified>2019-01-31</dcterms:modified>
        <rdfs:comment>A class to describe dates, times and time spans in the Gregorian calendar.</rdfs:comment>
        <skos:definition>A class to describe dates, times and time spans in the Gregorian calendar.</skos:definition>
        <vann:termGroup rdf:resource="General"/>
    </owl:Class>

    <owl:Class rdf:about="FieldNumber">
        <rdfs:label xml:lang="en">Field Number</rdfs:label>
        <rdfs:isDefinedBy rdf:resource="http://rs.tdwg.org/abcd/terms/"/>
        <dwcattributes:status>recommended</dwcattributes:status>
        <dcterms:issued>2019-01-31</dcterms:issued>
        <dcterms:modified>2019-01-31</dcterms:modified>
        <rdfs:comment>A class joining a Gathering Agent (Contact) and a number or other identifier assigned to a Unit during the collection or observation event.</rdfs:comment>
        <skos:definition>A class joining a Gathering Agent (Contact) and a number or other identifier assigned to a Unit during the collection or observation event.</skos:definition>
        <vann:termGroup rdf:resource="Unit"/>
    </owl:Class>

    <owl:Class rdf:about="Gathering">
        <rdfs:label xml:lang="en">Gathering</rdfs:label>
        <rdfs:isDefinedBy rdf:resource="http://rs.tdwg.org/abcd/terms/"/>
        <dwcattributes:status>recommended</dwcattributes:status>
        <dcterms:issued>2019-01-31</dcterms:issued>
        <dcterms:modified>2019-01-31</dcterms:modified>
        <rdfs:comment>A class to describe a collection or observation event.</rdfs:comment>
        <skos:definition>A class to describe a collection or observation event.</skos:definition>
        <vann:termGroup rdf:resource="Gathering"/>
    </owl:Class>

    <owl:Class rdf:about="GrowthCondition">
        <rdfs:label xml:lang="en">Growth Condition</rdfs:label>
        <rdfs:isDefinedBy rdf:resource="http://rs.tdwg.org/abcd/terms/"/>
        <dwcattributes:status>recommended</dwcattributes:status>
        <dcterms:issued>2019-01-31</dcterms:issued>
        <dcterms:modified>2019-01-31</dcterms:modified>
        <rdfs:comment>Atomized elements describing the growth conditions of a culture unit.</rdfs:comment>
        <skos:definition>Atomized elements describing the growth conditions of a culture unit.</skos:definition>
        <vann:termGroup rdf:resource="Unit Type Classes"/>
    </owl:Class>

    <owl:Class rdf:about="HerbariumUnit">
        <rdfs:label xml:lang="en">Herbarium Unit</rdfs:label>
        <rdfs:isDefinedBy rdf:resource="http://rs.tdwg.org/abcd/terms/"/>
        <dwcattributes:status>recommended</dwcattributes:status>
        <dcterms:issued>2019-01-31</dcterms:issued>
        <dcterms:modified>2019-01-31</dcterms:modified>
        <rdfs:comment>Elements only used for herbarium units.</rdfs:comment>
        <skos:definition>Elements only used for herbarium units.</skos:definition>
        <rdfs:subClassOf rdf:resource="TypeSpecificInformation"/>
        <vann:termGroup rdf:resource="Unit Type Classes"/>
    </owl:Class>

    <owl:Class rdf:about="HigherTaxon">
        <rdfs:label xml:lang="en">Higher Taxon</rdfs:label>
        <rdfs:isDefinedBy rdf:resource="http://rs.tdwg.org/abcd/terms/"/>
        <dwcattributes:status>recommended</dwcattributes:status>
        <dcterms:issued>2019-01-31</dcterms:issued>
        <dcterms:modified>2019-01-31</dcterms:modified>
        <rdfs:comment>A class to describe a higher taxon used to classify the taxon name assigned to a Unit in the Identification.</rdfs:comment>
        <skos:definition>A class to describe a higher taxon used to classify the taxon name assigned to a Unit in the Identification.</skos:definition>
        <vann:termGroup rdf:resource="Identification"/>
    </owl:Class>

    <owl:Class rdf:about="HigherTaxonRank">
        <rdfs:label xml:lang="en">Higher Taxon Rank</rdfs:label>
        <rdfs:isDefinedBy rdf:resource="http://rs.tdwg.org/abcd/terms/"/>
        <dwcattributes:status>recommended</dwcattributes:status>
        <dcterms:issued>2019-01-31</dcterms:issued>
        <dcterms:modified>2019-01-31</dcterms:modified>
        <rdfs:comment>Taxonomic ranks above the rank of genus.</rdfs:comment>
        <skos:definition>Taxonomic ranks above the rank of genus.</skos:definition>
        <vann:termGroup rdf:resource="Identification"/>
    </owl:Class>

    <owl:Class rdf:about="Identification">
        <rdfs:label xml:lang="en">Identification</rdfs:label>
        <rdfs:isDefinedBy rdf:resource="http://rs.tdwg.org/abcd/terms/"/>
        <dwcattributes:status>recommended</dwcattributes:status>
        <dcterms:issued>2019-01-31</dcterms:issued>
        <dcterms:modified>2019-01-31</dcterms:modified>
        <rdfs:comment>Class to describe the identification event which assigns a scientific or vernacular name to a Unit.</rdfs:comment>
        <skos:definition>Class to describe the identification event which assigns a scientific or vernacular name to a Unit.</skos:definition>
        <vann:termGroup rdf:resource="Identification"/>
        <skos:exactMatch rdf:resource="http://rs.tdwg.org/dwc/terms/Identification"/>
    </owl:Class>

    <owl:Class rdf:about="IdentifiedTaxon">
        <rdfs:label xml:lang="en">Identified Taxon</rdfs:label>
        <rdfs:isDefinedBy rdf:resource="http://rs.tdwg.org/abcd/terms/"/>
        <dwcattributes:status>recommended</dwcattributes:status>
        <dcterms:issued>2019-01-31</dcterms:issued>
        <dcterms:modified>2019-01-31</dcterms:modified>
        <rdfs:comment>The taxon or taxonon (negative taxon assertion) name assigned to the unit (or excluded, "non") in the identification event.</rdfs:comment>
        <skos:definition>The taxon or taxonon (negative taxon assertion) name assigned to the unit (or excluded, "non") in the identification event.</skos:definition>
        <vann:termGroup rdf:resource="Identification"/>
        <skos:exactMatch rdf:resource="http://rs.tdwg.org/dwc/terms/Taxon"/>
    </owl:Class>

    <owl:Class rdf:about="ImageObject">
        <rdfs:label xml:lang="en">Image Object</rdfs:label>
        <rdfs:isDefinedBy rdf:resource="http://rs.tdwg.org/abcd/terms/"/>
        <dwcattributes:status>recommended</dwcattributes:status>
        <dcterms:issued>2019-01-31</dcterms:issued>
        <dcterms:modified>2019-01-31</dcterms:modified>
        <rdfs:comment>Class to describe an image.</rdfs:comment>
        <skos:definition>Class to describe an image.</skos:definition>
        <rdfs:subClassOf rdf:resource="MultimediaObject"/>
        <vann:termGroup rdf:resource="Multimedia Object"/>
    </owl:Class>

    <owl:Class rdf:about="LegalStatement">
        <rdfs:label xml:lang="en">Legal Statement</rdfs:label>
        <rdfs:isDefinedBy rdf:resource="http://rs.tdwg.org/abcd/terms/"/>
        <dwcattributes:status>recommended</dwcattributes:status>
        <dcterms:issued>2019-01-31</dcterms:issued>
        <dcterms:modified>2019-01-31</dcterms:modified>
        <rdfs:comment>Class to describe a legal statement like copyright, license, terms of use or disclaimer.</rdfs:comment>
        <skos:definition>Class to describe a legal statement like copyright, license, terms of use or disclaimer.</skos:definition>
        <vann:termGroup rdf:resource="General"/>
    </owl:Class>

    <owl:Class rdf:about="LoanRestrictions">
        <rdfs:label xml:lang="en">Loan Restrictions</rdfs:label>
        <rdfs:isDefinedBy rdf:resource="http://rs.tdwg.org/abcd/terms/"/>
        <dwcattributes:status>recommended</dwcattributes:status>
        <dcterms:issued>2019-01-31</dcterms:issued>
        <dcterms:modified>2019-01-31</dcterms:modified>
        <rdfs:comment>Restrictions for accessing or loaning a specimen or sample.</rdfs:comment>
        <skos:definition>Restrictions for accessing or loaning a specimen or sample.</skos:definition>
        <vann:termGroup rdf:resource="Specimen Unit"/>
    </owl:Class>

    <owl:Class rdf:about="Mark">
        <rdfs:label xml:lang="en">Mark</rdfs:label>
        <rdfs:isDefinedBy rdf:resource="http://rs.tdwg.org/abcd/terms/"/>
        <dwcattributes:status>recommended</dwcattributes:status>
        <dcterms:issued>2019-01-31</dcterms:issued>
        <dcterms:modified>2019-01-31</dcterms:modified>
        <rdfs:comment>Label text(s), writing, or inscriptions associated with the unit.</rdfs:comment>
        <skos:definition>Label text(s), writing, or inscriptions associated with the unit.</skos:definition>
        <vann:termGroup rdf:resource="Specimen Unit"/>
    </owl:Class>

    <owl:Class rdf:about="MeasurementOrFact">
        <rdfs:label xml:lang="en">Measurement Or Fact</rdfs:label>
        <rdfs:isDefinedBy rdf:resource="http://rs.tdwg.org/abcd/terms/"/>
        <dwcattributes:status>recommended</dwcattributes:status>
        <dcterms:issued>2019-01-31</dcterms:issued>
        <dcterms:modified>2019-01-31</dcterms:modified>
        <rdfs:comment>A class to describe a quantitative or categorical measurement.</rdfs:comment>
        <skos:definition>A class to describe a quantitative or categorical measurement.</skos:definition>
        <vann:termGroup rdf:resource="Measurement Or Fact"/>
        <skos:exactMatch rdf:resource="http://rs.tdwg.org/dwc/terms/MeasurementOrFact"/>
    </owl:Class>

    <owl:Class rdf:about="MultimediaObject">
        <rdfs:label xml:lang="en">Multimedia Object</rdfs:label>
        <rdfs:isDefinedBy rdf:resource="http://rs.tdwg.org/abcd/terms/"/>
        <dwcattributes:status>recommended</dwcattributes:status>
        <dcterms:issued>2019-01-31</dcterms:issued>
        <dcterms:modified>2019-01-31</dcterms:modified>
        <rdfs:comment>Class to describe digital images, sound recordings, etc.</rdfs:comment>
        <skos:definition>Class to describe digital images, sound recordings, etc.</skos:definition>
        <vann:termGroup rdf:resource="Multimedia Object"/>
    </owl:Class>

    <owl:Class rdf:about="MycologicalUnit">
        <rdfs:label xml:lang="en">Mycological Unit</rdfs:label>
        <rdfs:isDefinedBy rdf:resource="http://rs.tdwg.org/abcd/terms/"/>
        <dwcattributes:status>recommended</dwcattributes:status>
        <dcterms:issued>2019-01-31</dcterms:issued>
        <dcterms:modified>2019-01-31</dcterms:modified>
        <rdfs:comment>Elements only used for mycological units.</rdfs:comment>
        <skos:definition>Elements only used for mycological units.</skos:definition>
        <rdfs:subClassOf rdf:resource="TypeSpecificInformation"/>
        <vann:termGroup rdf:resource="Unit Type Classes"/>
    </owl:Class>

    <owl:Class rdf:about="NamedArea">
        <rdfs:label xml:lang="en">Named Area</rdfs:label>
        <rdfs:isDefinedBy rdf:resource="http://rs.tdwg.org/abcd/terms/"/>
        <dwcattributes:status>recommended</dwcattributes:status>
        <dcterms:issued>2019-01-31</dcterms:issued>
        <dcterms:modified>2019-01-31</dcterms:modified>
        <rdfs:comment>An atomized place name (an administrative or geoecological area) with possibility for hierarchical structuring.</rdfs:comment>
        <skos:definition>An atomized place name (an administrative or geoecological area) with possibility for hierarchical structuring.</skos:definition>
        <vann:termGroup rdf:resource="Gathering"/>
    </owl:Class>

    <owl:Class rdf:about="NamedPlaceRelation">
        <rdfs:label xml:lang="en">Named Place Relation</rdfs:label>
        <rdfs:isDefinedBy rdf:resource="http://rs.tdwg.org/abcd/terms/"/>
        <dwcattributes:status>recommended</dwcattributes:status>
        <dcterms:issued>2019-01-31</dcterms:issued>
        <dcterms:modified>2019-01-31</dcterms:modified>
        <rdfs:comment>The relationship of a location to a different place.</rdfs:comment>
        <skos:definition>The relationship of a location to a different place.</skos:definition>
        <vann:termGroup rdf:resource="Gathering"/>
    </owl:Class>

    <owl:Class rdf:about="NomenclaturalTypeDesignation">
        <rdfs:label xml:lang="en">Nomenclatural Type Designation</rdfs:label>
        <rdfs:isDefinedBy rdf:resource="http://rs.tdwg.org/abcd/terms/"/>
        <dwcattributes:status>recommended</dwcattributes:status>
        <dcterms:issued>2019-01-31</dcterms:issued>
        <dcterms:modified>2019-01-31</dcterms:modified>
        <rdfs:comment>Information on the type status of the specimen.</rdfs:comment>
        <skos:definition>Information on the type status of the specimen.</skos:definition>
        <vann:termGroup rdf:resource="Specimen Unit"/>
    </owl:Class>

    <owl:Class rdf:about="NomenclatureCode">
        <rdfs:label xml:lang="en">Nomenclature Code</rdfs:label>
        <rdfs:isDefinedBy rdf:resource="http://rs.tdwg.org/abcd/terms/"/>
        <dwcattributes:status>recommended</dwcattributes:status>
        <dcterms:issued>2019-01-31</dcterms:issued>
        <dcterms:modified>2019-01-31</dcterms:modified>
        <rdfs:comment>Code of nomenclature for Scientific Names that are the result of an Identification.</rdfs:comment>
        <skos:definition>Code of nomenclature for Scientific Names that are the result of an Identification.</skos:definition>
        <vann:termGroup rdf:resource="Identification"/>
    </owl:Class>

    <owl:Class rdf:about="ObservationUnit">
        <rdfs:label xml:lang="en">Observation Unit</rdfs:label>
        <rdfs:isDefinedBy rdf:resource="http://rs.tdwg.org/abcd/terms/"/>
        <dwcattributes:status>recommended</dwcattributes:status>
        <dcterms:issued>2019-01-31</dcterms:issued>
        <dcterms:modified>2019-01-31</dcterms:modified>
        <rdfs:comment>Data elements specific to observation (recording) units.</rdfs:comment>
        <skos:definition>Data elements specific to observation (recording) units.</skos:definition>
        <rdfs:subClassOf rdf:resource="TypeSpecificInformation"/>
        <vann:termGroup rdf:resource="Unit Type Classes"/>
    </owl:Class>

    <owl:Class rdf:about="Organization">
        <rdfs:label xml:lang="en">Organization</rdfs:label>
        <rdfs:isDefinedBy rdf:resource="http://rs.tdwg.org/abcd/terms/"/>
        <dwcattributes:status>recommended</dwcattributes:status>
        <dcterms:issued>2019-01-31</dcterms:issued>
        <dcterms:modified>2019-01-31</dcterms:modified>
        <rdfs:comment>Class to describe an organization.</rdfs:comment>
        <skos:definition>Class to describe an organization.</skos:definition>
        <rdfs:subClassOf rdf:resource="Contact"/>
        <vann:termGroup rdf:resource="Contact"/>
        <skos:exactMatch rdf:resource="http://xmlns.com/foaf/0.1/Organization"/>
    </owl:Class>

    <owl:Class rdf:about="PaleontologicalUnit">
        <rdfs:label xml:lang="en">Paleontological Unit</rdfs:label>
        <rdfs:isDefinedBy rdf:resource="http://rs.tdwg.org/abcd/terms/"/>
        <dwcattributes:status>recommended</dwcattributes:status>
        <dcterms:issued>2019-01-31</dcterms:issued>
        <dcterms:modified>2019-01-31</dcterms:modified>
        <rdfs:comment>Data specific to paleontological units.</rdfs:comment>
        <skos:definition>Data specific to paleontological units.</skos:definition>
        <rdfs:subClassOf rdf:resource="TypeSpecificInformation"/>
        <vann:termGroup rdf:resource="Unit Type Classes"/>
    </owl:Class>

    <owl:Class rdf:about="Permit">
        <rdfs:label xml:lang="en">Permit</rdfs:label>
        <rdfs:isDefinedBy rdf:resource="http://rs.tdwg.org/abcd/terms/"/>
        <dwcattributes:status>recommended</dwcattributes:status>
        <dcterms:issued>2019-01-31</dcterms:issued>
        <dcterms:modified>2019-01-31</dcterms:modified>
        <rdfs:comment>A class for information regarding acquired permits for specific actions which would not be allowed otherwise.</rdfs:comment>
        <skos:definition>A class for information regarding acquired permits for specific actions which would not be allowed otherwise.</skos:definition>
        <vann:termGroup rdf:resource="Gathering"/>
    </owl:Class>

    <owl:Class rdf:about="PermitStatus">
        <rdfs:label xml:lang="en">Permit Status</rdfs:label>
        <rdfs:isDefinedBy rdf:resource="http://rs.tdwg.org/abcd/terms/"/>
        <dwcattributes:status>recommended</dwcattributes:status>
        <dcterms:issued>2019-01-31</dcterms:issued>
        <dcterms:modified>2019-01-31</dcterms:modified>
        <rdfs:comment>Information about the presence, absence or other basic status of Permits associated with the sample(s). Material collected after 2014-10-12 cannot be in "Unknown" Permit Status!</rdfs:comment>
        <skos:definition>Information about the presence, absence or other basic status of Permits associated with the sample(s). Material collected after 2014-10-12 cannot be in "Unknown" Permit Status!</skos:definition>
        <vann:termGroup rdf:resource="Gathering"/>
    </owl:Class>

    <owl:Class rdf:about="PermitType">
        <rdfs:label xml:lang="en">Permit Type</rdfs:label>
        <rdfs:isDefinedBy rdf:resource="http://rs.tdwg.org/abcd/terms/"/>
        <dwcattributes:status>recommended</dwcattributes:status>
        <dcterms:issued>2019-01-31</dcterms:issued>
        <dcterms:modified>2019-01-31</dcterms:modified>
        <rdfs:comment>Description of a permit type.</rdfs:comment>
        <skos:definition>Description of a permit type.</skos:definition>
        <vann:termGroup rdf:resource="Gathering"/>
    </owl:Class>

    <owl:Class rdf:about="Person">
        <rdfs:label xml:lang="en">Person</rdfs:label>
        <rdfs:isDefinedBy rdf:resource="http://rs.tdwg.org/abcd/terms/"/>
        <dwcattributes:status>recommended</dwcattributes:status>
        <dcterms:issued>2019-01-31</dcterms:issued>
        <dcterms:modified>2019-01-31</dcterms:modified>
        <rdfs:comment>Class to describe a natural Person.</rdfs:comment>
        <skos:definition>Class to describe a natural Person.</skos:definition>
        <rdfs:subClassOf rdf:resource="Contact"/>
        <vann:termGroup rdf:resource="Contact"/>
        <skos:exactMatch rdf:resource="http://xmlns.com/foaf/0.1/Person"/>
    </owl:Class>

    <owl:Class rdf:about="PlantGeneticResourcesUnit">
        <rdfs:label xml:lang="en">Plant Genetic Resources Unit</rdfs:label>
        <rdfs:isDefinedBy rdf:resource="http://rs.tdwg.org/abcd/terms/"/>
        <dwcattributes:status>recommended</dwcattributes:status>
        <dcterms:issued>2019-01-31</dcterms:issued>
        <dcterms:modified>2019-01-31</dcterms:modified>
        <rdfs:comment>Class for elements only used in plant genetic resource collections. Currently, all elements represent EURISCO descriptors.</rdfs:comment>
        <skos:definition>Class for elements only used in plant genetic resource collections. Currently, all elements represent EURISCO descriptors.</skos:definition>
        <rdfs:subClassOf rdf:resource="TypeSpecificInformation"/>
        <vann:termGroup rdf:resource="Unit Type Classes"/>
    </owl:Class>

    <owl:Class rdf:about="Preparation">
        <rdfs:label xml:lang="en">Preparation</rdfs:label>
        <rdfs:isDefinedBy rdf:resource="http://rs.tdwg.org/abcd/terms/"/>
        <dwcattributes:status>recommended</dwcattributes:status>
        <dcterms:issued>2019-01-31</dcterms:issued>
        <dcterms:modified>2019-01-31</dcterms:modified>
        <rdfs:comment>The specimen preparation details.</rdfs:comment>
        <skos:definition>The specimen preparation details.</skos:definition>
        <vann:termGroup rdf:resource="Specimen Unit"/>
    </owl:Class>

    <owl:Class rdf:about="Preservation">
        <rdfs:label xml:lang="en">Preservation</rdfs:label>
        <rdfs:isDefinedBy rdf:resource="http://rs.tdwg.org/abcd/terms/"/>
        <dwcattributes:status>recommended</dwcattributes:status>
        <dcterms:issued>2019-01-31</dcterms:issued>
        <dcterms:modified>2019-01-31</dcterms:modified>
        <rdfs:comment>A description of the preservation of a specimen.</rdfs:comment>
        <skos:definition>A description of the preservation of a specimen.</skos:definition>
        <vann:termGroup rdf:resource="Specimen Unit"/>
    </owl:Class>

    <owl:Class rdf:about="PreviousUnit">
        <rdfs:label xml:lang="en">Previous Unit</rdfs:label>
        <rdfs:isDefinedBy rdf:resource="http://rs.tdwg.org/abcd/terms/"/>
        <dwcattributes:status>recommended</dwcattributes:status>
        <dcterms:issued>2019-01-31</dcterms:issued>
        <dcterms:modified>2019-01-31</dcterms:modified>
        <rdfs:comment>A container for past identifiers and locations for this specimen.</rdfs:comment>
        <skos:definition>A container for past identifiers and locations for this specimen.</skos:definition>
        <vann:termGroup rdf:resource="Specimen Unit"/>
    </owl:Class>

    <owl:Class rdf:about="Project">
        <rdfs:label xml:lang="en">Project</rdfs:label>
        <rdfs:isDefinedBy rdf:resource="http://rs.tdwg.org/abcd/terms/"/>
        <dwcattributes:status>recommended</dwcattributes:status>
        <dcterms:issued>2019-01-31</dcterms:issued>
        <dcterms:modified>2019-01-31</dcterms:modified>
        <rdfs:comment>Class to describe a project.</rdfs:comment>
        <skos:definition>Class to describe a project.</skos:definition>
        <vann:termGroup rdf:resource="Gathering"/>
    </owl:Class>

    <owl:Class rdf:about="RecordBasis">
        <rdfs:label xml:lang="en">Record Basis</rdfs:label>
        <rdfs:isDefinedBy rdf:resource="http://rs.tdwg.org/abcd/terms/"/>
        <dwcattributes:status>recommended</dwcattributes:status>
        <dcterms:issued>2019-01-31</dcterms:issued>
        <dcterms:modified>2019-01-31</dcterms:modified>
        <rdfs:comment>A standard designator for the nature of the object of the record.</rdfs:comment>
        <skos:definition>A standard designator for the nature of the object of the record.</skos:definition>
        <vann:termGroup rdf:resource="Unit"/>
        <skos:exactMatch rdf:resource="http://rs.tdwg.org/dwc/terms/basisOfRecord"/>
    </owl:Class>

    <owl:Class rdf:about="Reference">
        <rdfs:label xml:lang="en">Reference</rdfs:label>
        <rdfs:isDefinedBy rdf:resource="http://rs.tdwg.org/abcd/terms/"/>
        <dwcattributes:status>recommended</dwcattributes:status>
        <dcterms:issued>2019-01-31</dcterms:issued>
        <dcterms:modified>2019-01-31</dcterms:modified>
        <rdfs:comment>A class to describe a scientific reference or citation.</rdfs:comment>
        <skos:definition>A class to describe a scientific reference or citation.</skos:definition>
        <vann:termGroup rdf:resource="General"/>
        <skos:relatedMatch rdf:resource="http://purl.org/dc/terms/references"/>
    </owl:Class>

    <owl:Class rdf:about="ScientificName">
        <rdfs:label xml:lang="en">Scientific Name</rdfs:label>
        <rdfs:isDefinedBy rdf:resource="http://rs.tdwg.org/abcd/terms/"/>
        <dwcattributes:status>recommended</dwcattributes:status>
        <dcterms:issued>2019-01-31</dcterms:issued>
        <dcterms:modified>2019-01-31</dcterms:modified>
        <rdfs:comment>The name of an Identified Taxon. Formed according to the different codes of nomenclature which apply to scientific names.</rdfs:comment>
        <skos:definition>The name of an Identified Taxon. Formed according to the different codes of nomenclature which apply to scientific names.</skos:definition>
        <vann:termGroup rdf:resource="Identification"/>
    </owl:Class>

    <owl:Class rdf:about="Sequence">
        <rdfs:label xml:lang="en">Sequence</rdfs:label>
        <rdfs:isDefinedBy rdf:resource="http://rs.tdwg.org/abcd/terms/"/>
        <dwcattributes:status>recommended</dwcattributes:status>
        <dcterms:issued>2019-01-31</dcterms:issued>
        <dcterms:modified>2019-01-31</dcterms:modified>
        <rdfs:comment>A genomic sequence.</rdfs:comment>
        <skos:definition>A genomic sequence.</skos:definition>
        <vann:termGroup rdf:resource="Unit"/>
    </owl:Class>

    <owl:Class rdf:about="Sex">
        <rdfs:label xml:lang="en">Sex</rdfs:label>
        <rdfs:isDefinedBy rdf:resource="http://rs.tdwg.org/abcd/terms/"/>
        <dwcattributes:status>recommended</dwcattributes:status>
        <dcterms:issued>2019-01-31</dcterms:issued>
        <dcterms:modified>2019-01-31</dcterms:modified>
        <rdfs:comment>The sex of an organism.</rdfs:comment>
        <skos:definition>The sex of an organism.</skos:definition>
        <vann:termGroup rdf:resource="Unit"/>
        <skos:exactMatch rdf:resource="http://rs.tdwg.org/dwc/terms/sex"/>
    </owl:Class>

    <owl:Class rdf:about="SpecimenUnit">
        <rdfs:label xml:lang="en">Specimen Unit</rdfs:label>
        <rdfs:isDefinedBy rdf:resource="http://rs.tdwg.org/abcd/terms/"/>
        <dwcattributes:status>recommended</dwcattributes:status>
        <dcterms:issued>2019-01-31</dcterms:issued>
        <dcterms:modified>2019-01-31</dcterms:modified>
        <rdfs:comment>Class to contain data elements specific to physical specimens (living, fossil, or preserved).</rdfs:comment>
        <skos:definition>Class to contain data elements specific to physical specimens (living, fossil, or preserved).</skos:definition>
        <rdfs:subClassOf rdf:resource="TypeSpecificInformation"/>
        <vann:termGroup rdf:resource="Unit Type Classes"/>
        <vann:termGroup rdf:resource="Specimen Unit"/>
    </owl:Class>

    <owl:Class rdf:about="StratigraphicTerm">
        <rdfs:label xml:lang="en">Stratigraphic Term</rdfs:label>
        <rdfs:isDefinedBy rdf:resource="http://rs.tdwg.org/abcd/terms/"/>
        <dwcattributes:status>recommended</dwcattributes:status>
        <dcterms:issued>2019-01-31</dcterms:issued>
        <dcterms:modified>2019-01-31</dcterms:modified>
        <rdfs:comment>Concept to describe a stratigraphic term.</rdfs:comment>
        <skos:definition>Concept to describe a stratigraphic term.</skos:definition>
        <vann:termGroup rdf:resource="Unit Type Classes"/>
    </owl:Class>

    <owl:Class rdf:about="Synecology">
        <rdfs:label xml:lang="en">Synecology</rdfs:label>
        <rdfs:isDefinedBy rdf:resource="http://rs.tdwg.org/abcd/terms/"/>
        <dwcattributes:status>recommended</dwcattributes:status>
        <dcterms:issued>2019-01-31</dcterms:issued>
        <dcterms:modified>2019-01-31</dcterms:modified>
        <rdfs:comment>The relationship of a Unit gathered with other taxa at the gathering site.</rdfs:comment>
        <skos:definition>The relationship of a Unit gathered with other taxa at the gathering site.</skos:definition>
        <vann:termGroup rdf:resource="Gathering"/>
        <dc:description>Note that this relationship can be recorded as a feature of the location (e.g. a syntaxon, or certain species known to grow together at the site). It can also be used to record an observed relationship (e.g. caterpillar and observed food plant, parasite and host etc.), but this would be better expressed as abcd:Association of the Unit.</dc:description>
    </owl:Class>

    <owl:Class rdf:about="Temperature">
        <rdfs:label xml:lang="en">Temperature</rdfs:label>
        <rdfs:isDefinedBy rdf:resource="http://rs.tdwg.org/abcd/terms/"/>
        <dwcattributes:status>recommended</dwcattributes:status>
        <dcterms:issued>2019-01-31</dcterms:issued>
        <dcterms:modified>2019-01-31</dcterms:modified>
        <rdfs:comment>Concept for a temperature.</rdfs:comment>
        <skos:definition>Concept for a temperature.</skos:definition>
        <vann:termGroup rdf:resource="Unit Type Classes"/>
    </owl:Class>

    <owl:Class rdf:about="temperatureScale">
        <rdfs:label xml:lang="en">Temperature Scale</rdfs:label>
        <rdfs:isDefinedBy rdf:resource="http://rs.tdwg.org/abcd/terms/"/>
        <dwcattributes:status>recommended</dwcattributes:status>
        <dcterms:issued>2019-01-31</dcterms:issued>
        <dcterms:modified>2019-01-31</dcterms:modified>
        <rdfs:comment>The type of temperature scale used for preservation (Celsius or Fahrenheit).</rdfs:comment>
        <skos:definition>The type of temperature scale used for preservation (Celsius or Fahrenheit).</skos:definition>
        <vann:termGroup rdf:resource="Unit Type Classes"/>
    </owl:Class>

    <owl:Class rdf:about="TypeSpecificInformation">
        <rdfs:label xml:lang="en">Type Specific Information</rdfs:label>
        <rdfs:isDefinedBy rdf:resource="http://rs.tdwg.org/abcd/terms/"/>
        <dwcattributes:status>recommended</dwcattributes:status>
        <dcterms:issued>2019-01-31</dcterms:issued>
        <dcterms:modified>2019-01-31</dcterms:modified>
        <rdfs:comment>A super class to create and link to type specific information about a unit.</rdfs:comment>
        <skos:definition>A super class to create and link to type specific information about a unit.</skos:definition>
        <vann:termGroup rdf:resource="Unit"/>
    </owl:Class>

    <owl:Class rdf:about="Unit">
        <rdfs:label xml:lang="en">Unit</rdfs:label>
        <rdfs:isDefinedBy rdf:resource="http://rs.tdwg.org/abcd/terms/"/>
        <dwcattributes:status>recommended</dwcattributes:status>
        <dcterms:issued>2019-01-31</dcterms:issued>
        <dcterms:modified>2019-01-31</dcterms:modified>
        <rdfs:comment>A class to join all data referring to a unit such as specimen or observation record.</rdfs:comment>
        <skos:definition>A class to join all data referring to a unit such as specimen or observation record.</skos:definition>
        <vann:termGroup rdf:resource="Unit"/>
    </owl:Class>

    <owl:Class rdf:about="Version">
        <rdfs:label xml:lang="en">Version</rdfs:label>
        <rdfs:isDefinedBy rdf:resource="http://rs.tdwg.org/abcd/terms/"/>
        <dwcattributes:status>recommended</dwcattributes:status>
        <dcterms:issued>2019-01-31</dcterms:issued>
        <dcterms:modified>2019-01-31</dcterms:modified>
        <rdfs:comment>The number and date of the current version of a class.</rdfs:comment>
        <skos:definition>The number and date of the current version of a class.</skos:definition>
        <vann:termGroup rdf:resource="General"/>
    </owl:Class>

    <owl:Class rdf:about="VideoObject">
        <rdfs:label xml:lang="en">Video Object</rdfs:label>
        <rdfs:isDefinedBy rdf:resource="http://rs.tdwg.org/abcd/terms/"/>
        <dwcattributes:status>recommended</dwcattributes:status>
        <dcterms:issued>2019-01-31</dcterms:issued>
        <dcterms:modified>2019-01-31</dcterms:modified>
        <rdfs:comment>Concept to bundle information about a video object.</rdfs:comment>
        <skos:definition>Concept to bundle information about a video object.</skos:definition>
        <rdfs:subClassOf rdf:resource="MultimediaObject"/>
        <vann:termGroup rdf:resource="Multimedia Object"/>
    </owl:Class>

    <owl:Class rdf:about="ViralScientificName">
        <rdfs:label xml:lang="en">Viral Scientific Name</rdfs:label>
        <rdfs:isDefinedBy rdf:resource="http://rs.tdwg.org/abcd/terms/"/>
        <dwcattributes:status>recommended</dwcattributes:status>
        <dcterms:issued>2019-01-31</dcterms:issued>
        <dcterms:modified>2019-01-31</dcterms:modified>
        <rdfs:comment>Atomized viral name formed in the unit identification, with elements according to the International Committee on Taxonomy of Viruses.</rdfs:comment>
        <skos:definition>Atomized viral name formed in the unit identification, with elements according to the International Committee on Taxonomy of Viruses.</skos:definition>
        <rdfs:subClassOf rdf:resource="ScientificName"/>
        <vann:termGroup rdf:resource="Identification"/>
    </owl:Class>

    <owl:Class rdf:about="ZoologicalScientificName">
        <rdfs:label xml:lang="en">Zoological Scientific Name</rdfs:label>
        <rdfs:isDefinedBy rdf:resource="http://rs.tdwg.org/abcd/terms/"/>
        <dwcattributes:status>recommended</dwcattributes:status>
        <dcterms:issued>2019-01-31</dcterms:issued>
        <dcterms:modified>2019-01-31</dcterms:modified>
        <rdfs:comment>Atomized zoological name formed in the unit identification with elements according to the International Code of Zoological Nomenclature.</rdfs:comment>
        <skos:definition>Atomized zoological name formed in the unit identification with elements according to the International Code of Zoological Nomenclature.</skos:definition>
        <rdfs:subClassOf rdf:resource="ScientificName"/>
        <vann:termGroup rdf:resource="Identification"/>
    </owl:Class>

    <owl:Class rdf:about="ZoologicalUnit">
        <rdfs:label xml:lang="en">Zoological Unit</rdfs:label>
        <rdfs:isDefinedBy rdf:resource="http://rs.tdwg.org/abcd/terms/"/>
        <dwcattributes:status>recommended</dwcattributes:status>
        <dcterms:issued>2019-01-31</dcterms:issued>
        <dcterms:modified>2019-01-31</dcterms:modified>
        <rdfs:comment>Data specific to zoological units.</rdfs:comment>
        <skos:definition>Data specific to zoological units.</skos:definition>
        <rdfs:subClassOf rdf:resource="TypeSpecificInformation"/>
        <vann:termGroup rdf:resource="Unit Type Classes"/>
    </owl:Class>

    <owl:DatatypeProperty rdf:about="abbreviation">
        <rdfs:label xml:lang="en">Abbreviation</rdfs:label>
        <rdfs:isDefinedBy rdf:resource="http://rs.tdwg.org/abcd/terms/"/>
        <dwcattributes:status>recommended</dwcattributes:status>
        <dcterms:issued>2019-01-31</dcterms:issued>
        <dcterms:modified>2019-01-31</dcterms:modified>
        <rdfs:comment>A common abbreviation for the name or label of a class.</rdfs:comment>
        <skos:definition>A common abbreviation for the name or label of a class.</skos:definition>
        <rdfs:domain rdf:resource="http://www.w3.org/2002/07/owl#Thing"/>
        <rdfs:range rdf:resource="http://www.w3.org/2001/XMLSchema#string"/>
    </owl:DatatypeProperty>

    <owl:DatatypeProperty rdf:about="accessionCatalogue">
        <rdfs:label xml:lang="en">Accession Catalogue</rdfs:label>
        <rdfs:isDefinedBy rdf:resource="http://rs.tdwg.org/abcd/terms/"/>
        <dwcattributes:status>recommended</dwcattributes:status>
        <dcterms:issued>2019-01-31</dcterms:issued>
        <dcterms:modified>2019-01-31</dcterms:modified>
        <rdfs:comment>Identifier of an accessions catalogue or numbering scheme which contains the SpecimenUnit</rdfs:comment>
        <skos:definition>Identifier of an accessions catalogue or numbering scheme which contains the SpecimenUnit</skos:definition>
        <rdfs:domain rdf:resource="http://www.w3.org/2002/07/owl#Thing"/>
        <rdfs:range rdf:resource="http://www.w3.org/2001/XMLSchema#string"/>
    </owl:DatatypeProperty>

    <owl:FunctionalProperty rdf:about="accessionCatalogue"/>

    <owl:DatatypeProperty rdf:about="accessionLineage">
        <rdfs:label xml:lang="en">Accession Lineage</rdfs:label>
        <rdfs:isDefinedBy rdf:resource="http://rs.tdwg.org/abcd/terms/"/>
        <dwcattributes:status>recommended</dwcattributes:status>
        <dcterms:issued>2019-01-31</dcterms:issued>
        <dcterms:modified>2019-01-31</dcterms:modified>
        <rdfs:comment>The purpose of this property is to trace the lineage of an accession to either one or two immediate parent unit ID's.</rdfs:comment>
        <skos:definition>The purpose of this property is to trace the lineage of an accession to either one or two immediate parent unit ID's.</skos:definition>
        <dc:description>The Unit IDs are preceded by the garden code (Heywood and Heywood).</dc:description>
        <rdfs:domain rdf:resource="http://www.w3.org/2002/07/owl#Thing"/>
        <rdfs:range rdf:resource="http://www.w3.org/2001/XMLSchema#string"/>
    </owl:DatatypeProperty>

    <owl:FunctionalProperty rdf:about="accessionLineage"/>

    <owl:DatatypeProperty rdf:about="accessionMaterialType">
        <rdfs:label xml:lang="en">Accession Material Type</rdfs:label>
        <rdfs:isDefinedBy rdf:resource="http://rs.tdwg.org/abcd/terms/"/>
        <dwcattributes:status>recommended</dwcattributes:status>
        <dcterms:issued>2019-01-31</dcterms:issued>
        <dcterms:modified>2019-01-31</dcterms:modified>
        <rdfs:comment>The type of material the current living accession is composed of.</rdfs:comment>
        <skos:definition>The type of material the current living accession is composed of.</skos:definition>
        <rdfs:domain rdf:resource="http://www.w3.org/2002/07/owl#Thing"/>
        <rdfs:range rdf:resource="http://www.w3.org/2001/XMLSchema#string"/>
    </owl:DatatypeProperty>

    <owl:FunctionalProperty rdf:about="accessionMaterialType"/>

    <owl:DatatypeProperty rdf:about="accessionName">
        <rdfs:label xml:lang="en">Accession Name</rdfs:label>
        <rdfs:isDefinedBy rdf:resource="http://rs.tdwg.org/abcd/terms/"/>
        <dwcattributes:status>recommended</dwcattributes:status>
        <dcterms:issued>2019-01-31</dcterms:issued>
        <dcterms:modified>2019-01-31</dcterms:modified>
        <rdfs:comment>A name given to the accession that cannot be covered by abcd:BotanicalScientificName (i.e. not a formal cultivar or trade designation name).</rdfs:comment>
        <skos:definition>A name given to the accession that cannot be covered by abcd:BotanicalScientificName (i.e. not a formal cultivar or trade designation name).</skos:definition>
        <rdfs:domain rdf:resource="http://www.w3.org/2002/07/owl#Thing"/>
        <rdfs:range rdf:resource="http://www.w3.org/2001/XMLSchema#string"/>
    </owl:DatatypeProperty>

    <owl:DatatypeProperty rdf:about="accessionNameText">
        <rdfs:label xml:lang="en">Accession Name Text</rdfs:label>
        <rdfs:isDefinedBy rdf:resource="http://rs.tdwg.org/abcd/terms/"/>
        <dwcattributes:status>recommended</dwcattributes:status>
        <dcterms:issued>2019-01-31</dcterms:issued>
        <dcterms:modified>2019-01-31</dcterms:modified>
        <rdfs:comment>Alternative concatenated representation for Accession Names.</rdfs:comment>
        <skos:definition>Alternative concatenated representation for Accession Names.</skos:definition>
        <rdfs:domain rdf:resource="http://www.w3.org/2002/07/owl#Thing"/>
        <rdfs:range rdf:resource="http://www.w3.org/2001/XMLSchema#string"/>
    </owl:DatatypeProperty>

    <owl:FunctionalProperty rdf:about="accessionNameText"/>

    <owl:DatatypeProperty rdf:about="accessionNumber">
        <rdfs:label xml:lang="en">Accession Number</rdfs:label>
        <rdfs:isDefinedBy rdf:resource="http://rs.tdwg.org/abcd/terms/"/>
        <dwcattributes:status>recommended</dwcattributes:status>
        <dcterms:issued>2019-01-31</dcterms:issued>
        <dcterms:modified>2019-01-31</dcterms:modified>
        <rdfs:comment>The institutional number applied to the accession and recorded in the accessions register.</rdfs:comment>
        <skos:definition>The institutional number applied to the accession and recorded in the accessions register.</skos:definition>
        <rdfs:domain rdf:resource="http://www.w3.org/2002/07/owl#Thing"/>
        <rdfs:range rdf:resource="http://www.w3.org/2001/XMLSchema#string"/>
    </owl:DatatypeProperty>

    <owl:FunctionalProperty rdf:about="accessionNumber"/>

    <owl:DatatypeProperty rdf:about="accessionSpecimenNumbers">
        <rdfs:label xml:lang="en">Accession Specimen Numbers</rdfs:label>
        <rdfs:isDefinedBy rdf:resource="http://rs.tdwg.org/abcd/terms/"/>
        <dwcattributes:status>recommended</dwcattributes:status>
        <dcterms:issued>2019-01-31</dcterms:issued>
        <dcterms:modified>2019-01-31</dcterms:modified>
        <rdfs:comment>The minimum numbers of individuals the garden is holding under the UnitID.</rdfs:comment>
        <skos:definition>The minimum numbers of individuals the garden is holding under the UnitID.</skos:definition>
        <dc:description>Accession status must not be D (dead).</dc:description>
        <rdfs:domain rdf:resource="http://www.w3.org/2002/07/owl#Thing"/>
        <rdfs:range rdf:resource="http://www.w3.org/2001/XMLSchema#integer"/>
    </owl:DatatypeProperty>

    <owl:FunctionalProperty rdf:about="accessionSpecimenNumbers"/>

    <owl:DatatypeProperty rdf:about="accessionStatus">
        <rdfs:label xml:lang="en">Accession Status</rdfs:label>
        <rdfs:isDefinedBy rdf:resource="http://rs.tdwg.org/abcd/terms/"/>
        <dwcattributes:status>recommended</dwcattributes:status>
        <dcterms:issued>2019-01-31</dcterms:issued>
        <dcterms:modified>2019-01-31</dcterms:modified>
        <rdfs:comment>The current status of the accession in the garden (current or not current).</rdfs:comment>
        <skos:definition>The current status of the accession in the garden (current or not current).</skos:definition>
        <rdfs:domain rdf:resource="http://www.w3.org/2002/07/owl#Thing"/>
        <rdfs:range rdf:resource="http://www.w3.org/2001/XMLSchema#byte"/>
    </owl:DatatypeProperty>

    <owl:FunctionalProperty rdf:about="accessionStatus"/>

    <owl:DatatypeProperty rdf:about="accuracy">
        <rdfs:label xml:lang="en">Accuracy</rdfs:label>
        <rdfs:isDefinedBy rdf:resource="http://rs.tdwg.org/abcd/terms/"/>
        <dwcattributes:status>recommended</dwcattributes:status>
        <dcterms:issued>2019-01-31</dcterms:issued>
        <dcterms:modified>2019-01-31</dcterms:modified>
        <rdfs:comment>A statement of accuracy concerning the measurement.</rdfs:comment>
        <skos:definition>A statement of accuracy concerning the measurement.</skos:definition>
        <dc:description>If the unit of measurement is the same as denoted in abcd:UnitOfMeasurment it should be omitted.</dc:description>
        <rdfs:domain rdf:resource="http://www.w3.org/2002/07/owl#Thing"/>
        <rdfs:range rdf:resource="http://www.w3.org/2001/XMLSchema#string"/>
        <skos:exactMatch rdf:resource="http://rs.tdwg.org/dwc/terms/measurementAccuracy"/>
    </owl:DatatypeProperty>

    <owl:FunctionalProperty rdf:about="accuracy"/>

    <owl:DatatypeProperty rdf:about="acquisitionSourceText">
        <rdfs:label xml:lang="en">Acquisition Source Text</rdfs:label>
        <rdfs:isDefinedBy rdf:resource="http://rs.tdwg.org/abcd/terms/"/>
        <dwcattributes:status>recommended</dwcattributes:status>
        <dcterms:issued>2019-01-31</dcterms:issued>
        <dcterms:modified>2019-01-31</dcterms:modified>
        <rdfs:comment>Free text field for unformatted recording of acquisition source details.</rdfs:comment>
        <skos:definition>Free text field for unformatted recording of acquisition source details.</skos:definition>
        <rdfs:domain rdf:resource="http://www.w3.org/2002/07/owl#Thing"/>
        <rdfs:range rdf:resource="http://www.w3.org/2001/XMLSchema#string"/>
    </owl:DatatypeProperty>

    <owl:FunctionalProperty rdf:about="acquisitionSourceText"/>

    <owl:DatatypeProperty rdf:about="acquisitionType">
        <rdfs:label xml:lang="en">Acquisition Type</rdfs:label>
        <rdfs:isDefinedBy rdf:resource="http://rs.tdwg.org/abcd/terms/"/>
        <dwcattributes:status>recommended</dwcattributes:status>
        <dcterms:issued>2019-01-31</dcterms:issued>
        <dcterms:modified>2019-01-31</dcterms:modified>
        <rdfs:comment>Type of acquisition of specimen.</rdfs:comment>
        <skos:definition>Type of acquisition of specimen.</skos:definition>
        <rdfs:domain rdf:resource="http://www.w3.org/2002/07/owl#Thing"/>
        <rdfs:range rdf:resource="http://www.w3.org/2001/XMLSchema#string"/>
    </owl:DatatypeProperty>

    <owl:FunctionalProperty rdf:about="acquisitionType"/>

    <owl:DatatypeProperty rdf:about="acronym">
        <rdfs:label xml:lang="en">Acronym</rdfs:label>
        <rdfs:isDefinedBy rdf:resource="http://rs.tdwg.org/abcd/terms/"/>
        <dwcattributes:status>recommended</dwcattributes:status>
        <dcterms:issued>2019-01-31</dcterms:issued>
        <dcterms:modified>2019-01-31</dcterms:modified>
        <rdfs:comment>The accepted acronym for the virus.</rdfs:comment>
        <skos:definition>The accepted acronym for the virus.</skos:definition>
        <rdfs:domain rdf:resource="http://www.w3.org/2002/07/owl#Thing"/>
        <rdfs:range rdf:resource="http://www.w3.org/2001/XMLSchema#string"/>
    </owl:DatatypeProperty>

    <owl:FunctionalProperty rdf:about="acronym"/>

    <owl:DatatypeProperty rdf:about="address">
        <rdfs:label xml:lang="en">Address</rdfs:label>
        <rdfs:isDefinedBy rdf:resource="http://rs.tdwg.org/abcd/terms/"/>
        <dwcattributes:status>recommended</dwcattributes:status>
        <dcterms:issued>2019-01-31</dcterms:issued>
        <dcterms:modified>2019-01-31</dcterms:modified>
        <rdfs:comment>A string representing a postal address.</rdfs:comment>
        <skos:definition>A string representing a postal address.</skos:definition>
        <rdfs:domain rdf:resource="http://www.w3.org/2002/07/owl#Thing"/>
        <rdfs:range rdf:resource="http://www.w3.org/2001/XMLSchema#string"/>
    </owl:DatatypeProperty>

    <owl:DatatypeProperty rdf:about="aerobicity">
        <rdfs:label xml:lang="en">Aerobicity</rdfs:label>
        <rdfs:isDefinedBy rdf:resource="http://rs.tdwg.org/abcd/terms/"/>
        <dwcattributes:status>recommended</dwcattributes:status>
        <dcterms:issued>2019-01-31</dcterms:issued>
        <dcterms:modified>2019-01-31</dcterms:modified>
        <rdfs:domain rdf:resource="http://www.w3.org/2002/07/owl#Thing"/>
        <rdfs:range rdf:resource="http://www.w3.org/2001/XMLSchema#string"/>
    </owl:DatatypeProperty>

    <owl:FunctionalProperty rdf:about="aerobicity"/>

    <owl:DatatypeProperty rdf:about="age">
        <rdfs:label xml:lang="en">Age</rdfs:label>
        <rdfs:isDefinedBy rdf:resource="http://rs.tdwg.org/abcd/terms/"/>
        <dwcattributes:status>recommended</dwcattributes:status>
        <dcterms:issued>2019-01-31</dcterms:issued>
        <dcterms:modified>2019-01-31</dcterms:modified>
        <rdfs:comment>The age of the organism at the time of collection or observation.</rdfs:comment>
        <skos:definition>The age of the organism at the time of collection or observation.</skos:definition>
        <dc:description>Note that atomized counts for different age (e.g. "26 years by counting tree rings") classes can be provided in the abcd:MeasurementOrFact class of the Unit.</dc:description>
        <rdfs:domain rdf:resource="http://www.w3.org/2002/07/owl#Thing"/>
        <rdfs:range rdf:resource="http://www.w3.org/2001/XMLSchema#string"/>
    </owl:DatatypeProperty>

    <owl:FunctionalProperty rdf:about="age"/>

    <owl:DatatypeProperty rdf:about="ancestralData">
        <rdfs:label xml:lang="en">Ancestral Data</rdfs:label>
        <rdfs:isDefinedBy rdf:resource="http://rs.tdwg.org/abcd/terms/"/>
        <dwcattributes:status>recommended</dwcattributes:status>
        <dcterms:issued>2019-01-31</dcterms:issued>
        <dcterms:modified>2019-01-31</dcterms:modified>
        <rdfs:comment>Information about either pedigree or other description of ancestral information (i.e. parent variety in case of mutant or selection). [FAO/IPGRI multi-crop passport descriptor (MCPD)]</rdfs:comment>
        <skos:definition>Information about either pedigree or other description of ancestral information (i.e. parent variety in case of mutant or selection). [FAO/IPGRI multi-crop passport descriptor (MCPD)]</skos:definition>
        <rdfs:domain rdf:resource="http://www.w3.org/2002/07/owl#Thing"/>
        <rdfs:range rdf:resource="http://www.w3.org/2001/XMLSchema#string"/>
    </owl:DatatypeProperty>

    <owl:FunctionalProperty rdf:about="ancestralData"/>

    <owl:DatatypeProperty rdf:about="applications">
        <rdfs:label xml:lang="en">Applications</rdfs:label>
        <rdfs:isDefinedBy rdf:resource="http://rs.tdwg.org/abcd/terms/"/>
        <dwcattributes:status>recommended</dwcattributes:status>
        <dcterms:issued>2019-01-31</dcterms:issued>
        <dcterms:modified>2019-01-31</dcterms:modified>
        <rdfs:domain rdf:resource="http://www.w3.org/2002/07/owl#Thing"/>
        <rdfs:range rdf:resource="http://www.w3.org/2001/XMLSchema#string"/>
    </owl:DatatypeProperty>

    <owl:FunctionalProperty rdf:about="applications"/>

    <owl:DatatypeProperty rdf:about="appliesTo">
        <rdfs:label xml:lang="en">Applies To</rdfs:label>
        <rdfs:isDefinedBy rdf:resource="http://rs.tdwg.org/abcd/terms/"/>
        <dwcattributes:status>recommended</dwcattributes:status>
        <dcterms:issued>2019-01-31</dcterms:issued>
        <dcterms:modified>2019-01-31</dcterms:modified>
        <rdfs:comment>Property to specify the actual part of a subject that was measured.</rdfs:comment>
        <skos:definition>Property to specify the actual part of a subject that was measured.</skos:definition>
        <rdfs:domain rdf:resource="http://www.w3.org/2002/07/owl#Thing"/>
        <rdfs:range rdf:resource="http://www.w3.org/2001/XMLSchema#string"/>
    </owl:DatatypeProperty>

    <owl:FunctionalProperty rdf:about="appliesTo"/>

    <owl:DatatypeProperty rdf:about="areaClass">
        <rdfs:label xml:lang="en">Area Class</rdfs:label>
        <rdfs:isDefinedBy rdf:resource="http://rs.tdwg.org/abcd/terms/"/>
        <dwcattributes:status>recommended</dwcattributes:status>
        <dcterms:issued>2019-01-31</dcterms:issued>
        <dcterms:modified>2019-01-31</dcterms:modified>
        <rdfs:comment>Allows the recording of classification categories for the class of the gathering named area (local or national subdivision levels, geomorphological units, protected areas, etc.)</rdfs:comment>
        <skos:definition>Allows the recording of classification categories for the class of the gathering named area (local or national subdivision levels, geomorphological units, protected areas, etc.)</skos:definition>
        <dc:description>These classification categories are often treated as individual elements in other standards.</dc:description>
        <rdfs:domain rdf:resource="http://www.w3.org/2002/07/owl#Thing"/>
        <rdfs:range rdf:resource="http://www.w3.org/2001/XMLSchema#string"/>
        <skos:relatedMatch rdf:resource="http://www.geonames.org/ontology#featureClass"/>
    </owl:DatatypeProperty>

    <owl:FunctionalProperty rdf:about="areaClass"/>

    <owl:DatatypeProperty rdf:about="aspectRatio">
        <rdfs:label xml:lang="en">Aspect Ratio</rdfs:label>
        <rdfs:isDefinedBy rdf:resource="http://rs.tdwg.org/abcd/terms/"/>
        <dwcattributes:status>recommended</dwcattributes:status>
        <dcterms:issued>2019-01-31</dcterms:issued>
        <dcterms:modified>2019-01-31</dcterms:modified>
        <rdfs:comment>The ratio of the frame dimensions expressed as a fraction of width and height.</rdfs:comment>
        <skos:definition>The ratio of the frame dimensions expressed as a fraction of width and height.</skos:definition>
        <rdfs:domain rdf:resource="http://www.w3.org/2002/07/owl#Thing"/>
        <rdfs:range rdf:resource="http://www.w3.org/2001/XMLSchema#string"/>
    </owl:DatatypeProperty>

    <owl:FunctionalProperty rdf:about="aspectRatio"/>

    <owl:DatatypeProperty rdf:about="associationType">
        <rdfs:label xml:lang="en">Association Type</rdfs:label>
        <rdfs:isDefinedBy rdf:resource="http://rs.tdwg.org/abcd/terms/"/>
        <dwcattributes:status>recommended</dwcattributes:status>
        <dcterms:issued>2019-01-31</dcterms:issued>
        <dcterms:modified>2019-01-31</dcterms:modified>
        <rdfs:comment>Description of the type of association which the associated Unit has to a Unit.</rdfs:comment>
        <skos:definition>Description of the type of association which the associated Unit has to a Unit.</skos:definition>
        <rdfs:domain rdf:resource="http://www.w3.org/2002/07/owl#Thing"/>
        <rdfs:range rdf:resource="http://www.w3.org/2001/XMLSchema#string"/>
    </owl:DatatypeProperty>

    <owl:FunctionalProperty rdf:about="associationType"/>

    <owl:DatatypeProperty rdf:about="audioBitrate">
        <rdfs:label xml:lang="en">Audio Bitrate</rdfs:label>
        <rdfs:isDefinedBy rdf:resource="http://rs.tdwg.org/abcd/terms/"/>
        <dwcattributes:status>recommended</dwcattributes:status>
        <dcterms:issued>2019-01-31</dcterms:issued>
        <dcterms:modified>2019-01-31</dcterms:modified>
        <rdfs:comment>The bit rate of the audio stream, usually expressed in kBit/s.</rdfs:comment>
        <skos:definition>The bit rate of the audio stream, usually expressed in kBit/s.</skos:definition>
        <rdfs:domain rdf:resource="http://www.w3.org/2002/07/owl#Thing"/>
        <rdfs:range rdf:resource="http://www.w3.org/2001/XMLSchema#string"/>
    </owl:DatatypeProperty>

    <owl:FunctionalProperty rdf:about="audioBitrate"/>

    <owl:DatatypeProperty rdf:about="audioChannel">
        <rdfs:label xml:lang="en">Audio Channel</rdfs:label>
        <rdfs:isDefinedBy rdf:resource="http://rs.tdwg.org/abcd/terms/"/>
        <dwcattributes:status>recommended</dwcattributes:status>
        <dcterms:issued>2019-01-31</dcterms:issued>
        <dcterms:modified>2019-01-31</dcterms:modified>
        <rdfs:comment>Channel(s) used for recording audio track.</rdfs:comment>
        <skos:definition>Channel(s) used for recording audio track.</skos:definition>
        <dc:description>Recommended vocabulary: "mono", "stereo".</dc:description>
        <rdfs:domain rdf:resource="http://www.w3.org/2002/07/owl#Thing"/>
        <rdfs:range rdf:resource="http://www.w3.org/2001/XMLSchema#string"/>
    </owl:DatatypeProperty>

    <owl:FunctionalProperty rdf:about="audioChannel"/>

    <owl:DatatypeProperty rdf:about="audioEncoding">
        <rdfs:label xml:lang="en">Audio Encoding</rdfs:label>
        <rdfs:isDefinedBy rdf:resource="http://rs.tdwg.org/abcd/terms/"/>
        <dwcattributes:status>recommended</dwcattributes:status>
        <dcterms:issued>2019-01-31</dcterms:issued>
        <dcterms:modified>2019-01-31</dcterms:modified>
        <rdfs:domain rdf:resource="http://www.w3.org/2002/07/owl#Thing"/>
        <rdfs:range rdf:resource="http://www.w3.org/2001/XMLSchema#string"/>
    </owl:DatatypeProperty>

    <owl:FunctionalProperty rdf:about="audioEncoding"/>

    <owl:DatatypeProperty rdf:about="authorTeam">
        <rdfs:label xml:lang="en">Author Team</rdfs:label>
        <rdfs:isDefinedBy rdf:resource="http://rs.tdwg.org/abcd/terms/"/>
        <dwcattributes:status>recommended</dwcattributes:status>
        <dcterms:issued>2019-01-31</dcterms:issued>
        <dcterms:modified>2019-01-31</dcterms:modified>
        <rdfs:comment>The author(s) who published the full name as it stands.</rdfs:comment>
        <skos:definition>The author(s) who published the full name as it stands.</skos:definition>
        <rdfs:domain rdf:resource="http://www.w3.org/2002/07/owl#Thing"/>
        <rdfs:range rdf:resource="http://www.w3.org/2001/XMLSchema#string"/>
    </owl:DatatypeProperty>

    <owl:FunctionalProperty rdf:about="authorTeam"/>

    <owl:DatatypeProperty rdf:about="authorTeamAndYear">
        <rdfs:label xml:lang="en">Author Team And Year</rdfs:label>
        <rdfs:isDefinedBy rdf:resource="http://rs.tdwg.org/abcd/terms/"/>
        <dwcattributes:status>recommended</dwcattributes:status>
        <dcterms:issued>2019-01-31</dcterms:issued>
        <dcterms:modified>2019-01-31</dcterms:modified>
        <rdfs:comment>The author(s) who published the full name as it stands and its year.</rdfs:comment>
        <skos:definition>The author(s) who published the full name as it stands and its year.</skos:definition>
        <dc:description>For the author team notation with parenthesis please use abcd:parentheticalAuthorTeamAndYear.</dc:description>
        <rdfs:domain rdf:resource="http://www.w3.org/2002/07/owl#Thing"/>
        <rdfs:range rdf:resource="http://www.w3.org/2001/XMLSchema#string"/>
    </owl:DatatypeProperty>

    <owl:FunctionalProperty rdf:about="authorTeamAndYear"/>

    <owl:DatatypeProperty rdf:about="authorTeamOriginalAndYear">
        <rdfs:label xml:lang="en">Author Team Original And Year</rdfs:label>
        <rdfs:isDefinedBy rdf:resource="http://rs.tdwg.org/abcd/terms/"/>
        <dwcattributes:status>recommended</dwcattributes:status>
        <dcterms:issued>2019-01-31</dcterms:issued>
        <dcterms:modified>2019-01-31</dcterms:modified>
        <rdfs:comment>The first person(s) who validly published the species-group name and the year of publication.</rdfs:comment>
        <skos:definition>The first person(s) who validly published the species-group name and the year of publication.</skos:definition>
        <rdfs:domain rdf:resource="http://www.w3.org/2002/07/owl#Thing"/>
        <rdfs:range rdf:resource="http://www.w3.org/2001/XMLSchema#string"/>
    </owl:DatatypeProperty>

    <owl:FunctionalProperty rdf:about="authorTeamOriginalAndYear"/>

    <owl:DatatypeProperty rdf:about="authorTeamParenthesis">
        <rdfs:label xml:lang="en">Author Team Parenthesis</rdfs:label>
        <rdfs:isDefinedBy rdf:resource="http://rs.tdwg.org/abcd/terms/"/>
        <dwcattributes:status>recommended</dwcattributes:status>
        <dcterms:issued>2019-01-31</dcterms:issued>
        <dcterms:modified>2019-01-31</dcterms:modified>
        <rdfs:comment>Author team of the basionym of a species or subspecies combination.</rdfs:comment>
        <skos:definition>Author team of the basionym of a species or subspecies combination.</skos:definition>
        <rdfs:domain rdf:resource="http://www.w3.org/2002/07/owl#Thing"/>
        <rdfs:range rdf:resource="http://www.w3.org/2001/XMLSchema#string"/>
    </owl:DatatypeProperty>

    <owl:FunctionalProperty rdf:about="authorTeamParenthesis"/>

    <owl:DatatypeProperty rdf:about="authorTeamParenthesisAndYear">
        <rdfs:label xml:lang="en">Author Team Parenthesis And Year</rdfs:label>
        <rdfs:isDefinedBy rdf:resource="http://rs.tdwg.org/abcd/terms/"/>
        <dwcattributes:status>recommended</dwcattributes:status>
        <dcterms:issued>2019-01-31</dcterms:issued>
        <dcterms:modified>2019-01-31</dcterms:modified>
        <rdfs:comment>The parenthetical citation of the original author when a species-group was transferred to another genus and the year of the original publication.</rdfs:comment>
        <skos:definition>The parenthetical citation of the original author when a species-group was transferred to another genus and the year of the original publication.</skos:definition>
        <rdfs:domain rdf:resource="http://www.w3.org/2002/07/owl#Thing"/>
        <rdfs:range rdf:resource="http://www.w3.org/2001/XMLSchema#string"/>
    </owl:DatatypeProperty>

    <owl:FunctionalProperty rdf:about="authorTeamParenthesisAndYear"/>

    <owl:DatatypeProperty rdf:about="biologicalStatus">
        <rdfs:label xml:lang="en">Biological Status</rdfs:label>
        <rdfs:isDefinedBy rdf:resource="http://rs.tdwg.org/abcd/terms/"/>
        <dwcattributes:status>recommended</dwcattributes:status>
        <dcterms:issued>2019-01-31</dcterms:issued>
        <dcterms:modified>2019-01-31</dcterms:modified>
        <rdfs:comment>Code for the (propagation-)provenance of the unit.</rdfs:comment>
        <skos:definition>Code for the (propagation-)provenance of the unit.</skos:definition>
        <dc:description>100: Wild; 110: Natural; 120: Semi-natural/wild; 200: Weedy; 300: Traditional cultivar/landrace; 400: Breeding/research material; 410: Breeder's line; 411: Synthetic population; 412: Hybrid; 413: Founder stock/base population; 414: Inbred line (parent of hybrid cultivar); 415: Segregating population; 420: Mutant/genetic stock; 500: Advanced/improved cultivar; 999: Other</dc:description>
        <rdfs:domain rdf:resource="http://www.w3.org/2002/07/owl#Thing"/>
        <rdfs:range rdf:resource="http://www.w3.org/2001/XMLSchema#integer"/>
    </owl:DatatypeProperty>

    <owl:FunctionalProperty rdf:about="biologicalStatus"/>

    <owl:DatatypeProperty rdf:about="blocked">
        <rdfs:label xml:lang="en">Blocked</rdfs:label>
        <rdfs:isDefinedBy rdf:resource="http://rs.tdwg.org/abcd/terms/"/>
        <dwcattributes:status>recommended</dwcattributes:status>
        <dcterms:issued>2019-01-31</dcterms:issued>
        <dcterms:modified>2019-01-31</dcterms:modified>
        <rdfs:comment>Sample or specimen data can not be ordered/loaned in general, but are visible via portals.</rdfs:comment>
        <skos:definition>Sample or specimen data can not be ordered/loaned in general, but are visible via portals.</skos:definition>
        <dc:description>Note: Records/samples/specimens not to be published should be blocked on database level. If they are available via Darwin Core or ABCD, they are visible for everyone. This element is to be used for samples/specimens that cannot be loaned.</dc:description>
        <rdfs:domain rdf:resource="http://www.w3.org/2002/07/owl#Thing"/>
        <rdfs:range rdf:resource="http://www.w3.org/2001/XMLSchema#boolean"/>
    </owl:DatatypeProperty>

    <owl:FunctionalProperty rdf:about="blocked"/>

    <owl:DatatypeProperty rdf:about="breed">
        <rdfs:label xml:lang="en">Breed</rdfs:label>
        <rdfs:isDefinedBy rdf:resource="http://rs.tdwg.org/abcd/terms/"/>
        <dwcattributes:status>recommended</dwcattributes:status>
        <dcterms:issued>2019-01-31</dcterms:issued>
        <dcterms:modified>2019-01-31</dcterms:modified>
        <rdfs:comment>Name of the breed of an animal.</rdfs:comment>
        <skos:definition>Name of the breed of an animal.</skos:definition>
        <rdfs:domain rdf:resource="http://www.w3.org/2002/07/owl#Thing"/>
        <rdfs:range rdf:resource="http://www.w3.org/2001/XMLSchema#string"/>
    </owl:DatatypeProperty>

    <owl:FunctionalProperty rdf:about="breed"/>

    <owl:DatatypeProperty rdf:about="breedingCountryCode">
        <rdfs:label xml:lang="en">Breeding Country Code</rdfs:label>
        <rdfs:isDefinedBy rdf:resource="http://rs.tdwg.org/abcd/terms/"/>
        <dwcattributes:status>recommended</dwcattributes:status>
        <dcterms:issued>2019-01-31</dcterms:issued>
        <dcterms:modified>2019-01-31</dcterms:modified>
        <rdfs:comment>ISO 3-letter code for the country where the breeding institute is located.</rdfs:comment>
        <skos:definition>ISO 3-letter code for the country where the breeding institute is located.</skos:definition>
        <rdfs:domain rdf:resource="http://www.w3.org/2002/07/owl#Thing"/>
        <rdfs:range rdf:resource="http://www.w3.org/2001/XMLSchema#string"/>
    </owl:DatatypeProperty>

    <owl:FunctionalProperty rdf:about="breedingCountryCode"/>

    <owl:DatatypeProperty rdf:about="breedingInstitutionCode">
        <rdfs:label xml:lang="en">Breeding Institution Code</rdfs:label>
        <rdfs:isDefinedBy rdf:resource="http://rs.tdwg.org/abcd/terms/"/>
        <dwcattributes:status>recommended</dwcattributes:status>
        <dcterms:issued>2019-01-31</dcterms:issued>
        <dcterms:modified>2019-01-31</dcterms:modified>
        <rdfs:comment>FAO Institute Code of the institute that has bred the material.</rdfs:comment>
        <skos:definition>FAO Institute Code of the institute that has bred the material.</skos:definition>
        <dc:description>The codes consist of the 3-letter ISO 3166 country code of the country where the institute is located plus a three-digit number.</dc:description>
        <rdfs:domain rdf:resource="http://www.w3.org/2002/07/owl#Thing"/>
        <rdfs:range rdf:resource="http://www.w3.org/2001/XMLSchema#string"/>
    </owl:DatatypeProperty>

    <owl:FunctionalProperty rdf:about="breedingInstitutionCode"/>

    <owl:DatatypeProperty rdf:about="breedingSystem">
        <rdfs:label xml:lang="en">Breeding System</rdfs:label>
        <rdfs:isDefinedBy rdf:resource="http://rs.tdwg.org/abcd/terms/"/>
        <dwcattributes:status>recommended</dwcattributes:status>
        <dcterms:issued>2019-01-31</dcterms:issued>
        <dcterms:modified>2019-01-31</dcterms:modified>
        <rdfs:comment>A code to indicate the breeding system of the accession [ITF-2].</rdfs:comment>
        <skos:definition>A code to indicate the breeding system of the accession [ITF-2].</skos:definition>
        <rdfs:domain rdf:resource="http://www.w3.org/2002/07/owl#Thing"/>
        <rdfs:range rdf:resource="http://www.w3.org/2001/XMLSchema#string"/>
    </owl:DatatypeProperty>

    <owl:FunctionalProperty rdf:about="breedingSystem"/>

    <owl:DatatypeProperty rdf:about="brightness">
        <rdfs:label xml:lang="en">Brightness</rdfs:label>
        <rdfs:isDefinedBy rdf:resource="http://rs.tdwg.org/abcd/terms/"/>
        <dwcattributes:status>recommended</dwcattributes:status>
        <dcterms:issued>2019-01-31</dcterms:issued>
        <dcterms:modified>2019-01-31</dcterms:modified>
        <rdfs:comment>This property describes the average scene luminance ("brightness") of the APEX exposure model.</rdfs:comment>
        <skos:definition>This property describes the average scene luminance ("brightness") of the APEX exposure model.</skos:definition>
        <dc:description>Ordinarily it is given in the range of -99.99 to 99.99.</dc:description>
        <dc:description>Note that if the numerator of the recorded value is FFFFFFFF.H, Unknown shall be indicated.</dc:description>
        <rdfs:domain rdf:resource="http://www.w3.org/2002/07/owl#Thing"/>
        <rdfs:range rdf:resource="http://www.w3.org/2001/XMLSchema#string"/>
    </owl:DatatypeProperty>

    <owl:FunctionalProperty rdf:about="brightness"/>

    <owl:DatatypeProperty rdf:about="callType">
        <rdfs:label xml:lang="en">Call Type</rdfs:label>
        <rdfs:isDefinedBy rdf:resource="http://rs.tdwg.org/abcd/terms/"/>
        <dwcattributes:status>recommended</dwcattributes:status>
        <dcterms:issued>2019-01-31</dcterms:issued>
        <dcterms:modified>2019-01-31</dcterms:modified>
        <rdfs:comment>The type of animal call that is recorded.</rdfs:comment>
        <skos:definition>The type of animal call that is recorded.</skos:definition>
        <rdfs:domain rdf:resource="http://www.w3.org/2002/07/owl#Thing"/>
        <rdfs:range rdf:resource="http://www.w3.org/2001/XMLSchema#string"/>
    </owl:DatatypeProperty>

    <owl:DatatypeProperty rdf:about="captureEquipment">
        <rdfs:label xml:lang="en">Capture Equipment</rdfs:label>
        <rdfs:isDefinedBy rdf:resource="http://rs.tdwg.org/abcd/terms/"/>
        <dwcattributes:status>recommended</dwcattributes:status>
        <dcterms:issued>2019-01-31</dcterms:issued>
        <dcterms:modified>2019-01-31</dcterms:modified>
        <rdfs:comment>The equipment used to create this multimedia object.</rdfs:comment>
        <skos:definition>The equipment used to create this multimedia object.</skos:definition>
        <rdfs:domain rdf:resource="http://www.w3.org/2002/07/owl#Thing"/>
        <rdfs:range rdf:resource="http://www.w3.org/2001/XMLSchema#string"/>
    </owl:DatatypeProperty>

    <owl:FunctionalProperty rdf:about="captureEquipment"/>

    <owl:DatatypeProperty rdf:about="captureFramerate">
        <rdfs:label xml:lang="en">Capture Framerate</rdfs:label>
        <rdfs:isDefinedBy rdf:resource="http://rs.tdwg.org/abcd/terms/"/>
        <dwcattributes:status>recommended</dwcattributes:status>
        <dcterms:issued>2019-01-31</dcterms:issued>
        <dcterms:modified>2019-01-31</dcterms:modified>
        <rdfs:comment>The number of frames a video was captured with. If this number is higher than the (playback) framerate the video is a high-speed capture (slow-motion video) and if it is lower it is a time-lapse recording.</rdfs:comment>
        <skos:definition>The number of frames a video was captured with. If this number is higher than the (playback) framerate the video is a high-speed capture (slow-motion video) and if it is lower it is a time-lapse recording.</skos:definition>
        <rdfs:domain rdf:resource="http://www.w3.org/2002/07/owl#Thing"/>
        <rdfs:range rdf:resource="http://www.w3.org/2001/XMLSchema#string"/>
    </owl:DatatypeProperty>

    <owl:FunctionalProperty rdf:about="captureFramerate"/>

    <owl:DatatypeProperty rdf:about="carrierFrequency">
        <rdfs:label xml:lang="en">Carrier Frequency</rdfs:label>
        <rdfs:isDefinedBy rdf:resource="http://rs.tdwg.org/abcd/terms/"/>
        <dwcattributes:status>recommended</dwcattributes:status>
        <dcterms:issued>2019-01-31</dcterms:issued>
        <dcterms:modified>2019-01-31</dcterms:modified>
        <rdfs:comment>For describing the sound or call of an animal.</rdfs:comment>
        <skos:definition>For describing the sound or call of an animal.</skos:definition>
        <rdfs:domain rdf:resource="http://www.w3.org/2002/07/owl#Thing"/>
        <rdfs:range rdf:resource="http://www.w3.org/2001/XMLSchema#string"/>
    </owl:DatatypeProperty>

    <owl:DatatypeProperty rdf:about="chapters">
        <rdfs:label xml:lang="en">Chapters</rdfs:label>
        <rdfs:isDefinedBy rdf:resource="http://rs.tdwg.org/abcd/terms/"/>
        <dwcattributes:status>recommended</dwcattributes:status>
        <dcterms:issued>2019-01-31</dcterms:issued>
        <dcterms:modified>2019-01-31</dcterms:modified>
        <rdfs:domain rdf:resource="http://www.w3.org/2002/07/owl#Thing"/>
        <rdfs:range rdf:resource="http://www.w3.org/2001/XMLSchema#string"/>
    </owl:DatatypeProperty>

    <owl:DatatypeProperty rdf:about="classificationScheme">
        <rdfs:label xml:lang="en">Classification Scheme</rdfs:label>
        <rdfs:isDefinedBy rdf:resource="http://rs.tdwg.org/abcd/terms/"/>
        <dwcattributes:status>recommended</dwcattributes:status>
        <dcterms:issued>2019-01-31</dcterms:issued>
        <dcterms:modified>2019-01-31</dcterms:modified>
        <rdfs:comment>The classification system used to describe a concept. This can also be used to document the controlled vocabulary used.</rdfs:comment>
        <skos:definition>The classification system used to describe a concept. This can also be used to document the controlled vocabulary used.</skos:definition>
        <rdfs:domain rdf:resource="http://www.w3.org/2002/07/owl#Thing"/>
        <rdfs:range rdf:resource="http://www.w3.org/2001/XMLSchema#string"/>
    </owl:DatatypeProperty>

    <owl:FunctionalProperty rdf:about="classificationScheme"/>

    <owl:DatatypeProperty rdf:about="code">
        <rdfs:label xml:lang="en">Code</rdfs:label>
        <rdfs:isDefinedBy rdf:resource="http://rs.tdwg.org/abcd/terms/"/>
        <dwcattributes:status>recommended</dwcattributes:status>
        <dcterms:issued>2019-01-31</dcterms:issued>
        <dcterms:modified>2019-01-31</dcterms:modified>
        <rdfs:comment>An abbreviation or code for a concept.</rdfs:comment>
        <skos:definition>An abbreviation or code for a concept.</skos:definition>
        <dc:description>Unlike abcd:ID a Code usually refers to a defined code standard.</dc:description>
        <rdfs:domain rdf:resource="http://www.w3.org/2002/07/owl#Thing"/>
        <rdfs:range rdf:resource="http://www.w3.org/2001/XMLSchema#string"/>
    </owl:DatatypeProperty>

    <owl:FunctionalProperty rdf:about="code"/>

    <owl:DatatypeProperty rdf:about="codeAssessment">
        <rdfs:label xml:lang="en">Code Assessment</rdfs:label>
        <rdfs:isDefinedBy rdf:resource="http://rs.tdwg.org/abcd/terms/"/>
        <dwcattributes:status>recommended</dwcattributes:status>
        <dcterms:issued>2019-01-31</dcterms:issued>
        <dcterms:modified>2019-01-31</dcterms:modified>
        <rdfs:comment>An indication of whether the type is conserved or rejected/suppressed by the Code, or is proposed for conservation or suppression/rejection.</rdfs:comment>
        <skos:definition>An indication of whether the type is conserved or rejected/suppressed by the Code, or is proposed for conservation or suppression/rejection.</skos:definition>
        <rdfs:domain rdf:resource="http://www.w3.org/2002/07/owl#Thing"/>
        <rdfs:range rdf:resource="http://www.w3.org/2001/XMLSchema#string"/>
    </owl:DatatypeProperty>

    <owl:FunctionalProperty rdf:about="codeAssessment"/>

    <owl:DatatypeProperty rdf:about="codeStandard">
        <rdfs:label xml:lang="en">Code Standard</rdfs:label>
        <rdfs:isDefinedBy rdf:resource="http://rs.tdwg.org/abcd/terms/"/>
        <dwcattributes:status>recommended</dwcattributes:status>
        <dcterms:issued>2019-01-31</dcterms:issued>
        <dcterms:modified>2019-01-31</dcterms:modified>
        <rdfs:comment>The standard coding scheme an abcd:Code is using.</rdfs:comment>
        <skos:definition>The standard coding scheme an abcd:Code is using.</skos:definition>
        <rdfs:domain rdf:resource="http://www.w3.org/2002/07/owl#Thing"/>
        <rdfs:range rdf:resource="http://www.w3.org/2001/XMLSchema#string"/>
    </owl:DatatypeProperty>

    <owl:FunctionalProperty rdf:about="codeStandard"/>

    <owl:DatatypeProperty rdf:about="codecName">
        <rdfs:label xml:lang="en">Codec Name</rdfs:label>
        <rdfs:isDefinedBy rdf:resource="http://rs.tdwg.org/abcd/terms/"/>
        <dwcattributes:status>recommended</dwcattributes:status>
        <dcterms:issued>2019-01-31</dcterms:issued>
        <dcterms:modified>2019-01-31</dcterms:modified>
        <rdfs:comment>Name and version (or subtype) of the compression algorithm used.</rdfs:comment>
        <skos:definition>Name and version (or subtype) of the compression algorithm used.</skos:definition>
        <rdfs:domain rdf:resource="http://www.w3.org/2002/07/owl#Thing"/>
        <rdfs:range rdf:resource="http://www.w3.org/2001/XMLSchema#string"/>
    </owl:DatatypeProperty>

    <owl:FunctionalProperty rdf:about="codecName"/>

    <owl:DatatypeProperty rdf:about="codecQuality">
        <rdfs:label xml:lang="en">Codec Quality</rdfs:label>
        <rdfs:isDefinedBy rdf:resource="http://rs.tdwg.org/abcd/terms/"/>
        <dwcattributes:status>recommended</dwcattributes:status>
        <dcterms:issued>2019-01-31</dcterms:issued>
        <dcterms:modified>2019-01-31</dcterms:modified>
        <rdfs:comment>Impact of the compression on quality.</rdfs:comment>
        <skos:definition>Impact of the compression on quality.</skos:definition>
        <rdfs:domain rdf:resource="http://www.w3.org/2002/07/owl#Thing"/>
        <rdfs:range rdf:resource="http://www.w3.org/2001/XMLSchema#string"/>
    </owl:DatatypeProperty>

    <owl:DatatypeProperty rdf:about="collectingAcquisitionSource">
        <rdfs:label xml:lang="en">Collecting Acquisition Source</rdfs:label>
        <rdfs:isDefinedBy rdf:resource="http://rs.tdwg.org/abcd/terms/"/>
        <dwcattributes:status>recommended</dwcattributes:status>
        <dcterms:issued>2019-01-31</dcterms:issued>
        <dcterms:modified>2019-01-31</dcterms:modified>
        <rdfs:comment>Code for the (location-) provenance of the unit.</rdfs:comment>
        <skos:definition>Code for the (location-) provenance of the unit.</skos:definition>
        <dc:description>40: Institute, Experimental station, Research organisation, Genebank; 50: Seed company; 60: Weedy, disturbed or ruderal habitat; 61: Roadside; 62: Field margin; 99: Other</dc:description>
        <dc:description>The coding scheme proposed can be used at 2 different levels of detail: either by using the general codes such as 10, 20, 30, 40 or by using the more specific codes such as 11, 12 etc.</dc:description>
        <dc:description>10: Wild habitat; 11: Forest/woodland; 12: Shrubland; 13: Grassland; 14: Desert/tundra; 15: Aquatic habitat; 20: Farm or cultivated habitat; 21: Field; 22: Orchard; 23: Backyard, kitchen or home garden (urban, peri-urban or rural); 24: Fallow land; 25: Pasture; 26: Farm store; 27: Threshing floor; 28: Park; 30: Market or shop;</dc:description>
        <rdfs:domain rdf:resource="http://www.w3.org/2002/07/owl#Thing"/>
        <rdfs:range rdf:resource="http://www.w3.org/2001/XMLSchema#integer"/>
    </owl:DatatypeProperty>

    <owl:FunctionalProperty rdf:about="collectingAcquisitionSource"/>

    <owl:DatatypeProperty rdf:about="color">
        <rdfs:label xml:lang="en">Color</rdfs:label>
        <rdfs:isDefinedBy rdf:resource="http://rs.tdwg.org/abcd/terms/"/>
        <dwcattributes:status>recommended</dwcattributes:status>
        <dcterms:issued>2019-01-31</dcterms:issued>
        <dcterms:modified>2019-01-31</dcterms:modified>
        <rdfs:comment>Property to indicate the color range recorded in this image.</rdfs:comment>
        <skos:definition>Property to indicate the color range recorded in this image.</skos:definition>
        <rdfs:domain rdf:resource="http://www.w3.org/2002/07/owl#Thing"/>
        <rdfs:range rdf:resource="http://www.w3.org/2001/XMLSchema#string"/>
    </owl:DatatypeProperty>

    <owl:FunctionalProperty rdf:about="color"/>

    <owl:DatatypeProperty rdf:about="colorSpace">
        <rdfs:label xml:lang="en">Color Space</rdfs:label>
        <rdfs:isDefinedBy rdf:resource="http://rs.tdwg.org/abcd/terms/"/>
        <dwcattributes:status>recommended</dwcattributes:status>
        <dcterms:issued>2019-01-31</dcterms:issued>
        <dcterms:modified>2019-01-31</dcterms:modified>
        <rdfs:comment>The color space used to store the image in.</rdfs:comment>
        <skos:definition>The color space used to store the image in.</skos:definition>
        <rdfs:domain rdf:resource="http://www.w3.org/2002/07/owl#Thing"/>
        <rdfs:range rdf:resource="http://www.w3.org/2001/XMLSchema#string"/>
    </owl:DatatypeProperty>

    <owl:FunctionalProperty rdf:about="colorSpace"/>

    <owl:DatatypeProperty rdf:about="combinationAuthorTeamAndYear">
        <rdfs:label xml:lang="en">Combination Author Team And Year</rdfs:label>
        <rdfs:isDefinedBy rdf:resource="http://rs.tdwg.org/abcd/terms/"/>
        <dwcattributes:status>recommended</dwcattributes:status>
        <dcterms:issued>2019-01-31</dcterms:issued>
        <dcterms:modified>2019-01-31</dcterms:modified>
        <rdfs:comment>The citation of the authors responsible for the new combination and the year of its publication.</rdfs:comment>
        <skos:definition>The citation of the authors responsible for the new combination and the year of its publication.</skos:definition>
        <rdfs:domain rdf:resource="http://www.w3.org/2002/07/owl#Thing"/>
        <rdfs:range rdf:resource="http://www.w3.org/2001/XMLSchema#string"/>
    </owl:DatatypeProperty>

    <owl:FunctionalProperty rdf:about="combinationAuthorTeamAndYear"/>

    <owl:DatatypeProperty rdf:about="completeness">
        <rdfs:label xml:lang="en">Completeness</rdfs:label>
        <rdfs:isDefinedBy rdf:resource="http://rs.tdwg.org/abcd/terms/"/>
        <dwcattributes:status>recommended</dwcattributes:status>
        <dcterms:issued>2019-01-31</dcterms:issued>
        <dcterms:modified>2019-01-31</dcterms:modified>
        <rdfs:comment>An indication of the completeness of the representation of an organism in a paleontological specimen.</rdfs:comment>
        <skos:definition>An indication of the completeness of the representation of an organism in a paleontological specimen.</skos:definition>
        <rdfs:domain rdf:resource="http://www.w3.org/2002/07/owl#Thing"/>
        <rdfs:range rdf:resource="http://www.w3.org/2001/XMLSchema#string"/>
    </owl:DatatypeProperty>

    <owl:FunctionalProperty rdf:about="completeness"/>

    <owl:DatatypeProperty rdf:about="contrast">
        <rdfs:label xml:lang="en">Contrast</rdfs:label>
        <rdfs:isDefinedBy rdf:resource="http://rs.tdwg.org/abcd/terms/"/>
        <dwcattributes:status>recommended</dwcattributes:status>
        <dcterms:issued>2019-01-31</dcterms:issued>
        <dcterms:modified>2019-01-31</dcterms:modified>
        <rdfs:comment>This property indicates the direction of contrast processing applied by the camera when the image was shot.</rdfs:comment>
        <skos:definition>This property indicates the direction of contrast processing applied by the camera when the image was shot.</skos:definition>
        <rdfs:domain rdf:resource="http://www.w3.org/2002/07/owl#Thing"/>
        <rdfs:range rdf:resource="http://www.w3.org/2001/XMLSchema#string"/>
    </owl:DatatypeProperty>

    <owl:FunctionalProperty rdf:about="contrast"/>

    <owl:DatatypeProperty rdf:about="contributors">
        <rdfs:label xml:lang="en">Contributors</rdfs:label>
        <rdfs:isDefinedBy rdf:resource="http://rs.tdwg.org/abcd/terms/"/>
        <dwcattributes:status>recommended</dwcattributes:status>
        <dcterms:issued>2019-01-31</dcterms:issued>
        <dcterms:modified>2019-01-31</dcterms:modified>
        <rdfs:comment>Contributors or translators for a class expressed in a free text form.</rdfs:comment>
        <skos:definition>Contributors or translators for a class expressed in a free text form.</skos:definition>
        <rdfs:domain rdf:resource="http://www.w3.org/2002/07/owl#Thing"/>
        <rdfs:range rdf:resource="http://www.w3.org/2001/XMLSchema#string"/>
        <skos:relatedMatch rdf:resource="http://purl.org/dc/terms/contributor"/>
    </owl:DatatypeProperty>

    <owl:FunctionalProperty rdf:about="contributors"/>

    <owl:DatatypeProperty rdf:about="counter">
        <rdfs:label xml:lang="en">Counter</rdfs:label>
        <rdfs:isDefinedBy rdf:resource="http://rs.tdwg.org/abcd/terms/"/>
        <dwcattributes:status>recommended</dwcattributes:status>
        <dcterms:issued>2019-01-31</dcterms:issued>
        <dcterms:modified>2019-01-31</dcterms:modified>
        <rdfs:domain rdf:resource="http://www.w3.org/2002/07/owl#Thing"/>
        <rdfs:range rdf:resource="http://www.w3.org/2001/XMLSchema#string"/>
    </owl:DatatypeProperty>

    <owl:DatatypeProperty rdf:about="coverage">
        <rdfs:label xml:lang="en">Coverage</rdfs:label>
        <rdfs:isDefinedBy rdf:resource="http://rs.tdwg.org/abcd/terms/"/>
        <dwcattributes:status>recommended</dwcattributes:status>
        <dcterms:issued>2019-01-31</dcterms:issued>
        <dcterms:modified>2019-01-31</dcterms:modified>
        <rdfs:comment>Free-form text terminology or descriptions available in a data source (geographic, taxonomic, etc.).</rdfs:comment>
        <skos:definition>Free-form text terminology or descriptions available in a data source (geographic, taxonomic, etc.).</skos:definition>
        <dc:description>This element is used to give a broad overview of the content of the data set. More detailed information can be expressed in abcd:TaxonomicTerm and abcd:GeoecologicalTerm.</dc:description>
        <rdfs:domain rdf:resource="http://www.w3.org/2002/07/owl#Thing"/>
        <rdfs:range rdf:resource="http://www.w3.org/2001/XMLSchema#string"/>
        <skos:relatedMatch rdf:resource="http://purl.org/dc/terms/coverage"/>
    </owl:DatatypeProperty>

    <owl:FunctionalProperty rdf:about="coverage"/>

    <owl:DatatypeProperty rdf:about="creators">
        <rdfs:label xml:lang="en">Creators</rdfs:label>
        <rdfs:isDefinedBy rdf:resource="http://rs.tdwg.org/abcd/terms/"/>
        <dwcattributes:status>recommended</dwcattributes:status>
        <dcterms:issued>2019-01-31</dcterms:issued>
        <dcterms:modified>2019-01-31</dcterms:modified>
        <rdfs:comment>Author(s) or editor(s) of a class expressed in a free text format.</rdfs:comment>
        <skos:definition>Author(s) or editor(s) of a class expressed in a free text format.</skos:definition>
        <rdfs:domain rdf:resource="http://www.w3.org/2002/07/owl#Thing"/>
        <rdfs:range rdf:resource="http://www.w3.org/2001/XMLSchema#string"/>
        <skos:relatedMatch rdf:resource="http://purl.org/dc/terms/creator"/>
    </owl:DatatypeProperty>

    <owl:FunctionalProperty rdf:about="creators"/>

    <owl:DatatypeProperty rdf:about="cultivarGroupName">
        <rdfs:label xml:lang="en">Cultivar Group Name</rdfs:label>
        <rdfs:isDefinedBy rdf:resource="http://rs.tdwg.org/abcd/terms/"/>
        <dwcattributes:status>recommended</dwcattributes:status>
        <dcterms:issued>2019-01-31</dcterms:issued>
        <dcterms:modified>2019-01-31</dcterms:modified>
        <rdfs:comment>The cultivar group name.</rdfs:comment>
        <skos:definition>The cultivar group name.</skos:definition>
        <rdfs:domain rdf:resource="http://www.w3.org/2002/07/owl#Thing"/>
        <rdfs:range rdf:resource="http://www.w3.org/2001/XMLSchema#string"/>
    </owl:DatatypeProperty>

    <owl:FunctionalProperty rdf:about="cultivarGroupName"/>

    <owl:DatatypeProperty rdf:about="cultivarName">
        <rdfs:label xml:lang="en">Cultivar Name</rdfs:label>
        <rdfs:isDefinedBy rdf:resource="http://rs.tdwg.org/abcd/terms/"/>
        <dwcattributes:status>recommended</dwcattributes:status>
        <dcterms:issued>2019-01-31</dcterms:issued>
        <dcterms:modified>2019-01-31</dcterms:modified>
        <rdfs:comment>A cultivar name, as specified by the ICNCP.</rdfs:comment>
        <skos:definition>A cultivar name, as specified by the ICNCP.</skos:definition>
        <rdfs:domain rdf:resource="http://www.w3.org/2002/07/owl#Thing"/>
        <rdfs:range rdf:resource="http://www.w3.org/2001/XMLSchema#string"/>
    </owl:DatatypeProperty>

    <owl:FunctionalProperty rdf:about="cultivarName"/>

    <owl:DatatypeProperty rdf:about="cultivatedOccurrence">
        <rdfs:label xml:lang="en">Cultivated Occurrence</rdfs:label>
        <rdfs:isDefinedBy rdf:resource="http://rs.tdwg.org/abcd/terms/"/>
        <dwcattributes:status>recommended</dwcattributes:status>
        <dcterms:issued>2019-01-31</dcterms:issued>
        <dcterms:modified>2019-01-31</dcterms:modified>
        <rdfs:comment>Records whether the plant is established or not established (hence, only maintained as a cultivated plant), in the collection habitat. Equivalent to HISPID:poscul.</rdfs:comment>
        <skos:definition>Records whether the plant is established or not established (hence, only maintained as a cultivated plant), in the collection habitat. Equivalent to HISPID:poscul.</skos:definition>
        <dc:description>It is expected that this field will have values similar to the following: Cultivated, Not cultivated, Unknown</dc:description>
        <rdfs:domain rdf:resource="http://www.w3.org/2002/07/owl#Thing"/>
        <rdfs:range rdf:resource="http://www.w3.org/2001/XMLSchema#string"/>
    </owl:DatatypeProperty>

    <owl:FunctionalProperty rdf:about="cultivatedOccurrence"/>

    <owl:DatatypeProperty rdf:about="cultivation">
        <rdfs:label xml:lang="en">Cultivation</rdfs:label>
        <rdfs:isDefinedBy rdf:resource="http://rs.tdwg.org/abcd/terms/"/>
        <dwcattributes:status>recommended</dwcattributes:status>
        <dcterms:issued>2019-01-31</dcterms:issued>
        <dcterms:modified>2019-01-31</dcterms:modified>
        <rdfs:comment>Allows for cultivation information to be passed as free text in order to help the receiving garden care for the transferred accession [ITF-2] or to record the garden's experience made with this accession.</rdfs:comment>
        <skos:definition>Allows for cultivation information to be passed as free text in order to help the receiving garden care for the transferred accession [ITF-2] or to record the garden's experience made with this accession.</skos:definition>
        <rdfs:domain rdf:resource="http://www.w3.org/2002/07/owl#Thing"/>
        <rdfs:range rdf:resource="http://www.w3.org/2001/XMLSchema#string"/>
    </owl:DatatypeProperty>

    <owl:FunctionalProperty rdf:about="cultivation"/>

    <owl:DatatypeProperty rdf:about="cultureMedium">
        <rdfs:label xml:lang="en">Culture Medium</rdfs:label>
        <rdfs:isDefinedBy rdf:resource="http://rs.tdwg.org/abcd/terms/"/>
        <dwcattributes:status>recommended</dwcattributes:status>
        <dcterms:issued>2019-01-31</dcterms:issued>
        <dcterms:modified>2019-01-31</dcterms:modified>
        <rdfs:comment>The growth medium for a microbial or similar culture.</rdfs:comment>
        <skos:definition>The growth medium for a microbial or similar culture.</skos:definition>
        <rdfs:domain rdf:resource="http://www.w3.org/2002/07/owl#Thing"/>
        <rdfs:range rdf:resource="http://www.w3.org/2001/XMLSchema#string"/>
    </owl:DatatypeProperty>

    <owl:FunctionalProperty rdf:about="cultureMedium"/>

    <owl:DatatypeProperty rdf:about="cultureName">
        <rdfs:label xml:lang="en">Culture Name</rdfs:label>
        <rdfs:isDefinedBy rdf:resource="http://rs.tdwg.org/abcd/terms/"/>
        <dwcattributes:status>recommended</dwcattributes:status>
        <dcterms:issued>2019-01-31</dcterms:issued>
        <dcterms:modified>2019-01-31</dcterms:modified>
        <rdfs:comment>The reference or trade name for a microbial culture.</rdfs:comment>
        <skos:definition>The reference or trade name for a microbial culture.</skos:definition>
        <rdfs:domain rdf:resource="http://www.w3.org/2002/07/owl#Thing"/>
        <rdfs:range rdf:resource="http://www.w3.org/2001/XMLSchema#string"/>
    </owl:DatatypeProperty>

    <owl:DatatypeProperty rdf:about="dataCenter">
        <rdfs:label xml:lang="en">Data Center</rdfs:label>
        <rdfs:isDefinedBy rdf:resource="http://rs.tdwg.org/abcd/terms/"/>
        <dwcattributes:status>recommended</dwcattributes:status>
        <dcterms:issued>2019-01-31</dcterms:issued>
        <dcterms:modified>2019-01-31</dcterms:modified>
        <rdfs:comment>The name of the institution or data center which is hosting a dataset. This might be different from (the institution of) the owner.</rdfs:comment>
        <skos:definition>The name of the institution or data center which is hosting a dataset. This might be different from (the institution of) the owner.</skos:definition>
        <rdfs:domain rdf:resource="http://www.w3.org/2002/07/owl#Thing"/>
        <rdfs:range rdf:resource="http://www.w3.org/2001/XMLSchema#string"/>
    </owl:DatatypeProperty>

    <owl:DatatypeProperty rdf:about="decodedBreedingInstitute">
        <rdfs:label xml:lang="en">Decoded Breeding Institute</rdfs:label>
        <rdfs:isDefinedBy rdf:resource="http://rs.tdwg.org/abcd/terms/"/>
        <dwcattributes:status>recommended</dwcattributes:status>
        <dcterms:issued>2019-01-31</dcterms:issued>
        <dcterms:modified>2019-01-31</dcterms:modified>
        <rdfs:comment>A brief name and location for a breeding institute.</rdfs:comment>
        <skos:definition>A brief name and location for a breeding institute.</skos:definition>
        <rdfs:domain rdf:resource="http://www.w3.org/2002/07/owl#Thing"/>
        <rdfs:range rdf:resource="http://www.w3.org/2001/XMLSchema#string"/>
    </owl:DatatypeProperty>

    <owl:FunctionalProperty rdf:about="decodedBreedingInstitute"/>

    <owl:DatatypeProperty rdf:about="decodedGatheringInstitute">
        <rdfs:label xml:lang="en">Decoded Gathering Institute</rdfs:label>
        <rdfs:isDefinedBy rdf:resource="http://rs.tdwg.org/abcd/terms/"/>
        <dwcattributes:status>recommended</dwcattributes:status>
        <dcterms:issued>2019-01-31</dcterms:issued>
        <dcterms:modified>2019-01-31</dcterms:modified>
        <rdfs:comment>The brief name and location of a donor institute.</rdfs:comment>
        <skos:definition>The brief name and location of a donor institute.</skos:definition>
        <rdfs:domain rdf:resource="http://www.w3.org/2002/07/owl#Thing"/>
        <rdfs:range rdf:resource="http://www.w3.org/2001/XMLSchema#string"/>
    </owl:DatatypeProperty>

    <owl:FunctionalProperty rdf:about="decodedGatheringInstitute"/>

    <owl:DatatypeProperty rdf:about="decodedLocationSafetyDuplicates">
        <rdfs:label xml:lang="en">Decoded Location Safety Duplicates</rdfs:label>
        <rdfs:isDefinedBy rdf:resource="http://rs.tdwg.org/abcd/terms/"/>
        <dwcattributes:status>recommended</dwcattributes:status>
        <dcterms:issued>2019-01-31</dcterms:issued>
        <dcterms:modified>2019-01-31</dcterms:modified>
        <rdfs:comment>Brief name and location of the institute maintaining the safety duplicate.</rdfs:comment>
        <skos:definition>Brief name and location of the institute maintaining the safety duplicate.</skos:definition>
        <rdfs:domain rdf:resource="http://www.w3.org/2002/07/owl#Thing"/>
        <rdfs:range rdf:resource="http://www.w3.org/2001/XMLSchema#string"/>
    </owl:DatatypeProperty>

    <owl:FunctionalProperty rdf:about="decodedLocationSafetyDuplicates"/>

    <owl:DatatypeProperty rdf:about="derivedFlag">
        <rdfs:label xml:lang="en">Derived Flag</rdfs:label>
        <rdfs:isDefinedBy rdf:resource="http://rs.tdwg.org/abcd/terms/"/>
        <dwcattributes:status>recommended</dwcattributes:status>
        <dcterms:issued>2019-01-31</dcterms:issued>
        <dcterms:modified>2019-01-31</dcterms:modified>
        <rdfs:comment>A flag indicating that the information connected to a class is derived rather than original data.</rdfs:comment>
        <skos:definition>A flag indicating that the information connected to a class is derived rather than original data.</skos:definition>
        <dc:description>Allowed values are "true" or "false".</dc:description>
        <rdfs:domain rdf:resource="http://www.w3.org/2002/07/owl#Thing"/>
        <rdfs:range rdf:resource="http://www.w3.org/2001/XMLSchema#boolean"/>
    </owl:DatatypeProperty>

    <owl:FunctionalProperty rdf:about="derivedFlag"/>

    <owl:DatatypeProperty rdf:about="details">
        <rdfs:label xml:lang="en">Details</rdfs:label>
        <rdfs:isDefinedBy rdf:resource="http://rs.tdwg.org/abcd/terms/"/>
        <dwcattributes:status>recommended</dwcattributes:status>
        <dcterms:issued>2019-01-31</dcterms:issued>
        <dcterms:modified>2019-01-31</dcterms:modified>
        <rdfs:comment>Detailed information related to a class.</rdfs:comment>
        <skos:definition>Detailed information related to a class.</skos:definition>
        <rdfs:domain rdf:resource="http://www.w3.org/2002/07/owl#Thing"/>
        <rdfs:range rdf:resource="http://www.w3.org/2001/XMLSchema#string"/>
    </owl:DatatypeProperty>

    <owl:DatatypeProperty rdf:about="digitalZoomRatio">
        <rdfs:label xml:lang="en">Digital Zoom Ratio</rdfs:label>
        <rdfs:isDefinedBy rdf:resource="http://rs.tdwg.org/abcd/terms/"/>
        <dwcattributes:status>recommended</dwcattributes:status>
        <dcterms:issued>2019-01-31</dcterms:issued>
        <dcterms:modified>2019-01-31</dcterms:modified>
        <rdfs:comment>This property indicates the digital zoom ratio when the image was shot.</rdfs:comment>
        <skos:definition>This property indicates the digital zoom ratio when the image was shot.</skos:definition>
        <dc:description>If the numerator of the recorded value is 0, this indicates that digital zoom was not used.</dc:description>
        <rdfs:domain rdf:resource="http://www.w3.org/2002/07/owl#Thing"/>
        <rdfs:range rdf:resource="http://www.w3.org/2001/XMLSchema#float"/>
    </owl:DatatypeProperty>

    <owl:FunctionalProperty rdf:about="digitalZoomRatio"/>

    <owl:DatatypeProperty rdf:about="directAccessURL">
        <rdfs:label xml:lang="en">Direct Access URL</rdfs:label>
        <rdfs:isDefinedBy rdf:resource="http://rs.tdwg.org/abcd/terms/"/>
        <dwcattributes:status>recommended</dwcattributes:status>
        <dcterms:issued>2019-01-31</dcterms:issued>
        <dcterms:modified>2019-01-31</dcterms:modified>
        <rdfs:comment>An electronic source of the dataset that allows for querying and downloading of the data.</rdfs:comment>
        <skos:definition>An electronic source of the dataset that allows for querying and downloading of the data.</skos:definition>
        <dc:description>Not to be confused with the abcd:WebsiteURL of the dataset, which is primarily to get additional information about the dataset whereas this property is to quickly access the data of the dataset.</dc:description>
        <rdfs:domain rdf:resource="http://www.w3.org/2002/07/owl#Thing"/>
        <rdfs:range rdf:resource="http://www.w3.org/2001/XMLSchema#anyURI"/>
    </owl:DatatypeProperty>

    <owl:FunctionalProperty rdf:about="directAccessURL"/>

    <owl:DatatypeProperty rdf:about="disposition">
        <rdfs:label xml:lang="en">Disposition</rdfs:label>
        <rdfs:isDefinedBy rdf:resource="http://rs.tdwg.org/abcd/terms/"/>
        <dwcattributes:status>recommended</dwcattributes:status>
        <dcterms:issued>2019-01-31</dcterms:issued>
        <dcterms:modified>2019-01-31</dcterms:modified>
        <rdfs:comment>The current disposition of the catalogued item.</rdfs:comment>
        <skos:definition>The current disposition of the catalogued item.</skos:definition>
        <rdfs:domain rdf:resource="http://www.w3.org/2002/07/owl#Thing"/>
        <rdfs:range rdf:resource="http://www.w3.org/2001/XMLSchema#string"/>
        <skos:exactMatch rdf:resource="http://rs.tdwg.org/dwc/terms/disposition"/>
    </owl:DatatypeProperty>

    <owl:FunctionalProperty rdf:about="disposition"/>

    <owl:DatatypeProperty rdf:about="division">
        <rdfs:label xml:lang="en">Division</rdfs:label>
        <rdfs:isDefinedBy rdf:resource="http://rs.tdwg.org/abcd/terms/"/>
        <dwcattributes:status>recommended</dwcattributes:status>
        <dcterms:issued>2019-01-31</dcterms:issued>
        <dcterms:modified>2019-01-31</dcterms:modified>
        <rdfs:comment>Part of an Organization, e.g. department or section.</rdfs:comment>
        <skos:definition>Part of an Organization, e.g. department or section.</skos:definition>
        <rdfs:domain rdf:resource="http://www.w3.org/2002/07/owl#Thing"/>
        <rdfs:range rdf:resource="http://www.w3.org/2001/XMLSchema#string"/>
        <skos:exactMatch rdf:resource="http://www.w3.org/2006/vcard/ns#organizational-unit"/>
    </owl:DatatypeProperty>

    <owl:DatatypeProperty rdf:about="donorCategory">
        <rdfs:label xml:lang="en">Donor Category</rdfs:label>
        <rdfs:isDefinedBy rdf:resource="http://rs.tdwg.org/abcd/terms/"/>
        <dwcattributes:status>recommended</dwcattributes:status>
        <dcterms:issued>2019-01-31</dcterms:issued>
        <dcterms:modified>2019-01-31</dcterms:modified>
        <rdfs:comment>A code to indicate the type of the immediate donor from which the accession was obtained. This may not be necessarily the original collector of wild material. [ITF-2]</rdfs:comment>
        <skos:definition>A code to indicate the type of the immediate donor from which the accession was obtained. This may not be necessarily the original collector of wild material. [ITF-2]</skos:definition>
        <rdfs:domain rdf:resource="http://www.w3.org/2002/07/owl#Thing"/>
        <rdfs:range rdf:resource="http://www.w3.org/2001/XMLSchema#byte"/>
    </owl:DatatypeProperty>

    <owl:FunctionalProperty rdf:about="donorCategory"/>

    <owl:DatatypeProperty rdf:about="doubtfulFlag">
        <rdfs:label xml:lang="en">Doubtful Flag</rdfs:label>
        <rdfs:isDefinedBy rdf:resource="http://rs.tdwg.org/abcd/terms/"/>
        <dwcattributes:status>recommended</dwcattributes:status>
        <dcterms:issued>2019-01-31</dcterms:issued>
        <dcterms:modified>2019-01-31</dcterms:modified>
        <rdfs:comment>An indicator for unverified type status (kind and fact).</rdfs:comment>
        <skos:definition>An indicator for unverified type status (kind and fact).</skos:definition>
        <rdfs:domain rdf:resource="http://www.w3.org/2002/07/owl#Thing"/>
        <rdfs:range rdf:resource="http://www.w3.org/2001/XMLSchema#boolean"/>
    </owl:DatatypeProperty>

    <owl:FunctionalProperty rdf:about="doubtfulFlag"/>

    <owl:DatatypeProperty rdf:about="duplicatesDistributedTo">
        <rdfs:label xml:lang="en">Duplicates Distributed To</rdfs:label>
        <rdfs:isDefinedBy rdf:resource="http://rs.tdwg.org/abcd/terms/"/>
        <dwcattributes:status>recommended</dwcattributes:status>
        <dcterms:issued>2019-01-31</dcterms:issued>
        <dcterms:modified>2019-01-31</dcterms:modified>
        <rdfs:comment>Institutions that received duplicates of this specimen, preferably in the form of a delimited list of SourceInstitionIDs.</rdfs:comment>
        <skos:definition>Institutions that received duplicates of this specimen, preferably in the form of a delimited list of SourceInstitionIDs.</skos:definition>
        <rdfs:domain rdf:resource="http://www.w3.org/2002/07/owl#Thing"/>
        <rdfs:range rdf:resource="http://www.w3.org/2001/XMLSchema#string"/>
    </owl:DatatypeProperty>

    <owl:FunctionalProperty rdf:about="duplicatesDistributedTo"/>

    <owl:DatatypeProperty rdf:about="duration">
        <rdfs:label xml:lang="en">Duration</rdfs:label>
        <rdfs:isDefinedBy rdf:resource="http://rs.tdwg.org/abcd/terms/"/>
        <dwcattributes:status>recommended</dwcattributes:status>
        <dcterms:issued>2019-01-31</dcterms:issued>
        <dcterms:modified>2019-01-31</dcterms:modified>
        <rdfs:comment>The duration of a measurement or recording.</rdfs:comment>
        <skos:definition>The duration of a measurement or recording.</skos:definition>
        <rdfs:domain rdf:resource="http://www.w3.org/2002/07/owl#Thing"/>
        <rdfs:range rdf:resource="http://www.w3.org/2001/XMLSchema#string"/>
    </owl:DatatypeProperty>

    <owl:FunctionalProperty rdf:about="duration"/>

    <owl:DatatypeProperty rdf:about="durationTimeCode">
        <rdfs:label xml:lang="en">Duration Time Code</rdfs:label>
        <rdfs:isDefinedBy rdf:resource="http://rs.tdwg.org/abcd/terms/"/>
        <dwcattributes:status>recommended</dwcattributes:status>
        <dcterms:issued>2019-01-31</dcterms:issued>
        <dcterms:modified>2019-01-31</dcterms:modified>
        <rdfs:comment>The duration of the recording expressed as a time code.</rdfs:comment>
        <skos:definition>The duration of the recording expressed as a time code.</skos:definition>
        <dc:description>Pattern: [0-9][0-9]:[0-5][0-9]:[0-5][0-9].[0-9][0-9]</dc:description>
        <rdfs:domain rdf:resource="http://www.w3.org/2002/07/owl#Thing"/>
        <rdfs:range rdf:resource="http://www.w3.org/2001/XMLSchema#string"/>
    </owl:DatatypeProperty>

    <owl:DatatypeProperty rdf:about="epsgID">
        <rdfs:label xml:lang="en">EPSG ID</rdfs:label>
        <rdfs:isDefinedBy rdf:resource="http://rs.tdwg.org/abcd/terms/"/>
        <dwcattributes:status>recommended</dwcattributes:status>
        <dcterms:issued>2019-01-31</dcterms:issued>
        <dcterms:modified>2019-01-31</dcterms:modified>
        <rdfs:comment>The EPSG code of the coordinate reference system used for the coordinates.</rdfs:comment>
        <skos:definition>The EPSG code of the coordinate reference system used for the coordinates.</skos:definition>
        <rdfs:domain rdf:resource="http://www.w3.org/2002/07/owl#Thing"/>
        <rdfs:range rdf:resource="http://www.w3.org/2001/XMLSchema#integer"/>
    </owl:DatatypeProperty>

    <owl:DatatypeProperty rdf:about="emailAddress">
        <rdfs:label xml:lang="en">Email Address</rdfs:label>
        <rdfs:isDefinedBy rdf:resource="http://rs.tdwg.org/abcd/terms/"/>
        <dwcattributes:status>recommended</dwcattributes:status>
        <dcterms:issued>2019-01-31</dcterms:issued>
        <dcterms:modified>2019-01-31</dcterms:modified>
        <rdfs:comment>An e-mail address of a contact.</rdfs:comment>
        <skos:definition>An e-mail address of a contact.</skos:definition>
        <dc:description>Email addresses should be written WITHOUT the "mailto:" prefix.</dc:description>
        <rdfs:domain rdf:resource="http://www.w3.org/2002/07/owl#Thing"/>
        <rdfs:range rdf:resource="http://www.w3.org/2001/XMLSchema#string"/>
        <skos:exactMatch rdf:resource="http://xmlns.com/foaf/0.1/mbox"/>
    </owl:DatatypeProperty>

    <owl:DatatypeProperty rdf:about="errorDistanceInMeters">
        <rdfs:label xml:lang="en">Error Distance In Meters</rdfs:label>
        <rdfs:isDefinedBy rdf:resource="http://rs.tdwg.org/abcd/terms/"/>
        <dwcattributes:status>recommended</dwcattributes:status>
        <dcterms:issued>2019-01-31</dcterms:issued>
        <dcterms:modified>2019-01-31</dcterms:modified>
        <rdfs:comment>An estimate of how tightly the coordinates were specified, expressed as a distance in meters corresponding to a radius around the coordinates.</rdfs:comment>
        <skos:definition>An estimate of how tightly the coordinates were specified, expressed as a distance in meters corresponding to a radius around the coordinates.</skos:definition>
        <rdfs:domain rdf:resource="http://www.w3.org/2002/07/owl#Thing"/>
        <rdfs:range rdf:resource="http://www.w3.org/2001/XMLSchema#decimal"/>
        <skos:exactMatch rdf:resource="http://rs.tdwg.org/dwc/terms/coordinateUncertaintyInMeters"/>
    </owl:DatatypeProperty>

    <owl:FunctionalProperty rdf:about="errorDistanceInMeters"/>

    <owl:DatatypeProperty rdf:about="errorMethod">
        <rdfs:label xml:lang="en">Error Method</rdfs:label>
        <rdfs:isDefinedBy rdf:resource="http://rs.tdwg.org/abcd/terms/"/>
        <dwcattributes:status>recommended</dwcattributes:status>
        <dcterms:issued>2019-01-31</dcterms:issued>
        <dcterms:modified>2019-01-31</dcterms:modified>
        <rdfs:comment>A free text statement of how the Coordinate Error was determined.</rdfs:comment>
        <skos:definition>A free text statement of how the Coordinate Error was determined.</skos:definition>
        <rdfs:subPropertyOf rdf:resource="method"/>
        <rdfs:domain rdf:resource="http://www.w3.org/2002/07/owl#Thing"/>
        <rdfs:range rdf:resource="http://www.w3.org/2001/XMLSchema#string"/>
    </owl:DatatypeProperty>

    <owl:FunctionalProperty rdf:about="errorMethod"/>

    <owl:DatatypeProperty rdf:about="establishmentMeans">
        <rdfs:label xml:lang="en">Establishment Means</rdfs:label>
        <rdfs:isDefinedBy rdf:resource="http://rs.tdwg.org/abcd/terms/"/>
        <dwcattributes:status>recommended</dwcattributes:status>
        <dcterms:issued>2019-01-31</dcterms:issued>
        <dcterms:modified>2019-01-31</dcterms:modified>
        <rdfs:comment>The historical relationship of the occurrence to the cited time and place of collection or observation.</rdfs:comment>
        <skos:definition>The historical relationship of the occurrence to the cited time and place of collection or observation.</skos:definition>
        <rdfs:domain rdf:resource="http://www.w3.org/2002/07/owl#Thing"/>
        <rdfs:range rdf:resource="http://www.w3.org/2001/XMLSchema#string"/>
        <skos:exactMatch rdf:resource="http://rs.tdwg.org/dwc/terms/establishmentMeans"/>
    </owl:DatatypeProperty>

    <owl:DatatypeProperty rdf:about="exactValue">
        <rdfs:label xml:lang="en">Exact Value</rdfs:label>
        <rdfs:isDefinedBy rdf:resource="http://rs.tdwg.org/abcd/terms/"/>
        <dwcattributes:status>recommended</dwcattributes:status>
        <dcterms:issued>2019-01-31</dcterms:issued>
        <dcterms:modified>2019-01-31</dcterms:modified>
        <rdfs:comment>The exact value of a measurement.</rdfs:comment>
        <skos:definition>The exact value of a measurement.</skos:definition>
        <dc:description>Used for measurements yielding only one exact value. To denote value ranges use abcd:LowerValue and abcd:UpperValue.</dc:description>
        <rdfs:domain rdf:resource="http://www.w3.org/2002/07/owl#Thing"/>
        <rdfs:range rdf:resource="http://www.w3.org/2001/XMLSchema#string"/>
        <skos:exactMatch rdf:resource="http://rs.tdwg.org/dwc/terms/measurementValue"/>
    </owl:DatatypeProperty>

    <owl:FunctionalProperty rdf:about="exactValue"/>

    <owl:DatatypeProperty rdf:about="exposureMode">
        <rdfs:label xml:lang="en">Exposure Mode</rdfs:label>
        <rdfs:isDefinedBy rdf:resource="http://rs.tdwg.org/abcd/terms/"/>
        <dwcattributes:status>recommended</dwcattributes:status>
        <dcterms:issued>2019-01-31</dcterms:issued>
        <dcterms:modified>2019-01-31</dcterms:modified>
        <rdfs:comment>This property indicates the exposure mode set when the image was shot. This is an EXIF term.</rdfs:comment>
        <skos:definition>This property indicates the exposure mode set when the image was shot. This is an EXIF term.</skos:definition>
        <dc:description>In auto-bracketing mode, the camera shoots a series of frames of the same scene at different exposure settings.</dc:description>
        <dc:description>The specification defines three values: auto-exposure (0), manual exposure (1) and auto-bracket (2).</dc:description>
        <rdfs:domain rdf:resource="http://www.w3.org/2002/07/owl#Thing"/>
        <rdfs:range rdf:resource="http://www.w3.org/2001/XMLSchema#string"/>
    </owl:DatatypeProperty>

    <owl:DatatypeProperty rdf:about="exposureTime">
        <rdfs:label xml:lang="en">Exposure Time</rdfs:label>
        <rdfs:isDefinedBy rdf:resource="http://rs.tdwg.org/abcd/terms/"/>
        <dwcattributes:status>recommended</dwcattributes:status>
        <dcterms:issued>2019-01-31</dcterms:issued>
        <dcterms:modified>2019-01-31</dcterms:modified>
        <rdfs:comment>EXIF term. Exposure time, given in seconds.</rdfs:comment>
        <skos:definition>EXIF term. Exposure time, given in seconds.</skos:definition>
        <rdfs:domain rdf:resource="http://www.w3.org/2002/07/owl#Thing"/>
        <rdfs:range rdf:resource="http://www.w3.org/2001/XMLSchema#string"/>
    </owl:DatatypeProperty>

    <owl:DatatypeProperty rdf:about="exsiccatum">
        <rdfs:label xml:lang="en">Exsiccatum</rdfs:label>
        <rdfs:isDefinedBy rdf:resource="http://rs.tdwg.org/abcd/terms/"/>
        <dwcattributes:status>recommended</dwcattributes:status>
        <dcterms:issued>2019-01-31</dcterms:issued>
        <dcterms:modified>2019-01-31</dcterms:modified>
        <rdfs:comment>Information relating a specimen to an Exsiccatum.</rdfs:comment>
        <skos:definition>Information relating a specimen to an Exsiccatum.</skos:definition>
        <rdfs:domain rdf:resource="http://www.w3.org/2002/07/owl#Thing"/>
        <rdfs:range rdf:resource="http://www.w3.org/2001/XMLSchema#string"/>
    </owl:DatatypeProperty>

    <owl:FunctionalProperty rdf:about="exsiccatum"/>

    <owl:DatatypeProperty rdf:about="fieldNotes">
        <rdfs:label xml:lang="en">Field Notes</rdfs:label>
        <rdfs:isDefinedBy rdf:resource="http://rs.tdwg.org/abcd/terms/"/>
        <dwcattributes:status>recommended</dwcattributes:status>
        <dcterms:issued>2019-01-31</dcterms:issued>
        <dcterms:modified>2019-01-31</dcterms:modified>
        <rdfs:comment>Notes taken in the field for the object or observation.</rdfs:comment>
        <skos:definition>Notes taken in the field for the object or observation.</skos:definition>
        <dc:description>If field notes exist, but are not published (dwc:fieldNotes use case a), this property should not be used, instead it should be noted using the abcd:InformationWidthheld property either on the Unit or DataSet level.</dc:description>
        <rdfs:domain rdf:resource="http://www.w3.org/2002/07/owl#Thing"/>
        <rdfs:range rdf:resource="http://www.w3.org/2001/XMLSchema#string"/>
        <skos:relatedMatch rdf:resource="http://rs.tdwg.org/dwc/terms/fieldNotes"/>
    </owl:DatatypeProperty>

    <owl:DatatypeProperty rdf:about="fileFormat">
        <rdfs:label xml:lang="en">File Format</rdfs:label>
        <rdfs:isDefinedBy rdf:resource="http://rs.tdwg.org/abcd/terms/"/>
        <dwcattributes:status>recommended</dwcattributes:status>
        <dcterms:issued>2019-01-31</dcterms:issued>
        <dcterms:modified>2019-01-31</dcterms:modified>
        <rdfs:comment>A code or descriptive term for the file or object format.</rdfs:comment>
        <skos:definition>A code or descriptive term for the file or object format.</skos:definition>
        <rdfs:domain rdf:resource="http://www.w3.org/2002/07/owl#Thing"/>
        <rdfs:range rdf:resource="http://www.w3.org/2001/XMLSchema#string"/>
    </owl:DatatypeProperty>

    <owl:DatatypeProperty rdf:about="fileSize">
        <rdfs:label xml:lang="en">File Size</rdfs:label>
        <rdfs:isDefinedBy rdf:resource="http://rs.tdwg.org/abcd/terms/"/>
        <dwcattributes:status>recommended</dwcattributes:status>
        <dcterms:issued>2019-01-31</dcterms:issued>
        <dcterms:modified>2019-01-31</dcterms:modified>
        <rdfs:comment>The size of the file of the multimedia object.</rdfs:comment>
        <skos:definition>The size of the file of the multimedia object.</skos:definition>
        <dc:description>Sizes should be expressed in kB (kilo byte) or MB (mega byte) including the unit abbreviation.</dc:description>
        <rdfs:domain rdf:resource="http://www.w3.org/2002/07/owl#Thing"/>
        <rdfs:range rdf:resource="http://www.w3.org/2001/XMLSchema#string"/>
    </owl:DatatypeProperty>

    <owl:FunctionalProperty rdf:about="fileSize"/>

    <owl:DatatypeProperty rdf:about="fileURL">
        <rdfs:label xml:lang="en">File URL</rdfs:label>
        <rdfs:isDefinedBy rdf:resource="http://rs.tdwg.org/abcd/terms/"/>
        <dwcattributes:status>recommended</dwcattributes:status>
        <dcterms:issued>2019-01-31</dcterms:issued>
        <dcterms:modified>2019-01-31</dcterms:modified>
        <rdfs:comment>The URL to directly access the underlying multimedia file.</rdfs:comment>
        <skos:definition>The URL to directly access the underlying multimedia file.</skos:definition>
        <rdfs:domain rdf:resource="http://www.w3.org/2002/07/owl#Thing"/>
        <rdfs:range rdf:resource="http://www.w3.org/2001/XMLSchema#anyURI"/>
    </owl:DatatypeProperty>

    <owl:FunctionalProperty rdf:about="fileURL"/>

    <owl:DatatypeProperty rdf:about="filterUsedForRecording">
        <rdfs:label xml:lang="en">Filter Used For Recording</rdfs:label>
        <rdfs:isDefinedBy rdf:resource="http://rs.tdwg.org/abcd/terms/"/>
        <dwcattributes:status>recommended</dwcattributes:status>
        <dcterms:issued>2019-01-31</dcterms:issued>
        <dcterms:modified>2019-01-31</dcterms:modified>
        <rdfs:domain rdf:resource="http://www.w3.org/2002/07/owl#Thing"/>
        <rdfs:range rdf:resource="http://www.w3.org/2001/XMLSchema#string"/>
    </owl:DatatypeProperty>

    <owl:DatatypeProperty rdf:about="firstEpithet">
        <rdfs:label xml:lang="en">First Epithet</rdfs:label>
        <rdfs:isDefinedBy rdf:resource="http://rs.tdwg.org/abcd/terms/"/>
        <dwcattributes:status>recommended</dwcattributes:status>
        <dcterms:issued>2019-01-31</dcterms:issued>
        <dcterms:modified>2019-01-31</dcterms:modified>
        <rdfs:comment>The first epithet in a botanical name combination identified for the unit(species epithet or the epithet of the subdivision of a genus).</rdfs:comment>
        <skos:definition>The first epithet in a botanical name combination identified for the unit(species epithet or the epithet of the subdivision of a genus).</skos:definition>
        <rdfs:domain rdf:resource="http://www.w3.org/2002/07/owl#Thing"/>
        <rdfs:range rdf:resource="http://www.w3.org/2001/XMLSchema#string"/>
    </owl:DatatypeProperty>

    <owl:FunctionalProperty rdf:about="firstEpithet"/>

    <owl:DatatypeProperty rdf:about="flash">
        <rdfs:label xml:lang="en">Flash</rdfs:label>
        <rdfs:isDefinedBy rdf:resource="http://rs.tdwg.org/abcd/terms/"/>
        <dwcattributes:status>recommended</dwcattributes:status>
        <dcterms:issued>2019-01-31</dcterms:issued>
        <dcterms:modified>2019-01-31</dcterms:modified>
        <rdfs:comment>This tag indicates the flash status when the picture was taken, as a human readable value.</rdfs:comment>
        <skos:definition>This tag indicates the flash status when the picture was taken, as a human readable value.</skos:definition>
        <dc:description>This element is related to Flash in Exif/DCFwriter, however in there formats, a short value is used to denote the status of the flash in 6 bits. In this field the human readable interpretation of these bits is expected.</dc:description>
        <rdfs:domain rdf:resource="http://www.w3.org/2002/07/owl#Thing"/>
        <rdfs:range rdf:resource="http://www.w3.org/2001/XMLSchema#string"/>
    </owl:DatatypeProperty>

    <owl:DatatypeProperty rdf:about="flashEnergy">
        <rdfs:label xml:lang="en">Flash Energy</rdfs:label>
        <rdfs:isDefinedBy rdf:resource="http://rs.tdwg.org/abcd/terms/"/>
        <dwcattributes:status>recommended</dwcattributes:status>
        <dcterms:issued>2019-01-31</dcterms:issued>
        <dcterms:modified>2019-01-31</dcterms:modified>
        <rdfs:comment>Indicates the strobe energy at the time the image is captured, as measured in Beam Candle Power Seconds (BCPS).</rdfs:comment>
        <skos:definition>Indicates the strobe energy at the time the image is captured, as measured in Beam Candle Power Seconds (BCPS).</skos:definition>
        <rdfs:domain rdf:resource="http://www.w3.org/2002/07/owl#Thing"/>
        <rdfs:range rdf:resource="http://www.w3.org/2001/XMLSchema#string"/>
    </owl:DatatypeProperty>

    <owl:DatatypeProperty rdf:about="focalLength">
        <rdfs:label xml:lang="en">Focal Length</rdfs:label>
        <rdfs:isDefinedBy rdf:resource="http://rs.tdwg.org/abcd/terms/"/>
        <dwcattributes:status>recommended</dwcattributes:status>
        <dcterms:issued>2019-01-31</dcterms:issued>
        <dcterms:modified>2019-01-31</dcterms:modified>
        <rdfs:comment>The actual focal length of the lens, in mm.</rdfs:comment>
        <skos:definition>The actual focal length of the lens, in mm.</skos:definition>
        <dc:description>Conversion is not made to the focal length of a 35 mm film camera, use the property abcd:focalLengthIn35mmFilm for this instead.</dc:description>
        <rdfs:domain rdf:resource="http://www.w3.org/2002/07/owl#Thing"/>
        <rdfs:range rdf:resource="http://www.w3.org/2001/XMLSchema#decimal"/>
    </owl:DatatypeProperty>

    <owl:DatatypeProperty rdf:about="focalLengthIn35mmFilm">
        <rdfs:label xml:lang="en">Focal Length In 35 mm Film</rdfs:label>
        <rdfs:isDefinedBy rdf:resource="http://rs.tdwg.org/abcd/terms/"/>
        <dwcattributes:status>recommended</dwcattributes:status>
        <dcterms:issued>2019-01-31</dcterms:issued>
        <dcterms:modified>2019-01-31</dcterms:modified>
        <rdfs:comment>This tag indicates the equivalent focal length assuming a 35 mm film camera, in mm.</rdfs:comment>
        <skos:definition>This tag indicates the equivalent focal length assuming a 35 mm film camera, in mm.</skos:definition>
        <rdfs:subPropertyOf rdf:resource="focalLength"/>
        <dc:description>For the actual focal length of the camera, please use the property abcd:focalLength.</dc:description>
        <rdfs:domain rdf:resource="http://www.w3.org/2002/07/owl#Thing"/>
        <rdfs:range rdf:resource="http://www.w3.org/2001/XMLSchema#string"/>
    </owl:DatatypeProperty>

    <owl:DatatypeProperty rdf:about="footprintSpatialFit">
        <rdfs:label xml:lang="en">Footprint Spatial Fit</rdfs:label>
        <rdfs:isDefinedBy rdf:resource="http://rs.tdwg.org/abcd/terms/"/>
        <dwcattributes:status>recommended</dwcattributes:status>
        <dcterms:issued>2019-01-31</dcterms:issued>
        <dcterms:modified>2019-01-31</dcterms:modified>
        <rdfs:comment>A measure of how well the geometry expressed in the abcd:FootprintWKT match the original spatial representation, as a ratio of the area of the footprint given to the area of the original spatial representation.</rdfs:comment>
        <skos:definition>A measure of how well the geometry expressed in the abcd:FootprintWKT match the original spatial representation, as a ratio of the area of the footprint given to the area of the original spatial representation.</skos:definition>
        <dc:description>If both the original and the given georeference are the same point, the FootprintSpatialFit is 1. Detailed explanations with graphical examples can be found in the Guide to Best Practices for Georeferencing (Chapman and Wieczorek, eds. 2006)</dc:description>
        <dc:description>Legal values are 0, greater than or equal to 1, or undefined. A value of 1 is an exact match or 100% overlap. A value of 0 should be used if the given georeference does not completely contain the original representation. The FootprintSpatialFit is undefined if the original representation is a point without uncertainty and the given georeference is not that same point (without uncertainty).</dc:description>
        <rdfs:domain rdf:resource="http://www.w3.org/2002/07/owl#Thing"/>
        <rdfs:range rdf:resource="http://www.w3.org/2001/XMLSchema#string"/>
        <skos:exactMatch rdf:resource="http://rs.tdwg.org/dwc/terms/footprintSpatialFit"/>
    </owl:DatatypeProperty>

    <owl:FunctionalProperty rdf:about="footprintSpatialFit"/>

    <owl:DatatypeProperty rdf:about="footprintWKT">
        <rdfs:label xml:lang="en">Footprint WKT</rdfs:label>
        <rdfs:isDefinedBy rdf:resource="http://rs.tdwg.org/abcd/terms/"/>
        <dwcattributes:status>recommended</dwcattributes:status>
        <dcterms:issued>2019-01-31</dcterms:issued>
        <dcterms:modified>2019-01-31</dcterms:modified>
        <rdfs:comment>A Well-Known Text (WKT; see http://en.wikipedia.org/wiki/Well-known_text) representation of the shape (footprint) that defines the gathering site.</rdfs:comment>
        <skos:definition>A Well-Known Text (WKT; see http://en.wikipedia.org/wiki/Well-known_text) representation of the shape (footprint) that defines the gathering site.</skos:definition>
        <rdfs:domain rdf:resource="http://www.w3.org/2002/07/owl#Thing"/>
        <rdfs:range rdf:resource="http://www.w3.org/2001/XMLSchema#string"/>
        <skos:exactMatch rdf:resource="http://rs.tdwg.org/dwc/terms/footprintWKT"/>
    </owl:DatatypeProperty>

    <owl:FunctionalProperty rdf:about="footprintWKT"/>

    <owl:DatatypeProperty rdf:about="form">
        <rdfs:label xml:lang="en">Form</rdfs:label>
        <rdfs:isDefinedBy rdf:resource="http://rs.tdwg.org/abcd/terms/"/>
        <dwcattributes:status>recommended</dwcattributes:status>
        <dcterms:issued>2019-01-31</dcterms:issued>
        <dcterms:modified>2019-01-31</dcterms:modified>
        <rdfs:comment>The original or a mold, cast etc. of the specimen.</rdfs:comment>
        <skos:definition>The original or a mold, cast etc. of the specimen.</skos:definition>
        <rdfs:domain rdf:resource="http://www.w3.org/2002/07/owl#Thing"/>
        <rdfs:range rdf:resource="http://www.w3.org/2001/XMLSchema#string"/>
    </owl:DatatypeProperty>

    <owl:FunctionalProperty rdf:about="form"/>

    <owl:DatatypeProperty rdf:about="formOfSupply">
        <rdfs:label xml:lang="en">Form Of Supply</rdfs:label>
        <rdfs:isDefinedBy rdf:resource="http://rs.tdwg.org/abcd/terms/"/>
        <dwcattributes:status>recommended</dwcattributes:status>
        <dcterms:issued>2019-01-31</dcterms:issued>
        <dcterms:modified>2019-01-31</dcterms:modified>
        <rdfs:comment>Form in which the strain will be sent to the customer.</rdfs:comment>
        <skos:definition>Form in which the strain will be sent to the customer.</skos:definition>
        <rdfs:domain rdf:resource="http://www.w3.org/2002/07/owl#Thing"/>
        <rdfs:range rdf:resource="http://www.w3.org/2001/XMLSchema#string"/>
    </owl:DatatypeProperty>

    <owl:FunctionalProperty rdf:about="formOfSupply"/>

    <owl:DatatypeProperty rdf:about="framerate">
        <rdfs:label xml:lang="en">Framerate</rdfs:label>
        <rdfs:isDefinedBy rdf:resource="http://rs.tdwg.org/abcd/terms/"/>
        <dwcattributes:status>recommended</dwcattributes:status>
        <dcterms:issued>2019-01-31</dcterms:issued>
        <dcterms:modified>2019-01-31</dcterms:modified>
        <rdfs:comment>The number of frames per second a video file is supposed to be played at.</rdfs:comment>
        <skos:definition>The number of frames per second a video file is supposed to be played at.</skos:definition>
        <rdfs:domain rdf:resource="http://www.w3.org/2002/07/owl#Thing"/>
        <rdfs:range rdf:resource="http://www.w3.org/2001/XMLSchema#string"/>
    </owl:DatatypeProperty>

    <owl:FunctionalProperty rdf:about="framerate"/>

    <owl:DatatypeProperty rdf:about="fullName">
        <rdfs:label xml:lang="en">Full Name</rdfs:label>
        <rdfs:isDefinedBy rdf:resource="http://rs.tdwg.org/abcd/terms/"/>
        <dwcattributes:status>recommended</dwcattributes:status>
        <dcterms:issued>2019-01-31</dcterms:issued>
        <dcterms:modified>2019-01-31</dcterms:modified>
        <rdfs:comment>String of the preferred form of personal name for displaying.</rdfs:comment>
        <skos:definition>String of the preferred form of personal name for displaying.</skos:definition>
        <dc:description>To be used when no atomized name is available or to display the preferred combination of name particles. May include titles.</dc:description>
        <rdfs:domain rdf:resource="http://www.w3.org/2002/07/owl#Thing"/>
        <rdfs:range rdf:resource="http://www.w3.org/2001/XMLSchema#string"/>
        <skos:exactMatch rdf:resource="http://www.w3.org/2006/vcard/ns#fn"/>
        <skos:exactMatch rdf:resource="http://xmlns.com/foaf/0.1/name"/>
    </owl:DatatypeProperty>

    <owl:FunctionalProperty rdf:about="fullName"/>

    <owl:DatatypeProperty rdf:about="fullScientificName">
        <rdfs:label xml:lang="en">Full Scientific Name</rdfs:label>
        <rdfs:isDefinedBy rdf:resource="http://rs.tdwg.org/abcd/terms/"/>
        <dwcattributes:status>recommended</dwcattributes:status>
        <dcterms:issued>2019-01-31</dcterms:issued>
        <dcterms:modified>2019-01-31</dcterms:modified>
        <rdfs:comment>A concatenated scientific name formed in the unit identification.</rdfs:comment>
        <skos:definition>A concatenated scientific name formed in the unit identification.</skos:definition>
        <dc:description>The Full Scientific Name as preferably formed in accordance with a Code of Nomenclature as fully as possible (i. e. a monomial, bionomial, or trinomial plus author[s] or author team[s] and - where relevant - year, or the full name of a cultivar or cultivar group, or a hybrid formula or named hybrid).</dc:description>
        <rdfs:domain rdf:resource="http://www.w3.org/2002/07/owl#Thing"/>
        <rdfs:range rdf:resource="http://www.w3.org/2001/XMLSchema#string"/>
        <skos:exactMatch rdf:resource="http://rs.tdwg.org/dwc/terms/scientificName"/>
    </owl:DatatypeProperty>

    <owl:FunctionalProperty rdf:about="fullScientificName"/>

    <owl:DatatypeProperty rdf:about="guid">
        <rdfs:label xml:lang="en">GUID</rdfs:label>
        <rdfs:isDefinedBy rdf:resource="http://rs.tdwg.org/abcd/terms/"/>
        <dwcattributes:status>recommended</dwcattributes:status>
        <dcterms:issued>2019-01-31</dcterms:issued>
        <dcterms:modified>2019-01-31</dcterms:modified>
        <rdfs:comment>The globally unique identifier of a class.</rdfs:comment>
        <skos:definition>The globally unique identifier of a class.</skos:definition>
        <rdfs:domain rdf:resource="http://www.w3.org/2002/07/owl#Thing"/>
        <rdfs:range rdf:resource="http://www.w3.org/2001/XMLSchema#string"/>
    </owl:DatatypeProperty>

    <owl:DatatypeProperty rdf:about="gamma">
        <rdfs:label xml:lang="en">Gamma</rdfs:label>
        <rdfs:isDefinedBy rdf:resource="http://rs.tdwg.org/abcd/terms/"/>
        <dwcattributes:status>recommended</dwcattributes:status>
        <dcterms:issued>2019-01-31</dcterms:issued>
        <dcterms:modified>2019-01-31</dcterms:modified>
        <rdfs:comment>Indicates the value of coefficient gamma used in gamma correction.</rdfs:comment>
        <skos:definition>Indicates the value of coefficient gamma used in gamma correction.</skos:definition>
        <dc:description>The formula of transfer function used for image reproduction is expressed as follows: (Reproduced value) = (Input value)^gamma.</dc:description>
        <rdfs:domain rdf:resource="http://www.w3.org/2002/07/owl#Thing"/>
        <rdfs:range rdf:resource="http://www.w3.org/2001/XMLSchema#string"/>
    </owl:DatatypeProperty>

    <owl:DatatypeProperty rdf:about="gatheringInstitutionCode">
        <rdfs:label xml:lang="en">Gathering Institution Code</rdfs:label>
        <rdfs:isDefinedBy rdf:resource="http://rs.tdwg.org/abcd/terms/"/>
        <dwcattributes:status>recommended</dwcattributes:status>
        <dcterms:issued>2019-01-31</dcterms:issued>
        <dcterms:modified>2019-01-31</dcterms:modified>
        <rdfs:comment>FAO Code of the institution responsible for the collection of the unit.</rdfs:comment>
        <skos:definition>FAO Code of the institution responsible for the collection of the unit.</skos:definition>
        <rdfs:domain rdf:resource="http://www.w3.org/2002/07/owl#Thing"/>
        <rdfs:range rdf:resource="http://www.w3.org/2001/XMLSchema#integer"/>
    </owl:DatatypeProperty>

    <owl:FunctionalProperty rdf:about="gatheringInstitutionCode"/>

    <owl:DatatypeProperty rdf:about="genotype">
        <rdfs:label xml:lang="en">Genotype</rdfs:label>
        <rdfs:isDefinedBy rdf:resource="http://rs.tdwg.org/abcd/terms/"/>
        <dwcattributes:status>recommended</dwcattributes:status>
        <dcterms:issued>2019-01-31</dcterms:issued>
        <dcterms:modified>2019-01-31</dcterms:modified>
        <rdfs:comment>Names of chromosomal markers of the strain.</rdfs:comment>
        <skos:definition>Names of chromosomal markers of the strain.</skos:definition>
        <dc:description>Especially recommended for strains of species for which many genetically modified strains exist.</dc:description>
        <rdfs:domain rdf:resource="http://www.w3.org/2002/07/owl#Thing"/>
        <rdfs:range rdf:resource="http://www.w3.org/2001/XMLSchema#string"/>
    </owl:DatatypeProperty>

    <owl:FunctionalProperty rdf:about="genotype"/>

    <owl:DatatypeProperty rdf:about="genusOrMonomial">
        <rdfs:label xml:lang="en">Genus Or Monomial</rdfs:label>
        <rdfs:isDefinedBy rdf:resource="http://rs.tdwg.org/abcd/terms/"/>
        <dwcattributes:status>recommended</dwcattributes:status>
        <dcterms:issued>2019-01-31</dcterms:issued>
        <dcterms:modified>2019-01-31</dcterms:modified>
        <rdfs:comment>The genus as part or only result of an identification or a higher taxon name representing that result.</rdfs:comment>
        <skos:definition>The genus as part or only result of an identification or a higher taxon name representing that result.</skos:definition>
        <rdfs:domain rdf:resource="http://www.w3.org/2002/07/owl#Thing"/>
        <rdfs:range rdf:resource="http://www.w3.org/2001/XMLSchema#string"/>
        <skos:exactMatch rdf:resource="http://rs.tdwg.org/dwc/terms/genus"/>
    </owl:DatatypeProperty>

    <owl:FunctionalProperty rdf:about="genusOrMonomial"/>

    <owl:DatatypeProperty rdf:about="geoecologicalTerm">
        <rdfs:label xml:lang="en">Geoecological Term</rdfs:label>
        <rdfs:isDefinedBy rdf:resource="http://rs.tdwg.org/abcd/terms/"/>
        <dwcattributes:status>recommended</dwcattributes:status>
        <dcterms:issued>2019-01-31</dcterms:issued>
        <dcterms:modified>2019-01-31</dcterms:modified>
        <rdfs:comment>An area name describing the - or part of the - geoecological scope of a data set.</rdfs:comment>
        <skos:definition>An area name describing the - or part of the - geoecological scope of a data set.</skos:definition>
        <rdfs:subPropertyOf rdf:resource="scope"/>
        <rdfs:domain rdf:resource="http://www.w3.org/2002/07/owl#Thing"/>
        <rdfs:range rdf:resource="http://www.w3.org/2001/XMLSchema#string"/>
    </owl:DatatypeProperty>

    <owl:DatatypeProperty rdf:about="givenNames">
        <rdfs:label xml:lang="en">Given Names</rdfs:label>
        <rdfs:isDefinedBy rdf:resource="http://rs.tdwg.org/abcd/terms/"/>
        <dwcattributes:status>recommended</dwcattributes:status>
        <dcterms:issued>2019-01-31</dcterms:issued>
        <dcterms:modified>2019-01-31</dcterms:modified>
        <rdfs:comment>The name of a person, which is the first or Christian name in western cultures as well as any additional given names e.g. middle name.</rdfs:comment>
        <skos:definition>The name of a person, which is the first or Christian name in western cultures as well as any additional given names e.g. middle name.</skos:definition>
        <dc:description>May include several names separated by spaces.</dc:description>
        <rdfs:domain rdf:resource="http://www.w3.org/2002/07/owl#Thing"/>
        <rdfs:range rdf:resource="http://www.w3.org/2001/XMLSchema#string"/>
        <skos:relatedMatch rdf:resource="http://www.w3.org/2006/vcard/ns#additional-name"/>
        <skos:relatedMatch rdf:resource="http://www.w3.org/2006/vcard/ns#given-name"/>
        <skos:exactMatch rdf:resource="http://xmlns.com/foaf/0.1/givenName"/>
    </owl:DatatypeProperty>

    <owl:FunctionalProperty rdf:about="givenNames"/>

    <owl:DatatypeProperty rdf:about="gridCellCode">
        <rdfs:label xml:lang="en">Grid Cell Code</rdfs:label>
        <rdfs:isDefinedBy rdf:resource="http://rs.tdwg.org/abcd/terms/"/>
        <dwcattributes:status>recommended</dwcattributes:status>
        <dcterms:issued>2019-01-31</dcterms:issued>
        <dcterms:modified>2019-01-31</dcterms:modified>
        <rdfs:comment>The code of the grid system used to record coordinates.</rdfs:comment>
        <skos:definition>The code of the grid system used to record coordinates.</skos:definition>
        <rdfs:domain rdf:resource="http://www.w3.org/2002/07/owl#Thing"/>
        <rdfs:range rdf:resource="http://www.w3.org/2001/XMLSchema#string"/>
    </owl:DatatypeProperty>

    <owl:FunctionalProperty rdf:about="gridCellCode"/>

    <owl:DatatypeProperty rdf:about="gridCellSystem">
        <rdfs:label xml:lang="en">Grid Cell System</rdfs:label>
        <rdfs:isDefinedBy rdf:resource="http://rs.tdwg.org/abcd/terms/"/>
        <dwcattributes:status>recommended</dwcattributes:status>
        <dcterms:issued>2019-01-31</dcterms:issued>
        <dcterms:modified>2019-01-31</dcterms:modified>
        <rdfs:comment>The name of the grid system used for grid coordinates.</rdfs:comment>
        <skos:definition>The name of the grid system used for grid coordinates.</skos:definition>
        <rdfs:domain rdf:resource="http://www.w3.org/2002/07/owl#Thing"/>
        <rdfs:range rdf:resource="http://www.w3.org/2001/XMLSchema#string"/>
    </owl:DatatypeProperty>

    <owl:FunctionalProperty rdf:about="gridCellSystem"/>

    <owl:DatatypeProperty rdf:about="gridQualifier">
        <rdfs:label xml:lang="en">Grid Qualifier</rdfs:label>
        <rdfs:isDefinedBy rdf:resource="http://rs.tdwg.org/abcd/terms/"/>
        <dwcattributes:status>recommended</dwcattributes:status>
        <dcterms:issued>2019-01-31</dcterms:issued>
        <dcterms:modified>2019-01-31</dcterms:modified>
        <rdfs:comment>A grid reference precision qualifier for coordinates.</rdfs:comment>
        <skos:definition>A grid reference precision qualifier for coordinates.</skos:definition>
        <rdfs:domain rdf:resource="http://www.w3.org/2002/07/owl#Thing"/>
        <rdfs:range rdf:resource="http://www.w3.org/2001/XMLSchema#string"/>
    </owl:DatatypeProperty>

    <owl:FunctionalProperty rdf:about="gridQualifier"/>

    <owl:DatatypeProperty rdf:about="growthConditionsText">
        <rdfs:label xml:lang="en">Growth Conditions Text</rdfs:label>
        <rdfs:isDefinedBy rdf:resource="http://rs.tdwg.org/abcd/terms/"/>
        <dwcattributes:status>recommended</dwcattributes:status>
        <dcterms:issued>2019-01-31</dcterms:issued>
        <dcterms:modified>2019-01-31</dcterms:modified>
        <rdfs:comment>An alternative full text field for the culture medium, atmospheric and light conditions, temperature conditions, and additional remarks on the cultivation.</rdfs:comment>
        <skos:definition>An alternative full text field for the culture medium, atmospheric and light conditions, temperature conditions, and additional remarks on the cultivation.</skos:definition>
        <rdfs:domain rdf:resource="http://www.w3.org/2002/07/owl#Thing"/>
        <rdfs:range rdf:resource="http://www.w3.org/2001/XMLSchema#string"/>
    </owl:DatatypeProperty>

    <owl:FunctionalProperty rdf:about="growthConditionsText"/>

    <owl:DatatypeProperty rdf:about="hardiness">
        <rdfs:label xml:lang="en">Hardiness</rdfs:label>
        <rdfs:isDefinedBy rdf:resource="http://rs.tdwg.org/abcd/terms/"/>
        <dwcattributes:status>recommended</dwcattributes:status>
        <dcterms:issued>2019-01-31</dcterms:issued>
        <dcterms:modified>2019-01-31</dcterms:modified>
        <rdfs:comment>A flag indicating that the accession is grown outdoors in the botanical garden.</rdfs:comment>
        <skos:definition>A flag indicating that the accession is grown outdoors in the botanical garden.</skos:definition>
        <rdfs:domain rdf:resource="http://www.w3.org/2002/07/owl#Thing"/>
        <rdfs:range rdf:resource="http://www.w3.org/2001/XMLSchema#boolean"/>
    </owl:DatatypeProperty>

    <owl:FunctionalProperty rdf:about="hardiness"/>

    <owl:DatatypeProperty rdf:about="hazard">
        <rdfs:label xml:lang="en">Hazard</rdfs:label>
        <rdfs:isDefinedBy rdf:resource="http://rs.tdwg.org/abcd/terms/"/>
        <dwcattributes:status>recommended</dwcattributes:status>
        <dcterms:issued>2019-01-31</dcterms:issued>
        <dcterms:modified>2019-01-31</dcterms:modified>
        <rdfs:domain rdf:resource="http://www.w3.org/2002/07/owl#Thing"/>
        <rdfs:range rdf:resource="http://www.w3.org/2001/XMLSchema#string"/>
    </owl:DatatypeProperty>

    <owl:FunctionalProperty rdf:about="hazard"/>

    <owl:DatatypeProperty rdf:about="height">
        <rdfs:label xml:lang="en">Height</rdfs:label>
        <rdfs:isDefinedBy rdf:resource="http://rs.tdwg.org/abcd/terms/"/>
        <dwcattributes:status>recommended</dwcattributes:status>
        <dcterms:issued>2019-01-31</dcterms:issued>
        <dcterms:modified>2019-01-31</dcterms:modified>
        <rdfs:comment>An image or video height in pixels.</rdfs:comment>
        <skos:definition>An image or video height in pixels.</skos:definition>
        <rdfs:domain rdf:resource="http://www.w3.org/2002/07/owl#Thing"/>
        <rdfs:range rdf:resource="http://www.w3.org/2001/XMLSchema#integer"/>
    </owl:DatatypeProperty>

    <owl:FunctionalProperty rdf:about="height"/>

    <owl:DatatypeProperty rdf:about="hybridFlag">
        <rdfs:label xml:lang="en">Hybrid Flag</rdfs:label>
        <rdfs:isDefinedBy rdf:resource="http://rs.tdwg.org/abcd/terms/"/>
        <dwcattributes:status>recommended</dwcattributes:status>
        <dcterms:issued>2019-01-31</dcterms:issued>
        <dcterms:modified>2019-01-31</dcterms:modified>
        <rdfs:comment>A flag indicating that the unit identified is a named hybrid or a graft chimaera.</rdfs:comment>
        <skos:definition>A flag indicating that the unit identified is a named hybrid or a graft chimaera.</skos:definition>
        <rdfs:domain rdf:resource="http://www.w3.org/2002/07/owl#Thing"/>
        <rdfs:range rdf:resource="http://www.w3.org/2001/XMLSchema#string"/>
    </owl:DatatypeProperty>

    <owl:FunctionalProperty rdf:about="hybridFlag"/>

    <owl:DatatypeProperty rdf:about="hybridFlagInsertionPoint">
        <rdfs:label xml:lang="en">Hybrid Flag Insertion Point</rdfs:label>
        <rdfs:isDefinedBy rdf:resource="http://rs.tdwg.org/abcd/terms/"/>
        <dwcattributes:status>recommended</dwcattributes:status>
        <dcterms:issued>2019-01-31</dcterms:issued>
        <dcterms:modified>2019-01-31</dcterms:modified>
        <rdfs:comment>An indicator of the insertion point of the abcd:hybridFlag.</rdfs:comment>
        <skos:definition>An indicator of the insertion point of the abcd:hybridFlag.</skos:definition>
        <dc:description>The insertion point defines the name element in front of which the hybrid flag should be inserted (1 = before entire name, 2 = before first epithet, 3 = before second epithet)</dc:description>
        <rdfs:domain rdf:resource="http://www.w3.org/2002/07/owl#Thing"/>
        <rdfs:range rdf:resource="http://www.w3.org/2001/XMLSchema#integer"/>
    </owl:DatatypeProperty>

    <owl:FunctionalProperty rdf:about="hybridFlagInsertionPoint"/>

    <owl:DatatypeProperty rdf:about="id">
        <rdfs:label xml:lang="en">ID</rdfs:label>
        <rdfs:isDefinedBy rdf:resource="http://rs.tdwg.org/abcd/terms/"/>
        <dwcattributes:status>recommended</dwcattributes:status>
        <dcterms:issued>2019-01-31</dcterms:issued>
        <dcterms:modified>2019-01-31</dcterms:modified>
        <rdfs:comment>Code or Identifier of a class (unique within its local context).</rdfs:comment>
        <skos:definition>Code or Identifier of a class (unique within its local context).</skos:definition>
        <dc:description>For globally unique identifiers (e.g. resolvable HTTP URIs) use abcd:GUID.</dc:description>
        <rdfs:domain rdf:resource="http://www.w3.org/2002/07/owl#Thing"/>
        <rdfs:range rdf:resource="http://www.w3.org/2001/XMLSchema#string"/>
        <skos:exactMatch rdf:resource="http://purl.org/dc/terms/identifier"/>
    </owl:DatatypeProperty>

    <owl:FunctionalProperty rdf:about="id"/>

    <owl:DatatypeProperty rdf:about="ipen">
        <rdfs:label xml:lang="en">IPEN</rdfs:label>
        <rdfs:isDefinedBy rdf:resource="http://rs.tdwg.org/abcd/terms/"/>
        <dwcattributes:status>recommended</dwcattributes:status>
        <dcterms:issued>2019-01-31</dcterms:issued>
        <dcterms:modified>2019-01-31</dcterms:modified>
        <rdfs:comment>A unique number given to plant materials accessioned in conformance with the rules of the International Plant Exchange Network.</rdfs:comment>
        <skos:definition>A unique number given to plant materials accessioned in conformance with the rules of the International Plant Exchange Network.</skos:definition>
        <dc:description>For additional information see https://www.bgci.org/policy/ipen/</dc:description>
        <rdfs:domain rdf:resource="http://www.w3.org/2002/07/owl#Thing"/>
        <rdfs:range rdf:resource="http://www.w3.org/2001/XMLSchema#string"/>
    </owl:DatatypeProperty>

    <owl:FunctionalProperty rdf:about="ipen"/>

    <owl:DatatypeProperty rdf:about="isoSpeed">
        <rdfs:label xml:lang="en">ISO Speed</rdfs:label>
        <rdfs:isDefinedBy rdf:resource="http://rs.tdwg.org/abcd/terms/"/>
        <dwcattributes:status>recommended</dwcattributes:status>
        <dcterms:issued>2019-01-31</dcterms:issued>
        <dcterms:modified>2019-01-31</dcterms:modified>
        <rdfs:comment>This tag indicates the ISO speed value of a camera or input device that is defined in ISO 12232. When recording this tag, the abcd:PhotographicSensitivity properties shall also be recorded.</rdfs:comment>
        <skos:definition>This tag indicates the ISO speed value of a camera or input device that is defined in ISO 12232. When recording this tag, the abcd:PhotographicSensitivity properties shall also be recorded.</skos:definition>
        <rdfs:domain rdf:resource="http://www.w3.org/2002/07/owl#Thing"/>
        <rdfs:range rdf:resource="http://www.w3.org/2001/XMLSchema#string"/>
    </owl:DatatypeProperty>

    <owl:DatatypeProperty rdf:about="iso3166Code">
        <rdfs:label xml:lang="en">ISO3166Code</rdfs:label>
        <rdfs:isDefinedBy rdf:resource="http://rs.tdwg.org/abcd/terms/"/>
        <dwcattributes:status>recommended</dwcattributes:status>
        <dcterms:issued>2019-01-31</dcterms:issued>
        <dcterms:modified>2019-01-31</dcterms:modified>
        <rdfs:comment>A 2-letter (ISO3166-1) or 4-letter (ISO3166-3, for historic countries) code for representation of the name of the country or origin.</rdfs:comment>
        <skos:definition>A 2-letter (ISO3166-1) or 4-letter (ISO3166-3, for historic countries) code for representation of the name of the country or origin.</skos:definition>
        <dc:description>Common used exceptions from the ISO standard are: XA (unknown or unspecified Africa), XB (unknown or unspecified Middle or South America), XC (unknown or unspecified Asia), XD (unknown or unspecified Australia and Oceania), XE (unknown or unspecified Europe), XF (unknown or unspecified North America)</dc:description>
        <rdfs:domain rdf:resource="http://www.w3.org/2002/07/owl#Thing"/>
        <rdfs:range rdf:resource="http://www.w3.org/2001/XMLSchema#string"/>
        <skos:exactMatch rdf:resource="http://rs.tdwg.org/dwc/terms/countryCode"/>
        <skos:exactMatch rdf:resource="http://www.geonames.org/ontology#countryCode"/>
    </owl:DatatypeProperty>

    <owl:FunctionalProperty rdf:about="iso3166Code"/>

    <owl:DatatypeProperty rdf:about="identificationHistory">
        <rdfs:label xml:lang="en">Identification History</rdfs:label>
        <rdfs:isDefinedBy rdf:resource="http://rs.tdwg.org/abcd/terms/"/>
        <dwcattributes:status>recommended</dwcattributes:status>
        <dcterms:issued>2019-01-31</dcterms:issued>
        <dcterms:modified>2019-01-31</dcterms:modified>
        <rdfs:comment>The history of identifications for a Unit (assigned identification results).</rdfs:comment>
        <skos:definition>The history of identifications for a Unit (assigned identification results).</skos:definition>
        <dc:description>This is a free text field for use when extracting data from data sources where the identification or verification history (or part of it) is a free text field. Under normal circumstances the history can be constructed by sorting identification events by date and reference to the preferred identification flag.</dc:description>
        <rdfs:domain rdf:resource="http://www.w3.org/2002/07/owl#Thing"/>
        <rdfs:range rdf:resource="http://www.w3.org/2001/XMLSchema#string"/>
    </owl:DatatypeProperty>

    <owl:FunctionalProperty rdf:about="identificationHistory"/>

    <owl:DatatypeProperty rdf:about="identificationQualifier">
        <rdfs:label xml:lang="en">Identification Qualifier</rdfs:label>
        <rdfs:isDefinedBy rdf:resource="http://rs.tdwg.org/abcd/terms/"/>
        <dwcattributes:status>recommended</dwcattributes:status>
        <dcterms:issued>2019-01-31</dcterms:issued>
        <dcterms:modified>2019-01-31</dcterms:modified>
        <rdfs:comment>A term to qualify the Identification of a Unit when doubts have arisen as to its identity (e.g. "cf." or "aff.").</rdfs:comment>
        <skos:definition>A term to qualify the Identification of a Unit when doubts have arisen as to its identity (e.g. "cf." or "aff.").</skos:definition>
        <rdfs:domain rdf:resource="http://www.w3.org/2002/07/owl#Thing"/>
        <rdfs:range rdf:resource="http://www.w3.org/2001/XMLSchema#string"/>
        <skos:exactMatch rdf:resource="http://rs.tdwg.org/dwc/terms/identificationQualifier"/>
    </owl:DatatypeProperty>

    <owl:FunctionalProperty rdf:about="identificationQualifier"/>

    <owl:DatatypeProperty rdf:about="identificationQualifierInsertionPoint">
        <rdfs:label xml:lang="en">Identification Qualifier Insertion Point</rdfs:label>
        <rdfs:isDefinedBy rdf:resource="http://rs.tdwg.org/abcd/terms/"/>
        <dwcattributes:status>recommended</dwcattributes:status>
        <dcterms:issued>2019-01-31</dcterms:issued>
        <dcterms:modified>2019-01-31</dcterms:modified>
        <rdfs:comment>An indicator of the insertion point of the abcd:identificationQualifier.</rdfs:comment>
        <skos:definition>An indicator of the insertion point of the abcd:identificationQualifier.</skos:definition>
        <dc:description>The attribute @Insertion-Point defines the name element in the scientific name identified for the unit before which the identification qualifier should be inserted (1 = before entire name, 2 =  before first epithet, 3 = before second epithet)</dc:description>
        <rdfs:domain rdf:resource="http://www.w3.org/2002/07/owl#Thing"/>
        <rdfs:range rdf:resource="http://www.w3.org/2001/XMLSchema#nonNegativeInteger"/>
    </owl:DatatypeProperty>

    <owl:FunctionalProperty rdf:about="identificationQualifierInsertionPoint"/>

    <owl:DatatypeProperty rdf:about="identifiedMaterial">
        <rdfs:label xml:lang="en">Identified Material</rdfs:label>
        <rdfs:isDefinedBy rdf:resource="http://rs.tdwg.org/abcd/terms/"/>
        <dwcattributes:status>recommended</dwcattributes:status>
        <dcterms:issued>2019-01-31</dcterms:issued>
        <dcterms:modified>2019-01-31</dcterms:modified>
        <rdfs:comment>A material identified as the result of the unit identification event (e.g. a non-organismic substrate of a microorganism).</rdfs:comment>
        <skos:definition>A material identified as the result of the unit identification event (e.g. a non-organismic substrate of a microorganism).</skos:definition>
        <rdfs:domain rdf:resource="http://www.w3.org/2002/07/owl#Thing"/>
        <rdfs:range rdf:resource="http://www.w3.org/2001/XMLSchema#string"/>
    </owl:DatatypeProperty>

    <owl:DatatypeProperty rdf:about="imageResolution">
        <rdfs:label xml:lang="en">Image Resolution</rdfs:label>
        <rdfs:isDefinedBy rdf:resource="http://rs.tdwg.org/abcd/terms/"/>
        <dwcattributes:status>recommended</dwcattributes:status>
        <dcterms:issued>2019-01-31</dcterms:issued>
        <dcterms:modified>2019-01-31</dcterms:modified>
        <rdfs:comment>The resolution of an image resolution expressed in dots per inch.</rdfs:comment>
        <skos:definition>The resolution of an image resolution expressed in dots per inch.</skos:definition>
        <dc:description>This should only be recorded for images that are either scans from pages or for photographs from flat objects taken in a standardized non-distorting way, e.g. digitized herbarium sheets.</dc:description>
        <rdfs:domain rdf:resource="http://www.w3.org/2002/07/owl#Thing"/>
        <rdfs:range rdf:resource="http://www.w3.org/2001/XMLSchema#integer"/>
    </owl:DatatypeProperty>

    <owl:FunctionalProperty rdf:about="imageResolution"/>

    <owl:DatatypeProperty rdf:about="informalName">
        <rdfs:label xml:lang="en">Informal Name</rdfs:label>
        <rdfs:isDefinedBy rdf:resource="http://rs.tdwg.org/abcd/terms/"/>
        <dwcattributes:status>recommended</dwcattributes:status>
        <dcterms:issued>2019-01-31</dcterms:issued>
        <dcterms:modified>2019-01-31</dcterms:modified>
        <rdfs:comment>The outcome of an Identification event for a Unit that does not adhere to the rule of a Code of Nomenclature. This includes common or vernacular names.</rdfs:comment>
        <skos:definition>The outcome of an Identification event for a Unit that does not adhere to the rule of a Code of Nomenclature. This includes common or vernacular names.</skos:definition>
        <rdfs:domain rdf:resource="http://www.w3.org/2002/07/owl#Thing"/>
        <rdfs:range rdf:resource="http://www.w3.org/2001/XMLSchema#string"/>
        <skos:exactMatch rdf:resource="http://rs.tdwg.org/dwc/terms/vernacularName"/>
    </owl:DatatypeProperty>

    <owl:FunctionalProperty rdf:about="informalName"/>

    <owl:DatatypeProperty rdf:about="informationWithheld">
        <rdfs:label xml:lang="en">Information Withheld</rdfs:label>
        <rdfs:isDefinedBy rdf:resource="http://rs.tdwg.org/abcd/terms/"/>
        <dwcattributes:status>recommended</dwcattributes:status>
        <dcterms:issued>2019-01-31</dcterms:issued>
        <dcterms:modified>2019-01-31</dcterms:modified>
        <rdfs:comment>Brief descriptions of additional information that may exist, but that has not been made public.</rdfs:comment>
        <skos:definition>Brief descriptions of additional information that may exist, but that has not been made public.</skos:definition>
        <dc:description>Information about obtaining the withheld information should be sought from the corresponding Contact (e.g. abcd:hasContentContact for the Data Set).</dc:description>
        <rdfs:domain rdf:resource="http://www.w3.org/2002/07/owl#Thing"/>
        <rdfs:range rdf:resource="http://www.w3.org/2001/XMLSchema#string"/>
        <skos:exactMatch rdf:resource="http://rs.tdwg.org/dwc/iri/informationWithheld"/>
    </owl:DatatypeProperty>

    <owl:DatatypeProperty rdf:about="infraspecificEpithet">
        <rdfs:label xml:lang="en">Infraspecific Epithet</rdfs:label>
        <rdfs:isDefinedBy rdf:resource="http://rs.tdwg.org/abcd/terms/"/>
        <dwcattributes:status>recommended</dwcattributes:status>
        <dcterms:issued>2019-01-31</dcterms:issued>
        <dcterms:modified>2019-01-31</dcterms:modified>
        <rdfs:comment>The final epithet of a botanical name of infraspecific rank.</rdfs:comment>
        <skos:definition>The final epithet of a botanical name of infraspecific rank.</skos:definition>
        <rdfs:domain rdf:resource="http://www.w3.org/2002/07/owl#Thing"/>
        <rdfs:range rdf:resource="http://www.w3.org/2001/XMLSchema#string"/>
        <skos:exactMatch rdf:resource="http://rs.tdwg.org/dwc/terms/infraspecificEpithet"/>
    </owl:DatatypeProperty>

    <owl:FunctionalProperty rdf:about="infraspecificEpithet"/>

    <owl:DatatypeProperty rdf:about="infrasubspecificName">
        <rdfs:label xml:lang="en">Infrasubspecific Name</rdfs:label>
        <rdfs:isDefinedBy rdf:resource="http://rs.tdwg.org/abcd/terms/"/>
        <dwcattributes:status>recommended</dwcattributes:status>
        <dcterms:issued>2019-01-31</dcterms:issued>
        <dcterms:modified>2019-01-31</dcterms:modified>
        <rdfs:comment>The variety designation, epithet, authors and reference for the unit.</rdfs:comment>
        <skos:definition>The variety designation, epithet, authors and reference for the unit.</skos:definition>
        <dc:description>This field excludes the pathovar name and the serovar name, which are both infrasubspecific names but are to be entered using abcd:pathovar and abcd:serovarOrSerotype respectivly.</dc:description>
        <rdfs:domain rdf:resource="http://www.w3.org/2002/07/owl#Thing"/>
        <rdfs:range rdf:resource="http://www.w3.org/2001/XMLSchema#string"/>
    </owl:DatatypeProperty>

    <owl:FunctionalProperty rdf:about="infrasubspecificName"/>

    <owl:DatatypeProperty rdf:about="inheritedName">
        <rdfs:label xml:lang="en">Inherited Name</rdfs:label>
        <rdfs:isDefinedBy rdf:resource="http://rs.tdwg.org/abcd/terms/"/>
        <dwcattributes:status>recommended</dwcattributes:status>
        <dcterms:issued>2019-01-31</dcterms:issued>
        <dcterms:modified>2019-01-31</dcterms:modified>
        <rdfs:comment>The inherited part of the name of a person. This may consist of family names, generational names, a clan name, parents or grandparents personal names, etc.</rdfs:comment>
        <skos:definition>The inherited part of the name of a person. This may consist of family names, generational names, a clan name, parents or grandparents personal names, etc.</skos:definition>
        <dc:description>The inherited name (this being the lastname in western cultures) may be compound (e.g. 'Fischer von Waldheim', 'da Selva', 'Silvano Morales'). Depending on culture, the inherited name is not necessarily the name of the parents nor common to a married couple. Therefore, 'family name' should be avoided even though used in other ontologies.</dc:description>
        <rdfs:domain rdf:resource="http://www.w3.org/2002/07/owl#Thing"/>
        <rdfs:range rdf:resource="http://www.w3.org/2001/XMLSchema#string"/>
        <skos:exactMatch rdf:resource="http://www.w3.org/2006/vcard/ns#family-name"/>
        <skos:exactMatch rdf:resource="http://xmlns.com/foaf/0.1/familyName"/>
    </owl:DatatypeProperty>

    <owl:FunctionalProperty rdf:about="inheritedName"/>

    <owl:DatatypeProperty rdf:about="isQuantitative">
        <rdfs:label xml:lang="en">Is Quantitative</rdfs:label>
        <rdfs:isDefinedBy rdf:resource="http://rs.tdwg.org/abcd/terms/"/>
        <dwcattributes:status>recommended</dwcattributes:status>
        <dcterms:issued>2019-01-31</dcterms:issued>
        <dcterms:modified>2019-01-31</dcterms:modified>
        <rdfs:comment>A flag indicating whether values given for a measurement represent the numerical result of a quantitative measurement ("true") or a descriptor with textual or categorical result ("false").</rdfs:comment>
        <skos:definition>A flag indicating whether values given for a measurement represent the numerical result of a quantitative measurement ("true") or a descriptor with textual or categorical result ("false").</skos:definition>
        <dc:description>Allowed values are "true" and "false" (in lower case).</dc:description>
        <rdfs:domain rdf:resource="http://www.w3.org/2002/07/owl#Thing"/>
        <rdfs:range rdf:resource="http://www.w3.org/2001/XMLSchema#boolean"/>
    </owl:DatatypeProperty>

    <owl:FunctionalProperty rdf:about="isQuantitative"/>

    <owl:DatatypeProperty rdf:about="kindOfUnit">
        <rdfs:label xml:lang="en">Kind Of Unit</rdfs:label>
        <rdfs:isDefinedBy rdf:resource="http://rs.tdwg.org/abcd/terms/"/>
        <dwcattributes:status>recommended</dwcattributes:status>
        <dcterms:issued>2019-01-31</dcterms:issued>
        <dcterms:modified>2019-01-31</dcterms:modified>
        <rdfs:comment>Part(s), physical state, or class of materials represented by the Unit.</rdfs:comment>
        <skos:definition>Part(s), physical state, or class of materials represented by the Unit.</skos:definition>
        <dc:description>Note that sex, stages etc. should normally be recorded using the respective elements, but may also end up here if the source database mixes them with other data.</dc:description>
        <rdfs:domain rdf:resource="http://www.w3.org/2002/07/owl#Thing"/>
        <rdfs:range rdf:resource="http://www.w3.org/2001/XMLSchema#string"/>
    </owl:DatatypeProperty>

    <owl:DatatypeProperty rdf:about="latitudeDecimal">
        <rdfs:label xml:lang="en">Latitude Decimal</rdfs:label>
        <rdfs:isDefinedBy rdf:resource="http://rs.tdwg.org/abcd/terms/"/>
        <dwcattributes:status>recommended</dwcattributes:status>
        <dcterms:issued>2019-01-31</dcterms:issued>
        <dcterms:modified>2019-01-31</dcterms:modified>
        <rdfs:comment>The latitude of a location (north-south component), expressed in decimal degrees. The values range from -90 to 90.</rdfs:comment>
        <skos:definition>The latitude of a location (north-south component), expressed in decimal degrees. The values range from -90 to 90.</skos:definition>
        <dc:description>To store a latitude expressed in a non decimal way (e.g. by using Degrees, Minutes and Seconds), please use abcd:VerbatimLatitude.</dc:description>
        <rdfs:domain rdf:resource="http://www.w3.org/2002/07/owl#Thing"/>
        <rdfs:range rdf:resource="http://www.w3.org/2001/XMLSchema#decimal"/>
        <skos:exactMatch rdf:resource="http://www.w3.org/2003/01/geo/wgs84_pos#lat"/>
        <skos:exactMatch rdf:resource="http://rs.tdwg.org/dwc/terms/decimalLatitude"/>
    </owl:DatatypeProperty>

    <owl:FunctionalProperty rdf:about="latitudeDecimal"/>

    <owl:DatatypeProperty rdf:about="latitudeText">
        <rdfs:label xml:lang="en">Latitude Text</rdfs:label>
        <rdfs:isDefinedBy rdf:resource="http://rs.tdwg.org/abcd/terms/"/>
        <dwcattributes:status>recommended</dwcattributes:status>
        <dcterms:issued>2019-01-31</dcterms:issued>
        <dcterms:modified>2019-01-31</dcterms:modified>
        <rdfs:comment>A free text format for the latitude component of the coordinates that are not expressed in a pure decimal format.</rdfs:comment>
        <skos:definition>A free text format for the latitude component of the coordinates that are not expressed in a pure decimal format.</skos:definition>
        <rdfs:subPropertyOf rdf:resource="unformattedValue"/>
        <rdfs:domain rdf:resource="http://www.w3.org/2002/07/owl#Thing"/>
        <rdfs:range rdf:resource="http://www.w3.org/2001/XMLSchema#string"/>
        <skos:exactMatch rdf:resource="http://rs.tdwg.org/dwc/terms/verbatimLatitude"/>
    </owl:DatatypeProperty>

    <owl:FunctionalProperty rdf:about="latitudeText"/>

    <owl:DatatypeProperty rdf:about="lensModel">
        <rdfs:label xml:lang="en">Lens Model</rdfs:label>
        <rdfs:isDefinedBy rdf:resource="http://rs.tdwg.org/abcd/terms/"/>
        <dwcattributes:status>recommended</dwcattributes:status>
        <dcterms:issued>2019-01-31</dcterms:issued>
        <dcterms:modified>2019-01-31</dcterms:modified>
        <rdfs:comment>This element records the lens&#8217;s model name and model number as an ASCII string.</rdfs:comment>
        <skos:definition>This element records the lens&#8217;s model name and model number as an ASCII string.</skos:definition>
        <rdfs:domain rdf:resource="http://www.w3.org/2002/07/owl#Thing"/>
        <rdfs:range rdf:resource="http://www.w3.org/2001/XMLSchema#string"/>
    </owl:DatatypeProperty>

    <owl:DatatypeProperty rdf:about="lichenMorphotype">
        <rdfs:label xml:lang="en">Lichen Morphotype</rdfs:label>
        <rdfs:isDefinedBy rdf:resource="http://rs.tdwg.org/abcd/terms/"/>
        <dwcattributes:status>recommended</dwcattributes:status>
        <dcterms:issued>2019-01-31</dcterms:issued>
        <dcterms:modified>2019-01-31</dcterms:modified>
        <rdfs:comment>The name of an algal or cyanobacterial component of lichen.</rdfs:comment>
        <skos:definition>The name of an algal or cyanobacterial component of lichen.</skos:definition>
        <rdfs:domain rdf:resource="http://www.w3.org/2002/07/owl#Thing"/>
        <rdfs:range rdf:resource="http://www.w3.org/2001/XMLSchema#string"/>
    </owl:DatatypeProperty>

    <owl:FunctionalProperty rdf:about="lichenMorphotype"/>

    <owl:DatatypeProperty rdf:about="lightCondition">
        <rdfs:label xml:lang="en">Light Condition</rdfs:label>
        <rdfs:isDefinedBy rdf:resource="http://rs.tdwg.org/abcd/terms/"/>
        <dwcattributes:status>recommended</dwcattributes:status>
        <dcterms:issued>2019-01-31</dcterms:issued>
        <dcterms:modified>2019-01-31</dcterms:modified>
        <rdfs:comment>Description of light conditions during recording.</rdfs:comment>
        <skos:definition>Description of light conditions during recording.</skos:definition>
        <rdfs:domain rdf:resource="http://www.w3.org/2002/07/owl#Thing"/>
        <rdfs:range rdf:resource="http://www.w3.org/2001/XMLSchema#string"/>
    </owl:DatatypeProperty>

    <owl:DatatypeProperty rdf:about="lightSource">
        <rdfs:label xml:lang="en">Light Source</rdfs:label>
        <rdfs:isDefinedBy rdf:resource="http://rs.tdwg.org/abcd/terms/"/>
        <dwcattributes:status>recommended</dwcattributes:status>
        <dcterms:issued>2019-01-31</dcterms:issued>
        <dcterms:modified>2019-01-31</dcterms:modified>
        <rdfs:comment>The kind of light source.</rdfs:comment>
        <skos:definition>The kind of light source.</skos:definition>
        <rdfs:domain rdf:resource="http://www.w3.org/2002/07/owl#Thing"/>
        <rdfs:range rdf:resource="http://www.w3.org/2001/XMLSchema#string"/>
    </owl:DatatypeProperty>

    <owl:DatatypeProperty rdf:about="loanConditions">
        <rdfs:label xml:lang="en">Loan Conditions</rdfs:label>
        <rdfs:isDefinedBy rdf:resource="http://rs.tdwg.org/abcd/terms/"/>
        <dwcattributes:status>recommended</dwcattributes:status>
        <dcterms:issued>2019-01-31</dcterms:issued>
        <dcterms:modified>2019-01-31</dcterms:modified>
        <rdfs:comment>Certain conditions for loaning this specimen or sample.</rdfs:comment>
        <skos:definition>Certain conditions for loaning this specimen or sample.</skos:definition>
        <rdfs:domain rdf:resource="http://www.w3.org/2002/07/owl#Thing"/>
        <rdfs:range rdf:resource="http://www.w3.org/2001/XMLSchema#string"/>
    </owl:DatatypeProperty>

    <owl:FunctionalProperty rdf:about="loanConditions"/>

    <owl:DatatypeProperty rdf:about="loanDestination">
        <rdfs:label xml:lang="en">Loan Destination</rdfs:label>
        <rdfs:isDefinedBy rdf:resource="http://rs.tdwg.org/abcd/terms/"/>
        <dwcattributes:status>recommended</dwcattributes:status>
        <dcterms:issued>2019-01-31</dcterms:issued>
        <dcterms:modified>2019-01-31</dcterms:modified>
        <rdfs:comment>Institution to which the loan is being sent [HISPID3].</rdfs:comment>
        <skos:definition>Institution to which the loan is being sent [HISPID3].</skos:definition>
        <rdfs:domain rdf:resource="http://www.w3.org/2002/07/owl#Thing"/>
        <rdfs:range rdf:resource="http://www.w3.org/2001/XMLSchema#string"/>
    </owl:DatatypeProperty>

    <owl:FunctionalProperty rdf:about="loanDestination"/>

    <owl:DatatypeProperty rdf:about="loanDispatchMethod">
        <rdfs:label xml:lang="en">Loan Dispatch Method</rdfs:label>
        <rdfs:isDefinedBy rdf:resource="http://rs.tdwg.org/abcd/terms/"/>
        <dwcattributes:status>recommended</dwcattributes:status>
        <dcterms:issued>2019-01-31</dcterms:issued>
        <dcterms:modified>2019-01-31</dcterms:modified>
        <rdfs:comment>The means by which the loan is being dispatched from the home institution [HISPID3].</rdfs:comment>
        <skos:definition>The means by which the loan is being dispatched from the home institution [HISPID3].</skos:definition>
        <rdfs:domain rdf:resource="http://www.w3.org/2002/07/owl#Thing"/>
        <rdfs:range rdf:resource="http://www.w3.org/2001/XMLSchema#string"/>
    </owl:DatatypeProperty>

    <owl:FunctionalProperty rdf:about="loanDispatchMethod"/>

    <owl:DatatypeProperty rdf:about="loanForBotanist">
        <rdfs:label xml:lang="en">Loan For Botanist</rdfs:label>
        <rdfs:isDefinedBy rdf:resource="http://rs.tdwg.org/abcd/terms/"/>
        <dwcattributes:status>recommended</dwcattributes:status>
        <dcterms:issued>2019-01-31</dcterms:issued>
        <dcterms:modified>2019-01-31</dcterms:modified>
        <rdfs:comment>Name of the botanist for whom the loan is destined [HISPID3].</rdfs:comment>
        <skos:definition>Name of the botanist for whom the loan is destined [HISPID3].</skos:definition>
        <rdfs:domain rdf:resource="http://www.w3.org/2002/07/owl#Thing"/>
        <rdfs:range rdf:resource="http://www.w3.org/2001/XMLSchema#string"/>
    </owl:DatatypeProperty>

    <owl:FunctionalProperty rdf:about="loanForBotanist"/>

    <owl:DatatypeProperty rdf:about="loanID">
        <rdfs:label xml:lang="en">Loan ID</rdfs:label>
        <rdfs:isDefinedBy rdf:resource="http://rs.tdwg.org/abcd/terms/"/>
        <dwcattributes:status>recommended</dwcattributes:status>
        <dcterms:issued>2019-01-31</dcterms:issued>
        <dcterms:modified>2019-01-31</dcterms:modified>
        <rdfs:comment>The unique institutional loan number applied with the loan sequence number to uniquely identify a specimen on loan [HISPID3].</rdfs:comment>
        <skos:definition>The unique institutional loan number applied with the loan sequence number to uniquely identify a specimen on loan [HISPID3].</skos:definition>
        <rdfs:domain rdf:resource="http://www.w3.org/2002/07/owl#Thing"/>
        <rdfs:range rdf:resource="http://www.w3.org/2001/XMLSchema#string"/>
    </owl:DatatypeProperty>

    <owl:FunctionalProperty rdf:about="loanID"/>

    <owl:DatatypeProperty rdf:about="loanSequenceNumber">
        <rdfs:label xml:lang="en">Loan Sequence Number</rdfs:label>
        <rdfs:isDefinedBy rdf:resource="http://rs.tdwg.org/abcd/terms/"/>
        <dwcattributes:status>recommended</dwcattributes:status>
        <dcterms:issued>2019-01-31</dcterms:issued>
        <dcterms:modified>2019-01-31</dcterms:modified>
        <rdfs:comment>The sequence of a specimen within a given loan, assigned with the Loan Identification to uniquely identify a specimen on loan [HISPID3].</rdfs:comment>
        <skos:definition>The sequence of a specimen within a given loan, assigned with the Loan Identification to uniquely identify a specimen on loan [HISPID3].</skos:definition>
        <rdfs:domain rdf:resource="http://www.w3.org/2002/07/owl#Thing"/>
        <rdfs:range rdf:resource="http://www.w3.org/2001/XMLSchema#string"/>
    </owl:DatatypeProperty>

    <owl:FunctionalProperty rdf:about="loanSequenceNumber"/>

    <owl:DatatypeProperty rdf:about="localityText">
        <rdfs:label xml:lang="en">Locality Text</rdfs:label>
        <rdfs:isDefinedBy rdf:resource="http://rs.tdwg.org/abcd/terms/"/>
        <dwcattributes:status>recommended</dwcattributes:status>
        <dcterms:issued>2019-01-31</dcterms:issued>
        <dcterms:modified>2019-01-31</dcterms:modified>
        <rdfs:comment>The original gathering locality data as appearing on a label or in an original entry. It should contain the information below the country level that describes where the accession was collected.</rdfs:comment>
        <skos:definition>The original gathering locality data as appearing on a label or in an original entry. It should contain the information below the country level that describes where the accession was collected.</skos:definition>
        <rdfs:subPropertyOf rdf:resource="text"/>
        <dc:description>The value may include the distance in kilometers and direction from the nearest town, village or map grid reference point. Editorial omissions for brevity, etc. should be indicated with an ellipsis (...) and interpreted or implied text should be included in square brackets [ ].</dc:description>
        <rdfs:domain rdf:resource="http://www.w3.org/2002/07/owl#Thing"/>
        <rdfs:range rdf:resource="http://www.w3.org/2001/XMLSchema#string"/>
        <skos:exactMatch rdf:resource="http://rs.tdwg.org/dwc/terms/verbatimLocality"/>
    </owl:DatatypeProperty>

    <owl:FunctionalProperty rdf:about="localityText"/>

    <owl:DatatypeProperty rdf:about="locationInGarden">
        <rdfs:label xml:lang="en">Location In Garden</rdfs:label>
        <rdfs:isDefinedBy rdf:resource="http://rs.tdwg.org/abcd/terms/"/>
        <dwcattributes:status>recommended</dwcattributes:status>
        <dcterms:issued>2019-01-31</dcterms:issued>
        <dcterms:modified>2019-01-31</dcterms:modified>
        <rdfs:comment>The current location of the living plant in the botanical garden.</rdfs:comment>
        <skos:definition>The current location of the living plant in the botanical garden.</skos:definition>
        <rdfs:domain rdf:resource="http://www.w3.org/2002/07/owl#Thing"/>
        <rdfs:range rdf:resource="http://www.w3.org/2001/XMLSchema#string"/>
    </owl:DatatypeProperty>

    <owl:FunctionalProperty rdf:about="locationInGarden"/>

    <owl:DatatypeProperty rdf:about="locationSafetyDuplicates">
        <rdfs:label xml:lang="en">Location Safety Duplicates</rdfs:label>
        <rdfs:isDefinedBy rdf:resource="http://rs.tdwg.org/abcd/terms/"/>
        <dwcattributes:status>recommended</dwcattributes:status>
        <dcterms:issued>2019-01-31</dcterms:issued>
        <dcterms:modified>2019-01-31</dcterms:modified>
        <rdfs:comment>The FAO Institute Code of the institute where a safety duplicate of the accession is maintained.</rdfs:comment>
        <skos:definition>The FAO Institute Code of the institute where a safety duplicate of the accession is maintained.</skos:definition>
        <rdfs:domain rdf:resource="http://www.w3.org/2002/07/owl#Thing"/>
        <rdfs:range rdf:resource="http://www.w3.org/2001/XMLSchema#integer"/>
    </owl:DatatypeProperty>

    <owl:FunctionalProperty rdf:about="locationSafetyDuplicates"/>

    <owl:DatatypeProperty rdf:about="logoURL">
        <rdfs:label xml:lang="en">Logo URL</rdfs:label>
        <rdfs:isDefinedBy rdf:resource="http://rs.tdwg.org/abcd/terms/"/>
        <dwcattributes:status>recommended</dwcattributes:status>
        <dcterms:issued>2019-01-31</dcterms:issued>
        <dcterms:modified>2019-01-31</dcterms:modified>
        <rdfs:comment>URL of an icon/logo symbolizing the associated class.</rdfs:comment>
        <skos:definition>URL of an icon/logo symbolizing the associated class.</skos:definition>
        <rdfs:domain rdf:resource="http://www.w3.org/2002/07/owl#Thing"/>
        <rdfs:range rdf:resource="http://www.w3.org/2001/XMLSchema#anyURI"/>
    </owl:DatatypeProperty>

    <owl:FunctionalProperty rdf:about="logoURL"/>

    <owl:DatatypeProperty rdf:about="longitudeDecimal">
        <rdfs:label xml:lang="en">Longitude Decimal</rdfs:label>
        <rdfs:isDefinedBy rdf:resource="http://rs.tdwg.org/abcd/terms/"/>
        <dwcattributes:status>recommended</dwcattributes:status>
        <dcterms:issued>2019-01-31</dcterms:issued>
        <dcterms:modified>2019-01-31</dcterms:modified>
        <rdfs:comment>The longitude of a location (east-west component), expressed in decimal degrees. The values range from -180 to 180.</rdfs:comment>
        <skos:definition>The longitude of a location (east-west component), expressed in decimal degrees. The values range from -180 to 180.</skos:definition>
        <dc:description>To store a longitude expressed in a non decimal way (e.g. by using Degrees, Minutes and Seconds), please use abcd:VerbatimLongitude.</dc:description>
        <rdfs:domain rdf:resource="http://www.w3.org/2002/07/owl#Thing"/>
        <rdfs:range rdf:resource="http://www.w3.org/2001/XMLSchema#decimal"/>
        <skos:exactMatch rdf:resource="http://rs.tdwg.org/dwc/terms/decimalLongitude"/>
        <skos:exactMatch rdf:resource="http://www.w3.org/2003/01/geo/wgs84_pos#long"/>
    </owl:DatatypeProperty>

    <owl:FunctionalProperty rdf:about="longitudeDecimal"/>

    <owl:DatatypeProperty rdf:about="longitudeText">
        <rdfs:label xml:lang="en">Longitude Text</rdfs:label>
        <rdfs:isDefinedBy rdf:resource="http://rs.tdwg.org/abcd/terms/"/>
        <dwcattributes:status>recommended</dwcattributes:status>
        <dcterms:issued>2019-01-31</dcterms:issued>
        <dcterms:modified>2019-01-31</dcterms:modified>
        <rdfs:comment>A free text format for the longitude component of the coordinates that are not expressed in a pure decimal format.</rdfs:comment>
        <skos:definition>A free text format for the longitude component of the coordinates that are not expressed in a pure decimal format.</skos:definition>
        <rdfs:subPropertyOf rdf:resource="unformattedValue"/>
        <rdfs:domain rdf:resource="http://www.w3.org/2002/07/owl#Thing"/>
        <rdfs:range rdf:resource="http://www.w3.org/2001/XMLSchema#string"/>
        <skos:exactMatch rdf:resource="http://rs.tdwg.org/dwc/terms/verbatimLongitude"/>
    </owl:DatatypeProperty>

    <owl:FunctionalProperty rdf:about="longitudeText"/>

    <owl:DatatypeProperty rdf:about="lowerValue">
        <rdfs:label xml:lang="en">Lower Value</rdfs:label>
        <rdfs:isDefinedBy rdf:resource="http://rs.tdwg.org/abcd/terms/"/>
        <dwcattributes:status>recommended</dwcattributes:status>
        <dcterms:issued>2019-01-31</dcterms:issued>
        <dcterms:modified>2019-01-31</dcterms:modified>
        <rdfs:comment>The lower value of a measurement when it yields a range of values.</rdfs:comment>
        <skos:definition>The lower value of a measurement when it yields a range of values.</skos:definition>
        <dc:description>The unit of the measurement should be expressed in abcd:UnitOfMeasurement. When a measurement yields an exact value and no range, use abcd:ExactValue instead. When no lower value of a range can be determined, this property should be omitted and only abcd:UpperValue should be filled.</dc:description>
        <rdfs:domain rdf:resource="http://www.w3.org/2002/07/owl#Thing"/>
        <rdfs:range rdf:resource="http://www.w3.org/2001/XMLSchema#string"/>
        <skos:relatedMatch rdf:resource="http://rs.tdwg.org/dwc/terms/measurementValue"/>
    </owl:DatatypeProperty>

    <owl:FunctionalProperty rdf:about="lowerValue"/>

    <owl:DatatypeProperty rdf:about="major">
        <rdfs:label xml:lang="en">Major</rdfs:label>
        <rdfs:isDefinedBy rdf:resource="http://rs.tdwg.org/abcd/terms/"/>
        <dwcattributes:status>recommended</dwcattributes:status>
        <dcterms:issued>2019-01-31</dcterms:issued>
        <dcterms:modified>2019-01-31</dcterms:modified>
        <rdfs:comment>A major version number.</rdfs:comment>
        <skos:definition>A major version number.</skos:definition>
        <rdfs:domain rdf:resource="http://www.w3.org/2002/07/owl#Thing"/>
        <rdfs:range rdf:resource="http://www.w3.org/2001/XMLSchema#nonNegativeInteger"/>
    </owl:DatatypeProperty>

    <owl:FunctionalProperty rdf:about="major"/>

    <owl:DatatypeProperty rdf:about="makerNote">
        <rdfs:label xml:lang="en">Maker Note</rdfs:label>
        <rdfs:isDefinedBy rdf:resource="http://rs.tdwg.org/abcd/terms/"/>
        <dwcattributes:status>recommended</dwcattributes:status>
        <dcterms:issued>2019-01-31</dcterms:issued>
        <dcterms:modified>2019-01-31</dcterms:modified>
        <rdfs:comment>A tag for manufacturers of e.g. Exif/DCF writers to record any desired information. The contents are up to the manufacturer, but this tag shall not be used for any other than its intended purpose.</rdfs:comment>
        <skos:definition>A tag for manufacturers of e.g. Exif/DCF writers to record any desired information. The contents are up to the manufacturer, but this tag shall not be used for any other than its intended purpose.</skos:definition>
        <rdfs:domain rdf:resource="http://www.w3.org/2002/07/owl#Thing"/>
        <rdfs:range rdf:resource="http://www.w3.org/2001/XMLSchema#string"/>
    </owl:DatatypeProperty>

    <owl:DatatypeProperty rdf:about="markType">
        <rdfs:label xml:lang="en">Mark Type</rdfs:label>
        <rdfs:isDefinedBy rdf:resource="http://rs.tdwg.org/abcd/terms/"/>
        <dwcattributes:status>recommended</dwcattributes:status>
        <dcterms:issued>2019-01-31</dcterms:issued>
        <dcterms:modified>2019-01-31</dcterms:modified>
        <rdfs:comment>The type of mark on or associated to the unit - a label or an inscription.</rdfs:comment>
        <skos:definition>The type of mark on or associated to the unit - a label or an inscription.</skos:definition>
        <rdfs:domain rdf:resource="http://www.w3.org/2002/07/owl#Thing"/>
        <rdfs:range rdf:resource="http://www.w3.org/2001/XMLSchema#string"/>
    </owl:DatatypeProperty>

    <owl:FunctionalProperty rdf:about="markType"/>

    <owl:DatatypeProperty rdf:about="matrix">
        <rdfs:label xml:lang="en">Matrix</rdfs:label>
        <rdfs:isDefinedBy rdf:resource="http://rs.tdwg.org/abcd/terms/"/>
        <dwcattributes:status>recommended</dwcattributes:status>
        <dcterms:issued>2019-01-31</dcterms:issued>
        <dcterms:modified>2019-01-31</dcterms:modified>
        <rdfs:comment>The sediment or mineral matrix enclosing the fossil.</rdfs:comment>
        <skos:definition>The sediment or mineral matrix enclosing the fossil.</skos:definition>
        <rdfs:domain rdf:resource="http://www.w3.org/2002/07/owl#Thing"/>
        <rdfs:range rdf:resource="http://www.w3.org/2001/XMLSchema#string"/>
    </owl:DatatypeProperty>

    <owl:FunctionalProperty rdf:about="matrix"/>

    <owl:DatatypeProperty rdf:about="method">
        <rdfs:label xml:lang="en">Method</rdfs:label>
        <rdfs:isDefinedBy rdf:resource="http://rs.tdwg.org/abcd/terms/"/>
        <dwcattributes:status>recommended</dwcattributes:status>
        <dcterms:issued>2019-01-31</dcterms:issued>
        <dcterms:modified>2019-01-31</dcterms:modified>
        <rdfs:comment>Property to describe the method used to determine a corresponding result.</rdfs:comment>
        <skos:definition>Property to describe the method used to determine a corresponding result.</skos:definition>
        <rdfs:domain rdf:resource="http://www.w3.org/2002/07/owl#Thing"/>
        <rdfs:range rdf:resource="http://www.w3.org/2001/XMLSchema#string"/>
        <skos:exactMatch rdf:resource="http://rs.tdwg.org/dwc/terms/measurementMethod"/>
    </owl:DatatypeProperty>

    <owl:DatatypeProperty rdf:about="microphone">
        <rdfs:label xml:lang="en">Microphone</rdfs:label>
        <rdfs:isDefinedBy rdf:resource="http://rs.tdwg.org/abcd/terms/"/>
        <dwcattributes:status>recommended</dwcattributes:status>
        <dcterms:issued>2019-01-31</dcterms:issued>
        <dcterms:modified>2019-01-31</dcterms:modified>
        <rdfs:comment>Microphone equipment used for recording audio track.</rdfs:comment>
        <skos:definition>Microphone equipment used for recording audio track.</skos:definition>
        <rdfs:domain rdf:resource="http://www.w3.org/2002/07/owl#Thing"/>
        <rdfs:range rdf:resource="http://www.w3.org/2001/XMLSchema#string"/>
    </owl:DatatypeProperty>

    <owl:DatatypeProperty rdf:about="mineralization">
        <rdfs:label xml:lang="en">Mineralization</rdfs:label>
        <rdfs:isDefinedBy rdf:resource="http://rs.tdwg.org/abcd/terms/"/>
        <dwcattributes:status>recommended</dwcattributes:status>
        <dcterms:issued>2019-01-31</dcterms:issued>
        <dcterms:modified>2019-01-31</dcterms:modified>
        <rdfs:comment>The form of mineralization.</rdfs:comment>
        <skos:definition>The form of mineralization.</skos:definition>
        <rdfs:domain rdf:resource="http://www.w3.org/2002/07/owl#Thing"/>
        <rdfs:range rdf:resource="http://www.w3.org/2001/XMLSchema#string"/>
    </owl:DatatypeProperty>

    <owl:FunctionalProperty rdf:about="mineralization"/>

    <owl:DatatypeProperty rdf:about="minor">
        <rdfs:label xml:lang="en">Minor</rdfs:label>
        <rdfs:isDefinedBy rdf:resource="http://rs.tdwg.org/abcd/terms/"/>
        <dwcattributes:status>recommended</dwcattributes:status>
        <dcterms:issued>2019-01-31</dcterms:issued>
        <dcterms:modified>2019-01-31</dcterms:modified>
        <rdfs:comment>An optional minor version number.</rdfs:comment>
        <skos:definition>An optional minor version number.</skos:definition>
        <rdfs:domain rdf:resource="http://www.w3.org/2002/07/owl#Thing"/>
        <rdfs:range rdf:resource="http://www.w3.org/2001/XMLSchema#nonNegativeInteger"/>
    </owl:DatatypeProperty>

    <owl:FunctionalProperty rdf:about="minor"/>

    <owl:DatatypeProperty rdf:about="modifier">
        <rdfs:label xml:lang="en">Modifier</rdfs:label>
        <rdfs:isDefinedBy rdf:resource="http://rs.tdwg.org/abcd/terms/"/>
        <dwcattributes:status>recommended</dwcattributes:status>
        <dcterms:issued>2019-01-31</dcterms:issued>
        <dcterms:modified>2019-01-31</dcterms:modified>
        <rdfs:comment>Text specifying a status and optional number for a version.</rdfs:comment>
        <skos:definition>Text specifying a status and optional number for a version.</skos:definition>
        <dc:description>If the modifier is missing, the standard release version &lt;Major&gt;.&lt;Minor&gt; is assumed.</dc:description>
        <rdfs:domain rdf:resource="http://www.w3.org/2002/07/owl#Thing"/>
        <rdfs:range rdf:resource="http://www.w3.org/2001/XMLSchema#string"/>
    </owl:DatatypeProperty>

    <owl:DatatypeProperty rdf:about="multimediaContext">
        <rdfs:label xml:lang="en">Multimedia Context</rdfs:label>
        <rdfs:isDefinedBy rdf:resource="http://rs.tdwg.org/abcd/terms/"/>
        <dwcattributes:status>recommended</dwcattributes:status>
        <dcterms:issued>2019-01-31</dcterms:issued>
        <dcterms:modified>2019-01-31</dcterms:modified>
        <rdfs:comment>The context of the multimedia object in relation to the specimen or observation.</rdfs:comment>
        <skos:definition>The context of the multimedia object in relation to the specimen or observation.</skos:definition>
        <rdfs:domain rdf:resource="http://www.w3.org/2002/07/owl#Thing"/>
        <rdfs:range rdf:resource="http://www.w3.org/2001/XMLSchema#string"/>
    </owl:DatatypeProperty>

    <owl:FunctionalProperty rdf:about="multimediaContext"/>

    <owl:DatatypeProperty rdf:about="mutant">
        <rdfs:label xml:lang="en">Mutant</rdfs:label>
        <rdfs:isDefinedBy rdf:resource="http://rs.tdwg.org/abcd/terms/"/>
        <dwcattributes:status>recommended</dwcattributes:status>
        <dcterms:issued>2019-01-31</dcterms:issued>
        <dcterms:modified>2019-01-31</dcterms:modified>
        <rdfs:comment>Type and parent of the mutant if the strain is a mutant strain.</rdfs:comment>
        <skos:definition>Type and parent of the mutant if the strain is a mutant strain.</skos:definition>
        <rdfs:domain rdf:resource="http://www.w3.org/2002/07/owl#Thing"/>
        <rdfs:range rdf:resource="http://www.w3.org/2001/XMLSchema#string"/>
    </owl:DatatypeProperty>

    <owl:FunctionalProperty rdf:about="mutant"/>

    <owl:DatatypeProperty rdf:about="mycologicalLiveStage">
        <rdfs:label xml:lang="en">Mycological Live Stage</rdfs:label>
        <rdfs:isDefinedBy rdf:resource="http://rs.tdwg.org/abcd/terms/"/>
        <dwcattributes:status>recommended</dwcattributes:status>
        <dcterms:issued>2019-01-31</dcterms:issued>
        <dcterms:modified>2019-01-31</dcterms:modified>
        <rdfs:comment>A spore state that is present in the sample.</rdfs:comment>
        <skos:definition>A spore state that is present in the sample.</skos:definition>
        <rdfs:domain rdf:resource="http://www.w3.org/2002/07/owl#Thing"/>
        <rdfs:range rdf:resource="http://www.w3.org/2001/XMLSchema#string"/>
    </owl:DatatypeProperty>

    <owl:DatatypeProperty rdf:about="mycologicalSexualStage">
        <rdfs:label xml:lang="en">Mycological Sexual Stage</rdfs:label>
        <rdfs:isDefinedBy rdf:resource="http://rs.tdwg.org/abcd/terms/"/>
        <dwcattributes:status>recommended</dwcattributes:status>
        <dcterms:issued>2019-01-31</dcterms:issued>
        <dcterms:modified>2019-01-31</dcterms:modified>
        <rdfs:domain rdf:resource="http://www.w3.org/2002/07/owl#Thing"/>
        <rdfs:range rdf:resource="http://www.w3.org/2001/XMLSchema#string"/>
    </owl:DatatypeProperty>

    <owl:FunctionalProperty rdf:about="mycologicalSexualStage"/>

    <owl:DatatypeProperty rdf:about="name">
        <rdfs:label xml:lang="en">Name</rdfs:label>
        <rdfs:isDefinedBy rdf:resource="http://rs.tdwg.org/abcd/terms/"/>
        <dwcattributes:status>recommended</dwcattributes:status>
        <dcterms:issued>2019-01-31</dcterms:issued>
        <dcterms:modified>2019-01-31</dcterms:modified>
        <rdfs:comment>The name of a class in a specific language.</rdfs:comment>
        <skos:definition>The name of a class in a specific language.</skos:definition>
        <dc:description>Not to be used for Persons. Use abcd:FullName, abcd:GivenNames, abcd:InheritedName, etc. instead.</dc:description>
        <rdfs:domain rdf:resource="http://www.w3.org/2002/07/owl#Thing"/>
        <rdfs:range rdf:resource="http://www.w3.org/2001/XMLSchema#string"/>
        <vann:termGroup rdf:resource="General"/>
        <skos:relatedMatch rdf:resource="http://www.w3.org/2000/01/rdf-schema#label"/>
    </owl:DatatypeProperty>

    <owl:FunctionalProperty rdf:about="name"/>

    <owl:DatatypeProperty rdf:about="nameAddendum">
        <rdfs:label xml:lang="en">Name Addendum</rdfs:label>
        <rdfs:isDefinedBy rdf:resource="http://rs.tdwg.org/abcd/terms/"/>
        <dwcattributes:status>recommended</dwcattributes:status>
        <dcterms:issued>2019-01-31</dcterms:issued>
        <dcterms:modified>2019-01-31</dcterms:modified>
        <rdfs:comment>A free-text suffix added to the Scientific Name of the Identified Taxon, including additional name element in common use but without formal nomenclatural standing (e.g. isolate names for viruses).</rdfs:comment>
        <skos:definition>A free-text suffix added to the Scientific Name of the Identified Taxon, including additional name element in common use but without formal nomenclatural standing (e.g. isolate names for viruses).</skos:definition>
        <rdfs:domain rdf:resource="http://www.w3.org/2002/07/owl#Thing"/>
        <rdfs:range rdf:resource="http://www.w3.org/2001/XMLSchema#string"/>
    </owl:DatatypeProperty>

    <owl:FunctionalProperty rdf:about="nameAddendum"/>

    <owl:DatatypeProperty rdf:about="nameApprobation">
        <rdfs:label xml:lang="en">Name Approbation</rdfs:label>
        <rdfs:isDefinedBy rdf:resource="http://rs.tdwg.org/abcd/terms/"/>
        <dwcattributes:status>recommended</dwcattributes:status>
        <dcterms:issued>2019-01-31</dcterms:issued>
        <dcterms:modified>2019-01-31</dcterms:modified>
        <rdfs:comment>Approbation of the name identified for a unit according to an approved list, validation list,or validly published, paper in IJSB after 1980.</rdfs:comment>
        <skos:definition>Approbation of the name identified for a unit according to an approved list, validation list,or validly published, paper in IJSB after 1980.</skos:definition>
        <rdfs:domain rdf:resource="http://www.w3.org/2002/07/owl#Thing"/>
        <rdfs:range rdf:resource="http://www.w3.org/2001/XMLSchema#string"/>
    </owl:DatatypeProperty>

    <owl:FunctionalProperty rdf:about="nameApprobation"/>

    <owl:DatatypeProperty rdf:about="namePrefix">
        <rdfs:label xml:lang="en">Name Prefix</rdfs:label>
        <rdfs:isDefinedBy rdf:resource="http://rs.tdwg.org/abcd/terms/"/>
        <dwcattributes:status>recommended</dwcattributes:status>
        <dcterms:issued>2019-01-31</dcterms:issued>
        <dcterms:modified>2019-01-31</dcterms:modified>
        <rdfs:comment>The prefix for the Inherited Name of a Person.</rdfs:comment>
        <skos:definition>The prefix for the Inherited Name of a Person.</skos:definition>
        <dc:description>The prefix should be output before the name, but is usually not included in sorting. Compare Title for 'Prof', 'Dr.'</dc:description>
        <rdfs:domain rdf:resource="http://www.w3.org/2002/07/owl#Thing"/>
        <rdfs:range rdf:resource="http://www.w3.org/2001/XMLSchema#string"/>
        <skos:relatedMatch rdf:resource="http://www.w3.org/2006/vcard/ns#honorific-prefix"/>
    </owl:DatatypeProperty>

    <owl:FunctionalProperty rdf:about="namePrefix"/>

    <owl:DatatypeProperty rdf:about="nameSuffix">
        <rdfs:label xml:lang="en">Name Suffix</rdfs:label>
        <rdfs:isDefinedBy rdf:resource="http://rs.tdwg.org/abcd/terms/"/>
        <dwcattributes:status>recommended</dwcattributes:status>
        <dcterms:issued>2019-01-31</dcterms:issued>
        <dcterms:modified>2019-01-31</dcterms:modified>
        <rdfs:comment>The suffix for the Inherited Name of a Person.</rdfs:comment>
        <skos:definition>The suffix for the Inherited Name of a Person.</skos:definition>
        <rdfs:domain rdf:resource="http://www.w3.org/2002/07/owl#Thing"/>
        <rdfs:range rdf:resource="http://www.w3.org/2001/XMLSchema#string"/>
        <skos:relatedMatch rdf:resource="http://www.w3.org/2006/vcard/ns#honorific-suffix"/>
    </owl:DatatypeProperty>

    <owl:FunctionalProperty rdf:about="nameSuffix"/>

    <owl:DatatypeProperty rdf:about="namedCollectionOrSurvey">
        <rdfs:label xml:lang="en">Named Collection Or Survey</rdfs:label>
        <rdfs:isDefinedBy rdf:resource="http://rs.tdwg.org/abcd/terms/"/>
        <dwcattributes:status>recommended</dwcattributes:status>
        <dcterms:issued>2019-01-31</dcterms:issued>
        <dcterms:modified>2019-01-31</dcterms:modified>
        <rdfs:comment>A named collection or survey project to which the Unit belongs, which may not match the abcd:SourceID.</rdfs:comment>
        <skos:definition>A named collection or survey project to which the Unit belongs, which may not match the abcd:SourceID.</skos:definition>
        <dc:description>Note that this element refers to the name accepted by the specimen or data holding institution and this may or may not be different from the project name given under abcd:ProjectTitle</dc:description>
        <rdfs:domain rdf:resource="http://www.w3.org/2002/07/owl#Thing"/>
        <rdfs:range rdf:resource="http://www.w3.org/2001/XMLSchema#string"/>
    </owl:DatatypeProperty>

    <owl:DatatypeProperty rdf:about="namedIndividual">
        <rdfs:label xml:lang="en">Named Individual</rdfs:label>
        <rdfs:isDefinedBy rdf:resource="http://rs.tdwg.org/abcd/terms/"/>
        <dwcattributes:status>recommended</dwcattributes:status>
        <dcterms:issued>2019-01-31</dcterms:issued>
        <dcterms:modified>2019-01-31</dcterms:modified>
        <rdfs:comment>The name of an individually named animal.</rdfs:comment>
        <skos:definition>The name of an individually named animal.</skos:definition>
        <rdfs:domain rdf:resource="http://www.w3.org/2002/07/owl#Thing"/>
        <rdfs:range rdf:resource="http://www.w3.org/2001/XMLSchema#string"/>
    </owl:DatatypeProperty>

    <owl:FunctionalProperty rdf:about="namedIndividual"/>

    <owl:DatatypeProperty rdf:about="nationalInventoryCode">
        <rdfs:label xml:lang="en">National Inventory Code</rdfs:label>
        <rdfs:isDefinedBy rdf:resource="http://rs.tdwg.org/abcd/terms/"/>
        <dwcattributes:status>recommended</dwcattributes:status>
        <dcterms:issued>2019-01-31</dcterms:issued>
        <dcterms:modified>2019-01-31</dcterms:modified>
        <rdfs:comment>A code identifying the National Inventory. The code of the country preparing the National Inventory. Exceptions are possible, if agreed with EURISCO such as NGB.</rdfs:comment>
        <skos:definition>A code identifying the National Inventory. The code of the country preparing the National Inventory. Exceptions are possible, if agreed with EURISCO such as NGB.</skos:definition>
        <rdfs:domain rdf:resource="http://www.w3.org/2002/07/owl#Thing"/>
        <rdfs:range rdf:resource="http://www.w3.org/2001/XMLSchema#string"/>
    </owl:DatatypeProperty>

    <owl:FunctionalProperty rdf:about="nationalInventoryCode"/>

    <owl:DatatypeProperty rdf:about="naturalOccurrence">
        <rdfs:label xml:lang="en">Natural Occurrence</rdfs:label>
        <rdfs:isDefinedBy rdf:resource="http://rs.tdwg.org/abcd/terms/"/>
        <dwcattributes:status>recommended</dwcattributes:status>
        <dcterms:issued>2019-01-31</dcterms:issued>
        <dcterms:modified>2019-01-31</dcterms:modified>
        <rdfs:comment>Records whether the plant is a native of the collection habitat or whether it is a naturalised introduction. Equivalent to HISPID:posnat.</rdfs:comment>
        <skos:definition>Records whether the plant is a native of the collection habitat or whether it is a naturalised introduction. Equivalent to HISPID:posnat.</skos:definition>
        <dc:description>It is expected that this field will have values similar to the following: Natural, Naturalised, Unknown.</dc:description>
        <rdfs:domain rdf:resource="http://www.w3.org/2002/07/owl#Thing"/>
        <rdfs:range rdf:resource="http://www.w3.org/2001/XMLSchema#string"/>
    </owl:DatatypeProperty>

    <owl:FunctionalProperty rdf:about="naturalOccurrence"/>

    <owl:DatatypeProperty rdf:about="nearbyPlaceName">
        <rdfs:label xml:lang="en">Nearby Place Name</rdfs:label>
        <rdfs:isDefinedBy rdf:resource="http://rs.tdwg.org/abcd/terms/"/>
        <dwcattributes:status>recommended</dwcattributes:status>
        <dcterms:issued>2019-01-31</dcterms:issued>
        <dcterms:modified>2019-01-31</dcterms:modified>
        <rdfs:comment>A named place near or otherwise related to - but not naming - the gathering site.</rdfs:comment>
        <skos:definition>A named place near or otherwise related to - but not naming - the gathering site.</skos:definition>
        <rdfs:subPropertyOf rdf:resource="name"/>
        <rdfs:domain rdf:resource="http://www.w3.org/2002/07/owl#Thing"/>
        <rdfs:range rdf:resource="http://www.w3.org/2001/XMLSchema#string"/>
    </owl:DatatypeProperty>

    <owl:FunctionalProperty rdf:about="nearbyPlaceName"/>

    <owl:DatatypeProperty rdf:about="nearbyPlaceRelation">
        <rdfs:label xml:lang="en">Nearby Place Relation</rdfs:label>
        <rdfs:isDefinedBy rdf:resource="http://rs.tdwg.org/abcd/terms/"/>
        <dwcattributes:status>recommended</dwcattributes:status>
        <dcterms:issued>2019-01-31</dcterms:issued>
        <dcterms:modified>2019-01-31</dcterms:modified>
        <rdfs:comment>The relation of the location to a nearby named place.</rdfs:comment>
        <skos:definition>The relation of the location to a nearby named place.</skos:definition>
        <rdfs:domain rdf:resource="http://www.w3.org/2002/07/owl#Thing"/>
        <rdfs:range rdf:resource="http://www.w3.org/2001/XMLSchema#string"/>
    </owl:DatatypeProperty>

    <owl:FunctionalProperty rdf:about="nearbyPlaceRelation"/>

    <owl:DatatypeProperty rdf:about="negativeIdentificationFlag">
        <rdfs:label xml:lang="en">Negative Identification Flag</rdfs:label>
        <rdfs:isDefinedBy rdf:resource="http://rs.tdwg.org/abcd/terms/"/>
        <dwcattributes:status>recommended</dwcattributes:status>
        <dcterms:issued>2019-01-31</dcterms:issued>
        <dcterms:modified>2019-01-31</dcterms:modified>
        <rdfs:comment>This flag is set to "true" to designate a negative identification.</rdfs:comment>
        <skos:definition>This flag is set to "true" to designate a negative identification.</skos:definition>
        <rdfs:domain rdf:resource="http://www.w3.org/2002/07/owl#Thing"/>
        <rdfs:range rdf:resource="http://www.w3.org/2001/XMLSchema#boolean"/>
    </owl:DatatypeProperty>

    <owl:FunctionalProperty rdf:about="negativeIdentificationFlag"/>

    <owl:DatatypeProperty rdf:about="nomenclaturalTypeText">
        <rdfs:label xml:lang="en">Nomenclatural Type Text</rdfs:label>
        <rdfs:isDefinedBy rdf:resource="http://rs.tdwg.org/abcd/terms/"/>
        <dwcattributes:status>recommended</dwcattributes:status>
        <dcterms:issued>2019-01-31</dcterms:issued>
        <dcterms:modified>2019-01-31</dcterms:modified>
        <rdfs:comment>A note detailing possible or verified type information related to the specimen.</rdfs:comment>
        <skos:definition>A note detailing possible or verified type information related to the specimen.</skos:definition>
        <rdfs:domain rdf:resource="http://www.w3.org/2002/07/owl#Thing"/>
        <rdfs:range rdf:resource="http://www.w3.org/2001/XMLSchema#string"/>
    </owl:DatatypeProperty>

    <owl:FunctionalProperty rdf:about="nomenclaturalTypeText"/>

    <owl:DatatypeProperty rdf:about="notes">
        <rdfs:label xml:lang="en">Notes</rdfs:label>
        <rdfs:isDefinedBy rdf:resource="http://rs.tdwg.org/abcd/terms/"/>
        <dwcattributes:status>recommended</dwcattributes:status>
        <dcterms:issued>2019-01-31</dcterms:issued>
        <dcterms:modified>2019-01-31</dcterms:modified>
        <rdfs:comment>Supplementary remarks about a concept.</rdfs:comment>
        <skos:definition>Supplementary remarks about a concept.</skos:definition>
        <rdfs:domain rdf:resource="http://www.w3.org/2002/07/owl#Thing"/>
        <rdfs:range rdf:resource="http://www.w3.org/2001/XMLSchema#string"/>
    </owl:DatatypeProperty>

    <owl:DatatypeProperty rdf:about="numberOfNotes">
        <rdfs:label xml:lang="en">Number Of Notes</rdfs:label>
        <rdfs:isDefinedBy rdf:resource="http://rs.tdwg.org/abcd/terms/"/>
        <dwcattributes:status>recommended</dwcattributes:status>
        <dcterms:issued>2019-01-31</dcterms:issued>
        <dcterms:modified>2019-01-31</dcterms:modified>
        <rdfs:comment>The number of notes the animal in the recording makes.</rdfs:comment>
        <skos:definition>The number of notes the animal in the recording makes.</skos:definition>
        <rdfs:domain rdf:resource="http://www.w3.org/2002/07/owl#Thing"/>
        <rdfs:range rdf:resource="http://www.w3.org/2001/XMLSchema#string"/>
    </owl:DatatypeProperty>

    <owl:FunctionalProperty rdf:about="numberOfNotes"/>

    <owl:DatatypeProperty rdf:about="numericUnitID">
        <rdfs:label xml:lang="en">Numeric Unit ID</rdfs:label>
        <rdfs:isDefinedBy rdf:resource="http://rs.tdwg.org/abcd/terms/"/>
        <dwcattributes:status>recommended</dwcattributes:status>
        <dcterms:issued>2019-01-31</dcterms:issued>
        <dcterms:modified>2019-01-31</dcterms:modified>
        <rdfs:comment>The numeric catalogue number for a Unit. Where present, the unit catalogue number facilitates sorting and allows for searches on a range of catalogue numbers.</rdfs:comment>
        <skos:definition>The numeric catalogue number for a Unit. Where present, the unit catalogue number facilitates sorting and allows for searches on a range of catalogue numbers.</skos:definition>
        <dc:description>The usage of this property still requires the usage of the general Unit ID. If the general Unit ID is by nature numeric, both properties should be filled with that value.</dc:description>
        <rdfs:domain rdf:resource="http://www.w3.org/2002/07/owl#Thing"/>
        <rdfs:range rdf:resource="http://www.w3.org/2001/XMLSchema#integer"/>
    </owl:DatatypeProperty>

    <owl:FunctionalProperty rdf:about="numericUnitID"/>

    <owl:DatatypeProperty rdf:about="observationUnitID">
        <rdfs:label xml:lang="en">Observation Unit ID</rdfs:label>
        <rdfs:isDefinedBy rdf:resource="http://rs.tdwg.org/abcd/terms/"/>
        <dwcattributes:status>recommended</dwcattributes:status>
        <dcterms:issued>2019-01-31</dcterms:issued>
        <dcterms:modified>2019-01-31</dcterms:modified>
        <rdfs:comment>Numbers or other registration mark associated with an observation record.</rdfs:comment>
        <skos:definition>Numbers or other registration mark associated with an observation record.</skos:definition>
        <dc:description>Separated from the equivalent AccessionNumber of specimen collections because of the more standardized approaches taken in physical collections.</dc:description>
        <rdfs:domain rdf:resource="http://www.w3.org/2002/07/owl#Thing"/>
        <rdfs:range rdf:resource="http://www.w3.org/2001/XMLSchema#string"/>
    </owl:DatatypeProperty>

    <owl:DatatypeProperty rdf:about="organismType">
        <rdfs:label xml:lang="en">Organism Type</rdfs:label>
        <rdfs:isDefinedBy rdf:resource="http://rs.tdwg.org/abcd/terms/"/>
        <dwcattributes:status>recommended</dwcattributes:status>
        <dcterms:issued>2019-01-31</dcterms:issued>
        <dcterms:modified>2019-01-31</dcterms:modified>
        <rdfs:comment>The type of organism.</rdfs:comment>
        <skos:definition>The type of organism.</skos:definition>
        <rdfs:domain rdf:resource="http://www.w3.org/2002/07/owl#Thing"/>
        <rdfs:range rdf:resource="http://www.w3.org/2001/XMLSchema#string"/>
    </owl:DatatypeProperty>

    <owl:FunctionalProperty rdf:about="organismType"/>

    <owl:DatatypeProperty rdf:about="otherIdentification">
        <rdfs:label xml:lang="en">Other Identification</rdfs:label>
        <rdfs:isDefinedBy rdf:resource="http://rs.tdwg.org/abcd/terms/"/>
        <dwcattributes:status>recommended</dwcattributes:status>
        <dcterms:issued>2019-01-31</dcterms:issued>
        <dcterms:modified>2019-01-31</dcterms:modified>
        <rdfs:comment>Any other identification (numbers) known to exist in other collections for this accession.</rdfs:comment>
        <skos:definition>Any other identification (numbers) known to exist in other collections for this accession.</skos:definition>
        <rdfs:domain rdf:resource="http://www.w3.org/2002/07/owl#Thing"/>
        <rdfs:range rdf:resource="http://www.w3.org/2001/XMLSchema#string"/>
    </owl:DatatypeProperty>

    <owl:FunctionalProperty rdf:about="otherIdentification"/>

    <owl:DatatypeProperty rdf:about="otherProvider">
        <rdfs:label xml:lang="en">Other Provider</rdfs:label>
        <rdfs:isDefinedBy rdf:resource="http://rs.tdwg.org/abcd/terms/"/>
        <dwcattributes:status>recommended</dwcattributes:status>
        <dcterms:issued>2019-01-31</dcterms:issued>
        <dcterms:modified>2019-01-31</dcterms:modified>
        <rdfs:comment>The URI of another provider known to serve this dataset, usually expressed as an http URI or a UUID.</rdfs:comment>
        <skos:definition>The URI of another provider known to serve this dataset, usually expressed as an http URI or a UUID.</skos:definition>
        <rdfs:domain rdf:resource="http://www.w3.org/2002/07/owl#Thing"/>
        <rdfs:range rdf:resource="http://www.w3.org/2001/XMLSchema#string"/>
    </owl:DatatypeProperty>

    <owl:DatatypeProperty rdf:about="paleontologicalTimeRange">
        <rdfs:label xml:lang="en">Paleontological Time Range</rdfs:label>
        <rdfs:isDefinedBy rdf:resource="http://rs.tdwg.org/abcd/terms/"/>
        <dwcattributes:status>recommended</dwcattributes:status>
        <dcterms:issued>2019-01-31</dcterms:issued>
        <dcterms:modified>2019-01-31</dcterms:modified>
        <rdfs:comment>Known or assumed time range of a fossil.</rdfs:comment>
        <skos:definition>Known or assumed time range of a fossil.</skos:definition>
        <rdfs:domain rdf:resource="http://www.w3.org/2002/07/owl#Thing"/>
        <rdfs:range rdf:resource="http://www.w3.org/2001/XMLSchema#string"/>
    </owl:DatatypeProperty>

    <owl:FunctionalProperty rdf:about="paleontologicalTimeRange"/>

    <owl:DatatypeProperty rdf:about="parabola">
        <rdfs:label xml:lang="en">Parabola</rdfs:label>
        <rdfs:isDefinedBy rdf:resource="http://rs.tdwg.org/abcd/terms/"/>
        <dwcattributes:status>recommended</dwcattributes:status>
        <dcterms:issued>2019-01-31</dcterms:issued>
        <dcterms:modified>2019-01-31</dcterms:modified>
        <rdfs:comment>The kind of parabola used for the microphone when recording from a distance.</rdfs:comment>
        <skos:definition>The kind of parabola used for the microphone when recording from a distance.</skos:definition>
        <rdfs:domain rdf:resource="http://www.w3.org/2002/07/owl#Thing"/>
        <rdfs:range rdf:resource="http://www.w3.org/2001/XMLSchema#string"/>
    </owl:DatatypeProperty>

    <owl:FunctionalProperty rdf:about="parabola"/>

    <owl:DatatypeProperty rdf:about="parameter">
        <rdfs:label xml:lang="en">Parameter</rdfs:label>
        <rdfs:isDefinedBy rdf:resource="http://rs.tdwg.org/abcd/terms/"/>
        <dwcattributes:status>recommended</dwcattributes:status>
        <dcterms:issued>2019-01-31</dcterms:issued>
        <dcterms:modified>2019-01-31</dcterms:modified>
        <rdfs:comment>A parameter to which the result of a measurement is assigned.</rdfs:comment>
        <skos:definition>A parameter to which the result of a measurement is assigned.</skos:definition>
        <rdfs:domain rdf:resource="http://www.w3.org/2002/07/owl#Thing"/>
        <rdfs:range rdf:resource="http://www.w3.org/2001/XMLSchema#string"/>
        <skos:exactMatch rdf:resource="http://rs.tdwg.org/dwc/terms/measurementType"/>
    </owl:DatatypeProperty>

    <owl:FunctionalProperty rdf:about="parameter"/>

    <owl:DatatypeProperty rdf:about="parentheticalAuthorTeamAndYear">
        <rdfs:label xml:lang="en">Parenthetical Author Team And Year</rdfs:label>
        <rdfs:isDefinedBy rdf:resource="http://rs.tdwg.org/abcd/terms/"/>
        <dwcattributes:status>recommended</dwcattributes:status>
        <dcterms:issued>2019-01-31</dcterms:issued>
        <dcterms:modified>2019-01-31</dcterms:modified>
        <rdfs:comment>Author team and Year of the basionym of a species or subspecies combination.</rdfs:comment>
        <skos:definition>Author team and Year of the basionym of a species or subspecies combination.</skos:definition>
        <rdfs:domain rdf:resource="http://www.w3.org/2002/07/owl#Thing"/>
        <rdfs:range rdf:resource="http://www.w3.org/2001/XMLSchema#string"/>
    </owl:DatatypeProperty>

    <owl:FunctionalProperty rdf:about="parentheticalAuthorTeamAndYear"/>

    <owl:DatatypeProperty rdf:about="pathovar">
        <rdfs:label xml:lang="en">Pathovar</rdfs:label>
        <rdfs:isDefinedBy rdf:resource="http://rs.tdwg.org/abcd/terms/"/>
        <dwcattributes:status>recommended</dwcattributes:status>
        <dcterms:issued>2019-01-31</dcterms:issued>
        <dcterms:modified>2019-01-31</dcterms:modified>
        <rdfs:comment>Name and author of a pathovar.</rdfs:comment>
        <skos:definition>Name and author of a pathovar.</skos:definition>
        <rdfs:domain rdf:resource="http://www.w3.org/2002/07/owl#Thing"/>
        <rdfs:range rdf:resource="http://www.w3.org/2001/XMLSchema#string"/>
    </owl:DatatypeProperty>

    <owl:FunctionalProperty rdf:about="pathovar"/>

    <owl:DatatypeProperty rdf:about="perennation">
        <rdfs:label xml:lang="en">Perennation</rdfs:label>
        <rdfs:isDefinedBy rdf:resource="http://rs.tdwg.org/abcd/terms/"/>
        <dwcattributes:status>recommended</dwcattributes:status>
        <dcterms:issued>2019-01-31</dcterms:issued>
        <dcterms:modified>2019-01-31</dcterms:modified>
        <rdfs:comment>A code to indicate the means of perennation, providing a means of noting living plant accessions that require regular curatorial monitoring [ITF-2].</rdfs:comment>
        <skos:definition>A code to indicate the means of perennation, providing a means of noting living plant accessions that require regular curatorial monitoring [ITF-2].</skos:definition>
        <rdfs:domain rdf:resource="http://www.w3.org/2002/07/owl#Thing"/>
        <rdfs:range rdf:resource="http://www.w3.org/2001/XMLSchema#string"/>
    </owl:DatatypeProperty>

    <owl:FunctionalProperty rdf:about="perennation"/>

    <owl:DatatypeProperty rdf:about="periodExplicit">
        <rdfs:label xml:lang="en">Period Explicit</rdfs:label>
        <rdfs:isDefinedBy rdf:resource="http://rs.tdwg.org/abcd/terms/"/>
        <dwcattributes:status>recommended</dwcattributes:status>
        <dcterms:issued>2019-01-31</dcterms:issued>
        <dcterms:modified>2019-01-31</dcterms:modified>
        <rdfs:comment>This is an indicator for the explicitness of a period.</rdfs:comment>
        <skos:definition>This is an indicator for the explicitness of a period.</skos:definition>
        <dc:description>Set to "true" if the event explicitly  takes place for the entire period indicated. Set to "false" if it occurs at some point of time during the period. Not filled if unknown or no period specified (abcd:timeSpanEnd not used).</dc:description>
        <rdfs:domain rdf:resource="http://www.w3.org/2002/07/owl#Thing"/>
        <rdfs:range rdf:resource="http://www.w3.org/2001/XMLSchema#boolean"/>
    </owl:DatatypeProperty>

    <owl:FunctionalProperty rdf:about="periodExplicit"/>

    <owl:DatatypeProperty rdf:about="phaseOrStage">
        <rdfs:label xml:lang="en">Phase Or Stage</rdfs:label>
        <rdfs:isDefinedBy rdf:resource="http://rs.tdwg.org/abcd/terms/"/>
        <dwcattributes:status>recommended</dwcattributes:status>
        <dcterms:issued>2019-01-31</dcterms:issued>
        <dcterms:modified>2019-01-31</dcterms:modified>
        <rdfs:comment>A property for a phase or a stage of the organism(s) in the unit.</rdfs:comment>
        <skos:definition>A property for a phase or a stage of the organism(s) in the unit.</skos:definition>
        <rdfs:domain rdf:resource="http://www.w3.org/2002/07/owl#Thing"/>
        <rdfs:range rdf:resource="http://www.w3.org/2001/XMLSchema#string"/>
    </owl:DatatypeProperty>

    <owl:DatatypeProperty rdf:about="photographicSensitivity">
        <rdfs:label xml:lang="en">Photographic Sensitivity</rdfs:label>
        <rdfs:isDefinedBy rdf:resource="http://rs.tdwg.org/abcd/terms/"/>
        <dwcattributes:status>recommended</dwcattributes:status>
        <dcterms:issued>2019-01-31</dcterms:issued>
        <dcterms:modified>2019-01-31</dcterms:modified>
        <rdfs:comment>EXIF term. This tag indicates the sensitivity of the camera or input device when the image was shot.</rdfs:comment>
        <skos:definition>EXIF term. This tag indicates the sensitivity of the camera or input device when the image was shot.</skos:definition>
        <dc:description>More specifically, it indicates one of the following values that are parameters defined in ISO 12232: standard output sensitivity (SOS), recommended exposure index (REI), or ISO speed.</dc:description>
        <dc:description>Note that this tag was referred to as &#8220;ISOSpeedRatings&#8221; in previous versions of the EXIF standard up to Version 2.21.</dc:description>
        <rdfs:domain rdf:resource="http://www.w3.org/2002/07/owl#Thing"/>
        <rdfs:range rdf:resource="http://www.w3.org/2001/XMLSchema#string"/>
    </owl:DatatypeProperty>

    <owl:DatatypeProperty rdf:about="physicalFormat">
        <rdfs:label xml:lang="en">Physical Format</rdfs:label>
        <rdfs:isDefinedBy rdf:resource="http://rs.tdwg.org/abcd/terms/"/>
        <dwcattributes:status>recommended</dwcattributes:status>
        <dcterms:issued>2019-01-31</dcterms:issued>
        <dcterms:modified>2019-01-31</dcterms:modified>
        <rdfs:comment>Code or descriptive term for physical format of record.</rdfs:comment>
        <skos:definition>Code or descriptive term for physical format of record.</skos:definition>
        <rdfs:domain rdf:resource="http://www.w3.org/2002/07/owl#Thing"/>
        <rdfs:range rdf:resource="http://www.w3.org/2001/XMLSchema#string"/>
    </owl:DatatypeProperty>

    <owl:DatatypeProperty rdf:about="physicalObjectID">
        <rdfs:label xml:lang="en">Physical Object ID</rdfs:label>
        <rdfs:isDefinedBy rdf:resource="http://rs.tdwg.org/abcd/terms/"/>
        <dwcattributes:status>recommended</dwcattributes:status>
        <dcterms:issued>2019-01-31</dcterms:issued>
        <dcterms:modified>2019-01-31</dcterms:modified>
        <rdfs:comment>Code or descriptive term for identifier of physical item in a collection like a tape number or catalog number of photograph.</rdfs:comment>
        <skos:definition>Code or descriptive term for identifier of physical item in a collection like a tape number or catalog number of photograph.</skos:definition>
        <rdfs:subPropertyOf rdf:resource="id"/>
        <rdfs:domain rdf:resource="http://www.w3.org/2002/07/owl#Thing"/>
        <rdfs:range rdf:resource="http://www.w3.org/2001/XMLSchema#string"/>
    </owl:DatatypeProperty>

    <owl:DatatypeProperty rdf:about="pitch">
        <rdfs:label xml:lang="en">Pitch</rdfs:label>
        <rdfs:isDefinedBy rdf:resource="http://rs.tdwg.org/abcd/terms/"/>
        <dwcattributes:status>recommended</dwcattributes:status>
        <dcterms:issued>2019-01-31</dcterms:issued>
        <dcterms:modified>2019-01-31</dcterms:modified>
        <rdfs:domain rdf:resource="http://www.w3.org/2002/07/owl#Thing"/>
        <rdfs:range rdf:resource="http://www.w3.org/2001/XMLSchema#string"/>
    </owl:DatatypeProperty>

    <owl:FunctionalProperty rdf:about="pitch"/>

    <owl:DatatypeProperty rdf:about="platformName">
        <rdfs:label xml:lang="en">Platform Name</rdfs:label>
        <rdfs:isDefinedBy rdf:resource="http://rs.tdwg.org/abcd/terms/"/>
        <dwcattributes:status>recommended</dwcattributes:status>
        <dcterms:issued>2019-01-31</dcterms:issued>
        <dcterms:modified>2019-01-31</dcterms:modified>
        <rdfs:comment>The platform from which observations or collections were made (e.g. the name of a research vessel or a remote operated vehicle).</rdfs:comment>
        <skos:definition>The platform from which observations or collections were made (e.g. the name of a research vessel or a remote operated vehicle).</skos:definition>
        <rdfs:domain rdf:resource="http://www.w3.org/2002/07/owl#Thing"/>
        <rdfs:range rdf:resource="http://www.w3.org/2001/XMLSchema#string"/>
    </owl:DatatypeProperty>

    <owl:DatatypeProperty rdf:about="playbackUsed">
        <rdfs:label xml:lang="en">Playback Used</rdfs:label>
        <rdfs:isDefinedBy rdf:resource="http://rs.tdwg.org/abcd/terms/"/>
        <dwcattributes:status>recommended</dwcattributes:status>
        <dcterms:issued>2019-01-31</dcterms:issued>
        <dcterms:modified>2019-01-31</dcterms:modified>
        <rdfs:comment>Boolean flag to indicate whether a playback was used to stimulate singing of the animal to be recorded.</rdfs:comment>
        <skos:definition>Boolean flag to indicate whether a playback was used to stimulate singing of the animal to be recorded.</skos:definition>
        <rdfs:domain rdf:resource="http://www.w3.org/2002/07/owl#Thing"/>
        <rdfs:range rdf:resource="http://www.w3.org/2001/XMLSchema#boolean"/>
    </owl:DatatypeProperty>

    <owl:DatatypeProperty rdf:about="pointRadiusSpatialFit">
        <rdfs:label xml:lang="en">Point Radius Spatial Fit</rdfs:label>
        <rdfs:isDefinedBy rdf:resource="http://rs.tdwg.org/abcd/terms/"/>
        <dwcattributes:status>recommended</dwcattributes:status>
        <dcterms:issued>2019-01-31</dcterms:issued>
        <dcterms:modified>2019-01-31</dcterms:modified>
        <rdfs:comment>A measure of how well the circle defined by the coordinates and uncertainty match the original spatial representation, as a ratio of the area of the circle to the area of the original spatial representation.</rdfs:comment>
        <skos:definition>A measure of how well the circle defined by the coordinates and uncertainty match the original spatial representation, as a ratio of the area of the circle to the area of the original spatial representation.</skos:definition>
        <dc:description>If both the original and the given georeference are the same point, the PointRadiusSpatialFit is 1. Detailed explanations with graphical examples can be found in the Guide to Best Practices for Georeferencing (Chapman and Wieczorek, eds. 2006).</dc:description>
        <dc:description>Legal values are 0, greater than or equal to 1, or undefined. A value of 1 is an exact match or 100% overlap. A value of 0 should be used if the given georeference does not completely contain the original representation. The PointRadiusSpatialFit is undefined if the original representation is a point without uncertainty and the given georeference is not that same point (without uncertainty).</dc:description>
        <rdfs:domain rdf:resource="http://www.w3.org/2002/07/owl#Thing"/>
        <rdfs:range rdf:resource="http://www.w3.org/2001/XMLSchema#string"/>
        <skos:exactMatch rdf:resource="http://rs.tdwg.org/dwc/terms/pointRadiusSpatialFit"/>
    </owl:DatatypeProperty>

    <owl:FunctionalProperty rdf:about="pointRadiusSpatialFit"/>

    <owl:DatatypeProperty rdf:about="positionOnObject">
        <rdfs:label xml:lang="en">Position On Object</rdfs:label>
        <rdfs:isDefinedBy rdf:resource="http://rs.tdwg.org/abcd/terms/"/>
        <dwcattributes:status>recommended</dwcattributes:status>
        <dcterms:issued>2019-01-31</dcterms:issued>
        <dcterms:modified>2019-01-31</dcterms:modified>
        <rdfs:comment>The position of the inscription, writing or label on the object.</rdfs:comment>
        <skos:definition>The position of the inscription, writing or label on the object.</skos:definition>
        <rdfs:domain rdf:resource="http://www.w3.org/2002/07/owl#Thing"/>
        <rdfs:range rdf:resource="http://www.w3.org/2001/XMLSchema#string"/>
    </owl:DatatypeProperty>

    <owl:FunctionalProperty rdf:about="positionOnObject"/>

    <owl:DatatypeProperty rdf:about="preferredName">
        <rdfs:label xml:lang="en">Preferred Name</rdfs:label>
        <rdfs:isDefinedBy rdf:resource="http://rs.tdwg.org/abcd/terms/"/>
        <dwcattributes:status>recommended</dwcattributes:status>
        <dcterms:issued>2019-01-31</dcterms:issued>
        <dcterms:modified>2019-01-31</dcterms:modified>
        <rdfs:comment>The preferred name of a Person.</rdfs:comment>
        <skos:definition>The preferred name of a Person.</skos:definition>
        <dc:description>The preferred name may differ from the first given name (e.g. second given name, nickname).</dc:description>
        <rdfs:domain rdf:resource="http://www.w3.org/2002/07/owl#Thing"/>
        <rdfs:range rdf:resource="http://www.w3.org/2001/XMLSchema#string"/>
        <skos:relatedMatch rdf:resource="http://www.w3.org/2006/vcard/ns#nickname"/>
    </owl:DatatypeProperty>

    <owl:FunctionalProperty rdf:about="preferredName"/>

    <owl:DatatypeProperty rdf:about="preparationMaterials">
        <rdfs:label xml:lang="en">Preparation Materials</rdfs:label>
        <rdfs:isDefinedBy rdf:resource="http://rs.tdwg.org/abcd/terms/"/>
        <dwcattributes:status>recommended</dwcattributes:status>
        <dcterms:issued>2019-01-31</dcterms:issued>
        <dcterms:modified>2019-01-31</dcterms:modified>
        <rdfs:comment>Materials and chemicals used in the preparation of the specimen, tissue, DNA or RNA sample.</rdfs:comment>
        <skos:definition>Materials and chemicals used in the preparation of the specimen, tissue, DNA or RNA sample.</skos:definition>
        <rdfs:domain rdf:resource="http://www.w3.org/2002/07/owl#Thing"/>
        <rdfs:range rdf:resource="http://www.w3.org/2001/XMLSchema#string"/>
    </owl:DatatypeProperty>

    <owl:FunctionalProperty rdf:about="preparationMaterials"/>

    <owl:DatatypeProperty rdf:about="preparationType">
        <rdfs:label xml:lang="en">Preparation Type</rdfs:label>
        <rdfs:isDefinedBy rdf:resource="http://rs.tdwg.org/abcd/terms/"/>
        <dwcattributes:status>recommended</dwcattributes:status>
        <dcterms:issued>2019-01-31</dcterms:issued>
        <dcterms:modified>2019-01-31</dcterms:modified>
        <rdfs:comment>Description of preparation type (specimens, tissues, DNA).</rdfs:comment>
        <skos:definition>Description of preparation type (specimens, tissues, DNA).</skos:definition>
        <rdfs:domain rdf:resource="http://www.w3.org/2002/07/owl#Thing"/>
        <rdfs:range rdf:resource="http://www.w3.org/2001/XMLSchema#string"/>
    </owl:DatatypeProperty>

    <owl:FunctionalProperty rdf:about="preparationType"/>

    <owl:DatatypeProperty rdf:about="preparationsText">
        <rdfs:label xml:lang="en">Preparations Text</rdfs:label>
        <rdfs:isDefinedBy rdf:resource="http://rs.tdwg.org/abcd/terms/"/>
        <dwcattributes:status>recommended</dwcattributes:status>
        <dcterms:issued>2019-01-31</dcterms:issued>
        <dcterms:modified>2019-01-31</dcterms:modified>
        <rdfs:comment>Textual account of preparation.</rdfs:comment>
        <skos:definition>Textual account of preparation.</skos:definition>
        <rdfs:domain rdf:resource="http://www.w3.org/2002/07/owl#Thing"/>
        <rdfs:range rdf:resource="http://www.w3.org/2001/XMLSchema#string"/>
    </owl:DatatypeProperty>

    <owl:FunctionalProperty rdf:about="preparationsText"/>

    <owl:DatatypeProperty rdf:about="preservationType">
        <rdfs:label xml:lang="en">Preservation Type</rdfs:label>
        <rdfs:isDefinedBy rdf:resource="http://rs.tdwg.org/abcd/terms/"/>
        <dwcattributes:status>recommended</dwcattributes:status>
        <dcterms:issued>2019-01-31</dcterms:issued>
        <dcterms:modified>2019-01-31</dcterms:modified>
        <rdfs:comment>Description of preservation type.</rdfs:comment>
        <skos:definition>Description of preservation type.</skos:definition>
        <rdfs:domain rdf:resource="http://www.w3.org/2002/07/owl#Thing"/>
        <rdfs:range rdf:resource="http://www.w3.org/2001/XMLSchema#string"/>
    </owl:DatatypeProperty>

    <owl:FunctionalProperty rdf:about="preservationType"/>

    <owl:DatatypeProperty rdf:about="previousUnitText">
        <rdfs:label xml:lang="en">Previous Unit Text</rdfs:label>
        <rdfs:isDefinedBy rdf:resource="http://rs.tdwg.org/abcd/terms/"/>
        <dwcattributes:status>recommended</dwcattributes:status>
        <dcterms:issued>2019-01-31</dcterms:issued>
        <dcterms:modified>2019-01-31</dcterms:modified>
        <rdfs:comment>Alternative text identifying the previous unit when no ABCD standard IDs can be assigned.</rdfs:comment>
        <skos:definition>Alternative text identifying the previous unit when no ABCD standard IDs can be assigned.</skos:definition>
        <rdfs:domain rdf:resource="http://www.w3.org/2002/07/owl#Thing"/>
        <rdfs:range rdf:resource="http://www.w3.org/2001/XMLSchema#string"/>
    </owl:DatatypeProperty>

    <owl:FunctionalProperty rdf:about="previousUnitText"/>

    <owl:DatatypeProperty rdf:about="previousUnitsText">
        <rdfs:label xml:lang="en">Previous Units Text</rdfs:label>
        <rdfs:isDefinedBy rdf:resource="http://rs.tdwg.org/abcd/terms/"/>
        <dwcattributes:status>recommended</dwcattributes:status>
        <dcterms:issued>2019-01-31</dcterms:issued>
        <dcterms:modified>2019-01-31</dcterms:modified>
        <rdfs:comment>An alternative text identifying the previous units.</rdfs:comment>
        <skos:definition>An alternative text identifying the previous units.</skos:definition>
        <rdfs:domain rdf:resource="http://www.w3.org/2002/07/owl#Thing"/>
        <rdfs:range rdf:resource="http://www.w3.org/2001/XMLSchema#string"/>
    </owl:DatatypeProperty>

    <owl:FunctionalProperty rdf:about="previousUnitsText"/>

    <owl:DatatypeProperty rdf:about="productURL">
        <rdfs:label xml:lang="en">Product URL</rdfs:label>
        <rdfs:isDefinedBy rdf:resource="http://rs.tdwg.org/abcd/terms/"/>
        <dwcattributes:status>recommended</dwcattributes:status>
        <dcterms:issued>2019-01-31</dcterms:issued>
        <dcterms:modified>2019-01-31</dcterms:modified>
        <rdfs:comment>The URL of a web page were the multimedia file is presented, including additional meta information, possibly with the support of web viewers or players.</rdfs:comment>
        <skos:definition>The URL of a web page were the multimedia file is presented, including additional meta information, possibly with the support of web viewers or players.</skos:definition>
        <rdfs:domain rdf:resource="http://www.w3.org/2002/07/owl#Thing"/>
        <rdfs:range rdf:resource="http://www.w3.org/2001/XMLSchema#anyURI"/>
    </owl:DatatypeProperty>

    <owl:DatatypeProperty rdf:about="propagation">
        <rdfs:label xml:lang="en">Propagation</rdfs:label>
        <rdfs:isDefinedBy rdf:resource="http://rs.tdwg.org/abcd/terms/"/>
        <dwcattributes:status>recommended</dwcattributes:status>
        <dcterms:issued>2019-01-31</dcterms:issued>
        <dcterms:modified>2019-01-31</dcterms:modified>
        <rdfs:comment>Allows for information about any propagation requirements to be passed as free text in order to help the receiving garden propagate the transferred accession [ITF-2] or to record the garden's experience made with this accession.</rdfs:comment>
        <skos:definition>Allows for information about any propagation requirements to be passed as free text in order to help the receiving garden propagate the transferred accession [ITF-2] or to record the garden's experience made with this accession.</skos:definition>
        <rdfs:domain rdf:resource="http://www.w3.org/2002/07/owl#Thing"/>
        <rdfs:range rdf:resource="http://www.w3.org/2001/XMLSchema#string"/>
    </owl:DatatypeProperty>

    <owl:FunctionalProperty rdf:about="propagation"/>

    <owl:DatatypeProperty rdf:about="propagationHistoryCode">
        <rdfs:label xml:lang="en">Propagation History Code</rdfs:label>
        <rdfs:isDefinedBy rdf:resource="http://rs.tdwg.org/abcd/terms/"/>
        <dwcattributes:status>recommended</dwcattributes:status>
        <dcterms:issued>2019-01-31</dcterms:issued>
        <dcterms:modified>2019-01-31</dcterms:modified>
        <rdfs:comment>A code to indicate the nature of the production of the plant material being accessioned, for use in association with the concept Provenance Category. [ITF-2]</rdfs:comment>
        <skos:definition>A code to indicate the nature of the production of the plant material being accessioned, for use in association with the concept Provenance Category. [ITF-2]</skos:definition>
        <rdfs:domain rdf:resource="http://www.w3.org/2002/07/owl#Thing"/>
        <rdfs:range rdf:resource="http://www.w3.org/2001/XMLSchema#string"/>
    </owl:DatatypeProperty>

    <owl:FunctionalProperty rdf:about="propagationHistoryCode"/>

    <owl:DatatypeProperty rdf:about="provenanceCategory">
        <rdfs:label xml:lang="en">Provenance Category</rdfs:label>
        <rdfs:isDefinedBy rdf:resource="http://rs.tdwg.org/abcd/terms/"/>
        <dwcattributes:status>recommended</dwcattributes:status>
        <dcterms:issued>2019-01-31</dcterms:issued>
        <dcterms:modified>2019-01-31</dcterms:modified>
        <rdfs:comment>A code to indicate the provenance of the accession [ITF-2].</rdfs:comment>
        <skos:definition>A code to indicate the provenance of the accession [ITF-2].</skos:definition>
        <rdfs:domain rdf:resource="http://www.w3.org/2002/07/owl#Thing"/>
        <rdfs:range rdf:resource="http://www.w3.org/2001/XMLSchema#string"/>
    </owl:DatatypeProperty>

    <owl:FunctionalProperty rdf:about="provenanceCategory"/>

    <owl:DatatypeProperty rdf:about="pulseDistanceRegularity">
        <rdfs:label xml:lang="en">Pulse Distance Regularity</rdfs:label>
        <rdfs:isDefinedBy rdf:resource="http://rs.tdwg.org/abcd/terms/"/>
        <dwcattributes:status>recommended</dwcattributes:status>
        <dcterms:issued>2019-01-31</dcterms:issued>
        <dcterms:modified>2019-01-31</dcterms:modified>
        <rdfs:comment>For describing the sound or call of an animal.</rdfs:comment>
        <skos:definition>For describing the sound or call of an animal.</skos:definition>
        <rdfs:domain rdf:resource="http://www.w3.org/2002/07/owl#Thing"/>
        <rdfs:range rdf:resource="http://www.w3.org/2001/XMLSchema#string"/>
    </owl:DatatypeProperty>

    <owl:FunctionalProperty rdf:about="pulseDistanceRegularity"/>

    <owl:DatatypeProperty rdf:about="pulseEnergyContour">
        <rdfs:label xml:lang="en">Pulse Energy Contour</rdfs:label>
        <rdfs:isDefinedBy rdf:resource="http://rs.tdwg.org/abcd/terms/"/>
        <dwcattributes:status>recommended</dwcattributes:status>
        <dcterms:issued>2019-01-31</dcterms:issued>
        <dcterms:modified>2019-01-31</dcterms:modified>
        <rdfs:comment>For describing the sound or call of an animal.</rdfs:comment>
        <skos:definition>For describing the sound or call of an animal.</skos:definition>
        <rdfs:domain rdf:resource="http://www.w3.org/2002/07/owl#Thing"/>
        <rdfs:range rdf:resource="http://www.w3.org/2001/XMLSchema#string"/>
    </owl:DatatypeProperty>

    <owl:FunctionalProperty rdf:about="pulseEnergyContour"/>

    <owl:DatatypeProperty rdf:about="pulseFrequencyContour">
        <rdfs:label xml:lang="en">Pulse Frequency Contour</rdfs:label>
        <rdfs:isDefinedBy rdf:resource="http://rs.tdwg.org/abcd/terms/"/>
        <dwcattributes:status>recommended</dwcattributes:status>
        <dcterms:issued>2019-01-31</dcterms:issued>
        <dcterms:modified>2019-01-31</dcterms:modified>
        <rdfs:comment>For describing the sound or call of an animal.</rdfs:comment>
        <skos:definition>For describing the sound or call of an animal.</skos:definition>
        <rdfs:domain rdf:resource="http://www.w3.org/2002/07/owl#Thing"/>
        <rdfs:range rdf:resource="http://www.w3.org/2001/XMLSchema#string"/>
    </owl:DatatypeProperty>

    <owl:FunctionalProperty rdf:about="pulseFrequencyContour"/>

    <owl:DatatypeProperty rdf:about="pulseFrequencyModulations">
        <rdfs:label xml:lang="en">Pulse Frequency Modulations</rdfs:label>
        <rdfs:isDefinedBy rdf:resource="http://rs.tdwg.org/abcd/terms/"/>
        <dwcattributes:status>recommended</dwcattributes:status>
        <dcterms:issued>2019-01-31</dcterms:issued>
        <dcterms:modified>2019-01-31</dcterms:modified>
        <rdfs:comment>For describing the sound or call of an animal.</rdfs:comment>
        <skos:definition>For describing the sound or call of an animal.</skos:definition>
        <rdfs:domain rdf:resource="http://www.w3.org/2002/07/owl#Thing"/>
        <rdfs:range rdf:resource="http://www.w3.org/2001/XMLSchema#string"/>
    </owl:DatatypeProperty>

    <owl:DatatypeProperty rdf:about="pulseGrouping">
        <rdfs:label xml:lang="en">Pulse Grouping</rdfs:label>
        <rdfs:isDefinedBy rdf:resource="http://rs.tdwg.org/abcd/terms/"/>
        <dwcattributes:status>recommended</dwcattributes:status>
        <dcterms:issued>2019-01-31</dcterms:issued>
        <dcterms:modified>2019-01-31</dcterms:modified>
        <rdfs:comment>For describing the sound or call of an animal.</rdfs:comment>
        <skos:definition>For describing the sound or call of an animal.</skos:definition>
        <rdfs:domain rdf:resource="http://www.w3.org/2002/07/owl#Thing"/>
        <rdfs:range rdf:resource="http://www.w3.org/2001/XMLSchema#string"/>
    </owl:DatatypeProperty>

    <owl:DatatypeProperty rdf:about="pulseLength">
        <rdfs:label xml:lang="en">Pulse Length</rdfs:label>
        <rdfs:isDefinedBy rdf:resource="http://rs.tdwg.org/abcd/terms/"/>
        <dwcattributes:status>recommended</dwcattributes:status>
        <dcterms:issued>2019-01-31</dcterms:issued>
        <dcterms:modified>2019-01-31</dcterms:modified>
        <rdfs:comment>For describing the sound or call of an animal.</rdfs:comment>
        <skos:definition>For describing the sound or call of an animal.</skos:definition>
        <rdfs:domain rdf:resource="http://www.w3.org/2002/07/owl#Thing"/>
        <rdfs:range rdf:resource="http://www.w3.org/2001/XMLSchema#string"/>
    </owl:DatatypeProperty>

    <owl:DatatypeProperty rdf:about="pulseMaximumAmplitude">
        <rdfs:label xml:lang="en">Pulse Maximum Amplitude</rdfs:label>
        <rdfs:isDefinedBy rdf:resource="http://rs.tdwg.org/abcd/terms/"/>
        <dwcattributes:status>recommended</dwcattributes:status>
        <dcterms:issued>2019-01-31</dcterms:issued>
        <dcterms:modified>2019-01-31</dcterms:modified>
        <rdfs:comment>For describing the sound or call of an animal.</rdfs:comment>
        <skos:definition>For describing the sound or call of an animal.</skos:definition>
        <rdfs:domain rdf:resource="http://www.w3.org/2002/07/owl#Thing"/>
        <rdfs:range rdf:resource="http://www.w3.org/2001/XMLSchema#string"/>
    </owl:DatatypeProperty>

    <owl:FunctionalProperty rdf:about="pulseMaximumAmplitude"/>

    <owl:DatatypeProperty rdf:about="pulseRepetitionRate">
        <rdfs:label xml:lang="en">Pulse Repetition Rate</rdfs:label>
        <rdfs:isDefinedBy rdf:resource="http://rs.tdwg.org/abcd/terms/"/>
        <dwcattributes:status>recommended</dwcattributes:status>
        <dcterms:issued>2019-01-31</dcterms:issued>
        <dcterms:modified>2019-01-31</dcterms:modified>
        <rdfs:comment>For describing the sound or call of an animal.</rdfs:comment>
        <skos:definition>For describing the sound or call of an animal.</skos:definition>
        <rdfs:domain rdf:resource="http://www.w3.org/2002/07/owl#Thing"/>
        <rdfs:range rdf:resource="http://www.w3.org/2001/XMLSchema#string"/>
    </owl:DatatypeProperty>

    <owl:FunctionalProperty rdf:about="pulseRepetitionRate"/>

    <owl:DatatypeProperty rdf:about="pulseTimeEncodedSignal">
        <rdfs:label xml:lang="en">Pulse Time Encoded Signal</rdfs:label>
        <rdfs:isDefinedBy rdf:resource="http://rs.tdwg.org/abcd/terms/"/>
        <dwcattributes:status>recommended</dwcattributes:status>
        <dcterms:issued>2019-01-31</dcterms:issued>
        <dcterms:modified>2019-01-31</dcterms:modified>
        <rdfs:comment>For describing the sound or call of an animal.</rdfs:comment>
        <skos:definition>For describing the sound or call of an animal.</skos:definition>
        <rdfs:domain rdf:resource="http://www.w3.org/2002/07/owl#Thing"/>
        <rdfs:range rdf:resource="http://www.w3.org/2001/XMLSchema#string"/>
    </owl:DatatypeProperty>

    <owl:DatatypeProperty rdf:about="recordingEnvironment">
        <rdfs:label xml:lang="en">Recording Environment</rdfs:label>
        <rdfs:isDefinedBy rdf:resource="http://rs.tdwg.org/abcd/terms/"/>
        <dwcattributes:status>recommended</dwcattributes:status>
        <dcterms:issued>2019-01-31</dcterms:issued>
        <dcterms:modified>2019-01-31</dcterms:modified>
        <rdfs:comment>The context or surrounding in which the multimedia object was created.</rdfs:comment>
        <skos:definition>The context or surrounding in which the multimedia object was created.</skos:definition>
        <rdfs:domain rdf:resource="http://www.w3.org/2002/07/owl#Thing"/>
        <rdfs:range rdf:resource="http://www.w3.org/2001/XMLSchema#string"/>
    </owl:DatatypeProperty>

    <owl:DatatypeProperty rdf:about="referenceSystem">
        <rdfs:label xml:lang="en">Reference System</rdfs:label>
        <rdfs:isDefinedBy rdf:resource="http://rs.tdwg.org/abcd/terms/"/>
        <dwcattributes:status>recommended</dwcattributes:status>
        <dcterms:issued>2019-01-31</dcterms:issued>
        <dcterms:modified>2019-01-31</dcterms:modified>
        <rdfs:comment>The reference system used for measuring, such as the geodetic datum.</rdfs:comment>
        <skos:definition>The reference system used for measuring, such as the geodetic datum.</skos:definition>
        <dc:description>Particularly to be used with the special Measurement Or Fact assertions: abcd:hasHeight, abcd:hasAltitude and abcd:hasDepth.</dc:description>
        <rdfs:domain rdf:resource="http://www.w3.org/2002/07/owl#Thing"/>
        <rdfs:range rdf:resource="http://www.w3.org/2001/XMLSchema#string"/>
        <vann:termGroup rdf:resource="Measurement Or Fact"/>
    </owl:DatatypeProperty>

    <owl:DatatypeProperty rdf:about="resourceURI">
        <rdfs:label xml:lang="en">Resource URI</rdfs:label>
        <rdfs:isDefinedBy rdf:resource="http://rs.tdwg.org/abcd/terms/"/>
        <dwcattributes:status>recommended</dwcattributes:status>
        <dcterms:issued>2019-01-31</dcterms:issued>
        <dcterms:modified>2019-01-31</dcterms:modified>
        <rdfs:comment>An preferably resolvable URI to uniquely identify a concept.</rdfs:comment>
        <skos:definition>An preferably resolvable URI to uniquely identify a concept.</skos:definition>
        <rdfs:subPropertyOf rdf:resource="guid"/>
        <dc:description>Common identifiers are ORCIDs for person identifiers or stable CETAF identifiers for specimen.</dc:description>
        <rdfs:domain rdf:resource="http://www.w3.org/2002/07/owl#Thing"/>
        <rdfs:range rdf:resource="http://www.w3.org/2001/XMLSchema#anyURI"/>
    </owl:DatatypeProperty>

    <owl:DatatypeProperty rdf:about="resultRole">
        <rdfs:label xml:lang="en">Result Role</rdfs:label>
        <rdfs:isDefinedBy rdf:resource="http://rs.tdwg.org/abcd/terms/"/>
        <dwcattributes:status>recommended</dwcattributes:status>
        <dcterms:issued>2019-01-31</dcterms:issued>
        <dcterms:modified>2019-01-31</dcterms:modified>
        <rdfs:comment>The result role is used to designate the role of the identification result (e.g. substrate, isolate, host, parasite, etc.)</rdfs:comment>
        <skos:definition>The result role is used to designate the role of the identification result (e.g. substrate, isolate, host, parasite, etc.)</skos:definition>
        <rdfs:domain rdf:resource="http://www.w3.org/2002/07/owl#Thing"/>
        <rdfs:range rdf:resource="http://www.w3.org/2001/XMLSchema#string"/>
    </owl:DatatypeProperty>

    <owl:FunctionalProperty rdf:about="resultRole"/>

    <owl:DatatypeProperty rdf:about="role">
        <rdfs:label xml:lang="en">Role</rdfs:label>
        <rdfs:isDefinedBy rdf:resource="http://rs.tdwg.org/abcd/terms/"/>
        <dwcattributes:status>recommended</dwcattributes:status>
        <dcterms:issued>2019-01-31</dcterms:issued>
        <dcterms:modified>2019-01-31</dcterms:modified>
        <rdfs:comment>The function a Contact fulfills.</rdfs:comment>
        <skos:definition>The function a Contact fulfills.</skos:definition>
        <rdfs:domain rdf:resource="http://www.w3.org/2002/07/owl#Thing"/>
        <rdfs:range rdf:resource="http://www.w3.org/2001/XMLSchema#string"/>
        <skos:exactMatch rdf:resource="http://www.w3.org/2006/vcard/ns#role"/>
    </owl:DatatypeProperty>

    <owl:DatatypeProperty rdf:about="sampleDesignation">
        <rdfs:label xml:lang="en">Sample Designation</rdfs:label>
        <rdfs:isDefinedBy rdf:resource="http://rs.tdwg.org/abcd/terms/"/>
        <dwcattributes:status>recommended</dwcattributes:status>
        <dcterms:issued>2019-01-31</dcterms:issued>
        <dcterms:modified>2019-01-31</dcterms:modified>
        <rdfs:comment>Designated number or identifier of sample, usually project number used in the lab.</rdfs:comment>
        <skos:definition>Designated number or identifier of sample, usually project number used in the lab.</skos:definition>
        <rdfs:domain rdf:resource="http://www.w3.org/2002/07/owl#Thing"/>
        <rdfs:range rdf:resource="http://www.w3.org/2001/XMLSchema#string"/>
    </owl:DatatypeProperty>

    <owl:DatatypeProperty rdf:about="sampleSize">
        <rdfs:label xml:lang="en">Sample Size</rdfs:label>
        <rdfs:isDefinedBy rdf:resource="http://rs.tdwg.org/abcd/terms/"/>
        <dwcattributes:status>recommended</dwcattributes:status>
        <dcterms:issued>2019-01-31</dcterms:issued>
        <dcterms:modified>2019-01-31</dcterms:modified>
        <rdfs:comment>MIxS element. Amount or size of sample (volume, mass or area) that was collected.</rdfs:comment>
        <skos:definition>MIxS element. Amount or size of sample (volume, mass or area) that was collected.</skos:definition>
        <rdfs:domain rdf:resource="http://www.w3.org/2002/07/owl#Thing"/>
        <rdfs:range rdf:resource="http://www.w3.org/2001/XMLSchema#string"/>
    </owl:DatatypeProperty>

    <owl:DatatypeProperty rdf:about="samplingRate">
        <rdfs:label xml:lang="en">Sampling Rate</rdfs:label>
        <rdfs:isDefinedBy rdf:resource="http://rs.tdwg.org/abcd/terms/"/>
        <dwcattributes:status>recommended</dwcattributes:status>
        <dcterms:issued>2019-01-31</dcterms:issued>
        <dcterms:modified>2019-01-31</dcterms:modified>
        <rdfs:comment>The number of times per second the analog signal is sampled when recording or converting into a digital format, expressed in Kilohertz (kHz).</rdfs:comment>
        <skos:definition>The number of times per second the analog signal is sampled when recording or converting into a digital format, expressed in Kilohertz (kHz).</skos:definition>
        <rdfs:domain rdf:resource="http://www.w3.org/2002/07/owl#Thing"/>
        <rdfs:range rdf:resource="http://www.w3.org/2001/XMLSchema#decimal"/>
    </owl:DatatypeProperty>

    <owl:FunctionalProperty rdf:about="samplingRate"/>

    <owl:DatatypeProperty rdf:about="saturation">
        <rdfs:label xml:lang="en">Saturation</rdfs:label>
        <rdfs:isDefinedBy rdf:resource="http://rs.tdwg.org/abcd/terms/"/>
        <dwcattributes:status>recommended</dwcattributes:status>
        <dcterms:issued>2019-01-31</dcterms:issued>
        <dcterms:modified>2019-01-31</dcterms:modified>
        <rdfs:comment>This property indicates the direction of saturation processing applied by the camera when the image was shot.</rdfs:comment>
        <skos:definition>This property indicates the direction of saturation processing applied by the camera when the image was shot.</skos:definition>
        <rdfs:domain rdf:resource="http://www.w3.org/2002/07/owl#Thing"/>
        <rdfs:range rdf:resource="http://www.w3.org/2001/XMLSchema#string"/>
    </owl:DatatypeProperty>

    <owl:DatatypeProperty rdf:about="scope">
        <rdfs:label xml:lang="en">Scope</rdfs:label>
        <rdfs:isDefinedBy rdf:resource="http://rs.tdwg.org/abcd/terms/"/>
        <dwcattributes:status>recommended</dwcattributes:status>
        <dcterms:issued>2019-01-31</dcterms:issued>
        <dcterms:modified>2019-01-31</dcterms:modified>
        <rdfs:comment>A keyword describing the scope of a class.</rdfs:comment>
        <skos:definition>A keyword describing the scope of a class.</skos:definition>
        <rdfs:domain rdf:resource="http://www.w3.org/2002/07/owl#Thing"/>
        <rdfs:range rdf:resource="http://www.w3.org/2001/XMLSchema#string"/>
        <vann:termGroup rdf:resource="Data Set"/>
    </owl:DatatypeProperty>

    <owl:DatatypeProperty rdf:about="sequenceDatabase">
        <rdfs:label xml:lang="en">Sequence Database</rdfs:label>
        <rdfs:isDefinedBy rdf:resource="http://rs.tdwg.org/abcd/terms/"/>
        <dwcattributes:status>recommended</dwcattributes:status>
        <dcterms:issued>2019-01-31</dcterms:issued>
        <dcterms:modified>2019-01-31</dcterms:modified>
        <rdfs:comment>The database holding the sequence data.</rdfs:comment>
        <skos:definition>The database holding the sequence data.</skos:definition>
        <dc:description>Use "Internal" for an unpublished sequence.</dc:description>
        <rdfs:domain rdf:resource="http://www.w3.org/2002/07/owl#Thing"/>
        <rdfs:range rdf:resource="http://www.w3.org/2001/XMLSchema#string"/>
    </owl:DatatypeProperty>

    <owl:FunctionalProperty rdf:about="sequenceDatabase"/>

    <owl:DatatypeProperty rdf:about="sequenceLength">
        <rdfs:label xml:lang="en">Sequence Length</rdfs:label>
        <rdfs:isDefinedBy rdf:resource="http://rs.tdwg.org/abcd/terms/"/>
        <dwcattributes:status>recommended</dwcattributes:status>
        <dcterms:issued>2019-01-31</dcterms:issued>
        <dcterms:modified>2019-01-31</dcterms:modified>
        <rdfs:comment>The length of the sequence in basepairs.</rdfs:comment>
        <skos:definition>The length of the sequence in basepairs.</skos:definition>
        <rdfs:domain rdf:resource="http://www.w3.org/2002/07/owl#Thing"/>
        <rdfs:range rdf:resource="http://www.w3.org/2001/XMLSchema#integer"/>
    </owl:DatatypeProperty>

    <owl:FunctionalProperty rdf:about="sequenceLength"/>

    <owl:DatatypeProperty rdf:about="sequencedPart">
        <rdfs:label xml:lang="en">Sequenced Part</rdfs:label>
        <rdfs:isDefinedBy rdf:resource="http://rs.tdwg.org/abcd/terms/"/>
        <dwcattributes:status>recommended</dwcattributes:status>
        <dcterms:issued>2019-01-31</dcterms:issued>
        <dcterms:modified>2019-01-31</dcterms:modified>
        <rdfs:comment>A description of the actually sequenced material  (DNA/RNA/Protein, Gene or part of gene, completeness, etc.).</rdfs:comment>
        <skos:definition>A description of the actually sequenced material  (DNA/RNA/Protein, Gene or part of gene, completeness, etc.).</skos:definition>
        <rdfs:domain rdf:resource="http://www.w3.org/2002/07/owl#Thing"/>
        <rdfs:range rdf:resource="http://www.w3.org/2001/XMLSchema#string"/>
    </owl:DatatypeProperty>

    <owl:FunctionalProperty rdf:about="sequencedPart"/>

    <owl:DatatypeProperty rdf:about="serovarOrSerotype">
        <rdfs:label xml:lang="en">Serovar Or Serotype</rdfs:label>
        <rdfs:isDefinedBy rdf:resource="http://rs.tdwg.org/abcd/terms/"/>
        <dwcattributes:status>recommended</dwcattributes:status>
        <dcterms:issued>2019-01-31</dcterms:issued>
        <dcterms:modified>2019-01-31</dcterms:modified>
        <rdfs:comment>Name and author of the serovar.</rdfs:comment>
        <skos:definition>Name and author of the serovar.</skos:definition>
        <rdfs:domain rdf:resource="http://www.w3.org/2002/07/owl#Thing"/>
        <rdfs:range rdf:resource="http://www.w3.org/2001/XMLSchema#string"/>
    </owl:DatatypeProperty>

    <owl:FunctionalProperty rdf:about="serovarOrSerotype"/>

    <owl:DatatypeProperty rdf:about="sharpness">
        <rdfs:label xml:lang="en">Sharpness</rdfs:label>
        <rdfs:isDefinedBy rdf:resource="http://rs.tdwg.org/abcd/terms/"/>
        <dwcattributes:status>recommended</dwcattributes:status>
        <dcterms:issued>2019-01-31</dcterms:issued>
        <dcterms:modified>2019-01-31</dcterms:modified>
        <rdfs:comment>This property indicates the direction of sharpness processing applied by the camera when the image was shot.</rdfs:comment>
        <skos:definition>This property indicates the direction of sharpness processing applied by the camera when the image was shot.</skos:definition>
        <rdfs:domain rdf:resource="http://www.w3.org/2002/07/owl#Thing"/>
        <rdfs:range rdf:resource="http://www.w3.org/2001/XMLSchema#string"/>
    </owl:DatatypeProperty>

    <owl:DatatypeProperty rdf:about="shutterSpeed">
        <rdfs:label xml:lang="en">Shutter Speed</rdfs:label>
        <rdfs:isDefinedBy rdf:resource="http://rs.tdwg.org/abcd/terms/"/>
        <dwcattributes:status>recommended</dwcattributes:status>
        <dcterms:issued>2019-01-31</dcterms:issued>
        <dcterms:modified>2019-01-31</dcterms:modified>
        <rdfs:comment>The APEX (Additive System of Photographic Exposure) value for the shutter speed setting.</rdfs:comment>
        <skos:definition>The APEX (Additive System of Photographic Exposure) value for the shutter speed setting.</skos:definition>
        <dc:description>To enter the time in seconds, please use abcd:exposureTime.</dc:description>
        <dc:description>Uses range -5 (30 seconds) to 11 (1/2000 second).</dc:description>
        <rdfs:domain rdf:resource="http://www.w3.org/2002/07/owl#Thing"/>
        <rdfs:range rdf:resource="http://www.w3.org/2001/XMLSchema#integer"/>
    </owl:DatatypeProperty>

    <owl:DatatypeProperty rdf:about="sortingName">
        <rdfs:label xml:lang="en">Sorting Name</rdfs:label>
        <rdfs:isDefinedBy rdf:resource="http://rs.tdwg.org/abcd/terms/"/>
        <dwcattributes:status>recommended</dwcattributes:status>
        <dcterms:issued>2019-01-31</dcterms:issued>
        <dcterms:modified>2019-01-31</dcterms:modified>
        <rdfs:comment>The Full Name of a Person in a form appropriate for sorting alphabetically.</rdfs:comment>
        <skos:definition>The Full Name of a Person in a form appropriate for sorting alphabetically.</skos:definition>
        <dc:description>The form consists of the following: inherited name (western cultures: last name) followed by a comma then a space then given names or initials separated by a space.</dc:description>
        <rdfs:domain rdf:resource="http://www.w3.org/2002/07/owl#Thing"/>
        <rdfs:range rdf:resource="http://www.w3.org/2001/XMLSchema#string"/>
        <skos:relatedMatch rdf:resource="http://www.w3.org/2006/vcard/ns#sort-string"/>
    </owl:DatatypeProperty>

    <owl:FunctionalProperty rdf:about="sortingName"/>

    <owl:DatatypeProperty rdf:about="sourceID">
        <rdfs:label xml:lang="en">Source ID</rdfs:label>
        <rdfs:isDefinedBy rdf:resource="http://rs.tdwg.org/abcd/terms/"/>
        <dwcattributes:status>recommended</dwcattributes:status>
        <dcterms:issued>2019-01-31</dcterms:issued>
        <dcterms:modified>2019-01-31</dcterms:modified>
        <rdfs:comment>The name or code of a data source (that is unique within the institution and constitutes the second part of the record identifier).</rdfs:comment>
        <skos:definition>The name or code of a data source (that is unique within the institution and constitutes the second part of the record identifier).</skos:definition>
        <rdfs:subPropertyOf rdf:resource="id"/>
        <dc:description>The source ID may be the name of a collection if all records stem from a single collection. Together with the element Source-Institution-Code it provides a unique identifier for the dataset's original source.</dc:description>
        <rdfs:domain rdf:resource="http://www.w3.org/2002/07/owl#Thing"/>
        <rdfs:range rdf:resource="http://www.w3.org/2001/XMLSchema#string"/>
        <skos:relatedMatch rdf:resource="http://rs.tdwg.org/dwc/terms/collectionID"/>
    </owl:DatatypeProperty>

    <owl:FunctionalProperty rdf:about="sourceID"/>

    <owl:DatatypeProperty rdf:about="sourceInstitutionID">
        <rdfs:label xml:lang="en">Source Institution ID</rdfs:label>
        <rdfs:isDefinedBy rdf:resource="http://rs.tdwg.org/abcd/terms/"/>
        <dwcattributes:status>recommended</dwcattributes:status>
        <dcterms:issued>2019-01-31</dcterms:issued>
        <dcterms:modified>2019-01-31</dcterms:modified>
        <rdfs:comment>The unique identifier (code or name) of an institution holding the original data source.</rdfs:comment>
        <skos:definition>The unique identifier (code or name) of an institution holding the original data source.</skos:definition>
        <rdfs:subPropertyOf rdf:resource="id"/>
        <dc:description>In specimen collections, this is normally the institution or private holder of the collection itself. For herbaria and botanical gardens, the standard abbreviations should be used.</dc:description>
        <dc:description>The units within the datasource are not necessarily all owned or administered by this institution.</dc:description>
        <rdfs:domain rdf:resource="http://www.w3.org/2002/07/owl#Thing"/>
        <rdfs:range rdf:resource="http://www.w3.org/2001/XMLSchema#string"/>
        <skos:relatedMatch rdf:resource="http://rs.tdwg.org/dwc/terms/institutionCode"/>
        <skos:relatedMatch rdf:resource="http://rs.tdwg.org/dwc/terms/institutionID"/>
    </owl:DatatypeProperty>

    <owl:FunctionalProperty rdf:about="sourceInstitutionID"/>

    <owl:DatatypeProperty rdf:about="spatialDatum">
        <rdfs:label xml:lang="en">Spatial Datum</rdfs:label>
        <rdfs:isDefinedBy rdf:resource="http://rs.tdwg.org/abcd/terms/"/>
        <dwcattributes:status>recommended</dwcattributes:status>
        <dcterms:issued>2019-01-31</dcterms:issued>
        <dcterms:modified>2019-01-31</dcterms:modified>
        <rdfs:comment>A mathematical surface on which the mapping and coordinate system used for the geolocation are based.</rdfs:comment>
        <skos:definition>A mathematical surface on which the mapping and coordinate system used for the geolocation are based.</skos:definition>
        <dc:description>The common abbreviations for spatial datum are to be used.</dc:description>
        <rdfs:domain rdf:resource="http://www.w3.org/2002/07/owl#Thing"/>
        <rdfs:range rdf:resource="http://www.w3.org/2001/XMLSchema#string"/>
        <skos:exactMatch rdf:resource="http://rs.tdwg.org/dwc/terms/geodeticDatum"/>
    </owl:DatatypeProperty>

    <owl:FunctionalProperty rdf:about="spatialDatum"/>

    <owl:DatatypeProperty rdf:about="speciesEpithet">
        <rdfs:label xml:lang="en">Species Epithet</rdfs:label>
        <rdfs:isDefinedBy rdf:resource="http://rs.tdwg.org/abcd/terms/"/>
        <dwcattributes:status>recommended</dwcattributes:status>
        <dcterms:issued>2019-01-31</dcterms:issued>
        <dcterms:modified>2019-01-31</dcterms:modified>
        <rdfs:comment>The first epithet occurring in a scientific name (after genus and, optionally, subgenus names).</rdfs:comment>
        <skos:definition>The first epithet occurring in a scientific name (after genus and, optionally, subgenus names).</skos:definition>
        <rdfs:domain rdf:resource="http://www.w3.org/2002/07/owl#Thing"/>
        <rdfs:range rdf:resource="http://www.w3.org/2001/XMLSchema#string"/>
        <skos:exactMatch rdf:resource="http://rs.tdwg.org/dwc/terms/specificEpithet"/>
    </owl:DatatypeProperty>

    <owl:FunctionalProperty rdf:about="speciesEpithet"/>

    <owl:DatatypeProperty rdf:about="spectralSensitivity">
        <rdfs:label xml:lang="en">Spectral Sensitivity</rdfs:label>
        <rdfs:isDefinedBy rdf:resource="http://rs.tdwg.org/abcd/terms/"/>
        <dwcattributes:status>recommended</dwcattributes:status>
        <dcterms:issued>2019-01-31</dcterms:issued>
        <dcterms:modified>2019-01-31</dcterms:modified>
        <rdfs:comment>EXIF term. Indicates the spectral sensitivity of each channel of the camera used. The value is an ASCII string compatible with the standard developed by the ASTM Technical committee.</rdfs:comment>
        <skos:definition>EXIF term. Indicates the spectral sensitivity of each channel of the camera used. The value is an ASCII string compatible with the standard developed by the ASTM Technical committee.</skos:definition>
        <rdfs:domain rdf:resource="http://www.w3.org/2002/07/owl#Thing"/>
        <rdfs:range rdf:resource="http://www.w3.org/2001/XMLSchema#string"/>
    </owl:DatatypeProperty>

    <owl:DatatypeProperty rdf:about="speed">
        <rdfs:label xml:lang="en">Speed</rdfs:label>
        <rdfs:isDefinedBy rdf:resource="http://rs.tdwg.org/abcd/terms/"/>
        <dwcattributes:status>recommended</dwcattributes:status>
        <dcterms:issued>2019-01-31</dcterms:issued>
        <dcterms:modified>2019-01-31</dcterms:modified>
        <rdfs:comment>The speed of the recording, indicating if the recording has been speed up (speed &gt; 1) or slowed (speed &lt; 1) down for better human analysis, expressed as a factor of the original speed.</rdfs:comment>
        <skos:definition>The speed of the recording, indicating if the recording has been speed up (speed &gt; 1) or slowed (speed &lt; 1) down for better human analysis, expressed as a factor of the original speed.</skos:definition>
        <rdfs:domain rdf:resource="http://www.w3.org/2002/07/owl#Thing"/>
        <rdfs:range rdf:resource="http://www.w3.org/2001/XMLSchema#string"/>
    </owl:DatatypeProperty>

    <owl:FunctionalProperty rdf:about="speed"/>

    <owl:DatatypeProperty rdf:about="storedUnderFlag">
        <rdfs:label xml:lang="en">Stored Under Flag</rdfs:label>
        <rdfs:isDefinedBy rdf:resource="http://rs.tdwg.org/abcd/terms/"/>
        <dwcattributes:status>recommended</dwcattributes:status>
        <dcterms:issued>2019-01-31</dcterms:issued>
        <dcterms:modified>2019-01-31</dcterms:modified>
        <rdfs:comment>This flag is set to "true" to designate the Identification under which the entire Unit is stored (in a physical collection) or otherwise preferably referenced.</rdfs:comment>
        <skos:definition>This flag is set to "true" to designate the Identification under which the entire Unit is stored (in a physical collection) or otherwise preferably referenced.</skos:definition>
        <rdfs:domain rdf:resource="http://www.w3.org/2002/07/owl#Thing"/>
        <rdfs:range rdf:resource="http://www.w3.org/2001/XMLSchema#boolean"/>
    </owl:DatatypeProperty>

    <owl:FunctionalProperty rdf:about="storedUnderFlag"/>

    <owl:DatatypeProperty rdf:about="strain">
        <rdfs:label xml:lang="en">Strain</rdfs:label>
        <rdfs:isDefinedBy rdf:resource="http://rs.tdwg.org/abcd/terms/"/>
        <dwcattributes:status>recommended</dwcattributes:status>
        <dcterms:issued>2019-01-31</dcterms:issued>
        <dcterms:modified>2019-01-31</dcterms:modified>
        <rdfs:comment>The name of a microbial or viral strain</rdfs:comment>
        <skos:definition>The name of a microbial or viral strain</skos:definition>
        <dc:description>Note that this name may also denote the unique identifier of the record in the collection, in which case it should also be used for Unit ID.</dc:description>
        <rdfs:domain rdf:resource="http://www.w3.org/2002/07/owl#Thing"/>
        <rdfs:range rdf:resource="http://www.w3.org/2001/XMLSchema#string"/>
    </owl:DatatypeProperty>

    <owl:FunctionalProperty rdf:about="strain"/>

    <owl:DatatypeProperty rdf:about="stratigraphy">
        <rdfs:label xml:lang="en">Stratigraphy</rdfs:label>
        <rdfs:isDefinedBy rdf:resource="http://rs.tdwg.org/abcd/terms/"/>
        <dwcattributes:status>recommended</dwcattributes:status>
        <dcterms:issued>2019-01-31</dcterms:issued>
        <dcterms:modified>2019-01-31</dcterms:modified>
        <rdfs:comment>A free text field for an informal record of the gathering site stratigraphy.</rdfs:comment>
        <skos:definition>A free text field for an informal record of the gathering site stratigraphy.</skos:definition>
        <rdfs:subPropertyOf rdf:resource="unformattedValue"/>
        <dc:description>The preferred way to specify stratigraphic terms is by using abcd:hasBiostratigraphicTerm,  abcd:hasChronostratigraphicTerm and abcd:hasLithostratigraphicTerm.</dc:description>
        <rdfs:domain rdf:resource="http://www.w3.org/2002/07/owl#Thing"/>
        <rdfs:range rdf:resource="http://www.w3.org/2001/XMLSchema#string"/>
    </owl:DatatypeProperty>

    <owl:FunctionalProperty rdf:about="stratigraphy"/>

    <owl:DatatypeProperty rdf:about="subgenus">
        <rdfs:label xml:lang="en">Subgenus</rdfs:label>
        <rdfs:isDefinedBy rdf:resource="http://rs.tdwg.org/abcd/terms/"/>
        <dwcattributes:status>recommended</dwcattributes:status>
        <dcterms:issued>2019-01-31</dcterms:issued>
        <dcterms:modified>2019-01-31</dcterms:modified>
        <rdfs:comment>The name of a subgenus.</rdfs:comment>
        <skos:definition>The name of a subgenus.</skos:definition>
        <rdfs:domain rdf:resource="http://www.w3.org/2002/07/owl#Thing"/>
        <rdfs:range rdf:resource="http://www.w3.org/2001/XMLSchema#string"/>
        <skos:exactMatch rdf:resource="http://rs.tdwg.org/dwc/terms/subgenus"/>
    </owl:DatatypeProperty>

    <owl:FunctionalProperty rdf:about="subgenus"/>

    <owl:DatatypeProperty rdf:about="subgenusAuthorAndYear">
        <rdfs:label xml:lang="en">Subgenus Author And Year</rdfs:label>
        <rdfs:isDefinedBy rdf:resource="http://rs.tdwg.org/abcd/terms/"/>
        <dwcattributes:status>recommended</dwcattributes:status>
        <dcterms:issued>2019-01-31</dcterms:issued>
        <dcterms:modified>2019-01-31</dcterms:modified>
        <rdfs:comment>Author and year of the subgenus name.</rdfs:comment>
        <skos:definition>Author and year of the subgenus name.</skos:definition>
        <rdfs:domain rdf:resource="http://www.w3.org/2002/07/owl#Thing"/>
        <rdfs:range rdf:resource="http://www.w3.org/2001/XMLSchema#string"/>
    </owl:DatatypeProperty>

    <owl:FunctionalProperty rdf:about="subgenusAuthorAndYear"/>

    <owl:DatatypeProperty rdf:about="subjectDistance">
        <rdfs:label xml:lang="en">Subject Distance</rdfs:label>
        <rdfs:isDefinedBy rdf:resource="http://rs.tdwg.org/abcd/terms/"/>
        <dwcattributes:status>recommended</dwcattributes:status>
        <dcterms:issued>2019-01-31</dcterms:issued>
        <dcterms:modified>2019-01-31</dcterms:modified>
        <rdfs:comment>Specific distance of the subject represented in the media resource with respect to the acquisition device.</rdfs:comment>
        <skos:definition>Specific distance of the subject represented in the media resource with respect to the acquisition device.</skos:definition>
        <rdfs:domain rdf:resource="http://www.w3.org/2002/07/owl#Thing"/>
        <rdfs:range rdf:resource="http://www.w3.org/2001/XMLSchema#string"/>
    </owl:DatatypeProperty>

    <owl:DatatypeProperty rdf:about="subspeciesEpithet">
        <rdfs:label xml:lang="en">Subspecies Epithet</rdfs:label>
        <rdfs:isDefinedBy rdf:resource="http://rs.tdwg.org/abcd/terms/"/>
        <dwcattributes:status>recommended</dwcattributes:status>
        <dcterms:issued>2019-01-31</dcterms:issued>
        <dcterms:modified>2019-01-31</dcterms:modified>
        <rdfs:comment>The second epithet of a scientific name of subspecies rank (after Genus, optional subgenus, and species epithet).</rdfs:comment>
        <skos:definition>The second epithet of a scientific name of subspecies rank (after Genus, optional subgenus, and species epithet).</skos:definition>
        <rdfs:domain rdf:resource="http://www.w3.org/2002/07/owl#Thing"/>
        <rdfs:range rdf:resource="http://www.w3.org/2001/XMLSchema#string"/>
        <skos:exactMatch rdf:resource="http://rs.tdwg.org/dwc/terms/infraspecificEpithet"/>
    </owl:DatatypeProperty>

    <owl:FunctionalProperty rdf:about="subspeciesEpithet"/>

    <owl:DatatypeProperty rdf:about="subtitles">
        <rdfs:label xml:lang="en">Subtitles</rdfs:label>
        <rdfs:isDefinedBy rdf:resource="http://rs.tdwg.org/abcd/terms/"/>
        <dwcattributes:status>recommended</dwcattributes:status>
        <dcterms:issued>2019-01-31</dcterms:issued>
        <dcterms:modified>2019-01-31</dcterms:modified>
        <rdfs:domain rdf:resource="http://www.w3.org/2002/07/owl#Thing"/>
        <rdfs:range rdf:resource="http://www.w3.org/2001/XMLSchema#string"/>
    </owl:DatatypeProperty>

    <owl:DatatypeProperty rdf:about="subtitlesFormat">
        <rdfs:label xml:lang="en">Subtitles Format</rdfs:label>
        <rdfs:isDefinedBy rdf:resource="http://rs.tdwg.org/abcd/terms/"/>
        <dwcattributes:status>recommended</dwcattributes:status>
        <dcterms:issued>2019-01-31</dcterms:issued>
        <dcterms:modified>2019-01-31</dcterms:modified>
        <rdfs:domain rdf:resource="http://www.w3.org/2002/07/owl#Thing"/>
        <rdfs:range rdf:resource="http://www.w3.org/2001/XMLSchema#string"/>
    </owl:DatatypeProperty>

    <owl:DatatypeProperty rdf:about="syntaxon">
        <rdfs:label xml:lang="en">Syntaxon</rdfs:label>
        <rdfs:isDefinedBy rdf:resource="http://rs.tdwg.org/abcd/terms/"/>
        <dwcattributes:status>recommended</dwcattributes:status>
        <dcterms:issued>2019-01-31</dcterms:issued>
        <dcterms:modified>2019-01-31</dcterms:modified>
        <rdfs:comment>A syntaxon name and category assigned to the gathering site.</rdfs:comment>
        <skos:definition>A syntaxon name and category assigned to the gathering site.</skos:definition>
        <rdfs:domain rdf:resource="http://www.w3.org/2002/07/owl#Thing"/>
        <rdfs:range rdf:resource="http://www.w3.org/2001/XMLSchema#string"/>
    </owl:DatatypeProperty>

    <owl:FunctionalProperty rdf:about="syntaxon"/>

    <owl:DatatypeProperty rdf:about="taphonomy">
        <rdfs:label xml:lang="en">Taphonomy</rdfs:label>
        <rdfs:isDefinedBy rdf:resource="http://rs.tdwg.org/abcd/terms/"/>
        <dwcattributes:status>recommended</dwcattributes:status>
        <dcterms:issued>2019-01-31</dcterms:issued>
        <dcterms:modified>2019-01-31</dcterms:modified>
        <rdfs:comment>The life position, allochthonous death assemblage, post mortem history details etc.</rdfs:comment>
        <skos:definition>The life position, allochthonous death assemblage, post mortem history details etc.</skos:definition>
        <rdfs:domain rdf:resource="http://www.w3.org/2002/07/owl#Thing"/>
        <rdfs:range rdf:resource="http://www.w3.org/2001/XMLSchema#string"/>
    </owl:DatatypeProperty>

    <owl:FunctionalProperty rdf:about="taphonomy"/>

    <owl:DatatypeProperty rdf:about="taxonomicTerm">
        <rdfs:label xml:lang="en">Taxonomic Term</rdfs:label>
        <rdfs:isDefinedBy rdf:resource="http://rs.tdwg.org/abcd/terms/"/>
        <dwcattributes:status>recommended</dwcattributes:status>
        <dcterms:issued>2019-01-31</dcterms:issued>
        <dcterms:modified>2019-01-31</dcterms:modified>
        <rdfs:comment>A taxonomic term (e.g. taxon name of higher rank) describing the taxonomic scope of a data set.</rdfs:comment>
        <skos:definition>A taxonomic term (e.g. taxon name of higher rank) describing the taxonomic scope of a data set.</skos:definition>
        <rdfs:subPropertyOf rdf:resource="scope"/>
        <rdfs:domain rdf:resource="http://www.w3.org/2002/07/owl#Thing"/>
        <rdfs:range rdf:resource="http://www.w3.org/2001/XMLSchema#string"/>
    </owl:DatatypeProperty>

    <owl:DatatypeProperty rdf:about="telephoneNumber">
        <rdfs:label xml:lang="en">Telephone Number</rdfs:label>
        <rdfs:isDefinedBy rdf:resource="http://rs.tdwg.org/abcd/terms/"/>
        <dwcattributes:status>recommended</dwcattributes:status>
        <dcterms:issued>2019-01-31</dcterms:issued>
        <dcterms:modified>2019-01-31</dcterms:modified>
        <rdfs:comment>Full telephone or fax number in standard international format.</rdfs:comment>
        <skos:definition>Full telephone or fax number in standard international format.</skos:definition>
        <dc:description>Numbers should be provided in the ITU Recommendation E.164 international format ("+Country-Code Area-Code Number").</dc:description>
        <rdfs:domain rdf:resource="http://www.w3.org/2002/07/owl#Thing"/>
        <rdfs:range rdf:resource="http://www.w3.org/2001/XMLSchema#string"/>
        <skos:relatedMatch rdf:resource="http://www.w3.org/2006/vcard/ns#hasValue"/>
        <skos:exactMatch rdf:resource="http://xmlns.com/foaf/0.1/phone"/>
    </owl:DatatypeProperty>

    <owl:FunctionalProperty rdf:about="telephoneNumber"/>

    <owl:DatatypeProperty rdf:about="temperatureValue">
        <rdfs:label xml:lang="en">Temperature Value</rdfs:label>
        <rdfs:isDefinedBy rdf:resource="http://rs.tdwg.org/abcd/terms/"/>
        <dwcattributes:status>recommended</dwcattributes:status>
        <dcterms:issued>2019-01-31</dcterms:issued>
        <dcterms:modified>2019-01-31</dcterms:modified>
        <rdfs:comment>Concept for a temperature value. Preferably a number.</rdfs:comment>
        <skos:definition>Concept for a temperature value. Preferably a number.</skos:definition>
        <dc:description>The used scale is not to be recorded with this property. Use abcd:TemperatureScale for this.</dc:description>
        <rdfs:domain rdf:resource="http://www.w3.org/2002/07/owl#Thing"/>
        <rdfs:range rdf:resource="http://www.w3.org/2001/XMLSchema#string"/>
    </owl:DatatypeProperty>

    <owl:FunctionalProperty rdf:about="temperatureValue"/>

    <owl:DatatypeProperty rdf:about="term">
        <rdfs:label xml:lang="en">Term</rdfs:label>
        <rdfs:isDefinedBy rdf:resource="http://rs.tdwg.org/abcd/terms/"/>
        <dwcattributes:status>recommended</dwcattributes:status>
        <dcterms:issued>2019-01-31</dcterms:issued>
        <dcterms:modified>2019-01-31</dcterms:modified>
        <rdfs:comment>A descriptive term to describe a concept.</rdfs:comment>
        <skos:definition>A descriptive term to describe a concept.</skos:definition>
        <rdfs:domain rdf:resource="http://www.w3.org/2002/07/owl#Thing"/>
        <rdfs:range rdf:resource="http://www.w3.org/2001/XMLSchema#string"/>
    </owl:DatatypeProperty>

    <owl:FunctionalProperty rdf:about="term"/>

    <owl:DatatypeProperty rdf:about="termDomain">
        <rdfs:label xml:lang="en">Term Domain</rdfs:label>
        <rdfs:isDefinedBy rdf:resource="http://rs.tdwg.org/abcd/terms/"/>
        <dwcattributes:status>recommended</dwcattributes:status>
        <dcterms:issued>2019-01-31</dcterms:issued>
        <dcterms:modified>2019-01-31</dcterms:modified>
        <rdfs:comment>The subject area of the term list from which the term is drawn.</rdfs:comment>
        <skos:definition>The subject area of the term list from which the term is drawn.</skos:definition>
        <rdfs:domain rdf:resource="http://www.w3.org/2002/07/owl#Thing"/>
        <rdfs:range rdf:resource="http://www.w3.org/2001/XMLSchema#string"/>
    </owl:DatatypeProperty>

    <owl:FunctionalProperty rdf:about="termDomain"/>

    <owl:DatatypeProperty rdf:about="text">
        <rdfs:label xml:lang="en">Text</rdfs:label>
        <rdfs:isDefinedBy rdf:resource="http://rs.tdwg.org/abcd/terms/"/>
        <dwcattributes:status>recommended</dwcattributes:status>
        <dcterms:issued>2019-01-31</dcterms:issued>
        <dcterms:modified>2019-01-31</dcterms:modified>
        <rdfs:comment>A generic text property to describe a class.</rdfs:comment>
        <skos:definition>A generic text property to describe a class.</skos:definition>
        <dc:description>Not to be used for information that can not be properly atomized to specific properties. Use the corresponding Unformatted Value elements instead.</dc:description>
        <rdfs:domain rdf:resource="http://www.w3.org/2002/07/owl#Thing"/>
        <rdfs:range rdf:resource="http://www.w3.org/2001/XMLSchema#string"/>
    </owl:DatatypeProperty>

    <owl:FunctionalProperty rdf:about="text"/>

    <owl:DatatypeProperty rdf:about="thumbnailURL">
        <rdfs:label xml:lang="en">Thumbnail URL</rdfs:label>
        <rdfs:isDefinedBy rdf:resource="http://rs.tdwg.org/abcd/terms/"/>
        <dwcattributes:status>recommended</dwcattributes:status>
        <dcterms:issued>2019-01-31</dcterms:issued>
        <dcterms:modified>2019-01-31</dcterms:modified>
        <rdfs:comment>The URL of a thumbnail representing the digital object.</rdfs:comment>
        <skos:definition>The URL of a thumbnail representing the digital object.</skos:definition>
        <rdfs:domain rdf:resource="http://www.w3.org/2002/07/owl#Thing"/>
        <rdfs:range rdf:resource="http://www.w3.org/2001/XMLSchema#anyURI"/>
    </owl:DatatypeProperty>

    <owl:DatatypeProperty rdf:about="timeOfDayBegin">
        <rdfs:label xml:lang="en">Time Of Day Begin</rdfs:label>
        <rdfs:isDefinedBy rdf:resource="http://rs.tdwg.org/abcd/terms/"/>
        <dwcattributes:status>recommended</dwcattributes:status>
        <dcterms:issued>2019-01-31</dcterms:issued>
        <dcterms:modified>2019-01-31</dcterms:modified>
        <rdfs:comment>The time of day in hours from midnight local time for the beginning of a period.</rdfs:comment>
        <skos:definition>The time of day in hours from midnight local time for the beginning of a period.</skos:definition>
        <rdfs:domain rdf:resource="http://www.w3.org/2002/07/owl#Thing"/>
        <rdfs:range rdf:resource="http://www.w3.org/2001/XMLSchema#string"/>
    </owl:DatatypeProperty>

    <owl:FunctionalProperty rdf:about="timeOfDayBegin"/>

    <owl:DatatypeProperty rdf:about="timeOfDayEnd">
        <rdfs:label xml:lang="en">Time Of Day End</rdfs:label>
        <rdfs:isDefinedBy rdf:resource="http://rs.tdwg.org/abcd/terms/"/>
        <dwcattributes:status>recommended</dwcattributes:status>
        <dcterms:issued>2019-01-31</dcterms:issued>
        <dcterms:modified>2019-01-31</dcterms:modified>
        <rdfs:comment>The time of day in hours from midnight for the end of a period.</rdfs:comment>
        <skos:definition>The time of day in hours from midnight for the end of a period.</skos:definition>
        <rdfs:domain rdf:resource="http://www.w3.org/2002/07/owl#Thing"/>
        <rdfs:range rdf:resource="http://www.w3.org/2001/XMLSchema#string"/>
    </owl:DatatypeProperty>

    <owl:FunctionalProperty rdf:about="timeOfDayEnd"/>

    <owl:DatatypeProperty rdf:about="timeSpanBegin">
        <rdfs:label xml:lang="en">Time Span Begin</rdfs:label>
        <rdfs:isDefinedBy rdf:resource="http://rs.tdwg.org/abcd/terms/"/>
        <dwcattributes:status>recommended</dwcattributes:status>
        <dcterms:issued>2019-01-31</dcterms:issued>
        <dcterms:modified>2019-01-31</dcterms:modified>
        <rdfs:comment>The beginning of a period or a single point in time expressed in a variant of the W3C DateTime format.</rdfs:comment>
        <skos:definition>The beginning of a period or a single point in time expressed in a variant of the W3C DateTime format.</skos:definition>
        <dc:description>To describe a single point in time, use this property and omit the abcd:timeSpanEnd property.</dc:description>
        <dc:description>The formatting holds to the W3C DateTime format (https://www.w3.org/TR/NOTE-datetime) with the exception, that the time zone designator can be omitted (though it is highly recommended). Dates or time spans that can not be properly mapped to this format due to potential ambiguities or missing information (e.g. indistinguishable writings) need to be expressed using the  unformatted value property.</dc:description>
        <rdfs:domain rdf:resource="http://www.w3.org/2002/07/owl#Thing"/>
        <rdfs:range rdf:resource="http://www.w3.org/2001/XMLSchema#string"/>
        <skos:relatedMatch rdf:resource="http://rs.tdwg.org/dwc/terms/eventDate"/>
    </owl:DatatypeProperty>

    <owl:FunctionalProperty rdf:about="timeSpanBegin"/>

    <owl:DatatypeProperty rdf:about="timeSpanEnd">
        <rdfs:label xml:lang="en">Time Span End</rdfs:label>
        <rdfs:isDefinedBy rdf:resource="http://rs.tdwg.org/abcd/terms/"/>
        <dwcattributes:status>recommended</dwcattributes:status>
        <dcterms:issued>2019-01-31</dcterms:issued>
        <dcterms:modified>2019-01-31</dcterms:modified>
        <rdfs:comment>The end of a period expressed in a variant of the W3C DateTime format.</rdfs:comment>
        <skos:definition>The end of a period expressed in a variant of the W3C DateTime format.</skos:definition>
        <dc:description>To describe a single point in time, omit this property and use the abcd:timeSpanBegin property.</dc:description>
        <dc:description>The formatting holds to the W3C DateTime format (https://www.w3.org/TR/NOTE-datetime) with the exception, that the time zone designator can be omitted (though it is highly recommended). Dates or time spans that can not be properly mapped to this format due to potential ambiguities or missing information (e.g. indistinguishable writings) need to be expressed using the unformatted value property.</dc:description>
        <rdfs:domain rdf:resource="http://www.w3.org/2002/07/owl#Thing"/>
        <rdfs:range rdf:resource="http://www.w3.org/2001/XMLSchema#string"/>
        <skos:relatedMatch rdf:resource="http://rs.tdwg.org/dwc/terms/eventDate"/>
    </owl:DatatypeProperty>

    <owl:FunctionalProperty rdf:about="timeSpanEnd"/>

    <owl:DatatypeProperty rdf:about="timeZone">
        <rdfs:label xml:lang="en">Time Zone</rdfs:label>
        <rdfs:isDefinedBy rdf:resource="http://rs.tdwg.org/abcd/terms/"/>
        <dwcattributes:status>recommended</dwcattributes:status>
        <dcterms:issued>2019-01-31</dcterms:issued>
        <dcterms:modified>2019-01-31</dcterms:modified>
        <rdfs:domain rdf:resource="http://www.w3.org/2002/07/owl#Thing"/>
        <rdfs:range rdf:resource="http://www.w3.org/2001/XMLSchema#string"/>
    </owl:DatatypeProperty>

    <owl:FunctionalProperty rdf:about="timeZone"/>

    <owl:DatatypeProperty rdf:about="title">
        <rdfs:label xml:lang="en">Title</rdfs:label>
        <rdfs:isDefinedBy rdf:resource="http://rs.tdwg.org/abcd/terms/"/>
        <dwcattributes:status>recommended</dwcattributes:status>
        <dcterms:issued>2019-01-31</dcterms:issued>
        <dcterms:modified>2019-01-31</dcterms:modified>
        <rdfs:comment>A short concise title for a class.</rdfs:comment>
        <skos:definition>A short concise title for a class.</skos:definition>
        <rdfs:domain rdf:resource="http://www.w3.org/2002/07/owl#Thing"/>
        <rdfs:range rdf:resource="http://www.w3.org/2001/XMLSchema#string"/>
        <skos:exactMatch rdf:resource="http://purl.org/dc/terms/title"/>
    </owl:DatatypeProperty>

    <owl:FunctionalProperty rdf:about="title"/>

    <owl:DatatypeProperty rdf:about="tradeDesignationName">
        <rdfs:label xml:lang="en">Trade Designation Name</rdfs:label>
        <rdfs:isDefinedBy rdf:resource="http://rs.tdwg.org/abcd/terms/"/>
        <dwcattributes:status>recommended</dwcattributes:status>
        <dcterms:issued>2019-01-31</dcterms:issued>
        <dcterms:modified>2019-01-31</dcterms:modified>
        <rdfs:comment>A trade name used for a specific cultivar.</rdfs:comment>
        <skos:definition>A trade name used for a specific cultivar.</skos:definition>
        <rdfs:domain rdf:resource="http://www.w3.org/2002/07/owl#Thing"/>
        <rdfs:range rdf:resource="http://www.w3.org/2001/XMLSchema#string"/>
    </owl:DatatypeProperty>

    <owl:DatatypeProperty rdf:about="typeGermplasmStorage">
        <rdfs:label xml:lang="en">Type Germplasm Storage</rdfs:label>
        <rdfs:isDefinedBy rdf:resource="http://rs.tdwg.org/abcd/terms/"/>
        <dwcattributes:status>recommended</dwcattributes:status>
        <dcterms:issued>2019-01-31</dcterms:issued>
        <dcterms:modified>2019-01-31</dcterms:modified>
        <rdfs:comment>Code for the type of storage of the unit in the collection.</rdfs:comment>
        <skos:definition>Code for the type of storage of the unit in the collection.</skos:definition>
        <dc:description>10: Seed collection; 11: Short term; 12: Medium term; 13: Long term; 20: Field collection; 30: In vitro collection (Slow growth); 40: Cryopreserved collection; 99: Other</dc:description>
        <dc:description>If germplasm is maintained under different types of storage, multiple choices are allowed (separated by a semicolon). (Refer to FAO/IPGRI Genebank Standards 1994 for details on storage type.)</dc:description>
        <rdfs:domain rdf:resource="http://www.w3.org/2002/07/owl#Thing"/>
        <rdfs:range rdf:resource="http://www.w3.org/2001/XMLSchema#integer"/>
    </owl:DatatypeProperty>

    <owl:FunctionalProperty rdf:about="typeGermplasmStorage"/>

    <owl:DatatypeProperty rdf:about="typeStatus">
        <rdfs:label xml:lang="en">Type Status</rdfs:label>
        <rdfs:isDefinedBy rdf:resource="http://rs.tdwg.org/abcd/terms/"/>
        <dwcattributes:status>recommended</dwcattributes:status>
        <dcterms:issued>2019-01-31</dcterms:issued>
        <dcterms:modified>2019-01-31</dcterms:modified>
        <rdfs:comment>A full term designating the status of the Nomenclatural Type Designation.</rdfs:comment>
        <skos:definition>A full term designating the status of the Nomenclatural Type Designation.</skos:definition>
        <rdfs:domain rdf:resource="http://www.w3.org/2002/07/owl#Thing"/>
        <rdfs:range rdf:resource="http://www.w3.org/2001/XMLSchema#string"/>
        <skos:exactMatch rdf:resource="http://rs.tdwg.org/dwc/terms/typeStatus"/>
    </owl:DatatypeProperty>

    <owl:FunctionalProperty rdf:about="typeStatus"/>

    <owl:DatatypeProperty rdf:about="utmDatum">
        <rdfs:label xml:lang="en">UTM Datum</rdfs:label>
        <rdfs:isDefinedBy rdf:resource="http://rs.tdwg.org/abcd/terms/"/>
        <dwcattributes:status>recommended</dwcattributes:status>
        <dcterms:issued>2019-01-31</dcterms:issued>
        <dcterms:modified>2019-01-31</dcterms:modified>
        <rdfs:comment>Mathematical surface on which the mapping and coordinate system used for geocodes are based.</rdfs:comment>
        <skos:definition>Mathematical surface on which the mapping and coordinate system used for geocodes are based.</skos:definition>
        <rdfs:domain rdf:resource="http://www.w3.org/2002/07/owl#Thing"/>
        <rdfs:range rdf:resource="http://www.w3.org/2001/XMLSchema#string"/>
    </owl:DatatypeProperty>

    <owl:FunctionalProperty rdf:about="utmDatum"/>

    <owl:DatatypeProperty rdf:about="utmEasting">
        <rdfs:label xml:lang="en">UTM Easting</rdfs:label>
        <rdfs:isDefinedBy rdf:resource="http://rs.tdwg.org/abcd/terms/"/>
        <dwcattributes:status>recommended</dwcattributes:status>
        <dcterms:issued>2019-01-31</dcterms:issued>
        <dcterms:modified>2019-01-31</dcterms:modified>
        <rdfs:comment>The distance in meters east of the origin of the UTM Zone.</rdfs:comment>
        <skos:definition>The distance in meters east of the origin of the UTM Zone.</skos:definition>
        <rdfs:domain rdf:resource="http://www.w3.org/2002/07/owl#Thing"/>
        <rdfs:range rdf:resource="http://www.w3.org/2001/XMLSchema#string"/>
    </owl:DatatypeProperty>

    <owl:FunctionalProperty rdf:about="utmEasting"/>

    <owl:DatatypeProperty rdf:about="utmNorthing">
        <rdfs:label xml:lang="en">UTM Northing</rdfs:label>
        <rdfs:isDefinedBy rdf:resource="http://rs.tdwg.org/abcd/terms/"/>
        <dwcattributes:status>recommended</dwcattributes:status>
        <dcterms:issued>2019-01-31</dcterms:issued>
        <dcterms:modified>2019-01-31</dcterms:modified>
        <rdfs:comment>The distance in meters north of the origin for the UTM Subzone.</rdfs:comment>
        <skos:definition>The distance in meters north of the origin for the UTM Subzone.</skos:definition>
        <rdfs:domain rdf:resource="http://www.w3.org/2002/07/owl#Thing"/>
        <rdfs:range rdf:resource="http://www.w3.org/2001/XMLSchema#string"/>
    </owl:DatatypeProperty>

    <owl:FunctionalProperty rdf:about="utmNorthing"/>

    <owl:DatatypeProperty rdf:about="utmSubzone">
        <rdfs:label xml:lang="en">UTM Subzone</rdfs:label>
        <rdfs:isDefinedBy rdf:resource="http://rs.tdwg.org/abcd/terms/"/>
        <dwcattributes:status>recommended</dwcattributes:status>
        <dcterms:issued>2019-01-31</dcterms:issued>
        <dcterms:modified>2019-01-31</dcterms:modified>
        <rdfs:comment>The Subzone letter corresponding to one of the 20 North-South divisions of the UTM grid system.</rdfs:comment>
        <skos:definition>The Subzone letter corresponding to one of the 20 North-South divisions of the UTM grid system.</skos:definition>
        <rdfs:domain rdf:resource="http://www.w3.org/2002/07/owl#Thing"/>
        <rdfs:range rdf:resource="http://www.w3.org/2001/XMLSchema#string"/>
    </owl:DatatypeProperty>

    <owl:FunctionalProperty rdf:about="utmSubzone"/>

    <owl:DatatypeProperty rdf:about="utmText">
        <rdfs:label xml:lang="en">UTM Text</rdfs:label>
        <rdfs:isDefinedBy rdf:resource="http://rs.tdwg.org/abcd/terms/"/>
        <dwcattributes:status>recommended</dwcattributes:status>
        <dcterms:issued>2019-01-31</dcterms:issued>
        <dcterms:modified>2019-01-31</dcterms:modified>
        <rdfs:comment>An alternative composite text to capture unatomized UTM coordinate data.</rdfs:comment>
        <skos:definition>An alternative composite text to capture unatomized UTM coordinate data.</skos:definition>
        <rdfs:domain rdf:resource="http://www.w3.org/2002/07/owl#Thing"/>
        <rdfs:range rdf:resource="http://www.w3.org/2001/XMLSchema#string"/>
    </owl:DatatypeProperty>

    <owl:FunctionalProperty rdf:about="utmText"/>

    <owl:DatatypeProperty rdf:about="utmZone">
        <rdfs:label xml:lang="en">UTM Zone</rdfs:label>
        <rdfs:isDefinedBy rdf:resource="http://rs.tdwg.org/abcd/terms/"/>
        <dwcattributes:status>recommended</dwcattributes:status>
        <dcterms:issued>2019-01-31</dcterms:issued>
        <dcterms:modified>2019-01-31</dcterms:modified>
        <rdfs:comment>The numerical Zone corresponding to the central meridian and origin upon which the UTMEasting is based.</rdfs:comment>
        <skos:definition>The numerical Zone corresponding to the central meridian and origin upon which the UTMEasting is based.</skos:definition>
        <rdfs:domain rdf:resource="http://www.w3.org/2002/07/owl#Thing"/>
        <rdfs:range rdf:resource="http://www.w3.org/2001/XMLSchema#integer"/>
    </owl:DatatypeProperty>

    <owl:FunctionalProperty rdf:about="utmZone"/>

    <owl:DatatypeProperty rdf:about="utmZoneFull">
        <rdfs:label xml:lang="en">UTM Zone Full</rdfs:label>
        <rdfs:isDefinedBy rdf:resource="http://rs.tdwg.org/abcd/terms/"/>
        <dwcattributes:status>recommended</dwcattributes:status>
        <dcterms:issued>2019-01-31</dcterms:issued>
        <dcterms:modified>2019-01-31</dcterms:modified>
        <rdfs:comment>An alternative composite text to capture a zone expressed as a combination of UTMZone and UTMSubzone.</rdfs:comment>
        <skos:definition>An alternative composite text to capture a zone expressed as a combination of UTMZone and UTMSubzone.</skos:definition>
        <rdfs:domain rdf:resource="http://www.w3.org/2002/07/owl#Thing"/>
        <rdfs:range rdf:resource="http://www.w3.org/2001/XMLSchema#string"/>
    </owl:DatatypeProperty>

    <owl:FunctionalProperty rdf:about="utmZoneFull"/>

    <owl:DatatypeProperty rdf:about="utmNS">
        <rdfs:label xml:lang="en">UTMNS</rdfs:label>
        <rdfs:isDefinedBy rdf:resource="http://rs.tdwg.org/abcd/terms/"/>
        <dwcattributes:status>recommended</dwcattributes:status>
        <dcterms:issued>2019-01-31</dcterms:issued>
        <dcterms:modified>2019-01-31</dcterms:modified>
        <rdfs:comment>The hemisphere to which the UTM Northing refers.</rdfs:comment>
        <skos:definition>The hemisphere to which the UTM Northing refers.</skos:definition>
        <rdfs:domain rdf:resource="http://www.w3.org/2002/07/owl#Thing"/>
        <rdfs:range rdf:resource="http://www.w3.org/2001/XMLSchema#string"/>
    </owl:DatatypeProperty>

    <owl:FunctionalProperty rdf:about="utmNS"/>

    <owl:DatatypeProperty rdf:about="unformattedValue">
        <rdfs:label xml:lang="en">Unformatted Value</rdfs:label>
        <rdfs:isDefinedBy rdf:resource="http://rs.tdwg.org/abcd/terms/"/>
        <dwcattributes:status>recommended</dwcattributes:status>
        <dcterms:issued>2019-01-31</dcterms:issued>
        <dcterms:modified>2019-01-31</dcterms:modified>
        <rdfs:comment>Information about a class in free text form that can not be expressed in atomized values.</rdfs:comment>
        <skos:definition>Information about a class in free text form that can not be expressed in atomized values.</skos:definition>
        <dc:description>To be used when no atomized information is available. Not to be confused with abcd:Text.</dc:description>
        <rdfs:domain rdf:resource="http://www.w3.org/2002/07/owl#Thing"/>
        <rdfs:range rdf:resource="http://www.w3.org/2001/XMLSchema#string"/>
    </owl:DatatypeProperty>

    <owl:DatatypeProperty rdf:about="unitOfMeasurement">
        <rdfs:label xml:lang="en">Unit Of Measurement</rdfs:label>
        <rdfs:isDefinedBy rdf:resource="http://rs.tdwg.org/abcd/terms/"/>
        <dwcattributes:status>recommended</dwcattributes:status>
        <dcterms:issued>2019-01-31</dcterms:issued>
        <dcterms:modified>2019-01-31</dcterms:modified>
        <rdfs:comment>The unit of measurement in which the values are expressed.</rdfs:comment>
        <skos:definition>The unit of measurement in which the values are expressed.</skos:definition>
        <dc:description>The usage of abbreviated SI units is highly recommended. An appropriate prefix can be added (e.g. 2 mm instead of 0.0002 m)</dc:description>
        <rdfs:domain rdf:resource="http://www.w3.org/2002/07/owl#Thing"/>
        <rdfs:range rdf:resource="http://www.w3.org/2001/XMLSchema#string"/>
        <skos:exactMatch rdf:resource="http://rs.tdwg.org/dwc/terms/measurementUnit"/>
    </owl:DatatypeProperty>

    <owl:FunctionalProperty rdf:about="unitOfMeasurement"/>

    <owl:DatatypeProperty rdf:about="upperValue">
        <rdfs:label xml:lang="en">Upper Value</rdfs:label>
        <rdfs:isDefinedBy rdf:resource="http://rs.tdwg.org/abcd/terms/"/>
        <dwcattributes:status>recommended</dwcattributes:status>
        <dcterms:issued>2019-01-31</dcterms:issued>
        <dcterms:modified>2019-01-31</dcterms:modified>
        <rdfs:comment>The upper value of a measurement when it yields a range of values.</rdfs:comment>
        <skos:definition>The upper value of a measurement when it yields a range of values.</skos:definition>
        <dc:description>The unit of the measurement should be expressed in abcd:UnitOfMeasurement. When no upper value of a range can be determined, this property should be omitted and only abcd:LowerValue should be filled.</dc:description>
        <rdfs:domain rdf:resource="http://www.w3.org/2002/07/owl#Thing"/>
        <rdfs:range rdf:resource="http://www.w3.org/2001/XMLSchema#string"/>
        <skos:relatedMatch rdf:resource="http://rs.tdwg.org/dwc/terms/measurementValue"/>
    </owl:DatatypeProperty>

    <owl:FunctionalProperty rdf:about="upperValue"/>

    <owl:DatatypeProperty rdf:about="validDistributionFlag">
        <rdfs:label xml:lang="en">Valid Distribution Flag</rdfs:label>
        <rdfs:isDefinedBy rdf:resource="http://rs.tdwg.org/abcd/terms/"/>
        <dwcattributes:status>recommended</dwcattributes:status>
        <dcterms:issued>2019-01-31</dcterms:issued>
        <dcterms:modified>2019-01-31</dcterms:modified>
        <rdfs:comment>A flag ("true" or "false") that indicates whether the locality information represents a valid distribution occurrence for a specimen.</rdfs:comment>
        <skos:definition>A flag ("true" or "false") that indicates whether the locality information represents a valid distribution occurrence for a specimen.</skos:definition>
        <dc:description>Specimens taken from captivity and showing the captive location should use the value "false".</dc:description>
        <rdfs:domain rdf:resource="http://www.w3.org/2002/07/owl#Thing"/>
        <rdfs:range rdf:resource="http://www.w3.org/2001/XMLSchema#boolean"/>
    </owl:DatatypeProperty>

    <owl:FunctionalProperty rdf:about="validDistributionFlag"/>

    <owl:DatatypeProperty rdf:about="verbatimText">
        <rdfs:label xml:lang="en">Verbatim Text</rdfs:label>
        <rdfs:isDefinedBy rdf:resource="http://rs.tdwg.org/abcd/terms/"/>
        <dwcattributes:status>recommended</dwcattributes:status>
        <dcterms:issued>2019-01-31</dcterms:issued>
        <dcterms:modified>2019-01-31</dcterms:modified>
        <rdfs:comment>The exact transcription of a written or printed text.</rdfs:comment>
        <skos:definition>The exact transcription of a written or printed text.</skos:definition>
        <rdfs:subPropertyOf rdf:resource="text"/>
        <rdfs:domain rdf:resource="http://www.w3.org/2002/07/owl#Thing"/>
        <rdfs:range rdf:resource="http://www.w3.org/2001/XMLSchema#string"/>
    </owl:DatatypeProperty>

    <owl:DatatypeProperty rdf:about="verificationLevel">
        <rdfs:label xml:lang="en">Verification Level</rdfs:label>
        <rdfs:isDefinedBy rdf:resource="http://rs.tdwg.org/abcd/terms/"/>
        <dwcattributes:status>recommended</dwcattributes:status>
        <dcterms:issued>2019-01-31</dcterms:issued>
        <dcterms:modified>2019-01-31</dcterms:modified>
        <rdfs:comment>The level to which the identification has been verified. Different standards may use different values here.</rdfs:comment>
        <skos:definition>The level to which the identification has been verified. Different standards may use different values here.</skos:definition>
        <dc:description>Verification Level from ITF 2 and HISPID 3 are commonly used.</dc:description>
        <rdfs:domain rdf:resource="http://www.w3.org/2002/07/owl#Thing"/>
        <rdfs:range rdf:resource="http://www.w3.org/2001/XMLSchema#string"/>
        <skos:exactMatch rdf:resource="http://rs.tdwg.org/dwc/terms/identificationVerificationStatus"/>
    </owl:DatatypeProperty>

    <owl:FunctionalProperty rdf:about="verificationLevel"/>

    <owl:DatatypeProperty rdf:about="verificationStatus">
        <rdfs:label xml:lang="en">Verification Status</rdfs:label>
        <rdfs:isDefinedBy rdf:resource="http://rs.tdwg.org/abcd/terms/"/>
        <dwcattributes:status>recommended</dwcattributes:status>
        <dcterms:issued>2019-01-31</dcterms:issued>
        <dcterms:modified>2019-01-31</dcterms:modified>
        <rdfs:comment>A categorical description of the extent to which the georeference has been verified to represent the location where the specimen or observation was collected. This element should be vocabulary-controlled.</rdfs:comment>
        <skos:definition>A categorical description of the extent to which the georeference has been verified to represent the location where the specimen or observation was collected. This element should be vocabulary-controlled.</skos:definition>
        <rdfs:domain rdf:resource="http://www.w3.org/2002/07/owl#Thing"/>
        <rdfs:range rdf:resource="http://www.w3.org/2001/XMLSchema#string"/>
        <skos:exactMatch rdf:resource="http://rs.tdwg.org/dwc/terms/georeferenceVerificationStatus"/>
    </owl:DatatypeProperty>

    <owl:FunctionalProperty rdf:about="verificationStatus"/>

    <owl:DatatypeProperty rdf:about="videoBitrate">
        <rdfs:label xml:lang="en">Video Bitrate</rdfs:label>
        <rdfs:isDefinedBy rdf:resource="http://rs.tdwg.org/abcd/terms/"/>
        <dwcattributes:status>recommended</dwcattributes:status>
        <dcterms:issued>2019-01-31</dcterms:issued>
        <dcterms:modified>2019-01-31</dcterms:modified>
        <rdfs:comment>The bit rate of a video stream, usually expressed in kBit/s or MBit/s.</rdfs:comment>
        <skos:definition>The bit rate of a video stream, usually expressed in kBit/s or MBit/s.</skos:definition>
        <rdfs:domain rdf:resource="http://www.w3.org/2002/07/owl#Thing"/>
        <rdfs:range rdf:resource="http://www.w3.org/2001/XMLSchema#string"/>
    </owl:DatatypeProperty>

    <owl:FunctionalProperty rdf:about="videoBitrate"/>

    <owl:DatatypeProperty rdf:about="videoEncoding">
        <rdfs:label xml:lang="en">Video Encoding</rdfs:label>
        <rdfs:isDefinedBy rdf:resource="http://rs.tdwg.org/abcd/terms/"/>
        <dwcattributes:status>recommended</dwcattributes:status>
        <dcterms:issued>2019-01-31</dcterms:issued>
        <dcterms:modified>2019-01-31</dcterms:modified>
        <rdfs:comment>The codec of a video.</rdfs:comment>
        <skos:definition>The codec of a video.</skos:definition>
        <rdfs:domain rdf:resource="http://www.w3.org/2002/07/owl#Thing"/>
        <rdfs:range rdf:resource="http://www.w3.org/2001/XMLSchema#string"/>
    </owl:DatatypeProperty>

    <owl:FunctionalProperty rdf:about="videoEncoding"/>

    <owl:DatatypeProperty rdf:about="viralSpeciesDesignation">
        <rdfs:label xml:lang="en">Viral Species Designation</rdfs:label>
        <rdfs:isDefinedBy rdf:resource="http://rs.tdwg.org/abcd/terms/"/>
        <dwcattributes:status>recommended</dwcattributes:status>
        <dcterms:issued>2019-01-31</dcterms:issued>
        <dcterms:modified>2019-01-31</dcterms:modified>
        <rdfs:comment>The formal name for a viral species.</rdfs:comment>
        <skos:definition>The formal name for a viral species.</skos:definition>
        <rdfs:domain rdf:resource="http://www.w3.org/2002/07/owl#Thing"/>
        <rdfs:range rdf:resource="http://www.w3.org/2001/XMLSchema#string"/>
    </owl:DatatypeProperty>

    <owl:FunctionalProperty rdf:about="viralSpeciesDesignation"/>

    <owl:DatatypeProperty rdf:about="volume">
        <rdfs:label xml:lang="en">Volume</rdfs:label>
        <rdfs:isDefinedBy rdf:resource="http://rs.tdwg.org/abcd/terms/"/>
        <dwcattributes:status>recommended</dwcattributes:status>
        <dcterms:issued>2019-01-31</dcterms:issued>
        <dcterms:modified>2019-01-31</dcterms:modified>
        <rdfs:domain rdf:resource="http://www.w3.org/2002/07/owl#Thing"/>
        <rdfs:range rdf:resource="http://www.w3.org/2001/XMLSchema#string"/>
    </owl:DatatypeProperty>

    <owl:FunctionalProperty rdf:about="volume"/>

    <owl:DatatypeProperty rdf:about="wmsURL">
        <rdfs:label xml:lang="en">WMSURL</rdfs:label>
        <rdfs:isDefinedBy rdf:resource="http://rs.tdwg.org/abcd/terms/"/>
        <dwcattributes:status>recommended</dwcattributes:status>
        <dcterms:issued>2019-01-31</dcterms:issued>
        <dcterms:modified>2019-01-31</dcterms:modified>
        <rdfs:comment>A URL for the location of a boundary polygon or centroid spatial reference relating to a gathering site, according to the Web Map Services (WMS) specification of the Open GIS Consortium.</rdfs:comment>
        <skos:definition>A URL for the location of a boundary polygon or centroid spatial reference relating to a gathering site, according to the Web Map Services (WMS) specification of the Open GIS Consortium.</skos:definition>
        <rdfs:subPropertyOf rdf:resource="websiteURL"/>
        <rdfs:domain rdf:resource="http://www.w3.org/2002/07/owl#Thing"/>
        <rdfs:range rdf:resource="http://www.w3.org/2001/XMLSchema#anyURI"/>
    </owl:DatatypeProperty>

    <owl:DatatypeProperty rdf:about="websiteURL">
        <rdfs:label xml:lang="en">Website URL</rdfs:label>
        <rdfs:isDefinedBy rdf:resource="http://rs.tdwg.org/abcd/terms/"/>
        <dwcattributes:status>recommended</dwcattributes:status>
        <dcterms:issued>2019-01-31</dcterms:issued>
        <dcterms:modified>2019-01-31</dcterms:modified>
        <rdfs:comment>The URL of a web page for the associated class.</rdfs:comment>
        <skos:definition>The URL of a web page for the associated class.</skos:definition>
        <dc:description>Not to be confused with URIs for external identifiers.</dc:description>
        <rdfs:domain rdf:resource="http://www.w3.org/2002/07/owl#Thing"/>
        <rdfs:range rdf:resource="http://www.w3.org/2001/XMLSchema#anyURI"/>
        <skos:exactMatch rdf:resource="http://xmlns.com/foaf/0.1/homepage"/>
    </owl:DatatypeProperty>

    <owl:DatatypeProperty rdf:about="whiteBalance">
        <rdfs:label xml:lang="en">White Balance</rdfs:label>
        <rdfs:isDefinedBy rdf:resource="http://rs.tdwg.org/abcd/terms/"/>
        <dwcattributes:status>recommended</dwcattributes:status>
        <dcterms:issued>2019-01-31</dcterms:issued>
        <dcterms:modified>2019-01-31</dcterms:modified>
        <rdfs:comment>This property indicates the white balance mode set when the image was shot.</rdfs:comment>
        <skos:definition>This property indicates the white balance mode set when the image was shot.</skos:definition>
        <rdfs:domain rdf:resource="http://www.w3.org/2002/07/owl#Thing"/>
        <rdfs:range rdf:resource="http://www.w3.org/2001/XMLSchema#string"/>
    </owl:DatatypeProperty>

    <owl:DatatypeProperty rdf:about="width">
        <rdfs:label xml:lang="en">Width</rdfs:label>
        <rdfs:isDefinedBy rdf:resource="http://rs.tdwg.org/abcd/terms/"/>
        <dwcattributes:status>recommended</dwcattributes:status>
        <dcterms:issued>2019-01-31</dcterms:issued>
        <dcterms:modified>2019-01-31</dcterms:modified>
        <rdfs:comment>An image or video width in pixels.</rdfs:comment>
        <skos:definition>An image or video width in pixels.</skos:definition>
        <rdfs:domain rdf:resource="http://www.w3.org/2002/07/owl#Thing"/>
        <rdfs:range rdf:resource="http://www.w3.org/2001/XMLSchema#integer"/>
    </owl:DatatypeProperty>

    <owl:FunctionalProperty rdf:about="width"/>

    <owl:DatatypeProperty rdf:about="fNumber">
        <rdfs:label xml:lang="en">f Number</rdfs:label>
        <rdfs:isDefinedBy rdf:resource="http://rs.tdwg.org/abcd/terms/"/>
        <dwcattributes:status>recommended</dwcattributes:status>
        <dcterms:issued>2019-01-31</dcterms:issued>
        <dcterms:modified>2019-01-31</dcterms:modified>
        <rdfs:comment>The ratio of the focal length of the camera to the diameter of the lens pupil (aperture).</rdfs:comment>
        <skos:definition>The ratio of the focal length of the camera to the diameter of the lens pupil (aperture).</skos:definition>
        <rdfs:domain rdf:resource="http://www.w3.org/2002/07/owl#Thing"/>
        <rdfs:range rdf:resource="http://www.w3.org/2001/XMLSchema#decimal"/>
    </owl:DatatypeProperty>

    <owl:DatatypeProperty rdf:about="preferred">
        <rdfs:label xml:lang="en">preferred</rdfs:label>
        <rdfs:isDefinedBy rdf:resource="http://rs.tdwg.org/abcd/terms/"/>
        <dwcattributes:status>recommended</dwcattributes:status>
        <dcterms:issued>2019-01-31</dcterms:issued>
        <dcterms:modified>2019-01-31</dcterms:modified>
        <rdfs:comment>Meta Property to denote the preferred statement if a property is used more than once for an instance of a class.</rdfs:comment>
        <skos:definition>Meta Property to denote the preferred statement if a property is used more than once for an instance of a class.</skos:definition>
        <rdfs:domain rdf:resource="http://www.w3.org/2002/07/owl#Thing"/>
        <rdfs:range rdf:resource="http://www.w3.org/2001/XMLSchema#boolean"/>
        <vann:termGroup rdf:resource="General"/>
    </owl:DatatypeProperty>

    <owl:DatatypeProperty rdf:about="sequence">
        <rdfs:label xml:lang="en">sequence</rdfs:label>
        <rdfs:isDefinedBy rdf:resource="http://rs.tdwg.org/abcd/terms/"/>
        <dwcattributes:status>recommended</dwcattributes:status>
        <dcterms:issued>2019-01-31</dcterms:issued>
        <dcterms:modified>2019-01-31</dcterms:modified>
        <rdfs:comment>Meta Property to denote the sequence of statements on a property which is used more than once for an instance of a class.</rdfs:comment>
        <skos:definition>Meta Property to denote the sequence of statements on a property which is used more than once for an instance of a class.</skos:definition>
        <dc:description>Not to be confused with abcd:Sequence, the class for a genomic sequence.</dc:description>
        <dc:description>This is commonly used to either denote the order of importance of statements (the lowest sequence number, usually 1, is considered the primary or most important one, e.g. the order of gathering agents) or the order in which they where gathered (e.g. the order of coordinate sets).</dc:description>
        <rdfs:domain rdf:resource="http://www.w3.org/2002/07/owl#Thing"/>
        <rdfs:range rdf:resource="http://www.w3.org/2001/XMLSchema#nonNegativeInteger"/>
        <vann:termGroup rdf:resource="General"/>
    </owl:DatatypeProperty>

    <owl:ObjectProperty rdf:about="hasAccession">
        <rdfs:label xml:lang="en">has Accession</rdfs:label>
        <rdfs:isDefinedBy rdf:resource="http://rs.tdwg.org/abcd/terms/"/>
        <dwcattributes:status>recommended</dwcattributes:status>
        <dcterms:issued>2019-01-31</dcterms:issued>
        <dcterms:modified>2019-01-31</dcterms:modified>
        <rdfs:comment>Property to connect a concept to an accession.</rdfs:comment>
        <skos:definition>Property to connect a concept to an accession.</skos:definition>
        <rdfs:domain rdf:resource="http://www.w3.org/2002/07/owl#Thing"/>
        <rdfs:range rdf:resource="Accession"/>
    </owl:ObjectProperty>

    <owl:ObjectProperty rdf:about="hasAcknowledgement">
        <rdfs:label xml:lang="en">has Acknowledgement</rdfs:label>
        <rdfs:isDefinedBy rdf:resource="http://rs.tdwg.org/abcd/terms/"/>
        <dwcattributes:status>recommended</dwcattributes:status>
        <dcterms:issued>2019-01-31</dcterms:issued>
        <dcterms:modified>2019-01-31</dcterms:modified>
        <rdfs:comment>Property to connect an instance of a class to acknowledgement information (e.g. to declare grant money, help, permissions to reuse published materials, related scientific work used).</rdfs:comment>
        <skos:definition>Property to connect an instance of a class to acknowledgement information (e.g. to declare grant money, help, permissions to reuse published materials, related scientific work used).</skos:definition>
        <dc:description>To suggest a citation format for the current instance please use abcd:hasSuggestedCitation.</dc:description>
        <rdfs:domain rdf:resource="http://www.w3.org/2002/07/owl#Thing"/>
        <rdfs:range rdf:resource="LegalStatement"/>
    </owl:ObjectProperty>

    <owl:ObjectProperty rdf:about="hasAcquisitionDate">
        <rdfs:label xml:lang="en">has Acquisition Date</rdfs:label>
        <rdfs:isDefinedBy rdf:resource="http://rs.tdwg.org/abcd/terms/"/>
        <dwcattributes:status>recommended</dwcattributes:status>
        <dcterms:issued>2019-01-31</dcterms:issued>
        <dcterms:modified>2019-01-31</dcterms:modified>
        <rdfs:comment>Property to connect a specimen to the date of acquisition of the specimen by the institution.</rdfs:comment>
        <skos:definition>Property to connect a specimen to the date of acquisition of the specimen by the institution.</skos:definition>
        <rdfs:subPropertyOf rdf:resource="hasDate"/>
        <rdfs:domain rdf:resource="http://www.w3.org/2002/07/owl#Thing"/>
        <rdfs:range rdf:resource="Date"/>
    </owl:ObjectProperty>

    <owl:FunctionalProperty rdf:about="hasAcquisitionDate"/>

    <owl:ObjectProperty rdf:about="hasAltitude">
        <rdfs:label xml:lang="en">has Altitude</rdfs:label>
        <rdfs:isDefinedBy rdf:resource="http://rs.tdwg.org/abcd/terms/"/>
        <dwcattributes:status>recommended</dwcattributes:status>
        <dcterms:issued>2019-01-31</dcterms:issued>
        <dcterms:modified>2019-01-31</dcterms:modified>
        <rdfs:comment>Property to connect an instance of a class to an altitude of a gathering site land or floor level given as distance above (positive) or below mean sea level. Represented as Measurement Or Fact.</rdfs:comment>
        <skos:definition>Property to connect an instance of a class to an altitude of a gathering site land or floor level given as distance above (positive) or below mean sea level. Represented as Measurement Or Fact.</skos:definition>
        <rdfs:domain rdf:resource="http://www.w3.org/2002/07/owl#Thing"/>
        <rdfs:range rdf:resource="MeasurementOrFact"/>
    </owl:ObjectProperty>

    <owl:FunctionalProperty rdf:about="hasAltitude"/>

    <owl:ObjectProperty rdf:about="hasAnnotation">
        <rdfs:label xml:lang="en">has Annotation</rdfs:label>
        <rdfs:isDefinedBy rdf:resource="http://rs.tdwg.org/abcd/terms/"/>
        <dwcattributes:status>recommended</dwcattributes:status>
        <dcterms:issued>2019-01-31</dcterms:issued>
        <dcterms:modified>2019-01-31</dcterms:modified>
        <rdfs:comment>Property to connect an instance of a class to an Annotation.</rdfs:comment>
        <skos:definition>Property to connect an instance of a class to an Annotation.</skos:definition>
        <rdfs:domain rdf:resource="http://www.w3.org/2002/07/owl#Thing"/>
        <rdfs:range rdf:resource="Annotation"/>
    </owl:ObjectProperty>

    <owl:ObjectProperty rdf:about="hasAnnotator">
        <rdfs:label xml:lang="en">has Annotator</rdfs:label>
        <rdfs:isDefinedBy rdf:resource="http://rs.tdwg.org/abcd/terms/"/>
        <dwcattributes:status>recommended</dwcattributes:status>
        <dcterms:issued>2019-01-31</dcterms:issued>
        <dcterms:modified>2019-01-31</dcterms:modified>
        <rdfs:comment>Property to connect an Annotation to a Contact as its author.</rdfs:comment>
        <skos:definition>Property to connect an Annotation to a Contact as its author.</skos:definition>
        <rdfs:subPropertyOf rdf:resource="hasContact"/>
        <rdfs:domain rdf:resource="http://www.w3.org/2002/07/owl#Thing"/>
        <rdfs:range rdf:resource="Person"/>
    </owl:ObjectProperty>

    <owl:ObjectProperty rdf:about="hasAspect">
        <rdfs:label xml:lang="en">has Aspect</rdfs:label>
        <rdfs:isDefinedBy rdf:resource="http://rs.tdwg.org/abcd/terms/"/>
        <dwcattributes:status>recommended</dwcattributes:status>
        <dcterms:issued>2019-01-31</dcterms:issued>
        <dcterms:modified>2019-01-31</dcterms:modified>
        <rdfs:comment>Property to connect to the facing direction (aspect) of whole site or sample point. Represented as Measurement Or Fact.</rdfs:comment>
        <skos:definition>Property to connect to the facing direction (aspect) of whole site or sample point. Represented as Measurement Or Fact.</skos:definition>
        <rdfs:domain rdf:resource="http://www.w3.org/2002/07/owl#Thing"/>
        <rdfs:range rdf:resource="MeasurementOrFact"/>
    </owl:ObjectProperty>

    <owl:FunctionalProperty rdf:about="hasAspect"/>

    <owl:ObjectProperty rdf:about="hasAssemblage">
        <rdfs:label xml:lang="en">has Assemblage</rdfs:label>
        <rdfs:isDefinedBy rdf:resource="http://rs.tdwg.org/abcd/terms/"/>
        <dwcattributes:status>recommended</dwcattributes:status>
        <dcterms:issued>2019-01-31</dcterms:issued>
        <dcterms:modified>2019-01-31</dcterms:modified>
        <rdfs:comment>Property to connect a Unit to an Assemblage to describe symmetric relationships between several Units.</rdfs:comment>
        <skos:definition>Property to connect a Unit to an Assemblage to describe symmetric relationships between several Units.</skos:definition>
        <rdfs:domain rdf:resource="http://www.w3.org/2002/07/owl#Thing"/>
        <rdfs:range rdf:resource="Assemblage"/>
    </owl:ObjectProperty>

    <owl:ObjectProperty rdf:about="hasAssociation">
        <rdfs:label xml:lang="en">has Association</rdfs:label>
        <rdfs:isDefinedBy rdf:resource="http://rs.tdwg.org/abcd/terms/"/>
        <dwcattributes:status>recommended</dwcattributes:status>
        <dcterms:issued>2019-01-31</dcterms:issued>
        <dcterms:modified>2019-01-31</dcterms:modified>
        <rdfs:comment>Property to connect a Unit to an Association to describe an asymmetric relationship between two Units.</rdfs:comment>
        <skos:definition>Property to connect a Unit to an Association to describe an asymmetric relationship between two Units.</skos:definition>
        <rdfs:domain rdf:resource="http://www.w3.org/2002/07/owl#Thing"/>
        <rdfs:range rdf:resource="Association"/>
    </owl:ObjectProperty>

    <owl:ObjectProperty rdf:about="hasAuthor">
        <rdfs:label xml:lang="en">has Author</rdfs:label>
        <rdfs:isDefinedBy rdf:resource="http://rs.tdwg.org/abcd/terms/"/>
        <dwcattributes:status>recommended</dwcattributes:status>
        <dcterms:issued>2019-01-31</dcterms:issued>
        <dcterms:modified>2019-01-31</dcterms:modified>
        <rdfs:comment>Property to connect a concept to a person as author.</rdfs:comment>
        <skos:definition>Property to connect a concept to a person as author.</skos:definition>
        <rdfs:subPropertyOf rdf:resource="hasPerson"/>
        <rdfs:domain rdf:resource="http://www.w3.org/2002/07/owl#Thing"/>
        <rdfs:range rdf:resource="Person"/>
    </owl:ObjectProperty>

    <owl:ObjectProperty rdf:about="hasBiostratigraphicTerm">
        <rdfs:label xml:lang="en">has Biostratigraphic Term</rdfs:label>
        <rdfs:isDefinedBy rdf:resource="http://rs.tdwg.org/abcd/terms/"/>
        <dwcattributes:status>recommended</dwcattributes:status>
        <dcterms:issued>2019-01-31</dcterms:issued>
        <dcterms:modified>2019-01-31</dcterms:modified>
        <rdfs:comment>Property to connect an instance of a class to a  biostratigraphic zonation term expressing stratigraphy at a location (e.g. Psiloceras planorbis zone).</rdfs:comment>
        <skos:definition>Property to connect an instance of a class to a  biostratigraphic zonation term expressing stratigraphy at a location (e.g. Psiloceras planorbis zone).</skos:definition>
        <rdfs:subPropertyOf rdf:resource="hasStratigraphicTerm"/>
        <rdfs:domain rdf:resource="http://www.w3.org/2002/07/owl#Thing"/>
        <rdfs:range rdf:resource="StratigraphicTerm"/>
    </owl:ObjectProperty>

    <owl:ObjectProperty rdf:about="hasBiotope">
        <rdfs:label xml:lang="en">has Biotope</rdfs:label>
        <rdfs:isDefinedBy rdf:resource="http://rs.tdwg.org/abcd/terms/"/>
        <dwcattributes:status>recommended</dwcattributes:status>
        <dcterms:issued>2019-01-31</dcterms:issued>
        <dcterms:modified>2019-01-31</dcterms:modified>
        <rdfs:comment>Property to connect an instance of a class to a Biotope.</rdfs:comment>
        <skos:definition>Property to connect an instance of a class to a Biotope.</skos:definition>
        <rdfs:domain rdf:resource="http://www.w3.org/2002/07/owl#Thing"/>
        <rdfs:range rdf:resource="Biotope"/>
    </owl:ObjectProperty>

    <owl:ObjectProperty rdf:about="hasBlockedUntilDate">
        <rdfs:label xml:lang="en">has Blocked Until Date</rdfs:label>
        <rdfs:isDefinedBy rdf:resource="http://rs.tdwg.org/abcd/terms/"/>
        <dwcattributes:status>recommended</dwcattributes:status>
        <dcterms:issued>2019-01-31</dcterms:issued>
        <dcterms:modified>2019-01-31</dcterms:modified>
        <rdfs:comment>Property to connect a concept to a date or year until a specimen or sample is not available for loan, often due to planned publications.</rdfs:comment>
        <skos:definition>Property to connect a concept to a date or year until a specimen or sample is not available for loan, often due to planned publications.</skos:definition>
        <rdfs:subPropertyOf rdf:resource="hasDate"/>
        <rdfs:domain rdf:resource="http://www.w3.org/2002/07/owl#Thing"/>
        <rdfs:range rdf:resource="Date"/>
    </owl:ObjectProperty>

    <owl:FunctionalProperty rdf:about="hasBlockedUntilDate"/>

    <owl:ObjectProperty rdf:about="hasBotanicalTaxonRank">
        <rdfs:label xml:lang="en">has Botanical Taxon Rank</rdfs:label>
        <rdfs:isDefinedBy rdf:resource="http://rs.tdwg.org/abcd/terms/"/>
        <dwcattributes:status>recommended</dwcattributes:status>
        <dcterms:issued>2019-01-31</dcterms:issued>
        <dcterms:modified>2019-01-31</dcterms:modified>
        <rdfs:comment>Property to connect a concept to a botanical taxon rank.</rdfs:comment>
        <skos:definition>Property to connect a concept to a botanical taxon rank.</skos:definition>
        <rdfs:domain rdf:resource="http://www.w3.org/2002/07/owl#Thing"/>
        <rdfs:range rdf:resource="BotanicalTaxonRank"/>
    </owl:ObjectProperty>

    <owl:FunctionalProperty rdf:about="hasBotanicalTaxonRank"/>

    <owl:ObjectProperty rdf:about="hasChronostratigraphicTerm">
        <rdfs:label xml:lang="en">has Chronostratigraphic Term</rdfs:label>
        <rdfs:isDefinedBy rdf:resource="http://rs.tdwg.org/abcd/terms/"/>
        <dwcattributes:status>recommended</dwcattributes:status>
        <dcterms:issued>2019-01-31</dcterms:issued>
        <dcterms:modified>2019-01-31</dcterms:modified>
        <rdfs:comment>Property to connect an instance of a class to a chronostratigraphic dating term expressing stratigraphy at a location.</rdfs:comment>
        <skos:definition>Property to connect an instance of a class to a chronostratigraphic dating term expressing stratigraphy at a location.</skos:definition>
        <rdfs:subPropertyOf rdf:resource="hasStratigraphicTerm"/>
        <rdfs:domain rdf:resource="http://www.w3.org/2002/07/owl#Thing"/>
        <rdfs:range rdf:resource="StratigraphicTerm"/>
    </owl:ObjectProperty>

    <owl:ObjectProperty rdf:about="hasContact">
        <rdfs:label xml:lang="en">has Contact</rdfs:label>
        <rdfs:isDefinedBy rdf:resource="http://rs.tdwg.org/abcd/terms/"/>
        <dwcattributes:status>recommended</dwcattributes:status>
        <dcterms:issued>2019-01-31</dcterms:issued>
        <dcterms:modified>2019-01-31</dcterms:modified>
        <rdfs:comment>Property to connect an instance of a class to a Contact.</rdfs:comment>
        <skos:definition>Property to connect an instance of a class to a Contact.</skos:definition>
        <rdfs:domain rdf:resource="http://www.w3.org/2002/07/owl#Thing"/>
        <rdfs:range rdf:resource="Contact"/>
    </owl:ObjectProperty>

    <owl:ObjectProperty rdf:about="hasContentContact">
        <rdfs:label xml:lang="en">has Content Contact</rdfs:label>
        <rdfs:isDefinedBy rdf:resource="http://rs.tdwg.org/abcd/terms/"/>
        <dwcattributes:status>recommended</dwcattributes:status>
        <dcterms:issued>2019-01-31</dcterms:issued>
        <dcterms:modified>2019-01-31</dcterms:modified>
        <rdfs:comment>Property to connect an instance of a class to a Contact that is responsible for its content.</rdfs:comment>
        <skos:definition>Property to connect an instance of a class to a Contact that is responsible for its content.</skos:definition>
        <rdfs:subPropertyOf rdf:resource="hasContact"/>
        <dc:description>In context of datasets  the content contact is usually representing the agent acting as the original supplier or custodian of the dataset.</dc:description>
        <rdfs:domain rdf:resource="http://www.w3.org/2002/07/owl#Thing"/>
        <rdfs:range rdf:resource="Contact"/>
    </owl:ObjectProperty>

    <owl:ObjectProperty rdf:about="hasCoordinates">
        <rdfs:label xml:lang="en">has Coordinates</rdfs:label>
        <rdfs:isDefinedBy rdf:resource="http://rs.tdwg.org/abcd/terms/"/>
        <dwcattributes:status>recommended</dwcattributes:status>
        <dcterms:issued>2019-01-31</dcterms:issued>
        <dcterms:modified>2019-01-31</dcterms:modified>
        <rdfs:comment>Property to connect an instance of a class to Coordinates.</rdfs:comment>
        <skos:definition>Property to connect an instance of a class to Coordinates.</skos:definition>
        <rdfs:domain rdf:resource="http://www.w3.org/2002/07/owl#Thing"/>
        <rdfs:range rdf:resource="Coordinates"/>
    </owl:ObjectProperty>

    <owl:ObjectProperty rdf:about="hasCountry">
        <rdfs:label xml:lang="en">has Country</rdfs:label>
        <rdfs:isDefinedBy rdf:resource="http://rs.tdwg.org/abcd/terms/"/>
        <dwcattributes:status>recommended</dwcattributes:status>
        <dcterms:issued>2019-01-31</dcterms:issued>
        <dcterms:modified>2019-01-31</dcterms:modified>
        <rdfs:comment>Property to connect an instance of a class to a Country.</rdfs:comment>
        <skos:definition>Property to connect an instance of a class to a Country.</skos:definition>
        <rdfs:domain rdf:resource="http://www.w3.org/2002/07/owl#Thing"/>
        <rdfs:range rdf:resource="Country"/>
    </owl:ObjectProperty>

    <owl:ObjectProperty rdf:about="hasCreator">
        <rdfs:label xml:lang="en">has Creator</rdfs:label>
        <rdfs:isDefinedBy rdf:resource="http://rs.tdwg.org/abcd/terms/"/>
        <dwcattributes:status>recommended</dwcattributes:status>
        <dcterms:issued>2019-01-31</dcterms:issued>
        <dcterms:modified>2019-01-31</dcterms:modified>
        <rdfs:comment>Property to connect a concept to its creator.</rdfs:comment>
        <skos:definition>Property to connect a concept to its creator.</skos:definition>
        <rdfs:subPropertyOf rdf:resource="hasContact"/>
        <rdfs:domain rdf:resource="http://www.w3.org/2002/07/owl#Thing"/>
        <rdfs:range rdf:resource="Contact"/>
    </owl:ObjectProperty>

    <owl:ObjectProperty rdf:about="hasDataSet">
        <rdfs:label xml:lang="en">has Data Set</rdfs:label>
        <rdfs:isDefinedBy rdf:resource="http://rs.tdwg.org/abcd/terms/"/>
        <dwcattributes:status>recommended</dwcattributes:status>
        <dcterms:issued>2019-01-31</dcterms:issued>
        <dcterms:modified>2019-01-31</dcterms:modified>
        <rdfs:comment>Property to connect an instance of a class to a data set.</rdfs:comment>
        <skos:definition>Property to connect an instance of a class to a data set.</skos:definition>
        <rdfs:domain rdf:resource="http://www.w3.org/2002/07/owl#Thing"/>
        <rdfs:range rdf:resource="DataSet"/>
    </owl:ObjectProperty>

    <owl:ObjectProperty rdf:about="hasDate">
        <rdfs:label xml:lang="en">has Date</rdfs:label>
        <rdfs:isDefinedBy rdf:resource="http://rs.tdwg.org/abcd/terms/"/>
        <dwcattributes:status>recommended</dwcattributes:status>
        <dcterms:issued>2019-01-31</dcterms:issued>
        <dcterms:modified>2019-01-31</dcterms:modified>
        <rdfs:comment>Connects an instance of a class to a Date.</rdfs:comment>
        <skos:definition>Connects an instance of a class to a Date.</skos:definition>
        <rdfs:domain rdf:resource="http://www.w3.org/2002/07/owl#Thing"/>
        <rdfs:range rdf:resource="Date"/>
    </owl:ObjectProperty>

    <owl:FunctionalProperty rdf:about="hasDate"/>

    <owl:ObjectProperty rdf:about="hasDateCreated">
        <rdfs:label xml:lang="en">has Date Created</rdfs:label>
        <rdfs:isDefinedBy rdf:resource="http://rs.tdwg.org/abcd/terms/"/>
        <dwcattributes:status>recommended</dwcattributes:status>
        <dcterms:issued>2019-01-31</dcterms:issued>
        <dcterms:modified>2019-01-31</dcterms:modified>
        <rdfs:comment>Connects a class to the date it was created.</rdfs:comment>
        <skos:definition>Connects a class to the date it was created.</skos:definition>
        <rdfs:subPropertyOf rdf:resource="hasDate"/>
        <rdfs:domain rdf:resource="http://www.w3.org/2002/07/owl#Thing"/>
        <rdfs:range rdf:resource="Date"/>
        <skos:exactMatch rdf:resource="http://purl.org/dc/terms/created"/>
    </owl:ObjectProperty>

    <owl:FunctionalProperty rdf:about="hasDateCreated"/>

    <owl:ObjectProperty rdf:about="hasDateModified">
        <rdfs:label xml:lang="en">has Date Modified</rdfs:label>
        <rdfs:isDefinedBy rdf:resource="http://rs.tdwg.org/abcd/terms/"/>
        <dwcattributes:status>recommended</dwcattributes:status>
        <dcterms:issued>2019-01-31</dcterms:issued>
        <dcterms:modified>2019-01-31</dcterms:modified>
        <rdfs:comment>Property to connect an instance of a class to the date it was last modified/edited.</rdfs:comment>
        <skos:definition>Property to connect an instance of a class to the date it was last modified/edited.</skos:definition>
        <rdfs:subPropertyOf rdf:resource="hasDate"/>
        <dc:description>Needs to be updated if any part of the data is changed.</dc:description>
        <rdfs:domain rdf:resource="http://www.w3.org/2002/07/owl#Thing"/>
        <rdfs:range rdf:resource="Date"/>
        <skos:exactMatch rdf:resource="http://purl.org/dc/terms/modified"/>
    </owl:ObjectProperty>

    <owl:ObjectProperty rdf:about="hasDepth">
        <rdfs:label xml:lang="en">has Depth</rdfs:label>
        <rdfs:isDefinedBy rdf:resource="http://rs.tdwg.org/abcd/terms/"/>
        <dwcattributes:status>recommended</dwcattributes:status>
        <dcterms:issued>2019-01-31</dcterms:issued>
        <dcterms:modified>2019-01-31</dcterms:modified>
        <rdfs:comment>Property to connect an instance of a class to the vertical distance point or range measurement in relation to a ground datum such as water level, or level of the sea floor for benthic samples.. Represented as Measurement Or Fact.</rdfs:comment>
        <skos:definition>Property to connect an instance of a class to the vertical distance point or range measurement in relation to a ground datum such as water level, or level of the sea floor for benthic samples.. Represented as Measurement Or Fact.</skos:definition>
        <rdfs:domain rdf:resource="http://www.w3.org/2002/07/owl#Thing"/>
        <rdfs:range rdf:resource="MeasurementOrFact"/>
    </owl:ObjectProperty>

    <owl:FunctionalProperty rdf:about="hasDepth"/>

    <owl:ObjectProperty rdf:about="hasFieldNoteReference">
        <rdfs:label xml:lang="en">has Field Note Reference</rdfs:label>
        <rdfs:isDefinedBy rdf:resource="http://rs.tdwg.org/abcd/terms/"/>
        <dwcattributes:status>recommended</dwcattributes:status>
        <dcterms:issued>2019-01-31</dcterms:issued>
        <dcterms:modified>2019-01-31</dcterms:modified>
        <rdfs:comment>Property to connect a Unit to a Reference where corresponding Field Notes are published.</rdfs:comment>
        <skos:definition>Property to connect a Unit to a Reference where corresponding Field Notes are published.</skos:definition>
        <rdfs:domain rdf:resource="http://www.w3.org/2002/07/owl#Thing"/>
        <rdfs:range rdf:resource="Reference"/>
    </owl:ObjectProperty>

    <owl:ObjectProperty rdf:about="hasFieldNumber">
        <rdfs:label xml:lang="en">has Field Number</rdfs:label>
        <rdfs:isDefinedBy rdf:resource="http://rs.tdwg.org/abcd/terms/"/>
        <dwcattributes:status>recommended</dwcattributes:status>
        <dcterms:issued>2019-01-31</dcterms:issued>
        <dcterms:modified>2019-01-31</dcterms:modified>
        <rdfs:comment>Property to connect a Unit or a Gathering Agent (Contact) to a Field Number.</rdfs:comment>
        <skos:definition>Property to connect a Unit or a Gathering Agent (Contact) to a Field Number.</skos:definition>
        <rdfs:domain rdf:resource="http://www.w3.org/2002/07/owl#Thing"/>
        <rdfs:range rdf:resource="FieldNumber"/>
    </owl:ObjectProperty>

    <owl:ObjectProperty rdf:about="hasFileFormatVersion">
        <rdfs:label xml:lang="en">has File Format Version</rdfs:label>
        <rdfs:isDefinedBy rdf:resource="http://rs.tdwg.org/abcd/terms/"/>
        <dwcattributes:status>recommended</dwcattributes:status>
        <dcterms:issued>2019-01-31</dcterms:issued>
        <dcterms:modified>2019-01-31</dcterms:modified>
        <rdfs:comment>Property to connect a concept to a File Format Version.</rdfs:comment>
        <skos:definition>Property to connect a concept to a File Format Version.</skos:definition>
        <rdfs:subPropertyOf rdf:resource="hasVersion"/>
        <rdfs:domain rdf:resource="http://www.w3.org/2002/07/owl#Thing"/>
        <rdfs:range rdf:resource="Version"/>
    </owl:ObjectProperty>

    <owl:ObjectProperty rdf:about="hasGathering">
        <rdfs:label xml:lang="en">has Gathering</rdfs:label>
        <rdfs:isDefinedBy rdf:resource="http://rs.tdwg.org/abcd/terms/"/>
        <dwcattributes:status>recommended</dwcattributes:status>
        <dcterms:issued>2019-01-31</dcterms:issued>
        <dcterms:modified>2019-01-31</dcterms:modified>
        <rdfs:comment>Property to connect an instance of a class to a gathering event.</rdfs:comment>
        <skos:definition>Property to connect an instance of a class to a gathering event.</skos:definition>
        <rdfs:domain rdf:resource="http://www.w3.org/2002/07/owl#Thing"/>
        <rdfs:range rdf:resource="Gathering"/>
    </owl:ObjectProperty>

    <owl:ObjectProperty rdf:about="hasGatheringAgent">
        <rdfs:label xml:lang="en">has Gathering Agent</rdfs:label>
        <rdfs:isDefinedBy rdf:resource="http://rs.tdwg.org/abcd/terms/"/>
        <dwcattributes:status>recommended</dwcattributes:status>
        <dcterms:issued>2019-01-31</dcterms:issued>
        <dcterms:modified>2019-01-31</dcterms:modified>
        <rdfs:comment>Property to connect an instance of a class to a Person as gathering agent.</rdfs:comment>
        <skos:definition>Property to connect an instance of a class to a Person as gathering agent.</skos:definition>
        <rdfs:subPropertyOf rdf:resource="hasContact"/>
        <rdfs:domain rdf:resource="http://www.w3.org/2002/07/owl#Thing"/>
        <rdfs:range rdf:resource="Person"/>
    </owl:ObjectProperty>

    <owl:ObjectProperty rdf:about="hasGrowthCondition">
        <rdfs:label xml:lang="en">has Growth Condition</rdfs:label>
        <rdfs:isDefinedBy rdf:resource="http://rs.tdwg.org/abcd/terms/"/>
        <dwcattributes:status>recommended</dwcattributes:status>
        <dcterms:issued>2019-01-31</dcterms:issued>
        <dcterms:modified>2019-01-31</dcterms:modified>
        <rdfs:comment>Property to connect a culture unit to growth conditions.</rdfs:comment>
        <skos:definition>Property to connect a culture unit to growth conditions.</skos:definition>
        <rdfs:domain rdf:resource="http://www.w3.org/2002/07/owl#Thing"/>
        <rdfs:range rdf:resource="GrowthCondition"/>
    </owl:ObjectProperty>

    <owl:ObjectProperty rdf:about="hasHeight">
        <rdfs:label xml:lang="en">has Height</rdfs:label>
        <rdfs:isDefinedBy rdf:resource="http://rs.tdwg.org/abcd/terms/"/>
        <dwcattributes:status>recommended</dwcattributes:status>
        <dcterms:issued>2019-01-31</dcterms:issued>
        <dcterms:modified>2019-01-31</dcterms:modified>
        <rdfs:comment>Property to connect an instance of a class to the vertical distance measure or range in relation to a ground datum, e.g. ground level. Represented as Measurement Or Fact.</rdfs:comment>
        <skos:definition>Property to connect an instance of a class to the vertical distance measure or range in relation to a ground datum, e.g. ground level. Represented as Measurement Or Fact.</skos:definition>
        <rdfs:domain rdf:resource="http://www.w3.org/2002/07/owl#Thing"/>
        <rdfs:range rdf:resource="MeasurementOrFact"/>
    </owl:ObjectProperty>

    <owl:FunctionalProperty rdf:about="hasHeight"/>

    <owl:ObjectProperty rdf:about="hasHigherTaxon">
        <rdfs:label xml:lang="en">has Higher Taxon</rdfs:label>
        <rdfs:isDefinedBy rdf:resource="http://rs.tdwg.org/abcd/terms/"/>
        <dwcattributes:status>recommended</dwcattributes:status>
        <dcterms:issued>2019-01-31</dcterms:issued>
        <dcterms:modified>2019-01-31</dcterms:modified>
        <rdfs:comment>Property to connect an Identified Taxon to a Higher Taxon.</rdfs:comment>
        <skos:definition>Property to connect an Identified Taxon to a Higher Taxon.</skos:definition>
        <rdfs:domain rdf:resource="http://www.w3.org/2002/07/owl#Thing"/>
        <rdfs:range rdf:resource="HigherTaxon"/>
    </owl:ObjectProperty>

    <owl:ObjectProperty rdf:about="hasHigherTaxonRank">
        <rdfs:label xml:lang="en">has Higher Taxon Rank</rdfs:label>
        <rdfs:isDefinedBy rdf:resource="http://rs.tdwg.org/abcd/terms/"/>
        <dwcattributes:status>recommended</dwcattributes:status>
        <dcterms:issued>2019-01-31</dcterms:issued>
        <dcterms:modified>2019-01-31</dcterms:modified>
        <rdfs:comment>Property to connect a Higher Taxon to a rank higher than genus.</rdfs:comment>
        <skos:definition>Property to connect a Higher Taxon to a rank higher than genus.</skos:definition>
        <rdfs:domain rdf:resource="http://www.w3.org/2002/07/owl#Thing"/>
        <rdfs:range rdf:resource="HigherTaxonRank"/>
    </owl:ObjectProperty>

    <owl:ObjectProperty rdf:about="hasIdentification">
        <rdfs:label xml:lang="en">has Identification</rdfs:label>
        <rdfs:isDefinedBy rdf:resource="http://rs.tdwg.org/abcd/terms/"/>
        <dwcattributes:status>recommended</dwcattributes:status>
        <dcterms:issued>2019-01-31</dcterms:issued>
        <dcterms:modified>2019-01-31</dcterms:modified>
        <rdfs:comment>Property to connect an instance of a class to an Identification.</rdfs:comment>
        <skos:definition>Property to connect an instance of a class to an Identification.</skos:definition>
        <rdfs:domain rdf:resource="http://www.w3.org/2002/07/owl#Thing"/>
        <rdfs:range rdf:resource="Identification"/>
    </owl:ObjectProperty>

    <owl:ObjectProperty rdf:about="hasIdentificationSource">
        <rdfs:label xml:lang="en">has Identification Source</rdfs:label>
        <rdfs:isDefinedBy rdf:resource="http://rs.tdwg.org/abcd/terms/"/>
        <dwcattributes:status>recommended</dwcattributes:status>
        <dcterms:issued>2019-01-31</dcterms:issued>
        <dcterms:modified>2019-01-31</dcterms:modified>
        <rdfs:comment>Property to connect an Identification to the Reference which has provided the Unit Identification (and - if present - the identifier's name and/or organization).</rdfs:comment>
        <skos:definition>Property to connect an Identification to the Reference which has provided the Unit Identification (and - if present - the identifier's name and/or organization).</skos:definition>
        <rdfs:subPropertyOf rdf:resource="hasReference"/>
        <dc:description>The entire identification event was taken from the source given here. It is not recommended to cite "field tag", or "determination slip" here as the source of the identification but to restrict this to published works. To cite published works that helped with the Identification, please use the abcd:hasReference property of the Identification.</dc:description>
        <rdfs:domain rdf:resource="http://www.w3.org/2002/07/owl#Thing"/>
        <rdfs:range rdf:resource="Reference"/>
    </owl:ObjectProperty>

    <owl:ObjectProperty rdf:about="hasIdentifiedTaxon">
        <rdfs:label xml:lang="en">has Identified Taxon</rdfs:label>
        <rdfs:isDefinedBy rdf:resource="http://rs.tdwg.org/abcd/terms/"/>
        <dwcattributes:status>recommended</dwcattributes:status>
        <dcterms:issued>2019-01-31</dcterms:issued>
        <dcterms:modified>2019-01-31</dcterms:modified>
        <rdfs:comment>Property to connect an Identification to the Identified Taxon.</rdfs:comment>
        <skos:definition>Property to connect an Identification to the Identified Taxon.</skos:definition>
        <rdfs:domain rdf:resource="http://www.w3.org/2002/07/owl#Thing"/>
        <rdfs:range rdf:resource="IdentifiedTaxon"/>
    </owl:ObjectProperty>

    <owl:FunctionalProperty rdf:about="hasIdentifiedTaxon"/>

    <owl:ObjectProperty rdf:about="hasIdentifier">
        <rdfs:label xml:lang="en">has Identifier</rdfs:label>
        <rdfs:isDefinedBy rdf:resource="http://rs.tdwg.org/abcd/terms/"/>
        <dwcattributes:status>recommended</dwcattributes:status>
        <dcterms:issued>2019-01-31</dcterms:issued>
        <dcterms:modified>2019-01-31</dcterms:modified>
        <rdfs:comment>Property to connect an Identification to the Person (Contact) who issued it.</rdfs:comment>
        <skos:definition>Property to connect an Identification to the Person (Contact) who issued it.</skos:definition>
        <rdfs:domain rdf:resource="http://www.w3.org/2002/07/owl#Thing"/>
        <rdfs:range rdf:resource="Person"/>
    </owl:ObjectProperty>

    <owl:ObjectProperty rdf:about="hasInverseAssociation">
        <rdfs:label xml:lang="en">has Inverse Association</rdfs:label>
        <rdfs:isDefinedBy rdf:resource="http://rs.tdwg.org/abcd/terms/"/>
        <dwcattributes:status>recommended</dwcattributes:status>
        <dcterms:issued>2019-01-31</dcterms:issued>
        <dcterms:modified>2019-01-31</dcterms:modified>
        <rdfs:comment>A property to link an Association to its inverse.</rdfs:comment>
        <skos:definition>A property to link an Association to its inverse.</skos:definition>
        <rdfs:domain rdf:resource="Association"/>
        <rdfs:range rdf:resource="Association"/>
    </owl:ObjectProperty>

    <owl:ObjectProperty rdf:about="hasLastEditor">
        <rdfs:label xml:lang="en">has Last Editor</rdfs:label>
        <rdfs:isDefinedBy rdf:resource="http://rs.tdwg.org/abcd/terms/"/>
        <dwcattributes:status>recommended</dwcattributes:status>
        <dcterms:issued>2019-01-31</dcterms:issued>
        <dcterms:modified>2019-01-31</dcterms:modified>
        <rdfs:comment>Property to connect an instance of a class to the Contact that created or last edited it.</rdfs:comment>
        <skos:definition>Property to connect an instance of a class to the Contact that created or last edited it.</skos:definition>
        <rdfs:subPropertyOf rdf:resource="hasContact"/>
        <rdfs:domain rdf:resource="http://www.w3.org/2002/07/owl#Thing"/>
        <rdfs:range rdf:resource="Person"/>
    </owl:ObjectProperty>

    <owl:ObjectProperty rdf:about="hasLicense">
        <rdfs:label xml:lang="en">has License</rdfs:label>
        <rdfs:isDefinedBy rdf:resource="http://rs.tdwg.org/abcd/terms/"/>
        <dwcattributes:status>recommended</dwcattributes:status>
        <dcterms:issued>2019-01-31</dcterms:issued>
        <dcterms:modified>2019-01-31</dcterms:modified>
        <rdfs:comment>Property to connect a class to the license that applies to it.</rdfs:comment>
        <skos:definition>Property to connect a class to the license that applies to it.</skos:definition>
        <dc:description>This should be used if the data is placed under a known and documented license (e.g. GNU Free Document License [GFDL], Creative Commons [CC], Open Database License [ODbL]). The corresponding properties for the Legal Statement class should be filled accordingly.</dc:description>
        <rdfs:domain rdf:resource="http://www.w3.org/2002/07/owl#Thing"/>
        <rdfs:range rdf:resource="LegalStatement"/>
    </owl:ObjectProperty>

    <owl:ObjectProperty rdf:about="hasLithostratigraphicTerm">
        <rdfs:label xml:lang="en">has Lithostratigraphic Term</rdfs:label>
        <rdfs:isDefinedBy rdf:resource="http://rs.tdwg.org/abcd/terms/"/>
        <dwcattributes:status>recommended</dwcattributes:status>
        <dcterms:issued>2019-01-31</dcterms:issued>
        <dcterms:modified>2019-01-31</dcterms:modified>
        <rdfs:comment>Property to connect an instance of a class to a lithostratigraphic term describing geology at a location (e.g. Mercia Mudstone Group).</rdfs:comment>
        <skos:definition>Property to connect an instance of a class to a lithostratigraphic term describing geology at a location (e.g. Mercia Mudstone Group).</skos:definition>
        <rdfs:subPropertyOf rdf:resource="hasStratigraphicTerm"/>
        <rdfs:domain rdf:resource="http://www.w3.org/2002/07/owl#Thing"/>
        <rdfs:range rdf:resource="StratigraphicTerm"/>
    </owl:ObjectProperty>

    <owl:ObjectProperty rdf:about="hasLoanDate">
        <rdfs:label xml:lang="en">has Loan Date</rdfs:label>
        <rdfs:isDefinedBy rdf:resource="http://rs.tdwg.org/abcd/terms/"/>
        <dwcattributes:status>recommended</dwcattributes:status>
        <dcterms:issued>2019-01-31</dcterms:issued>
        <dcterms:modified>2019-01-31</dcterms:modified>
        <rdfs:comment>Property to connect a concept to the date it was lent.</rdfs:comment>
        <skos:definition>Property to connect a concept to the date it was lent.</skos:definition>
        <rdfs:subPropertyOf rdf:resource="hasDate"/>
        <rdfs:domain rdf:resource="http://www.w3.org/2002/07/owl#Thing"/>
        <rdfs:range rdf:resource="Date"/>
    </owl:ObjectProperty>

    <owl:ObjectProperty rdf:about="hasLoanRestrictions">
        <rdfs:label xml:lang="en">has Loan Restrictions</rdfs:label>
        <rdfs:isDefinedBy rdf:resource="http://rs.tdwg.org/abcd/terms/"/>
        <dwcattributes:status>recommended</dwcattributes:status>
        <dcterms:issued>2019-01-31</dcterms:issued>
        <dcterms:modified>2019-01-31</dcterms:modified>
        <rdfs:comment>Property to connect a concept to restrictions for accessing or loaning a specimen or sample.</rdfs:comment>
        <skos:definition>Property to connect a concept to restrictions for accessing or loaning a specimen or sample.</skos:definition>
        <rdfs:domain rdf:resource="http://www.w3.org/2002/07/owl#Thing"/>
        <rdfs:range rdf:resource="LoanRestrictions"/>
    </owl:ObjectProperty>

    <owl:ObjectProperty rdf:about="hasLoanReturnDate">
        <rdfs:label xml:lang="en">has Loan Return Date</rdfs:label>
        <rdfs:isDefinedBy rdf:resource="http://rs.tdwg.org/abcd/terms/"/>
        <dwcattributes:status>recommended</dwcattributes:status>
        <dcterms:issued>2019-01-31</dcterms:issued>
        <dcterms:modified>2019-01-31</dcterms:modified>
        <rdfs:comment>Property to connect a concept to the date it has to be returned and the loan ends.</rdfs:comment>
        <skos:definition>Property to connect a concept to the date it has to be returned and the loan ends.</skos:definition>
        <rdfs:subPropertyOf rdf:resource="hasDate"/>
        <rdfs:domain rdf:resource="http://www.w3.org/2002/07/owl#Thing"/>
        <rdfs:range rdf:resource="Date"/>
    </owl:ObjectProperty>

    <owl:ObjectProperty rdf:about="hasMark">
        <rdfs:label xml:lang="en">has Mark</rdfs:label>
        <rdfs:isDefinedBy rdf:resource="http://rs.tdwg.org/abcd/terms/"/>
        <dwcattributes:status>recommended</dwcattributes:status>
        <dcterms:issued>2019-01-31</dcterms:issued>
        <dcterms:modified>2019-01-31</dcterms:modified>
        <rdfs:comment>Property to connect a concept to a mark.</rdfs:comment>
        <skos:definition>Property to connect a concept to a mark.</skos:definition>
        <rdfs:domain rdf:resource="http://www.w3.org/2002/07/owl#Thing"/>
        <rdfs:range rdf:resource="Mark"/>
    </owl:ObjectProperty>

    <owl:ObjectProperty rdf:about="hasMeasurementOrFact">
        <rdfs:label xml:lang="en">has Measurement Or Fact</rdfs:label>
        <rdfs:isDefinedBy rdf:resource="http://rs.tdwg.org/abcd/terms/"/>
        <dwcattributes:status>recommended</dwcattributes:status>
        <dcterms:issued>2019-01-31</dcterms:issued>
        <dcterms:modified>2019-01-31</dcterms:modified>
        <rdfs:comment>Property to connect an instance of a class to a Measurement Or Fact.</rdfs:comment>
        <skos:definition>Property to connect an instance of a class to a Measurement Or Fact.</skos:definition>
        <rdfs:domain rdf:resource="http://www.w3.org/2002/07/owl#Thing"/>
        <rdfs:range rdf:resource="MeasurementOrFact"/>
    </owl:ObjectProperty>

    <owl:ObjectProperty rdf:about="hasMeasuringAgent">
        <rdfs:label xml:lang="en">has Measuring Agent</rdfs:label>
        <rdfs:isDefinedBy rdf:resource="http://rs.tdwg.org/abcd/terms/"/>
        <dwcattributes:status>recommended</dwcattributes:status>
        <dcterms:issued>2019-01-31</dcterms:issued>
        <dcterms:modified>2019-01-31</dcterms:modified>
        <rdfs:comment>Property to connect a Measurement Or Fact to the Contact it was done by.</rdfs:comment>
        <skos:definition>Property to connect a Measurement Or Fact to the Contact it was done by.</skos:definition>
        <rdfs:subPropertyOf rdf:resource="hasContact"/>
        <rdfs:domain rdf:resource="http://www.w3.org/2002/07/owl#Thing"/>
        <rdfs:range rdf:resource="Person"/>
    </owl:ObjectProperty>

    <owl:ObjectProperty rdf:about="hasMultimediaObject">
        <rdfs:label xml:lang="en">has Multimedia Object</rdfs:label>
        <rdfs:isDefinedBy rdf:resource="http://rs.tdwg.org/abcd/terms/"/>
        <dwcattributes:status>recommended</dwcattributes:status>
        <dcterms:issued>2019-01-31</dcterms:issued>
        <dcterms:modified>2019-01-31</dcterms:modified>
        <rdfs:comment>Property to connect an instance of a class to a Multimedia Object.</rdfs:comment>
        <skos:definition>Property to connect an instance of a class to a Multimedia Object.</skos:definition>
        <rdfs:domain rdf:resource="http://www.w3.org/2002/07/owl#Thing"/>
        <rdfs:range rdf:resource="MultimediaObject"/>
    </owl:ObjectProperty>

    <owl:ObjectProperty rdf:about="hasNamedArea">
        <rdfs:label xml:lang="en">has Named Area</rdfs:label>
        <rdfs:isDefinedBy rdf:resource="http://rs.tdwg.org/abcd/terms/"/>
        <dwcattributes:status>recommended</dwcattributes:status>
        <dcterms:issued>2019-01-31</dcterms:issued>
        <dcterms:modified>2019-01-31</dcterms:modified>
        <rdfs:comment>Property to connect an instance of a class to a Named Area.</rdfs:comment>
        <skos:definition>Property to connect an instance of a class to a Named Area.</skos:definition>
        <rdfs:domain rdf:resource="http://www.w3.org/2002/07/owl#Thing"/>
        <rdfs:range rdf:resource="NamedArea"/>
    </owl:ObjectProperty>

    <owl:ObjectProperty rdf:about="hasNamedPlaceRelation">
        <rdfs:label xml:lang="en">has Named Place Relation</rdfs:label>
        <rdfs:isDefinedBy rdf:resource="http://rs.tdwg.org/abcd/terms/"/>
        <dwcattributes:status>recommended</dwcattributes:status>
        <dcterms:issued>2019-01-31</dcterms:issued>
        <dcterms:modified>2019-01-31</dcterms:modified>
        <rdfs:comment>Property to connect an instance of a class to a Named Place Relation.</rdfs:comment>
        <skos:definition>Property to connect an instance of a class to a Named Place Relation.</skos:definition>
        <rdfs:domain rdf:resource="http://www.w3.org/2002/07/owl#Thing"/>
        <rdfs:range rdf:resource="NamedPlaceRelation"/>
    </owl:ObjectProperty>

    <owl:ObjectProperty rdf:about="hasNomenclaturalTypeDesignation">
        <rdfs:label xml:lang="en">has Nomenclatural Type Designation</rdfs:label>
        <rdfs:isDefinedBy rdf:resource="http://rs.tdwg.org/abcd/terms/"/>
        <dwcattributes:status>recommended</dwcattributes:status>
        <dcterms:issued>2019-01-31</dcterms:issued>
        <dcterms:modified>2019-01-31</dcterms:modified>
        <rdfs:comment>Property to connect a concept to its nomenclatural type designation.</rdfs:comment>
        <skos:definition>Property to connect a concept to its nomenclatural type designation.</skos:definition>
        <rdfs:domain rdf:resource="http://www.w3.org/2002/07/owl#Thing"/>
        <rdfs:range rdf:resource="NomenclaturalTypeDesignation"/>
    </owl:ObjectProperty>

    <owl:ObjectProperty rdf:about="hasNomenclatureCode">
        <rdfs:label xml:lang="en">has Nomenclature Code</rdfs:label>
        <rdfs:isDefinedBy rdf:resource="http://rs.tdwg.org/abcd/terms/"/>
        <dwcattributes:status>recommended</dwcattributes:status>
        <dcterms:issued>2019-01-31</dcterms:issued>
        <dcterms:modified>2019-01-31</dcterms:modified>
        <rdfs:comment>Property to connect an Identified Taxon to a Nomenclature Code.</rdfs:comment>
        <skos:definition>Property to connect an Identified Taxon to a Nomenclature Code.</skos:definition>
        <rdfs:domain rdf:resource="http://www.w3.org/2002/07/owl#Thing"/>
        <rdfs:range rdf:resource="NomenclatureCode"/>
    </owl:ObjectProperty>

    <owl:FunctionalProperty rdf:about="hasNomenclatureCode"/>

    <owl:ObjectProperty rdf:about="hasOrganization">
        <rdfs:label xml:lang="en">has Organization</rdfs:label>
        <rdfs:isDefinedBy rdf:resource="http://rs.tdwg.org/abcd/terms/"/>
        <dwcattributes:status>recommended</dwcattributes:status>
        <dcterms:issued>2019-01-31</dcterms:issued>
        <dcterms:modified>2019-01-31</dcterms:modified>
        <rdfs:comment>Property to connect a class to an Organization.</rdfs:comment>
        <skos:definition>Property to connect a class to an Organization.</skos:definition>
        <rdfs:subPropertyOf rdf:resource="hasContact"/>
        <rdfs:domain rdf:resource="http://www.w3.org/2002/07/owl#Thing"/>
        <rdfs:range rdf:resource="Organization"/>
    </owl:ObjectProperty>

    <owl:ObjectProperty rdf:about="hasOtherLegalStatement">
        <rdfs:label xml:lang="en">has Other Legal Statement</rdfs:label>
        <rdfs:isDefinedBy rdf:resource="http://rs.tdwg.org/abcd/terms/"/>
        <dwcattributes:status>recommended</dwcattributes:status>
        <dcterms:issued>2019-01-31</dcterms:issued>
        <dcterms:modified>2019-01-31</dcterms:modified>
        <rdfs:comment>Connects an instance of a class to an associated Legal Statement that can not be expressed by abcd:hasLicense, abcd:hasAcknowledgement or abcd:hasSuggestedCitation such as disclaimers and usage restrictions.</rdfs:comment>
        <skos:definition>Connects an instance of a class to an associated Legal Statement that can not be expressed by abcd:hasLicense, abcd:hasAcknowledgement or abcd:hasSuggestedCitation such as disclaimers and usage restrictions.</skos:definition>
        <dc:description>To express which kind of information were withheld in the publication of the corresponding instance (e.g. removal of coordinates of threatened species) please use abcd:InformationWithheld.</dc:description>
        <rdfs:domain rdf:resource="http://www.w3.org/2002/07/owl#Thing"/>
        <rdfs:range rdf:resource="LegalStatement"/>
    </owl:ObjectProperty>

    <owl:ObjectProperty rdf:about="hasOwner">
        <rdfs:label xml:lang="en">has Owner</rdfs:label>
        <rdfs:isDefinedBy rdf:resource="http://rs.tdwg.org/abcd/terms/"/>
        <dwcattributes:status>recommended</dwcattributes:status>
        <dcterms:issued>2019-01-31</dcterms:issued>
        <dcterms:modified>2019-01-31</dcterms:modified>
        <rdfs:comment>Property to connect a class to a Contact acting as or representing the legal owner of it.</rdfs:comment>
        <skos:definition>Property to connect a class to a Contact acting as or representing the legal owner of it.</skos:definition>
        <rdfs:subPropertyOf rdf:resource="hasContact"/>
        <rdfs:domain rdf:resource="http://www.w3.org/2002/07/owl#Thing"/>
        <rdfs:range rdf:resource="Contact"/>
    </owl:ObjectProperty>

    <owl:ObjectProperty rdf:about="hasPermit">
        <rdfs:label xml:lang="en">has Permit</rdfs:label>
        <rdfs:isDefinedBy rdf:resource="http://rs.tdwg.org/abcd/terms/"/>
        <dwcattributes:status>recommended</dwcattributes:status>
        <dcterms:issued>2019-01-31</dcterms:issued>
        <dcterms:modified>2019-01-31</dcterms:modified>
        <rdfs:comment>Property to connect an instance of a class to a Permit.</rdfs:comment>
        <skos:definition>Property to connect an instance of a class to a Permit.</skos:definition>
        <rdfs:domain rdf:resource="http://www.w3.org/2002/07/owl#Thing"/>
        <rdfs:range rdf:resource="Permit"/>
    </owl:ObjectProperty>

    <owl:ObjectProperty rdf:about="hasPermitStatus">
        <rdfs:label xml:lang="en">has Permit Status</rdfs:label>
        <rdfs:isDefinedBy rdf:resource="http://rs.tdwg.org/abcd/terms/"/>
        <dwcattributes:status>recommended</dwcattributes:status>
        <dcterms:issued>2019-01-31</dcterms:issued>
        <dcterms:modified>2019-01-31</dcterms:modified>
        <rdfs:comment>Property to connect a Permit to a Permit Status. Material collected after 2014-10-12 cannot be in "Unknown" Permit Status!</rdfs:comment>
        <skos:definition>Property to connect a Permit to a Permit Status. Material collected after 2014-10-12 cannot be in "Unknown" Permit Status!</skos:definition>
        <rdfs:domain rdf:resource="Permit"/>
        <rdfs:range rdf:resource="PermitStatus"/>
    </owl:ObjectProperty>

    <owl:FunctionalProperty rdf:about="hasPermitStatus"/>

    <owl:ObjectProperty rdf:about="hasPermitType">
        <rdfs:label xml:lang="en">has Permit Type</rdfs:label>
        <rdfs:isDefinedBy rdf:resource="http://rs.tdwg.org/abcd/terms/"/>
        <dwcattributes:status>recommended</dwcattributes:status>
        <dcterms:issued>2019-01-31</dcterms:issued>
        <dcterms:modified>2019-01-31</dcterms:modified>
        <rdfs:comment>Property to connect a Permit to a Permit Type.</rdfs:comment>
        <skos:definition>Property to connect a Permit to a Permit Type.</skos:definition>
        <rdfs:domain rdf:resource="Permit"/>
        <rdfs:range rdf:resource="PermitType"/>
    </owl:ObjectProperty>

    <owl:FunctionalProperty rdf:about="hasPermitType"/>

    <owl:ObjectProperty rdf:about="hasPerson">
        <rdfs:label xml:lang="en">has Person</rdfs:label>
        <rdfs:isDefinedBy rdf:resource="http://rs.tdwg.org/abcd/terms/"/>
        <dwcattributes:status>recommended</dwcattributes:status>
        <dcterms:issued>2019-01-31</dcterms:issued>
        <dcterms:modified>2019-01-31</dcterms:modified>
        <rdfs:comment>Property to connect a class to a Person.</rdfs:comment>
        <skos:definition>Property to connect a class to a Person.</skos:definition>
        <rdfs:domain rdf:resource="http://www.w3.org/2002/07/owl#Thing"/>
        <rdfs:range rdf:resource="Person"/>
    </owl:ObjectProperty>

    <owl:ObjectProperty rdf:about="hasPlantingDate">
        <rdfs:label xml:lang="en">has Planting Date</rdfs:label>
        <rdfs:isDefinedBy rdf:resource="http://rs.tdwg.org/abcd/terms/"/>
        <dwcattributes:status>recommended</dwcattributes:status>
        <dcterms:issued>2019-01-31</dcterms:issued>
        <dcterms:modified>2019-01-31</dcterms:modified>
        <rdfs:comment>Property to connect a concept to the date it was planted.</rdfs:comment>
        <skos:definition>Property to connect a concept to the date it was planted.</skos:definition>
        <rdfs:subPropertyOf rdf:resource="hasDate"/>
        <rdfs:domain rdf:resource="http://www.w3.org/2002/07/owl#Thing"/>
        <rdfs:range rdf:resource="Date"/>
    </owl:ObjectProperty>

    <owl:ObjectProperty rdf:about="hasPreparation">
        <rdfs:label xml:lang="en">has Preparation</rdfs:label>
        <rdfs:isDefinedBy rdf:resource="http://rs.tdwg.org/abcd/terms/"/>
        <dwcattributes:status>recommended</dwcattributes:status>
        <dcterms:issued>2019-01-31</dcterms:issued>
        <dcterms:modified>2019-01-31</dcterms:modified>
        <rdfs:comment>Property to connect a concept to information about preparation.</rdfs:comment>
        <skos:definition>Property to connect a concept to information about preparation.</skos:definition>
        <rdfs:domain rdf:resource="http://www.w3.org/2002/07/owl#Thing"/>
        <rdfs:range rdf:resource="Preparation"/>
    </owl:ObjectProperty>

    <owl:ObjectProperty rdf:about="hasPreparationAgent">
        <rdfs:label xml:lang="en">has Preparation Agent</rdfs:label>
        <rdfs:isDefinedBy rdf:resource="http://rs.tdwg.org/abcd/terms/"/>
        <dwcattributes:status>recommended</dwcattributes:status>
        <dcterms:issued>2019-01-31</dcterms:issued>
        <dcterms:modified>2019-01-31</dcterms:modified>
        <rdfs:comment>Property to connect a preparation to the person and/or institution responsible for or effecting the preparation of the specimen.</rdfs:comment>
        <skos:definition>Property to connect a preparation to the person and/or institution responsible for or effecting the preparation of the specimen.</skos:definition>
        <rdfs:subPropertyOf rdf:resource="hasContact"/>
        <rdfs:domain rdf:resource="http://www.w3.org/2002/07/owl#Thing"/>
        <rdfs:range rdf:resource="Person"/>
    </owl:ObjectProperty>

    <owl:ObjectProperty rdf:about="hasPreservation">
        <rdfs:label xml:lang="en">has Preservation</rdfs:label>
        <rdfs:isDefinedBy rdf:resource="http://rs.tdwg.org/abcd/terms/"/>
        <dwcattributes:status>recommended</dwcattributes:status>
        <dcterms:issued>2019-01-31</dcterms:issued>
        <dcterms:modified>2019-01-31</dcterms:modified>
        <rdfs:comment>Property to connect a concept to a preservation.</rdfs:comment>
        <skos:definition>Property to connect a concept to a preservation.</skos:definition>
        <rdfs:domain rdf:resource="http://www.w3.org/2002/07/owl#Thing"/>
        <rdfs:range rdf:resource="Preservation"/>
    </owl:ObjectProperty>

    <owl:ObjectProperty rdf:about="hasPreviousUnit">
        <rdfs:label xml:lang="en">has Previous Unit</rdfs:label>
        <rdfs:isDefinedBy rdf:resource="http://rs.tdwg.org/abcd/terms/"/>
        <dwcattributes:status>recommended</dwcattributes:status>
        <dcterms:issued>2019-01-31</dcterms:issued>
        <dcterms:modified>2019-01-31</dcterms:modified>
        <rdfs:comment>Property to connect a unit to a predecessor.</rdfs:comment>
        <skos:definition>Property to connect a unit to a predecessor.</skos:definition>
        <rdfs:domain rdf:resource="http://www.w3.org/2002/07/owl#Thing"/>
        <rdfs:range rdf:resource="PreviousUnit"/>
    </owl:ObjectProperty>

    <owl:ObjectProperty rdf:about="hasProject">
        <rdfs:label xml:lang="en">has Project</rdfs:label>
        <rdfs:isDefinedBy rdf:resource="http://rs.tdwg.org/abcd/terms/"/>
        <dwcattributes:status>recommended</dwcattributes:status>
        <dcterms:issued>2019-01-31</dcterms:issued>
        <dcterms:modified>2019-01-31</dcterms:modified>
        <rdfs:comment>Property to connect an instance of a class to a Project.</rdfs:comment>
        <skos:definition>Property to connect an instance of a class to a Project.</skos:definition>
        <rdfs:domain rdf:resource="http://www.w3.org/2002/07/owl#Thing"/>
        <rdfs:range rdf:resource="Project"/>
    </owl:ObjectProperty>

    <owl:ObjectProperty rdf:about="hasRecordBasis">
        <rdfs:label xml:lang="en">has Record Basis</rdfs:label>
        <rdfs:isDefinedBy rdf:resource="http://rs.tdwg.org/abcd/terms/"/>
        <dwcattributes:status>recommended</dwcattributes:status>
        <dcterms:issued>2019-01-31</dcterms:issued>
        <dcterms:modified>2019-01-31</dcterms:modified>
        <rdfs:comment>Property to connect an instance of a class to a Record Basis.</rdfs:comment>
        <skos:definition>Property to connect an instance of a class to a Record Basis.</skos:definition>
        <rdfs:domain rdf:resource="http://www.w3.org/2002/07/owl#Thing"/>
        <rdfs:range rdf:resource="RecordBasis"/>
    </owl:ObjectProperty>

    <owl:ObjectProperty rdf:about="hasReference">
        <rdfs:label xml:lang="en">has Reference</rdfs:label>
        <rdfs:isDefinedBy rdf:resource="http://rs.tdwg.org/abcd/terms/"/>
        <dwcattributes:status>recommended</dwcattributes:status>
        <dcterms:issued>2019-01-31</dcterms:issued>
        <dcterms:modified>2019-01-31</dcterms:modified>
        <rdfs:comment>Property to connect an instance of a class to an associated Reference.</rdfs:comment>
        <skos:definition>Property to connect an instance of a class to an associated Reference.</skos:definition>
        <rdfs:domain rdf:resource="http://www.w3.org/2002/07/owl#Thing"/>
        <rdfs:range rdf:resource="Reference"/>
    </owl:ObjectProperty>

    <owl:ObjectProperty rdf:about="hasScientificName">
        <rdfs:label xml:lang="en">has Scientific Name</rdfs:label>
        <rdfs:isDefinedBy rdf:resource="http://rs.tdwg.org/abcd/terms/"/>
        <dwcattributes:status>recommended</dwcattributes:status>
        <dcterms:issued>2019-01-31</dcterms:issued>
        <dcterms:modified>2019-01-31</dcterms:modified>
        <rdfs:comment>Property to connect an Identified Taxon to its Scientific Name.</rdfs:comment>
        <skos:definition>Property to connect an Identified Taxon to its Scientific Name.</skos:definition>
        <rdfs:domain rdf:resource="http://www.w3.org/2002/07/owl#Thing"/>
        <rdfs:range rdf:resource="ScientificName"/>
    </owl:ObjectProperty>

    <owl:FunctionalProperty rdf:about="hasScientificName"/>

    <owl:ObjectProperty rdf:about="hasSequence">
        <rdfs:label xml:lang="en">has Sequence</rdfs:label>
        <rdfs:isDefinedBy rdf:resource="http://rs.tdwg.org/abcd/terms/"/>
        <dwcattributes:status>recommended</dwcattributes:status>
        <dcterms:issued>2019-01-31</dcterms:issued>
        <dcterms:modified>2019-01-31</dcterms:modified>
        <rdfs:comment>Property to connect an instance of a class to a genomic Sequence.</rdfs:comment>
        <skos:definition>Property to connect an instance of a class to a genomic Sequence.</skos:definition>
        <rdfs:domain rdf:resource="http://www.w3.org/2002/07/owl#Thing"/>
        <rdfs:range rdf:resource="Sequence"/>
    </owl:ObjectProperty>

    <owl:ObjectProperty rdf:about="hasSequencingAgent">
        <rdfs:label xml:lang="en">has Sequencing Agent</rdfs:label>
        <rdfs:isDefinedBy rdf:resource="http://rs.tdwg.org/abcd/terms/"/>
        <dwcattributes:status>recommended</dwcattributes:status>
        <dcterms:issued>2019-01-31</dcterms:issued>
        <dcterms:modified>2019-01-31</dcterms:modified>
        <rdfs:comment>Property to connect a Sequence to the responsible agent.</rdfs:comment>
        <skos:definition>Property to connect a Sequence to the responsible agent.</skos:definition>
        <rdfs:subPropertyOf rdf:resource="hasContact"/>
        <rdfs:domain rdf:resource="http://www.w3.org/2002/07/owl#Thing"/>
        <rdfs:range rdf:resource="Person"/>
    </owl:ObjectProperty>

    <owl:ObjectProperty rdf:about="hasSex">
        <rdfs:label xml:lang="en">has Sex</rdfs:label>
        <rdfs:isDefinedBy rdf:resource="http://rs.tdwg.org/abcd/terms/"/>
        <dwcattributes:status>recommended</dwcattributes:status>
        <dcterms:issued>2019-01-31</dcterms:issued>
        <dcterms:modified>2019-01-31</dcterms:modified>
        <rdfs:comment>Property to connect an instance of a class to a Sex.</rdfs:comment>
        <skos:definition>Property to connect an instance of a class to a Sex.</skos:definition>
        <rdfs:domain rdf:resource="http://www.w3.org/2002/07/owl#Thing"/>
        <rdfs:range rdf:resource="Sex"/>
        <skos:exactMatch rdf:resource="http://rs.tdwg.org/dwc/iri/sex"/>
    </owl:ObjectProperty>

    <owl:FunctionalProperty rdf:about="hasSex"/>

    <owl:ObjectProperty rdf:about="hasSourceReference">
        <rdfs:label xml:lang="en">has Source Reference</rdfs:label>
        <rdfs:isDefinedBy rdf:resource="http://rs.tdwg.org/abcd/terms/"/>
        <dwcattributes:status>recommended</dwcattributes:status>
        <dcterms:issued>2019-01-31</dcterms:issued>
        <dcterms:modified>2019-01-31</dcterms:modified>
        <rdfs:comment>Property to connect an instance of a class to  a reference to the source of the information connected to it. This is usually the published reference from where the information originated.</rdfs:comment>
        <skos:definition>Property to connect an instance of a class to  a reference to the source of the information connected to it. This is usually the published reference from where the information originated.</skos:definition>
        <rdfs:subPropertyOf rdf:resource="hasReference"/>
        <rdfs:domain rdf:resource="http://www.w3.org/2002/07/owl#Thing"/>
        <rdfs:range rdf:resource="Reference"/>
    </owl:ObjectProperty>

    <owl:FunctionalProperty rdf:about="hasSourceReference"/>

    <owl:ObjectProperty rdf:about="hasStratigraphicTerm">
        <rdfs:label xml:lang="en">has Stratigraphic Term</rdfs:label>
        <rdfs:isDefinedBy rdf:resource="http://rs.tdwg.org/abcd/terms/"/>
        <dwcattributes:status>recommended</dwcattributes:status>
        <dcterms:issued>2019-01-31</dcterms:issued>
        <dcterms:modified>2019-01-31</dcterms:modified>
        <rdfs:comment>Property to connect an instance of a class to a stratigraphic term.</rdfs:comment>
        <skos:definition>Property to connect an instance of a class to a stratigraphic term.</skos:definition>
        <rdfs:domain rdf:resource="http://www.w3.org/2002/07/owl#Thing"/>
        <rdfs:range rdf:resource="StratigraphicTerm"/>
    </owl:ObjectProperty>

    <owl:ObjectProperty rdf:about="hasSuggestedCitation">
        <rdfs:label xml:lang="en">has Suggested Citation</rdfs:label>
        <rdfs:isDefinedBy rdf:resource="http://rs.tdwg.org/abcd/terms/"/>
        <dwcattributes:status>recommended</dwcattributes:status>
        <dcterms:issued>2019-01-31</dcterms:issued>
        <dcterms:modified>2019-01-31</dcterms:modified>
        <rdfs:comment>Property to connect an instance of a class to a citation indicating how the instance should be attributed when cited externally.</rdfs:comment>
        <skos:definition>Property to connect an instance of a class to a citation indicating how the instance should be attributed when cited externally.</skos:definition>
        <rdfs:subPropertyOf rdf:resource="hasReference"/>
        <rdfs:domain rdf:resource="http://www.w3.org/2002/07/owl#Thing"/>
        <rdfs:range rdf:resource="Reference"/>
        <skos:exactMatch rdf:resource="http://purl.org/dc/terms/bibliographicCitation"/>
    </owl:ObjectProperty>

    <owl:ObjectProperty rdf:about="hasSynecology">
        <rdfs:label xml:lang="en">has Synecology</rdfs:label>
        <rdfs:isDefinedBy rdf:resource="http://rs.tdwg.org/abcd/terms/"/>
        <dwcattributes:status>recommended</dwcattributes:status>
        <dcterms:issued>2019-01-31</dcterms:issued>
        <dcterms:modified>2019-01-31</dcterms:modified>
        <rdfs:comment>Property to connect an instance of a class to a Synecology.</rdfs:comment>
        <skos:definition>Property to connect an instance of a class to a Synecology.</skos:definition>
        <rdfs:domain rdf:resource="http://www.w3.org/2002/07/owl#Thing"/>
        <rdfs:range rdf:resource="Synecology"/>
    </owl:ObjectProperty>

    <owl:ObjectProperty rdf:about="hasTaxonInBackground">
        <rdfs:label xml:lang="en">has Taxon In Background</rdfs:label>
        <rdfs:isDefinedBy rdf:resource="http://rs.tdwg.org/abcd/terms/"/>
        <dwcattributes:status>recommended</dwcattributes:status>
        <rdfs:comment>a property to denote a taxon in the background of a multimedia object</rdfs:comment>
        <skos:definition>a property to denote a taxon in the background of a multimedia object</skos:definition>
        <rdfs:subPropertyOf rdf:resource="hasIdentifiedTaxon"/>
        <rdfs:domain rdf:resource="http://www.w3.org/2002/07/owl#Thing"/>
        <rdfs:range rdf:resource="IdentifiedTaxon"/>
    </owl:ObjectProperty>

    <owl:ObjectProperty rdf:about="hasTechnicalContact">
        <rdfs:label xml:lang="en">has Technical Contact</rdfs:label>
        <rdfs:isDefinedBy rdf:resource="http://rs.tdwg.org/abcd/terms/"/>
        <dwcattributes:status>recommended</dwcattributes:status>
        <dcterms:issued>2019-01-31</dcterms:issued>
        <dcterms:modified>2019-01-31</dcterms:modified>
        <rdfs:comment>Property to connect an instance of a class to a Contact that is responsible for technical issues in its context.</rdfs:comment>
        <skos:definition>Property to connect an instance of a class to a Contact that is responsible for technical issues in its context.</skos:definition>
        <rdfs:subPropertyOf rdf:resource="hasContact"/>
        <dc:description>In context of datasets the technical contact normally is the agent acting as the publisher of the dataset in the network.</dc:description>
        <rdfs:domain rdf:resource="http://www.w3.org/2002/07/owl#Thing"/>
        <rdfs:range rdf:resource="Contact"/>
    </owl:ObjectProperty>

    <owl:ObjectProperty rdf:about="hasTemperature">
        <rdfs:label xml:lang="en">has Temperature</rdfs:label>
        <rdfs:isDefinedBy rdf:resource="http://rs.tdwg.org/abcd/terms/"/>
        <dwcattributes:status>recommended</dwcattributes:status>
        <dcterms:issued>2019-01-31</dcterms:issued>
        <dcterms:modified>2019-01-31</dcterms:modified>
        <rdfs:comment>Property to connect a concept to a temperature.</rdfs:comment>
        <skos:definition>Property to connect a concept to a temperature.</skos:definition>
        <rdfs:domain rdf:resource="http://www.w3.org/2002/07/owl#Thing"/>
        <rdfs:range rdf:resource="Temperature"/>
    </owl:ObjectProperty>

    <owl:FunctionalProperty rdf:about="hasTemperature"/>

    <owl:ObjectProperty rdf:about="hasTemperatureScale">
        <rdfs:label xml:lang="en">has Temperature Scale</rdfs:label>
        <rdfs:isDefinedBy rdf:resource="http://rs.tdwg.org/abcd/terms/"/>
        <dwcattributes:status>recommended</dwcattributes:status>
        <dcterms:issued>2019-01-31</dcterms:issued>
        <dcterms:modified>2019-01-31</dcterms:modified>
        <rdfs:comment>Property to connect a temperature to the temperature scale it uses.</rdfs:comment>
        <skos:definition>Property to connect a temperature to the temperature scale it uses.</skos:definition>
        <rdfs:domain rdf:resource="http://www.w3.org/2002/07/owl#Thing"/>
        <rdfs:range rdf:resource="temperatureScale"/>
    </owl:ObjectProperty>

    <owl:FunctionalProperty rdf:about="hasTemperatureScale"/>

    <owl:ObjectProperty rdf:about="hasTypeSpecificInformation">
        <rdfs:label xml:lang="en">has Type Specific Information</rdfs:label>
        <rdfs:isDefinedBy rdf:resource="http://rs.tdwg.org/abcd/terms/"/>
        <dwcattributes:status>recommended</dwcattributes:status>
        <dcterms:issued>2019-01-31</dcterms:issued>
        <dcterms:modified>2019-01-31</dcterms:modified>
        <rdfs:comment>Property to connect an instance of a class to information specific to the type of the Unit.</rdfs:comment>
        <skos:definition>Property to connect an instance of a class to information specific to the type of the Unit.</skos:definition>
        <rdfs:domain rdf:resource="Unit"/>
        <rdfs:range rdf:resource="TypeSpecificInformation"/>
    </owl:ObjectProperty>

    <owl:FunctionalProperty rdf:about="hasTypeSpecificInformation"/>

    <owl:ObjectProperty rdf:about="hasTypifiedName">
        <rdfs:label xml:lang="en">has Typified Name</rdfs:label>
        <rdfs:isDefinedBy rdf:resource="http://rs.tdwg.org/abcd/terms/"/>
        <dwcattributes:status>recommended</dwcattributes:status>
        <dcterms:issued>2019-01-31</dcterms:issued>
        <dcterms:modified>2019-01-31</dcterms:modified>
        <rdfs:comment>Property to connect a Nomenclatural Type Designation to a scientific name as its typified name.</rdfs:comment>
        <skos:definition>Property to connect a Nomenclatural Type Designation to a scientific name as its typified name.</skos:definition>
        <rdfs:subPropertyOf rdf:resource="hasScientificName"/>
        <rdfs:domain rdf:resource="http://www.w3.org/2002/07/owl#Thing"/>
        <rdfs:range rdf:resource="ScientificName"/>
    </owl:ObjectProperty>

    <owl:ObjectProperty rdf:about="hasUnit">
        <rdfs:label xml:lang="en">has Unit</rdfs:label>
        <rdfs:isDefinedBy rdf:resource="http://rs.tdwg.org/abcd/terms/"/>
        <dwcattributes:status>recommended</dwcattributes:status>
        <dcterms:issued>2019-01-31</dcterms:issued>
        <dcterms:modified>2019-01-31</dcterms:modified>
        <rdfs:comment>A property that connects an instance of a class to a Unit.</rdfs:comment>
        <skos:definition>A property that connects an instance of a class to a Unit.</skos:definition>
        <rdfs:domain rdf:resource="http://www.w3.org/2002/07/owl#Thing"/>
        <rdfs:range rdf:resource="Unit"/>
    </owl:ObjectProperty>

    <owl:ObjectProperty rdf:about="hasUnitReference">
        <rdfs:label xml:lang="en">has Unit Reference</rdfs:label>
        <rdfs:isDefinedBy rdf:resource="http://rs.tdwg.org/abcd/terms/"/>
        <dwcattributes:status>recommended</dwcattributes:status>
        <dcterms:issued>2019-01-31</dcterms:issued>
        <dcterms:modified>2019-01-31</dcterms:modified>
        <rdfs:comment>Property to connect a Unit to a published Reference citing it.</rdfs:comment>
        <skos:definition>Property to connect a Unit to a published Reference citing it.</skos:definition>
        <rdfs:subPropertyOf rdf:resource="hasReference"/>
        <dc:description>To cite the reference the information of the Unit came from, please  use abcd:hasSourceReference instead.</dc:description>
        <rdfs:domain rdf:resource="http://www.w3.org/2002/07/owl#Thing"/>
        <rdfs:range rdf:resource="Reference"/>
    </owl:ObjectProperty>

    <owl:ObjectProperty rdf:about="hasVerificationDate">
        <rdfs:label xml:lang="en">has Verification Date</rdfs:label>
        <rdfs:isDefinedBy rdf:resource="http://rs.tdwg.org/abcd/terms/"/>
        <dwcattributes:status>recommended</dwcattributes:status>
        <dcterms:issued>2019-01-31</dcterms:issued>
        <dcterms:modified>2019-01-31</dcterms:modified>
        <rdfs:comment>Property to connect a concept to a date of verification.</rdfs:comment>
        <skos:definition>Property to connect a concept to a date of verification.</skos:definition>
        <rdfs:subPropertyOf rdf:resource="hasDate"/>
        <rdfs:domain rdf:resource="http://www.w3.org/2002/07/owl#Thing"/>
        <rdfs:range rdf:resource="Date"/>
    </owl:ObjectProperty>

    <owl:ObjectProperty rdf:about="hasVerifier">
        <rdfs:label xml:lang="en">has Verifier</rdfs:label>
        <rdfs:isDefinedBy rdf:resource="http://rs.tdwg.org/abcd/terms/"/>
        <dwcattributes:status>recommended</dwcattributes:status>
        <dcterms:issued>2019-01-31</dcterms:issued>
        <dcterms:modified>2019-01-31</dcterms:modified>
        <rdfs:comment>Property to connect a concept to a person as its verifier.</rdfs:comment>
        <skos:definition>Property to connect a concept to a person as its verifier.</skos:definition>
        <rdfs:subPropertyOf rdf:resource="hasPerson"/>
        <rdfs:domain rdf:resource="http://www.w3.org/2002/07/owl#Thing"/>
        <rdfs:range rdf:resource="Person"/>
    </owl:ObjectProperty>

    <owl:ObjectProperty rdf:about="hasVersion">
        <rdfs:label xml:lang="en">has Version</rdfs:label>
        <rdfs:isDefinedBy rdf:resource="http://rs.tdwg.org/abcd/terms/"/>
        <dwcattributes:status>recommended</dwcattributes:status>
        <dcterms:issued>2019-01-31</dcterms:issued>
        <dcterms:modified>2019-01-31</dcterms:modified>
        <rdfs:comment>Connects an instance of a class to its version.</rdfs:comment>
        <skos:definition>Connects an instance of a class to its version.</skos:definition>
        <rdfs:domain rdf:resource="http://www.w3.org/2002/07/owl#Thing"/>
        <rdfs:range rdf:resource="Version"/>
    </owl:ObjectProperty>

    <owl:FunctionalProperty rdf:about="hasVersion"/>

    <owl:ObjectProperty rdf:about="wasAcquiredFrom">
        <rdfs:label xml:lang="en">was Acquired From</rdfs:label>
        <rdfs:isDefinedBy rdf:resource="http://rs.tdwg.org/abcd/terms/"/>
        <dwcattributes:status>recommended</dwcattributes:status>
        <dcterms:issued>2019-01-31</dcterms:issued>
        <dcterms:modified>2019-01-31</dcterms:modified>
        <rdfs:comment>Property to connect a concept to the contact it was acquired from.</rdfs:comment>
        <skos:definition>Property to connect a concept to the contact it was acquired from.</skos:definition>
        <rdfs:domain rdf:resource="http://www.w3.org/2002/07/owl#Thing"/>
        <rdfs:range rdf:resource="Contact"/>
    </owl:ObjectProperty>

    <abcd:HigherTaxonRank rdf:about="regnum">
        <rdfs:isDefinedBy rdf:resource="http://rs.tdwg.org/abcd/terms/"/>
        <dwcattributes:status>recommended</dwcattributes:status>
        <dcterms:issued>2019-01-31</dcterms:issued>
        <dcterms:modified>2019-01-31</dcterms:modified>
        <rdfs:comment>Higher Taxon Rank for the kingdom (lat. regnum).</rdfs:comment>
        <skos:definition>Higher Taxon Rank for the kingdom (lat. regnum).</skos:definition>
    </abcd:HigherTaxonRank>

    <abcd:HigherTaxonRank rdf:about="subregnum">
        <rdfs:isDefinedBy rdf:resource="http://rs.tdwg.org/abcd/terms/"/>
        <dwcattributes:status>recommended</dwcattributes:status>
        <dcterms:issued>2019-01-31</dcterms:issued>
        <dcterms:modified>2019-01-31</dcterms:modified>
        <rdfs:comment>Higher Taxon Rank for the subkingdom (lat. subregnum).</rdfs:comment>
        <skos:definition>Higher Taxon Rank for the subkingdom (lat. subregnum).</skos:definition>
    </abcd:HigherTaxonRank>

    <abcd:HigherTaxonRank rdf:about="superphylum">
        <rdfs:isDefinedBy rdf:resource="http://rs.tdwg.org/abcd/terms/"/>
        <dwcattributes:status>recommended</dwcattributes:status>
        <dcterms:issued>2019-01-31</dcterms:issued>
        <dcterms:modified>2019-01-31</dcterms:modified>
        <rdfs:comment>Higher Taxon Rank for the superphylum (or Superdivision in Botany).</rdfs:comment>
        <skos:definition>Higher Taxon Rank for the superphylum (or Superdivision in Botany).</skos:definition>
    </abcd:HigherTaxonRank>

    <abcd:HigherTaxonRank rdf:about="phylum">
        <rdfs:isDefinedBy rdf:resource="http://rs.tdwg.org/abcd/terms/"/>
        <dwcattributes:status>recommended</dwcattributes:status>
        <dcterms:issued>2019-01-31</dcterms:issued>
        <dcterms:modified>2019-01-31</dcterms:modified>
        <rdfs:comment>Higher Taxon Rank for the Phylum (or Division in Botany).</rdfs:comment>
        <skos:definition>Higher Taxon Rank for the Phylum (or Division in Botany).</skos:definition>
    </abcd:HigherTaxonRank>

    <abcd:HigherTaxonRank rdf:about="subphylum">
        <rdfs:isDefinedBy rdf:resource="http://rs.tdwg.org/abcd/terms/"/>
        <dwcattributes:status>recommended</dwcattributes:status>
        <dcterms:issued>2019-01-31</dcterms:issued>
        <dcterms:modified>2019-01-31</dcterms:modified>
        <rdfs:comment>Higher Taxon Rank for the subphylum (or Subdivision in Botany).</rdfs:comment>
        <skos:definition>Higher Taxon Rank for the subphylum (or Subdivision in Botany).</skos:definition>
    </abcd:HigherTaxonRank>

    <abcd:HigherTaxonRank rdf:about="superclassis">
        <rdfs:isDefinedBy rdf:resource="http://rs.tdwg.org/abcd/terms/"/>
        <dwcattributes:status>recommended</dwcattributes:status>
        <dcterms:issued>2019-01-31</dcterms:issued>
        <dcterms:modified>2019-01-31</dcterms:modified>
        <rdfs:comment>Higher Taxon Rank for the superclass (lat. superclassis).</rdfs:comment>
        <skos:definition>Higher Taxon Rank for the superclass (lat. superclassis).</skos:definition>
    </abcd:HigherTaxonRank>

    <abcd:HigherTaxonRank rdf:about="classis">
        <rdfs:isDefinedBy rdf:resource="http://rs.tdwg.org/abcd/terms/"/>
        <dwcattributes:status>recommended</dwcattributes:status>
        <dcterms:issued>2019-01-31</dcterms:issued>
        <dcterms:modified>2019-01-31</dcterms:modified>
        <rdfs:comment>Higher Taxon Rank for the class (lat. classis).</rdfs:comment>
        <skos:definition>Higher Taxon Rank for the class (lat. classis).</skos:definition>
    </abcd:HigherTaxonRank>

    <abcd:HigherTaxonRank rdf:about="subclassis">
        <rdfs:isDefinedBy rdf:resource="http://rs.tdwg.org/abcd/terms/"/>
        <dwcattributes:status>recommended</dwcattributes:status>
        <dcterms:issued>2019-01-31</dcterms:issued>
        <dcterms:modified>2019-01-31</dcterms:modified>
        <rdfs:comment>Higher Taxon Rank for the subclass (lat. subclassis).</rdfs:comment>
        <skos:definition>Higher Taxon Rank for the subclass (lat. subclassis).</skos:definition>
    </abcd:HigherTaxonRank>

    <abcd:HigherTaxonRank rdf:about="supercohors">
        <rdfs:isDefinedBy rdf:resource="http://rs.tdwg.org/abcd/terms/"/>
        <dwcattributes:status>recommended</dwcattributes:status>
        <dcterms:issued>2019-01-31</dcterms:issued>
        <dcterms:modified>2019-01-31</dcterms:modified>
        <rdfs:comment>Higher Taxon Rank for the supercohort (lat. supercohors).</rdfs:comment>
        <skos:definition>Higher Taxon Rank for the supercohort (lat. supercohors).</skos:definition>
    </abcd:HigherTaxonRank>

    <abcd:HigherTaxonRank rdf:about="cohors">
        <rdfs:isDefinedBy rdf:resource="http://rs.tdwg.org/abcd/terms/"/>
        <dwcattributes:status>recommended</dwcattributes:status>
        <dcterms:issued>2019-01-31</dcterms:issued>
        <dcterms:modified>2019-01-31</dcterms:modified>
        <rdfs:comment>Higher Taxon Rank for the outdated rank of cohort (lat. cohors).</rdfs:comment>
        <skos:definition>Higher Taxon Rank for the outdated rank of cohort (lat. cohors).</skos:definition>
    </abcd:HigherTaxonRank>

    <abcd:HigherTaxonRank rdf:about="subcohors">
        <rdfs:isDefinedBy rdf:resource="http://rs.tdwg.org/abcd/terms/"/>
        <dwcattributes:status>recommended</dwcattributes:status>
        <dcterms:issued>2019-01-31</dcterms:issued>
        <dcterms:modified>2019-01-31</dcterms:modified>
        <rdfs:comment>Higher Taxon Rank for the subcohort (lat. subcohors).</rdfs:comment>
        <skos:definition>Higher Taxon Rank for the subcohort (lat. subcohors).</skos:definition>
    </abcd:HigherTaxonRank>

    <abcd:HigherTaxonRank rdf:about="superordo">
        <rdfs:isDefinedBy rdf:resource="http://rs.tdwg.org/abcd/terms/"/>
        <dwcattributes:status>recommended</dwcattributes:status>
        <dcterms:issued>2019-01-31</dcterms:issued>
        <dcterms:modified>2019-01-31</dcterms:modified>
        <rdfs:comment>Higher Taxon Rank for the superorder (lat. superordo).</rdfs:comment>
        <skos:definition>Higher Taxon Rank for the superorder (lat. superordo).</skos:definition>
    </abcd:HigherTaxonRank>

    <abcd:HigherTaxonRank rdf:about="ordo">
        <rdfs:isDefinedBy rdf:resource="http://rs.tdwg.org/abcd/terms/"/>
        <dwcattributes:status>recommended</dwcattributes:status>
        <dcterms:issued>2019-01-31</dcterms:issued>
        <dcterms:modified>2019-01-31</dcterms:modified>
        <rdfs:comment>Higher Taxon Rank for the order (lat. ordo).</rdfs:comment>
        <skos:definition>Higher Taxon Rank for the order (lat. ordo).</skos:definition>
    </abcd:HigherTaxonRank>

    <abcd:HigherTaxonRank rdf:about="subordo">
        <rdfs:isDefinedBy rdf:resource="http://rs.tdwg.org/abcd/terms/"/>
        <dwcattributes:status>recommended</dwcattributes:status>
        <dcterms:issued>2019-01-31</dcterms:issued>
        <dcterms:modified>2019-01-31</dcterms:modified>
        <rdfs:comment>Higher Taxon Rank for the suborder (lat. subordo).</rdfs:comment>
        <skos:definition>Higher Taxon Rank for the suborder (lat. subordo).</skos:definition>
    </abcd:HigherTaxonRank>

    <abcd:HigherTaxonRank rdf:about="superfamilia">
        <rdfs:isDefinedBy rdf:resource="http://rs.tdwg.org/abcd/terms/"/>
        <dwcattributes:status>recommended</dwcattributes:status>
        <dcterms:issued>2019-01-31</dcterms:issued>
        <dcterms:modified>2019-01-31</dcterms:modified>
        <rdfs:comment>Higher Taxon Rank for the superfamily (lat. superfamilia).</rdfs:comment>
        <skos:definition>Higher Taxon Rank for the superfamily (lat. superfamilia).</skos:definition>
    </abcd:HigherTaxonRank>

    <abcd:HigherTaxonRank rdf:about="familia">
        <rdfs:isDefinedBy rdf:resource="http://rs.tdwg.org/abcd/terms/"/>
        <dwcattributes:status>recommended</dwcattributes:status>
        <dcterms:issued>2019-01-31</dcterms:issued>
        <dcterms:modified>2019-01-31</dcterms:modified>
        <rdfs:comment>Higher Taxon Rank for the family (lat. familia)</rdfs:comment>
        <skos:definition>Higher Taxon Rank for the family (lat. familia)</skos:definition>
    </abcd:HigherTaxonRank>

    <abcd:HigherTaxonRank rdf:about="subfamilia">
        <rdfs:isDefinedBy rdf:resource="http://rs.tdwg.org/abcd/terms/"/>
        <dwcattributes:status>recommended</dwcattributes:status>
        <dcterms:issued>2019-01-31</dcterms:issued>
        <dcterms:modified>2019-01-31</dcterms:modified>
        <rdfs:comment>Higher Taxon Rank for the subfamily (lat. subfamilia).</rdfs:comment>
        <skos:definition>Higher Taxon Rank for the subfamily (lat. subfamilia).</skos:definition>
    </abcd:HigherTaxonRank>

    <abcd:HigherTaxonRank rdf:about="tribus">
        <rdfs:isDefinedBy rdf:resource="http://rs.tdwg.org/abcd/terms/"/>
        <dwcattributes:status>recommended</dwcattributes:status>
        <dcterms:issued>2019-01-31</dcterms:issued>
        <dcterms:modified>2019-01-31</dcterms:modified>
        <rdfs:comment>Higher Taxon Rank for the tribe (lat. tribus).</rdfs:comment>
        <skos:definition>Higher Taxon Rank for the tribe (lat. tribus).</skos:definition>
    </abcd:HigherTaxonRank>

    <abcd:HigherTaxonRank rdf:about="genusgroup">
        <rdfs:isDefinedBy rdf:resource="http://rs.tdwg.org/abcd/terms/"/>
        <dwcattributes:status>recommended</dwcattributes:status>
        <dcterms:issued>2019-01-31</dcterms:issued>
        <dcterms:modified>2019-01-31</dcterms:modified>
        <rdfs:comment>Higher Taxon Rank element  for Higher Taxon Names that are in an unspecified genus-group in Zoology.</rdfs:comment>
        <skos:definition>Higher Taxon Rank element  for Higher Taxon Names that are in an unspecified genus-group in Zoology.</skos:definition>
    </abcd:HigherTaxonRank>

    <abcd:HigherTaxonRank rdf:about="unranked">
        <rdfs:isDefinedBy rdf:resource="http://rs.tdwg.org/abcd/terms/"/>
        <dwcattributes:status>recommended</dwcattributes:status>
        <dcterms:issued>2019-01-31</dcterms:issued>
        <dcterms:modified>2019-01-31</dcterms:modified>
        <rdfs:comment>Higher Taxon Rank element for Higher Taxon Names that are unranked.</rdfs:comment>
        <skos:definition>Higher Taxon Rank element for Higher Taxon Names that are unranked.</skos:definition>
    </abcd:HigherTaxonRank>

    <abcd:BotanicalTaxonRank rdf:about="subgen.">
        <rdfs:isDefinedBy rdf:resource="http://rs.tdwg.org/abcd/terms/"/>
        <dwcattributes:status>recommended</dwcattributes:status>
        <dcterms:issued>2019-01-31</dcterms:issued>
        <dcterms:modified>2019-01-31</dcterms:modified>
        <rdfs:comment>Abbreviation for the botanical taxonomic rank subgenus.</rdfs:comment>
        <skos:definition>Abbreviation for the botanical taxonomic rank subgenus.</skos:definition>
    </abcd:BotanicalTaxonRank>

    <abcd:BotanicalTaxonRank rdf:about="sect.">
        <rdfs:isDefinedBy rdf:resource="http://rs.tdwg.org/abcd/terms/"/>
        <dwcattributes:status>recommended</dwcattributes:status>
        <dcterms:issued>2019-01-31</dcterms:issued>
        <dcterms:modified>2019-01-31</dcterms:modified>
        <rdfs:comment>Abbreviation for the botanical taxonomic rank section (lat: sectio).</rdfs:comment>
        <skos:definition>Abbreviation for the botanical taxonomic rank section (lat: sectio).</skos:definition>
    </abcd:BotanicalTaxonRank>

    <abcd:BotanicalTaxonRank rdf:about="subsp.">
        <rdfs:isDefinedBy rdf:resource="http://rs.tdwg.org/abcd/terms/"/>
        <dwcattributes:status>recommended</dwcattributes:status>
        <dcterms:issued>2019-01-31</dcterms:issued>
        <dcterms:modified>2019-01-31</dcterms:modified>
        <rdfs:comment>Abbreviation for the botanical taxonomic rank subspecies.</rdfs:comment>
        <skos:definition>Abbreviation for the botanical taxonomic rank subspecies.</skos:definition>
    </abcd:BotanicalTaxonRank>

    <abcd:BotanicalTaxonRank rdf:about="var.">
        <rdfs:isDefinedBy rdf:resource="http://rs.tdwg.org/abcd/terms/"/>
        <dwcattributes:status>recommended</dwcattributes:status>
        <dcterms:issued>2019-01-31</dcterms:issued>
        <dcterms:modified>2019-01-31</dcterms:modified>
        <rdfs:comment>Abbreviation for the botanical taxonomic rank variety (lat: varietas).</rdfs:comment>
        <skos:definition>Abbreviation for the botanical taxonomic rank variety (lat: varietas).</skos:definition>
    </abcd:BotanicalTaxonRank>

    <abcd:BotanicalTaxonRank rdf:about="subvar.">
        <rdfs:isDefinedBy rdf:resource="http://rs.tdwg.org/abcd/terms/"/>
        <dwcattributes:status>recommended</dwcattributes:status>
        <dcterms:issued>2019-01-31</dcterms:issued>
        <dcterms:modified>2019-01-31</dcterms:modified>
        <rdfs:comment>Abbreviation for the botanical taxonomic rank subvariety (lat: subvarietas).</rdfs:comment>
        <skos:definition>Abbreviation for the botanical taxonomic rank subvariety (lat: subvarietas).</skos:definition>
    </abcd:BotanicalTaxonRank>

    <abcd:BotanicalTaxonRank rdf:about="forma">
        <rdfs:isDefinedBy rdf:resource="http://rs.tdwg.org/abcd/terms/"/>
        <dwcattributes:status>recommended</dwcattributes:status>
        <dcterms:issued>2019-01-31</dcterms:issued>
        <dcterms:modified>2019-01-31</dcterms:modified>
        <rdfs:comment>Latin name for the botanical taxonomic rank form (abbr.: f.).</rdfs:comment>
        <skos:definition>Latin name for the botanical taxonomic rank form (abbr.: f.).</skos:definition>
    </abcd:BotanicalTaxonRank>

    <abcd:BotanicalTaxonRank rdf:about="f.">
        <rdfs:isDefinedBy rdf:resource="http://rs.tdwg.org/abcd/terms/"/>
        <dwcattributes:status>recommended</dwcattributes:status>
        <dcterms:issued>2019-01-31</dcterms:issued>
        <dcterms:modified>2019-01-31</dcterms:modified>
        <rdfs:comment>Abbreviation for the botanical taxonomic rank form (lat: forma).</rdfs:comment>
        <skos:definition>Abbreviation for the botanical taxonomic rank form (lat: forma).</skos:definition>
    </abcd:BotanicalTaxonRank>

    <abcd:BotanicalTaxonRank rdf:about="subforma">
        <rdfs:isDefinedBy rdf:resource="http://rs.tdwg.org/abcd/terms/"/>
        <dwcattributes:status>recommended</dwcattributes:status>
        <dcterms:issued>2019-01-31</dcterms:issued>
        <dcterms:modified>2019-01-31</dcterms:modified>
        <rdfs:comment>Latin name for the botanical taxonomic rank subform (abbr.: subf.).</rdfs:comment>
        <skos:definition>Latin name for the botanical taxonomic rank subform (abbr.: subf.).</skos:definition>
    </abcd:BotanicalTaxonRank>

    <abcd:BotanicalTaxonRank rdf:about="subf.">
        <rdfs:isDefinedBy rdf:resource="http://rs.tdwg.org/abcd/terms/"/>
        <dwcattributes:status>recommended</dwcattributes:status>
        <dcterms:issued>2019-01-31</dcterms:issued>
        <dcterms:modified>2019-01-31</dcterms:modified>
        <rdfs:comment>Abbreviation for the botanical taxonomic rank subform (lat: subforma).</rdfs:comment>
        <skos:definition>Abbreviation for the botanical taxonomic rank subform (lat: subforma).</skos:definition>
    </abcd:BotanicalTaxonRank>

    <abcd:BotanicalTaxonRank rdf:about="f.spec.">
        <rdfs:isDefinedBy rdf:resource="http://rs.tdwg.org/abcd/terms/"/>
        <dwcattributes:status>recommended</dwcattributes:status>
        <dcterms:issued>2019-01-31</dcterms:issued>
        <dcterms:modified>2019-01-31</dcterms:modified>
        <rdfs:comment>Abbreviation for the botanical taxonomic rank form species (lat: forma species).</rdfs:comment>
        <skos:definition>Abbreviation for the botanical taxonomic rank form species (lat: forma species).</skos:definition>
    </abcd:BotanicalTaxonRank>

    <abcd:NomenclatureCode rdf:about="Bacteriological">
        <rdfs:isDefinedBy rdf:resource="http://rs.tdwg.org/abcd/terms/"/>
        <dwcattributes:status>recommended</dwcattributes:status>
        <dcterms:issued>2019-01-31</dcterms:issued>
        <dcterms:modified>2019-01-31</dcterms:modified>
        <rdfs:comment>Nomenclature Code: Bacteriological.</rdfs:comment>
        <skos:definition>Nomenclature Code: Bacteriological.</skos:definition>
    </abcd:NomenclatureCode>

    <abcd:NomenclatureCode rdf:about="Botanical">
        <rdfs:isDefinedBy rdf:resource="http://rs.tdwg.org/abcd/terms/"/>
        <dwcattributes:status>recommended</dwcattributes:status>
        <dcterms:issued>2019-01-31</dcterms:issued>
        <dcterms:modified>2019-01-31</dcterms:modified>
        <rdfs:comment>Nomenclature Code: Botanical.</rdfs:comment>
        <skos:definition>Nomenclature Code: Botanical.</skos:definition>
    </abcd:NomenclatureCode>

    <abcd:NomenclatureCode rdf:about="Viral">
        <rdfs:isDefinedBy rdf:resource="http://rs.tdwg.org/abcd/terms/"/>
        <dwcattributes:status>recommended</dwcattributes:status>
        <dcterms:issued>2019-01-31</dcterms:issued>
        <dcterms:modified>2019-01-31</dcterms:modified>
        <rdfs:comment>Nomenclature Code: Viral.</rdfs:comment>
        <skos:definition>Nomenclature Code: Viral.</skos:definition>
    </abcd:NomenclatureCode>

    <abcd:NomenclatureCode rdf:about="Zoological">
        <rdfs:isDefinedBy rdf:resource="http://rs.tdwg.org/abcd/terms/"/>
        <dwcattributes:status>recommended</dwcattributes:status>
        <dcterms:issued>2019-01-31</dcterms:issued>
        <dcterms:modified>2019-01-31</dcterms:modified>
        <rdfs:comment>Nomenclature Code: Zoological.</rdfs:comment>
        <skos:definition>Nomenclature Code: Zoological.</skos:definition>
    </abcd:NomenclatureCode>

    <abcd:NomenclatureCode rdf:about="Cultivated">
        <rdfs:isDefinedBy rdf:resource="http://rs.tdwg.org/abcd/terms/"/>
        <dwcattributes:status>recommended</dwcattributes:status>
        <dcterms:issued>2019-01-31</dcterms:issued>
        <dcterms:modified>2019-01-31</dcterms:modified>
        <rdfs:comment>Nomenclature Code: Cultivated.</rdfs:comment>
        <skos:definition>Nomenclature Code: Cultivated.</skos:definition>
    </abcd:NomenclatureCode>

    <abcd:temperatureScale rdf:about="Celsius">
        <rdfs:isDefinedBy rdf:resource="http://rs.tdwg.org/abcd/terms/"/>
        <dwcattributes:status>recommended</dwcattributes:status>
        <dcterms:issued>2019-01-31</dcterms:issued>
        <dcterms:modified>2019-01-31</dcterms:modified>
        <rdfs:comment>Temperature Scale Celsius for expressing temperatures in &#176;C.</rdfs:comment>
        <skos:definition>Temperature Scale Celsius for expressing temperatures in &#176;C.</skos:definition>
    </abcd:temperatureScale>

    <abcd:temperatureScale rdf:about="Fahrenheit">
        <rdfs:isDefinedBy rdf:resource="http://rs.tdwg.org/abcd/terms/"/>
        <dwcattributes:status>recommended</dwcattributes:status>
        <dcterms:issued>2019-01-31</dcterms:issued>
        <dcterms:modified>2019-01-31</dcterms:modified>
        <rdfs:comment>Temperature Scale Fahrenheit for expressing temperatures in &#176;F.</rdfs:comment>
        <skos:definition>Temperature Scale Fahrenheit for expressing temperatures in &#176;F.</skos:definition>
    </abcd:temperatureScale>

    <abcd:temperatureScale rdf:about="Kelvin">
        <rdfs:isDefinedBy rdf:resource="http://rs.tdwg.org/abcd/terms/"/>
        <dwcattributes:status>recommended</dwcattributes:status>
        <dcterms:issued>2019-01-31</dcterms:issued>
        <dcterms:modified>2019-01-31</dcterms:modified>
        <rdfs:comment>Temperature Scale Kelvin for expressing temperatures in K.</rdfs:comment>
        <skos:definition>Temperature Scale Kelvin for expressing temperatures in K.</skos:definition>
    </abcd:temperatureScale>

    <abcd:RecordBasis rdf:about="PreservedSpecimen">
        <rdfs:isDefinedBy rdf:resource="http://rs.tdwg.org/abcd/terms/"/>
        <dwcattributes:status>recommended</dwcattributes:status>
        <dcterms:issued>2019-01-31</dcterms:issued>
        <dcterms:modified>2019-01-31</dcterms:modified>
        <rdfs:comment>A record describing a preserved specimen (not living).</rdfs:comment>
        <skos:definition>A record describing a preserved specimen (not living).</skos:definition>
    </abcd:RecordBasis>

    <abcd:RecordBasis rdf:about="LivingSpecimen">
        <rdfs:isDefinedBy rdf:resource="http://rs.tdwg.org/abcd/terms/"/>
        <dwcattributes:status>recommended</dwcattributes:status>
        <dcterms:issued>2019-01-31</dcterms:issued>
        <dcterms:modified>2019-01-31</dcterms:modified>
        <rdfs:comment>A record describing a specimen which is alive (not preserved).</rdfs:comment>
        <skos:definition>A record describing a specimen which is alive (not preserved).</skos:definition>
    </abcd:RecordBasis>

    <abcd:RecordBasis rdf:about="FossilSpecimen">
        <rdfs:isDefinedBy rdf:resource="http://rs.tdwg.org/abcd/terms/"/>
        <dwcattributes:status>recommended</dwcattributes:status>
        <dcterms:issued>2019-01-31</dcterms:issued>
        <dcterms:modified>2019-01-31</dcterms:modified>
        <rdfs:comment>A record describing a preserved specimen that is a fossil.</rdfs:comment>
        <skos:definition>A record describing a preserved specimen that is a fossil.</skos:definition>
    </abcd:RecordBasis>

    <abcd:RecordBasis rdf:about="MineralSpecimen">
        <rdfs:isDefinedBy rdf:resource="http://rs.tdwg.org/abcd/terms/"/>
        <dwcattributes:status>recommended</dwcattributes:status>
        <dcterms:issued>2019-01-31</dcterms:issued>
        <dcterms:modified>2019-01-31</dcterms:modified>
        <rdfs:comment>A record describing a preserved specimen which is a mineral.</rdfs:comment>
        <skos:definition>A record describing a preserved specimen which is a mineral.</skos:definition>
    </abcd:RecordBasis>

    <abcd:RecordBasis rdf:about="OtherSpecimen">
        <rdfs:isDefinedBy rdf:resource="http://rs.tdwg.org/abcd/terms/"/>
        <dwcattributes:status>recommended</dwcattributes:status>
        <dcterms:issued>2019-01-31</dcterms:issued>
        <dcterms:modified>2019-01-31</dcterms:modified>
        <rdfs:comment>A record describing a specimen which is not covered by any of the other values in the Record Basis vocabulary.</rdfs:comment>
        <skos:definition>A record describing a specimen which is not covered by any of the other values in the Record Basis vocabulary.</skos:definition>
    </abcd:RecordBasis>

    <abcd:RecordBasis rdf:about="MaterialSample">
        <rdfs:isDefinedBy rdf:resource="http://rs.tdwg.org/abcd/terms/"/>
        <dwcattributes:status>recommended</dwcattributes:status>
        <dcterms:issued>2019-01-31</dcterms:issued>
        <dcterms:modified>2019-01-31</dcterms:modified>
        <rdfs:comment>A record describing the physical result of a sampling (or subsampling) event (sample either preserved or destructively processed).</rdfs:comment>
        <skos:definition>A record describing the physical result of a sampling (or subsampling) event (sample either preserved or destructively processed).</skos:definition>
    </abcd:RecordBasis>

    <abcd:RecordBasis rdf:about="HumanObservation">
        <rdfs:isDefinedBy rdf:resource="http://rs.tdwg.org/abcd/terms/"/>
        <dwcattributes:status>recommended</dwcattributes:status>
        <dcterms:issued>2019-01-31</dcterms:issued>
        <dcterms:modified>2019-01-31</dcterms:modified>
        <rdfs:comment>A record describing an output of a human observation process.</rdfs:comment>
        <skos:definition>A record describing an output of a human observation process.</skos:definition>
    </abcd:RecordBasis>

    <abcd:RecordBasis rdf:about="MachineObservation">
        <rdfs:isDefinedBy rdf:resource="http://rs.tdwg.org/abcd/terms/"/>
        <dwcattributes:status>recommended</dwcattributes:status>
        <dcterms:issued>2019-01-31</dcterms:issued>
        <dcterms:modified>2019-01-31</dcterms:modified>
        <rdfs:comment>A record describing an output of a machine observation process.</rdfs:comment>
        <skos:definition>A record describing an output of a machine observation process.</skos:definition>
    </abcd:RecordBasis>

    <abcd:RecordBasis rdf:about="DrawingOrPhotograph">
        <rdfs:isDefinedBy rdf:resource="http://rs.tdwg.org/abcd/terms/"/>
        <dwcattributes:status>recommended</dwcattributes:status>
        <dcterms:issued>2019-01-31</dcterms:issued>
        <dcterms:modified>2019-01-31</dcterms:modified>
        <rdfs:comment>A record describing a static visual representation (digital or physical).</rdfs:comment>
        <skos:definition>A record describing a static visual representation (digital or physical).</skos:definition>
        <dc:description>For sets of multiple images (image stacks) or films, please use abcd:MultimediaObject.</dc:description>
    </abcd:RecordBasis>

    <abcd:RecordBasis rdf:about="MultimediaRecord">
        <rdfs:isDefinedBy rdf:resource="http://rs.tdwg.org/abcd/terms/"/>
        <dwcattributes:status>recommended</dwcattributes:status>
        <dcterms:issued>2019-01-31</dcterms:issued>
        <dcterms:modified>2019-01-31</dcterms:modified>
        <rdfs:comment>A record describing a multimedia representation (digital or physical).</rdfs:comment>
        <skos:definition>A record describing a multimedia representation (digital or physical).</skos:definition>
        <dc:description>For single static images as a Record Basis please use the term abcd:DrawingOrPhotograph.</dc:description>
    </abcd:RecordBasis>

    <abcd:RecordBasis rdf:about="AbsenceObservation">
        <rdfs:isDefinedBy rdf:resource="http://rs.tdwg.org/abcd/terms/"/>
        <dwcattributes:status>recommended</dwcattributes:status>
        <dcterms:issued>2019-01-31</dcterms:issued>
        <dcterms:modified>2019-01-31</dcterms:modified>
        <rdfs:comment>A record describing an output of an observation process with indication of the absence of an observation</rdfs:comment>
        <skos:definition>A record describing an output of an observation process with indication of the absence of an observation</skos:definition>
    </abcd:RecordBasis>

    <abcd:Sex rdf:about="Male">
        <rdfs:isDefinedBy rdf:resource="http://rs.tdwg.org/abcd/terms/"/>
        <dwcattributes:status>recommended</dwcattributes:status>
        <dcterms:issued>2019-01-31</dcterms:issued>
        <dcterms:modified>2019-01-31</dcterms:modified>
        <rdfs:comment>Sex: Male.</rdfs:comment>
        <skos:definition>Sex: Male.</skos:definition>
    </abcd:Sex>

    <abcd:Sex rdf:about="Female">
        <rdfs:isDefinedBy rdf:resource="http://rs.tdwg.org/abcd/terms/"/>
        <dwcattributes:status>recommended</dwcattributes:status>
        <dcterms:issued>2019-01-31</dcterms:issued>
        <dcterms:modified>2019-01-31</dcterms:modified>
        <rdfs:comment>Sex: Female.</rdfs:comment>
        <skos:definition>Sex: Female.</skos:definition>
    </abcd:Sex>

    <abcd:Sex rdf:about="SexUnknown">
        <rdfs:isDefinedBy rdf:resource="http://rs.tdwg.org/abcd/terms/"/>
        <dwcattributes:status>recommended</dwcattributes:status>
        <dcterms:issued>2019-01-31</dcterms:issued>
        <dcterms:modified>2019-01-31</dcterms:modified>
        <rdfs:comment>Sex: Unknown.</rdfs:comment>
        <skos:definition>Sex: Unknown.</skos:definition>
    </abcd:Sex>

    <abcd:Sex rdf:about="SexNotApplicable">
        <rdfs:isDefinedBy rdf:resource="http://rs.tdwg.org/abcd/terms/"/>
        <dwcattributes:status>recommended</dwcattributes:status>
        <dcterms:issued>2019-01-31</dcterms:issued>
        <dcterms:modified>2019-01-31</dcterms:modified>
        <rdfs:comment>Sex: Not applicable, e.g. for a fungus in a herbarium.</rdfs:comment>
        <skos:definition>Sex: Not applicable, e.g. for a fungus in a herbarium.</skos:definition>
    </abcd:Sex>

    <abcd:Sex rdf:about="MixedSex">
        <rdfs:isDefinedBy rdf:resource="http://rs.tdwg.org/abcd/terms/"/>
        <dwcattributes:status>recommended</dwcattributes:status>
        <dcterms:issued>2019-01-31</dcterms:issued>
        <dcterms:modified>2019-01-31</dcterms:modified>
        <rdfs:comment>Sex: Mixed, like hermaphrodite or dioecious reproduction</rdfs:comment>
        <skos:definition>Sex: Mixed, like hermaphrodite or dioecious reproduction</skos:definition>
    </abcd:Sex>

    <abcd:PermitStatus rdf:about="PermitAvailable">
        <rdfs:isDefinedBy rdf:resource="http://rs.tdwg.org/abcd/terms/"/>
        <dwcattributes:status>recommended</dwcattributes:status>
        <dcterms:issued>2019-01-31</dcterms:issued>
        <dcterms:modified>2019-01-31</dcterms:modified>
        <rdfs:comment>Permit Status: Permit available</rdfs:comment>
        <skos:definition>Permit Status: Permit available</skos:definition>
    </abcd:PermitStatus>

    <abcd:PermitStatus rdf:about="PermitNotRequired">
        <rdfs:isDefinedBy rdf:resource="http://rs.tdwg.org/abcd/terms/"/>
        <dwcattributes:status>recommended</dwcattributes:status>
        <dcterms:issued>2019-01-31</dcterms:issued>
        <dcterms:modified>2019-01-31</dcterms:modified>
        <rdfs:comment>Permit Status: Permit not required</rdfs:comment>
        <skos:definition>Permit Status: Permit not required</skos:definition>
        <dc:description>Please use abcd:Details of the Permit class to explain why no permit was required.</dc:description>
    </abcd:PermitStatus>

    <abcd:PermitStatus rdf:about="PermitNotAvailable">
        <rdfs:isDefinedBy rdf:resource="http://rs.tdwg.org/abcd/terms/"/>
        <dwcattributes:status>recommended</dwcattributes:status>
        <dcterms:issued>2019-01-31</dcterms:issued>
        <dcterms:modified>2019-01-31</dcterms:modified>
        <rdfs:comment>Permit Status: Permit not available</rdfs:comment>
        <skos:definition>Permit Status: Permit not available</skos:definition>
    </abcd:PermitStatus>

    <abcd:PermitStatus rdf:about="PermitStatusUnknown">
        <rdfs:isDefinedBy rdf:resource="http://rs.tdwg.org/abcd/terms/"/>
        <dwcattributes:status>recommended</dwcattributes:status>
        <dcterms:issued>2019-01-31</dcterms:issued>
        <dcterms:modified>2019-01-31</dcterms:modified>
        <rdfs:comment>Permit Status: Unknown</rdfs:comment>
        <skos:definition>Permit Status: Unknown</skos:definition>
        <dc:description>Material collected after 2014-10-12 cannot be in "Unknown" Permit Status!</dc:description>
    </abcd:PermitStatus>

    <abcd:PermitType rdf:about="Contract">
        <rdfs:isDefinedBy rdf:resource="http://rs.tdwg.org/abcd/terms/"/>
        <dwcattributes:status>recommended</dwcattributes:status>
        <dcterms:issued>2019-01-31</dcterms:issued>
        <dcterms:modified>2019-01-31</dcterms:modified>
        <rdfs:comment>Permit Type: Contract</rdfs:comment>
        <skos:definition>Permit Type: Contract</skos:definition>
    </abcd:PermitType>

    <abcd:PermitType rdf:about="Copyright">
        <rdfs:isDefinedBy rdf:resource="http://rs.tdwg.org/abcd/terms/"/>
        <dwcattributes:status>recommended</dwcattributes:status>
        <dcterms:issued>2019-01-31</dcterms:issued>
        <dcterms:modified>2019-01-31</dcterms:modified>
        <rdfs:comment>Permit Type: Copyright</rdfs:comment>
        <skos:definition>Permit Type: Copyright</skos:definition>
    </abcd:PermitType>

    <abcd:PermitType rdf:about="DataUse">
        <rdfs:isDefinedBy rdf:resource="http://rs.tdwg.org/abcd/terms/"/>
        <dwcattributes:status>recommended</dwcattributes:status>
        <dcterms:issued>2019-01-31</dcterms:issued>
        <dcterms:modified>2019-01-31</dcterms:modified>
        <rdfs:comment>Permit Type: Data use</rdfs:comment>
        <skos:definition>Permit Type: Data use</skos:definition>
    </abcd:PermitType>

    <abcd:PermitType rdf:about="ExemptionPermit">
        <rdfs:isDefinedBy rdf:resource="http://rs.tdwg.org/abcd/terms/"/>
        <dwcattributes:status>recommended</dwcattributes:status>
        <dcterms:issued>2019-01-31</dcterms:issued>
        <dcterms:modified>2019-01-31</dcterms:modified>
        <rdfs:comment>Permit Type:  Exemption Permit</rdfs:comment>
        <skos:definition>Permit Type:  Exemption Permit</skos:definition>
    </abcd:PermitType>

    <abcd:PermitType rdf:about="ExportPermit">
        <rdfs:isDefinedBy rdf:resource="http://rs.tdwg.org/abcd/terms/"/>
        <dwcattributes:status>recommended</dwcattributes:status>
        <dcterms:issued>2019-01-31</dcterms:issued>
        <dcterms:modified>2019-01-31</dcterms:modified>
        <rdfs:comment>Permit Type: Export Permit</rdfs:comment>
        <skos:definition>Permit Type: Export Permit</skos:definition>
    </abcd:PermitType>

    <abcd:PermitType rdf:about="GeneticallyModifiedOrganism">
        <rdfs:isDefinedBy rdf:resource="http://rs.tdwg.org/abcd/terms/"/>
        <dwcattributes:status>recommended</dwcattributes:status>
        <dcterms:issued>2019-01-31</dcterms:issued>
        <dcterms:modified>2019-01-31</dcterms:modified>
        <rdfs:comment>Permit Type: Genetically Modified Organism</rdfs:comment>
        <skos:definition>Permit Type: Genetically Modified Organism</skos:definition>
    </abcd:PermitType>

    <abcd:PermitType rdf:about="HumanPathogens">
        <rdfs:isDefinedBy rdf:resource="http://rs.tdwg.org/abcd/terms/"/>
        <dwcattributes:status>recommended</dwcattributes:status>
        <dcterms:issued>2019-01-31</dcterms:issued>
        <dcterms:modified>2019-01-31</dcterms:modified>
        <rdfs:comment>Permit Type: Human Pathogens</rdfs:comment>
        <skos:definition>Permit Type: Human Pathogens</skos:definition>
    </abcd:PermitType>

    <abcd:PermitType rdf:about="IntellectualPropertyRights">
        <rdfs:isDefinedBy rdf:resource="http://rs.tdwg.org/abcd/terms/"/>
        <dwcattributes:status>recommended</dwcattributes:status>
        <dcterms:issued>2019-01-31</dcterms:issued>
        <dcterms:modified>2019-01-31</dcterms:modified>
        <rdfs:comment>Permit Type: Intellectual Property Rights</rdfs:comment>
        <skos:definition>Permit Type: Intellectual Property Rights</skos:definition>
    </abcd:PermitType>

    <abcd:PermitType rdf:about="InternationallyRecognizedCertificateOfCompliance">
        <rdfs:isDefinedBy rdf:resource="http://rs.tdwg.org/abcd/terms/"/>
        <dwcattributes:status>recommended</dwcattributes:status>
        <dcterms:issued>2019-01-31</dcterms:issued>
        <dcterms:modified>2019-01-31</dcterms:modified>
        <rdfs:comment>Permit Type: Internationally Recognized Certificate of Compliance</rdfs:comment>
        <skos:definition>Permit Type: Internationally Recognized Certificate of Compliance</skos:definition>
    </abcd:PermitType>

    <abcd:PermitType rdf:about="ImportPermit">
        <rdfs:isDefinedBy rdf:resource="http://rs.tdwg.org/abcd/terms/"/>
        <dwcattributes:status>recommended</dwcattributes:status>
        <dcterms:issued>2019-01-31</dcterms:issued>
        <dcterms:modified>2019-01-31</dcterms:modified>
        <rdfs:comment>Permit Type: Import Permit</rdfs:comment>
        <skos:definition>Permit Type: Import Permit</skos:definition>
    </abcd:PermitType>

    <abcd:PermitType rdf:about="CollectingPermit">
        <rdfs:isDefinedBy rdf:resource="http://rs.tdwg.org/abcd/terms/"/>
        <dwcattributes:status>recommended</dwcattributes:status>
        <dcterms:issued>2019-01-31</dcterms:issued>
        <dcterms:modified>2019-01-31</dcterms:modified>
        <rdfs:comment>Permit Type: Collecting Permit</rdfs:comment>
        <skos:definition>Permit Type: Collecting Permit</skos:definition>
    </abcd:PermitType>

    <abcd:PermitType rdf:about="MaterialTransferAgreement">
        <rdfs:isDefinedBy rdf:resource="http://rs.tdwg.org/abcd/terms/"/>
        <dwcattributes:status>recommended</dwcattributes:status>
        <dcterms:issued>2019-01-31</dcterms:issued>
        <dcterms:modified>2019-01-31</dcterms:modified>
        <rdfs:comment>Permit Type: Material Transfer Agreement</rdfs:comment>
        <skos:definition>Permit Type: Material Transfer Agreement</skos:definition>
    </abcd:PermitType>

    <abcd:PermitType rdf:about="MemorandumOfCooperation">
        <rdfs:isDefinedBy rdf:resource="http://rs.tdwg.org/abcd/terms/"/>
        <dwcattributes:status>recommended</dwcattributes:status>
        <dcterms:issued>2019-01-31</dcterms:issued>
        <dcterms:modified>2019-01-31</dcterms:modified>
        <rdfs:comment>Permit Type: Memorandum of Cooperation</rdfs:comment>
        <skos:definition>Permit Type: Memorandum of Cooperation</skos:definition>
    </abcd:PermitType>

    <abcd:PermitType rdf:about="MemorandumOfUnderstanding">
        <rdfs:isDefinedBy rdf:resource="http://rs.tdwg.org/abcd/terms/"/>
        <dwcattributes:status>recommended</dwcattributes:status>
        <dcterms:issued>2019-01-31</dcterms:issued>
        <dcterms:modified>2019-01-31</dcterms:modified>
        <rdfs:comment>Permit Type: Memorandum of Understanding</rdfs:comment>
        <skos:definition>Permit Type: Memorandum of Understanding</skos:definition>
    </abcd:PermitType>

    <abcd:PermitType rdf:about="Patent">
        <rdfs:isDefinedBy rdf:resource="http://rs.tdwg.org/abcd/terms/"/>
        <dwcattributes:status>recommended</dwcattributes:status>
        <dcterms:issued>2019-01-31</dcterms:issued>
        <dcterms:modified>2019-01-31</dcterms:modified>
        <rdfs:comment>Permit Type: Patent</rdfs:comment>
        <skos:definition>Permit Type: Patent</skos:definition>
    </abcd:PermitType>

    <abcd:PermitType rdf:about="Phytosanitary">
        <rdfs:isDefinedBy rdf:resource="http://rs.tdwg.org/abcd/terms/"/>
        <dwcattributes:status>recommended</dwcattributes:status>
        <dcterms:issued>2019-01-31</dcterms:issued>
        <dcterms:modified>2019-01-31</dcterms:modified>
        <rdfs:comment>Permit Type: Phytosanitary</rdfs:comment>
        <skos:definition>Permit Type: Phytosanitary</skos:definition>
    </abcd:PermitType>

    <abcd:PermitType rdf:about="Salvage">
        <rdfs:isDefinedBy rdf:resource="http://rs.tdwg.org/abcd/terms/"/>
        <dwcattributes:status>recommended</dwcattributes:status>
        <dcterms:issued>2019-01-31</dcterms:issued>
        <dcterms:modified>2019-01-31</dcterms:modified>
        <rdfs:comment>Permit Type: Salvage</rdfs:comment>
        <skos:definition>Permit Type: Salvage</skos:definition>
    </abcd:PermitType>

    <abcd:PermitType rdf:about="VeterinaryCertificate">
        <rdfs:isDefinedBy rdf:resource="http://rs.tdwg.org/abcd/terms/"/>
        <dwcattributes:status>recommended</dwcattributes:status>
        <dcterms:issued>2019-01-31</dcterms:issued>
        <dcterms:modified>2019-01-31</dcterms:modified>
        <rdfs:comment>Permit Type: Veterinary Certificate</rdfs:comment>
        <skos:definition>Permit Type: Veterinary Certificate</skos:definition>
    </abcd:PermitType>

    <abcd:RecordBasis rdf:about="EarthScienceSpecimen">
        <rdfs:isDefinedBy rdf:resource="http://rs.tdwg.org/abcd/terms/"/>
        <dwcattributes:status>recommended</dwcattributes:status>
        <dcterms:issued>2019-01-31</dcterms:issued>
        <dcterms:modified>2019-01-31</dcterms:modified>
        <rdfs:comment>A record describing a geo-scientific object which is no pure mineral, rock or fossil specimen (but a mixture), or a geo-scientific specimen with unknown trait.</rdfs:comment>
        <skos:definition>A record describing a geo-scientific object which is no pure mineral, rock or fossil specimen (but a mixture), or a geo-scientific specimen with unknown trait.</skos:definition>
    </abcd:RecordBasis>

    <abcd:RecordBasis rdf:about="Literature">
        <rdfs:isDefinedBy rdf:resource="http://rs.tdwg.org/abcd/terms/"/>
        <dwcattributes:status>recommended</dwcattributes:status>
        <dcterms:issued>2019-01-31</dcterms:issued>
        <dcterms:modified>2019-01-31</dcterms:modified>
        <rdfs:comment>A record describing an output of a literature research.</rdfs:comment>
        <skos:definition>A record describing an output of a literature research.</skos:definition>
    </abcd:RecordBasis>

    <abcd:RecordBasis rdf:about="Unknown">
        <rdfs:isDefinedBy rdf:resource="http://rs.tdwg.org/abcd/terms/"/>
        <dwcattributes:status>recommended</dwcattributes:status>
        <dcterms:issued>2019-01-31</dcterms:issued>
        <dcterms:modified>2019-01-31</dcterms:modified>
        <rdfs:comment>A record where the indication (basis) of the record is unknown.</rdfs:comment>
        <skos:definition>A record where the indication (basis) of the record is unknown.</skos:definition>
    </abcd:RecordBasis>

    <rdf:Property rdf:about="http://gensc.org/ns/mixs/sieving">
        <rdfs:comment>Collection design of pooled samples and/or sieve size and amount of sample sieved. Is of interest for metagenomic focus e.g. design name and/or size;amount.</rdfs:comment>
        <skos:definition>Collection design of pooled samples and/or sieve size and amount of sample sieved. Is of interest for metagenomic focus e.g. design name and/or size;amount.</skos:definition>
    </rdf:Property>

    <rdf:Property rdf:about="http://rs.tdwg.org/ac/terms/IDofContainingCollection">
        <rdfs:comment>If the resource is contained in a Collection, this field identifies that Collection uniquely. Its form is not specified by this normative document, but is left to implementers of specific implementations.</rdfs:comment>
        <skos:definition>If the resource is contained in a Collection, this field identifies that Collection uniquely. Its form is not specified by this normative document, but is left to implementers of specific implementations.</skos:definition>
    </rdf:Property>

    <rdf:Property rdf:about="http://purl.org/dc/elements/1.1/type">
        <rdfs:comment>Recommended terms are Collection, StillImage, Sound, MovingImage, InteractiveResource, Text.</rdfs:comment>
        <skos:definition>Recommended terms are Collection, StillImage, Sound, MovingImage, InteractiveResource, Text.</skos:definition>
        <dc:description>At least one of dc:type and dcterms:type must be supplied but, when feasible, supplying both may make the metadata more widely useful. The values of each should designate the same type, but in case of ambiguity dcterms:type prevails.</dc:description>
        <dc:description>Values may be used either in their literal form, or with a full namespace (e. g. http://purl.org/dc/dcmitype/StillImage) from a controlled vocabulary, but the best practice is to use the literal form when using dc:type and use dcterms:type when you can supply the URI from a controlled vocabulary and implementers may require this practice.</dc:description>
    </rdf:Property>

    <rdf:Property rdf:about="http://rs.tdwg.org/ac/terms/provider">
        <rdfs:comment>URI for person or organization responsible for presenting the media resource. If no separate Metadata Provider is given, this also attributes the metadata.</rdfs:comment>
        <skos:definition>URI for person or organization responsible for presenting the media resource. If no separate Metadata Provider is given, this also attributes the metadata.</skos:definition>
    </rdf:Property>

    <rdf:Property rdf:about="http://rs.tdwg.org/ac/terms/tag">
        <rdfs:comment>General keywords or tags. Tags may be multi-worded phrases. Where scientific names, common names, geographic locations, etc. are separable, those should go into the more specific coverage metadata items provided further below.</rdfs:comment>
        <skos:definition>General keywords or tags. Tags may be multi-worded phrases. Where scientific names, common names, geographic locations, etc. are separable, those should go into the more specific coverage metadata items provided further below.</skos:definition>
        <dc:description>Examples: "flower diagram". Character or part keywords like "leaf", or "flower color" are especially desirable.</dc:description>
    </rdf:Property>

    <rdf:Property rdf:about="http://ns.adobe.com/xap/1.0/Rating">
        <rdfs:comment>A rating of the media resources, provided by record originators or editors, with -1 defining &#8220;rejected&#8221;, &#8220;0&#8221; defining &#8220;unrated&#8221;, and &#8220;1&#8221; (worst) to &#8220;5&#8221; (best).</rdfs:comment>
        <skos:definition>A rating of the media resources, provided by record originators or editors, with -1 defining &#8220;rejected&#8221;, &#8220;0&#8221; defining &#8220;unrated&#8221;, and &#8220;1&#8221; (worst) to &#8220;5&#8221; (best).</skos:definition>
        <dc:description>The origin of the rating is not communicated. It may, e. g., be based on user feedback or on editorial ratings. If Rating is not present, a value of 0 may be assumed. By "user-assigned" is meant assigned by the originator or editor of the record using the term.</dc:description>
    </rdf:Property>

    <rdf:Property rdf:about="http://rs.tdwg.org/dwc/terms/sex">
        <rdfs:comment>A description of the sex of any organisms featured within the media, when relevant to the subject of the media, e. g., male, female, hermaphrodite, dioecious.</rdfs:comment>
        <skos:definition>A description of the sex of any organisms featured within the media, when relevant to the subject of the media, e. g., male, female, hermaphrodite, dioecious.</skos:definition>
    </rdf:Property>

    <rdf:Property rdf:about="http://rs.tdwg.org/dwc/terms/lifeStage">
        <rdfs:comment>A description of the life-cycle stage of any organisms featured within the media, when relevant to the subject of the media, e. g., larvae, juvenile, adult.</rdfs:comment>
        <skos:definition>A description of the life-cycle stage of any organisms featured within the media, when relevant to the subject of the media, e. g., larvae, juvenile, adult.</skos:definition>
    </rdf:Property>

    <rdf:Property rdf:about="http://rs.tdwg.org/ac/terms/subjectPart">
        <rdfs:comment>The portion or product of organism morphology, behavior, environment, etc. that is either predominantly shown or particularly well exemplified by the media resource.</rdfs:comment>
        <skos:definition>The portion or product of organism morphology, behavior, environment, etc. that is either predominantly shown or particularly well exemplified by the media resource.</skos:definition>
        <dc:description>No formal encoding scheme as yet exists. Examples are "whole body", "head", "flower", "leaf", "canopy" (of a rain forest stand). Several anatomical ontologies are emerging in http://www.obofoundry.org/</dc:description>
    </rdf:Property>

    <rdf:Property rdf:about="http://rs.tdwg.org/ac/terms/subjectOrientation">
        <rdfs:comment>Specific orientation (= direction, view angle) of the subject represented in the media resource with respect to the acquisition device.</rdfs:comment>
        <skos:definition>Specific orientation (= direction, view angle) of the subject represented in the media resource with respect to the acquisition device.</skos:definition>
        <dc:description>Examples: "dorsal", "ventral", "frontal", etc. No formal encoding scheme as yet exists. The term is repeatable e.g., in the case of a composite image, consisting of a combination of different view orientations.</dc:description>
    </rdf:Property>
</rdf:RDF>

